<?xml version="1.0"?>
<rdf:RDF xmlns="http://www.semanticweb.org/marthinust/ontologies/2022/8/untitled-ontology-7#"
     xml:base="http://www.semanticweb.org/marthinust/ontologies/2022/8/untitled-ontology-7"
     xmlns:owl="http://www.w3.org/2002/07/owl#"
     xmlns:rdf="http://www.w3.org/1999/02/22-rdf-syntax-ns#"
     xmlns:xml="http://www.w3.org/XML/1998/namespace"
     xmlns:xsd="http://www.w3.org/2001/XMLSchema#"
     xmlns:rdfs="http://www.w3.org/2000/01/rdf-schema#"
     xmlns:opla-sd="http://ontologydesignpatterns.org/opla-sd#"
     xmlns:Gait_Ontology="http://www.semanticweb.org/marthinust/ontologies/2022/8/Gait_Ontology#">
    <owl:Ontology rdf:about="http://www.semanticweb.org/marthinust/ontologies/2022/8/Gait_Ontology">
        <rdfs:comment xml:lang="en">This is the Gait Analysis Domain Ontology (GADO) for gait-related diseases.</rdfs:comment>
    </owl:Ontology>
    


    <!-- 
    ///////////////////////////////////////////////////////////////////////////////////////
    //
    // Annotation properties
    //
    ///////////////////////////////////////////////////////////////////////////////////////
     -->

    


    <!-- http://ontologydesignpatterns.org/opla-sd#entityPosition -->

    <owl:AnnotationProperty rdf:about="http://ontologydesignpatterns.org/opla-sd#entityPosition"/>
    


    <!-- http://ontologydesignpatterns.org/opla-sd#entityPositionX -->

    <owl:AnnotationProperty rdf:about="http://ontologydesignpatterns.org/opla-sd#entityPositionX"/>
    


    <!-- http://ontologydesignpatterns.org/opla-sd#entityPositionY -->

    <owl:AnnotationProperty rdf:about="http://ontologydesignpatterns.org/opla-sd#entityPositionY"/>
    


    <!-- 
    ///////////////////////////////////////////////////////////////////////////////////////
    //
    // Object Properties
    //
    ///////////////////////////////////////////////////////////////////////////////////////
     -->

    


    <!-- http://www.semanticweb.org/marthinust/ontologies/2022/8/Gait_Ontology#administers -->

    <owl:ObjectProperty rdf:about="http://www.semanticweb.org/marthinust/ontologies/2022/8/Gait_Ontology#administers">
        <owl:inverseOf rdf:resource="http://www.semanticweb.org/marthinust/ontologies/2022/8/Gait_Ontology#isAdministeredBy"/>
        <rdf:type rdf:resource="http://www.w3.org/2002/07/owl#InverseFunctionalProperty"/>
        <rdfs:domain rdf:resource="http://www.semanticweb.org/marthinust/ontologies/2022/8/Gait_Ontology#Gait_expert"/>
        <rdfs:range rdf:resource="http://www.semanticweb.org/marthinust/ontologies/2022/8/Gait_Ontology#Gait-based_Process"/>
        <rdfs:comment xml:lang="en">The gait expert administers the gait -based process</rdfs:comment>
        <rdfs:label xml:lang="en">administers</rdfs:label>
    </owl:ObjectProperty>
    


    <!-- http://www.semanticweb.org/marthinust/ontologies/2022/8/Gait_Ontology#affects -->

    <owl:ObjectProperty rdf:about="http://www.semanticweb.org/marthinust/ontologies/2022/8/Gait_Ontology#affects">
        <owl:inverseOf rdf:resource="http://www.semanticweb.org/marthinust/ontologies/2022/8/Gait_Ontology#isAffectedBy"/>
        <rdf:type rdf:resource="http://www.w3.org/2002/07/owl#InverseFunctionalProperty"/>
        <rdfs:domain rdf:resource="http://www.semanticweb.org/marthinust/ontologies/2022/8/Gait_Ontology#Gait_Disturbance"/>
        <rdfs:range rdf:resource="http://www.semanticweb.org/marthinust/ontologies/2022/8/Gait_Ontology#Gait_patient"/>
        <rdfs:comment xml:lang="en">A gait disturbance that affects a patient</rdfs:comment>
        <rdfs:label xml:lang="en">affects</rdfs:label>
    </owl:ObjectProperty>
    


    <!-- http://www.semanticweb.org/marthinust/ontologies/2022/8/Gait_Ontology#analyzes -->

    <owl:ObjectProperty rdf:about="http://www.semanticweb.org/marthinust/ontologies/2022/8/Gait_Ontology#analyzes">
        <owl:inverseOf rdf:resource="http://www.semanticweb.org/marthinust/ontologies/2022/8/Gait_Ontology#isAnalysedBy"/>
        <rdf:type rdf:resource="http://www.w3.org/2002/07/owl#InverseFunctionalProperty"/>
        <rdfs:domain rdf:resource="http://www.semanticweb.org/marthinust/ontologies/2022/8/Gait_Ontology#Gait_expert"/>
        <rdfs:range rdf:resource="http://www.semanticweb.org/marthinust/ontologies/2022/8/Gait_Ontology#Gait_data"/>
        <rdfs:comment xml:lang="en">The gait expert analyzes the collected gait data.</rdfs:comment>
        <rdfs:label xml:lang="en">analyzes</rdfs:label>
    </owl:ObjectProperty>
    


    <!-- http://www.semanticweb.org/marthinust/ontologies/2022/8/Gait_Ontology#collects -->

    <owl:ObjectProperty rdf:about="http://www.semanticweb.org/marthinust/ontologies/2022/8/Gait_Ontology#collects">
        <owl:inverseOf rdf:resource="http://www.semanticweb.org/marthinust/ontologies/2022/8/Gait_Ontology#isCollectedBy"/>
        <rdf:type rdf:resource="http://www.w3.org/2002/07/owl#InverseFunctionalProperty"/>
        <rdfs:domain rdf:resource="http://www.semanticweb.org/marthinust/ontologies/2022/8/Gait_Ontology#Gait_acquisition"/>
        <rdfs:range rdf:resource="http://www.semanticweb.org/marthinust/ontologies/2022/8/Gait_Ontology#Gait_data"/>
        <rdfs:comment xml:lang="en">The gait acquisition session collects gait data.</rdfs:comment>
        <rdfs:label xml:lang="en">collects</rdfs:label>
    </owl:ObjectProperty>
    


    <!-- http://www.semanticweb.org/marthinust/ontologies/2022/8/Gait_Ontology#demonstrates -->

    <owl:ObjectProperty rdf:about="http://www.semanticweb.org/marthinust/ontologies/2022/8/Gait_Ontology#demonstrates">
        <owl:inverseOf rdf:resource="http://www.semanticweb.org/marthinust/ontologies/2022/8/Gait_Ontology#isDemonstratedBy"/>
        <rdf:type rdf:resource="http://www.w3.org/2002/07/owl#InverseFunctionalProperty"/>
        <rdfs:domain rdf:resource="http://www.semanticweb.org/marthinust/ontologies/2022/8/Gait_Ontology#Gait_patient"/>
        <rdfs:range rdf:resource="http://www.semanticweb.org/marthinust/ontologies/2022/8/Gait_Ontology#Gait_Cycle"/>
        <rdfs:comment xml:lang="en">The (gait) patient demonstrates a gait cycle.</rdfs:comment>
        <rdfs:label xml:lang="en">demonstrates</rdfs:label>
    </owl:ObjectProperty>
    


    <!-- http://www.semanticweb.org/marthinust/ontologies/2022/8/Gait_Ontology#exhibits -->

    <owl:ObjectProperty rdf:about="http://www.semanticweb.org/marthinust/ontologies/2022/8/Gait_Ontology#exhibits">
        <owl:inverseOf rdf:resource="http://www.semanticweb.org/marthinust/ontologies/2022/8/Gait_Ontology#isExhibitedBy"/>
        <rdf:type rdf:resource="http://www.w3.org/2002/07/owl#InverseFunctionalProperty"/>
        <rdfs:domain rdf:resource="http://www.semanticweb.org/marthinust/ontologies/2022/8/Gait_Ontology#Gait_patient"/>
        <rdfs:range rdf:resource="http://www.semanticweb.org/marthinust/ontologies/2022/8/Gait_Ontology#Type_of_Gait"/>
        <rdfs:comment xml:lang="en">The (gait) patient exhibits the type of gait.</rdfs:comment>
        <rdfs:label xml:lang="en">exhibits</rdfs:label>
    </owl:ObjectProperty>
    


    <!-- http://www.semanticweb.org/marthinust/ontologies/2022/8/Gait_Ontology#facilitates -->

    <owl:ObjectProperty rdf:about="http://www.semanticweb.org/marthinust/ontologies/2022/8/Gait_Ontology#facilitates">
        <owl:inverseOf rdf:resource="http://www.semanticweb.org/marthinust/ontologies/2022/8/Gait_Ontology#isFacilitatedBy"/>
        <rdf:type rdf:resource="http://www.w3.org/2002/07/owl#InverseFunctionalProperty"/>
        <rdfs:domain rdf:resource="http://www.semanticweb.org/marthinust/ontologies/2022/8/Gait_Ontology#Gait_expert"/>
        <rdfs:range rdf:resource="http://www.semanticweb.org/marthinust/ontologies/2022/8/Gait_Ontology#Gait_analysis"/>
        <rdfs:comment xml:lang="en">The gait expert facilitates the gait analysis process.</rdfs:comment>
        <rdfs:label xml:lang="en">facilitates</rdfs:label>
    </owl:ObjectProperty>
    


    <!-- http://www.semanticweb.org/marthinust/ontologies/2022/8/Gait_Ontology#hasAgeGroup -->

    <owl:ObjectProperty rdf:about="http://www.semanticweb.org/marthinust/ontologies/2022/8/Gait_Ontology#hasAgeGroup">
        <rdf:type rdf:resource="http://www.w3.org/2002/07/owl#FunctionalProperty"/>
        <rdfs:domain rdf:resource="http://www.semanticweb.org/marthinust/ontologies/2022/8/Gait_Ontology#Gait_Person"/>
        <rdfs:range rdf:resource="http://www.semanticweb.org/marthinust/ontologies/2022/8/Gait_Ontology#Gait_patient"/>
        <rdfs:comment xml:lang="en">Age group classification refers to the practice of dividing people into groups based on their age. This is often done for statistical or research purposes, as well as for the development of age-specific policies, research and programmes. 

Age group classifications can vary depending on the context, but some common examples include:

Children: usually considered to be between the ages of newborn and 12 years old
Adolescents: people who are going through puberty and the transition from childhood to adulthood, typically between the ages of 11 and 20
Adults: people who have reached physical and mental maturity, usually considered to be 18 or 21 years and older
Elderly: people who are older, usually in their later years of life; the age at which someone is considered elderly can vary, but it is often used to describe people who are in their 60s or older.
Other age group classifications may include infants, toddlers, pre-adolescents, young adults, middle-aged adults, and seniors.</rdfs:comment>
        <rdfs:label xml:lang="en">hasAgeGroup</rdfs:label>
    </owl:ObjectProperty>
    


    <!-- http://www.semanticweb.org/marthinust/ontologies/2022/8/Gait_Ontology#involves -->

    <owl:ObjectProperty rdf:about="http://www.semanticweb.org/marthinust/ontologies/2022/8/Gait_Ontology#involves">
        <owl:inverseOf rdf:resource="http://www.semanticweb.org/marthinust/ontologies/2022/8/Gait_Ontology#isInvolvedIn"/>
        <rdf:type rdf:resource="http://www.w3.org/2002/07/owl#InverseFunctionalProperty"/>
        <rdfs:domain rdf:resource="http://www.semanticweb.org/marthinust/ontologies/2022/8/Gait_Ontology#Gait_acquisition"/>
        <rdfs:range rdf:resource="http://www.semanticweb.org/marthinust/ontologies/2022/8/Gait_Ontology#Gait_patient"/>
        <rdfs:comment xml:lang="en">The gait acquisition (session) involves a patient.</rdfs:comment>
        <rdfs:label xml:lang="en">involves</rdfs:label>
    </owl:ObjectProperty>
    


    <!-- http://www.semanticweb.org/marthinust/ontologies/2022/8/Gait_Ontology#isAcquiredFrom -->

    <owl:ObjectProperty rdf:about="http://www.semanticweb.org/marthinust/ontologies/2022/8/Gait_Ontology#isAcquiredFrom">
        <rdf:type rdf:resource="http://www.w3.org/2002/07/owl#FunctionalProperty"/>
        <rdfs:domain rdf:resource="http://www.semanticweb.org/marthinust/ontologies/2022/8/Gait_Ontology#Gait_data"/>
        <rdfs:range rdf:resource="http://www.semanticweb.org/marthinust/ontologies/2022/8/Gait_Ontology#Gait_patient"/>
        <rdfs:comment xml:lang="en">Clinical gait data isAcquiredFrom a (gait) patient.</rdfs:comment>
        <rdfs:label xml:lang="en">isAcquiredFrom</rdfs:label>
    </owl:ObjectProperty>
    


    <!-- http://www.semanticweb.org/marthinust/ontologies/2022/8/Gait_Ontology#isAdministeredBy -->

    <owl:ObjectProperty rdf:about="http://www.semanticweb.org/marthinust/ontologies/2022/8/Gait_Ontology#isAdministeredBy">
        <rdf:type rdf:resource="http://www.w3.org/2002/07/owl#FunctionalProperty"/>
        <rdfs:domain rdf:resource="http://www.semanticweb.org/marthinust/ontologies/2022/8/Gait_Ontology#Gait-based_Process"/>
        <rdfs:range rdf:resource="http://www.semanticweb.org/marthinust/ontologies/2022/8/Gait_Ontology#Gait_expert"/>
        <rdfs:comment xml:lang="en">The gait-based process isAdministeredBy the gait expert.</rdfs:comment>
        <rdfs:label xml:lang="en">isAdministeredBy</rdfs:label>
    </owl:ObjectProperty>
    


    <!-- http://www.semanticweb.org/marthinust/ontologies/2022/8/Gait_Ontology#isAffectedBy -->

    <owl:ObjectProperty rdf:about="http://www.semanticweb.org/marthinust/ontologies/2022/8/Gait_Ontology#isAffectedBy">
        <rdf:type rdf:resource="http://www.w3.org/2002/07/owl#FunctionalProperty"/>
        <rdfs:domain rdf:resource="http://www.semanticweb.org/marthinust/ontologies/2022/8/Gait_Ontology#Gait_patient"/>
        <rdfs:range rdf:resource="http://www.semanticweb.org/marthinust/ontologies/2022/8/Gait_Ontology#Gait_Disturbance"/>
        <rdfs:comment xml:lang="en">Gait patient isAffectedBy Gait Disturbance.</rdfs:comment>
        <rdfs:label xml:lang="en">isAffectedBy</rdfs:label>
    </owl:ObjectProperty>
    


    <!-- http://www.semanticweb.org/marthinust/ontologies/2022/8/Gait_Ontology#isAnalysedBy -->

    <owl:ObjectProperty rdf:about="http://www.semanticweb.org/marthinust/ontologies/2022/8/Gait_Ontology#isAnalysedBy">
        <rdf:type rdf:resource="http://www.w3.org/2002/07/owl#FunctionalProperty"/>
        <rdfs:domain rdf:resource="http://www.semanticweb.org/marthinust/ontologies/2022/8/Gait_Ontology#Gait_data"/>
        <rdfs:range rdf:resource="http://www.semanticweb.org/marthinust/ontologies/2022/8/Gait_Ontology#Gait_expert"/>
        <rdfs:comment xml:lang="en">Gait data isAnalysedBy a (gait) expert.</rdfs:comment>
        <rdfs:label xml:lang="en">isAnalysedBy</rdfs:label>
    </owl:ObjectProperty>
    


    <!-- http://www.semanticweb.org/marthinust/ontologies/2022/8/Gait_Ontology#isAnalysedIn -->

    <owl:ObjectProperty rdf:about="http://www.semanticweb.org/marthinust/ontologies/2022/8/Gait_Ontology#isAnalysedIn">
        <rdf:type rdf:resource="http://www.w3.org/2002/07/owl#FunctionalProperty"/>
        <rdfs:domain rdf:resource="http://www.semanticweb.org/marthinust/ontologies/2022/8/Gait_Ontology#Gait_Measurement_Point"/>
        <rdfs:range rdf:resource="http://www.semanticweb.org/marthinust/ontologies/2022/8/Gait_Ontology#Gait_Cycle"/>
        <rdfs:comment xml:lang="en">Gait Measurement Point isAnalysedIn Gait Cycle.</rdfs:comment>
        <rdfs:label xml:lang="en">isAnalysedIn</rdfs:label>
    </owl:ObjectProperty>
    


    <!-- http://www.semanticweb.org/marthinust/ontologies/2022/8/Gait_Ontology#isAscertainedIn -->

    <owl:ObjectProperty rdf:about="http://www.semanticweb.org/marthinust/ontologies/2022/8/Gait_Ontology#isAscertainedIn">
        <rdf:type rdf:resource="http://www.w3.org/2002/07/owl#FunctionalProperty"/>
        <rdfs:domain rdf:resource="http://www.semanticweb.org/marthinust/ontologies/2022/8/Gait_Ontology#Gait_Assistive_Technology"/>
        <rdfs:range rdf:resource="http://www.semanticweb.org/marthinust/ontologies/2022/8/Gait_Ontology#Gait-based_Process"/>
        <rdfs:comment xml:lang="en">The type of Gait Assistive device solution isAscertainedIn the Gait-based process.</rdfs:comment>
        <rdfs:label xml:lang="en">isAscertainedIn</rdfs:label>
    </owl:ObjectProperty>
    


    <!-- http://www.semanticweb.org/marthinust/ontologies/2022/8/Gait_Ontology#isAssessedIn -->

    <owl:ObjectProperty rdf:about="http://www.semanticweb.org/marthinust/ontologies/2022/8/Gait_Ontology#isAssessedIn">
        <rdf:type rdf:resource="http://www.w3.org/2002/07/owl#FunctionalProperty"/>
        <rdfs:domain rdf:resource="http://www.semanticweb.org/marthinust/ontologies/2022/8/Gait_Ontology#Gait_patient"/>
        <rdfs:range rdf:resource="http://www.semanticweb.org/marthinust/ontologies/2022/8/Gait_Ontology#Gait-based_Process"/>
        <rdfs:comment xml:lang="en">The (gait) patient isAssessedIn the gait-based process.</rdfs:comment>
        <rdfs:label xml:lang="en">isAssessedIn</rdfs:label>
    </owl:ObjectProperty>
    


    <!-- http://www.semanticweb.org/marthinust/ontologies/2022/8/Gait_Ontology#isAssignedWith -->

    <owl:ObjectProperty rdf:about="http://www.semanticweb.org/marthinust/ontologies/2022/8/Gait_Ontology#isAssignedWith">
        <owl:inverseOf rdf:resource="http://www.semanticweb.org/marthinust/ontologies/2022/8/Gait_Ontology#isRecommendedTo"/>
        <rdf:type rdf:resource="http://www.w3.org/2002/07/owl#InverseFunctionalProperty"/>
        <rdfs:domain rdf:resource="http://www.semanticweb.org/marthinust/ontologies/2022/8/Gait_Ontology#Gait_patient"/>
        <rdfs:range rdf:resource="http://www.semanticweb.org/marthinust/ontologies/2022/8/Gait_Ontology#Gait_Assistive_Technology"/>
        <rdfs:comment xml:lang="en">A Gait patient isAssignedWith a Gait assistive technology</rdfs:comment>
        <rdfs:label xml:lang="en">isAssignedWith</rdfs:label>
    </owl:ObjectProperty>
    


    <!-- http://www.semanticweb.org/marthinust/ontologies/2022/8/Gait_Ontology#isAssociatedTo -->

    <owl:ObjectProperty rdf:about="http://www.semanticweb.org/marthinust/ontologies/2022/8/Gait_Ontology#isAssociatedTo">
        <owl:inverseOf rdf:resource="http://www.semanticweb.org/marthinust/ontologies/2022/8/Gait_Ontology#isLinkedWith"/>
        <rdf:type rdf:resource="http://www.w3.org/2002/07/owl#FunctionalProperty"/>
        <rdfs:domain rdf:resource="http://www.semanticweb.org/marthinust/ontologies/2022/8/Gait_Ontology#Gait-related_Disease"/>
        <rdfs:range rdf:resource="http://www.semanticweb.org/marthinust/ontologies/2022/8/Gait_Ontology#Gait_patient"/>
        <rdfs:comment xml:lang="en">Gait-related disease that isAssociatedTo the Gait patient.</rdfs:comment>
        <rdfs:label xml:lang="en">isAssociatedTo</rdfs:label>
    </owl:ObjectProperty>
    


    <!-- http://www.semanticweb.org/marthinust/ontologies/2022/8/Gait_Ontology#isBasedOn -->

    <owl:ObjectProperty rdf:about="http://www.semanticweb.org/marthinust/ontologies/2022/8/Gait_Ontology#isBasedOn">
        <rdf:type rdf:resource="http://www.w3.org/2002/07/owl#FunctionalProperty"/>
        <rdfs:domain rdf:resource="http://www.semanticweb.org/marthinust/ontologies/2022/8/Gait_Ontology#Gait_Analysis_Method"/>
        <rdfs:range rdf:resource="http://www.semanticweb.org/marthinust/ontologies/2022/8/Gait_Ontology#Gait_Analysis_Equipment"/>
        <rdfs:comment xml:lang="en">Gait Analysis Method isBasedOn Gait Analysis Equipment</rdfs:comment>
        <rdfs:label xml:lang="en">isBasedOn</rdfs:label>
    </owl:ObjectProperty>
    


    <!-- http://www.semanticweb.org/marthinust/ontologies/2022/8/Gait_Ontology#isCapturedIn -->

    <owl:ObjectProperty rdf:about="http://www.semanticweb.org/marthinust/ontologies/2022/8/Gait_Ontology#isCapturedIn">
        <rdf:type rdf:resource="http://www.w3.org/2002/07/owl#FunctionalProperty"/>
        <rdfs:domain rdf:resource="http://www.semanticweb.org/marthinust/ontologies/2022/8/Gait_Ontology#Gait-based_Process"/>
        <rdfs:range rdf:resource="http://www.semanticweb.org/marthinust/ontologies/2022/8/Gait_Ontology#Gait_Analysis_Method"/>
        <rdfs:comment xml:lang="en">Gait-based Process isCapturedIn Gait Analysis Method.</rdfs:comment>
        <rdfs:label xml:lang="en">isCapturedIn</rdfs:label>
    </owl:ObjectProperty>
    


    <!-- http://www.semanticweb.org/marthinust/ontologies/2022/8/Gait_Ontology#isCategorisedIn -->

    <owl:ObjectProperty rdf:about="http://www.semanticweb.org/marthinust/ontologies/2022/8/Gait_Ontology#isCategorisedIn">
        <rdf:type rdf:resource="http://www.w3.org/2002/07/owl#FunctionalProperty"/>
        <rdfs:domain rdf:resource="http://www.semanticweb.org/marthinust/ontologies/2022/8/Gait_Ontology#Gait_Pathology"/>
        <rdfs:range rdf:resource="http://www.semanticweb.org/marthinust/ontologies/2022/8/Gait_Ontology#Gait_Classification"/>
        <rdfs:comment xml:lang="en">Gait Pathology isCategorisedIn Gait Classification

Gait classification is a key aspect of gait pathology, as it helps to identify and understand the specific features of different gait disorders.</rdfs:comment>
        <rdfs:label xml:lang="en">isCategorisedIn</rdfs:label>
    </owl:ObjectProperty>
    


    <!-- http://www.semanticweb.org/marthinust/ontologies/2022/8/Gait_Ontology#isClassedIn -->

    <owl:ObjectProperty rdf:about="http://www.semanticweb.org/marthinust/ontologies/2022/8/Gait_Ontology#isClassedIn">
        <rdf:type rdf:resource="http://www.w3.org/2002/07/owl#FunctionalProperty"/>
        <rdfs:domain rdf:resource="http://www.semanticweb.org/marthinust/ontologies/2022/8/Gait_Ontology#Gait_patient"/>
        <rdfs:range rdf:resource="http://www.semanticweb.org/marthinust/ontologies/2022/8/Gait_Ontology#Gait_Classification"/>
        <rdfs:comment xml:lang="en">Gait patient isClassedIn Gait Classification.</rdfs:comment>
        <rdfs:label xml:lang="en">isClassedIn</rdfs:label>
    </owl:ObjectProperty>
    


    <!-- http://www.semanticweb.org/marthinust/ontologies/2022/8/Gait_Ontology#isCollectedBy -->

    <owl:ObjectProperty rdf:about="http://www.semanticweb.org/marthinust/ontologies/2022/8/Gait_Ontology#isCollectedBy">
        <rdf:type rdf:resource="http://www.w3.org/2002/07/owl#FunctionalProperty"/>
        <rdfs:domain rdf:resource="http://www.semanticweb.org/marthinust/ontologies/2022/8/Gait_Ontology#Gait_data"/>
        <rdfs:range rdf:resource="http://www.semanticweb.org/marthinust/ontologies/2022/8/Gait_Ontology#Gait_acquisition"/>
        <rdfs:comment xml:lang="en">Gait data isCollectedBy gait acquistion during sessions.</rdfs:comment>
        <rdfs:label xml:lang="en">isCollectedBy</rdfs:label>
    </owl:ObjectProperty>
    


    <!-- http://www.semanticweb.org/marthinust/ontologies/2022/8/Gait_Ontology#isDemonstratedBy -->

    <owl:ObjectProperty rdf:about="http://www.semanticweb.org/marthinust/ontologies/2022/8/Gait_Ontology#isDemonstratedBy">
        <rdf:type rdf:resource="http://www.w3.org/2002/07/owl#FunctionalProperty"/>
        <rdfs:domain rdf:resource="http://www.semanticweb.org/marthinust/ontologies/2022/8/Gait_Ontology#Gait_Cycle"/>
        <rdfs:range rdf:resource="http://www.semanticweb.org/marthinust/ontologies/2022/8/Gait_Ontology#Gait_patient"/>
        <rdfs:comment xml:lang="en">The gait cycle isDemonstratedBy the (gait) patient.</rdfs:comment>
        <rdfs:label xml:lang="en">isDemonstratedBy</rdfs:label>
    </owl:ObjectProperty>
    


    <!-- http://www.semanticweb.org/marthinust/ontologies/2022/8/Gait_Ontology#isDetectedIn -->

    <owl:ObjectProperty rdf:about="http://www.semanticweb.org/marthinust/ontologies/2022/8/Gait_Ontology#isDetectedIn">
        <rdf:type rdf:resource="http://www.w3.org/2002/07/owl#FunctionalProperty"/>
        <rdfs:domain rdf:resource="http://www.semanticweb.org/marthinust/ontologies/2022/8/Gait_Ontology#Type_of_Gait"/>
        <rdfs:range rdf:resource="http://www.semanticweb.org/marthinust/ontologies/2022/8/Gait_Ontology#Gait_Analysis_Method"/>
        <rdfs:comment xml:lang="en">The type of gait isDetectedIn the gait analysis method.</rdfs:comment>
        <rdfs:label xml:lang="en">isDetectedIn</rdfs:label>
    </owl:ObjectProperty>
    


    <!-- http://www.semanticweb.org/marthinust/ontologies/2022/8/Gait_Ontology#isDeterminedBy -->

    <owl:ObjectProperty rdf:about="http://www.semanticweb.org/marthinust/ontologies/2022/8/Gait_Ontology#isDeterminedBy">
        <rdf:type rdf:resource="http://www.w3.org/2002/07/owl#FunctionalProperty"/>
        <rdfs:domain rdf:resource="http://www.semanticweb.org/marthinust/ontologies/2022/8/Gait_Ontology#Gait_Parameter"/>
        <rdfs:range rdf:resource="http://www.semanticweb.org/marthinust/ontologies/2022/8/Gait_Ontology#Gait_Measurement_Point"/>
        <rdfs:comment xml:lang="en">Gait Parameter isDeterminedBy Gait Measurement Point.</rdfs:comment>
        <rdfs:label xml:lang="en">isDeterminedBy</rdfs:label>
    </owl:ObjectProperty>
    


    <!-- http://www.semanticweb.org/marthinust/ontologies/2022/8/Gait_Ontology#isDiagnosedBy -->

    <owl:ObjectProperty rdf:about="http://www.semanticweb.org/marthinust/ontologies/2022/8/Gait_Ontology#isDiagnosedBy">
        <rdf:type rdf:resource="http://www.w3.org/2002/07/owl#FunctionalProperty"/>
        <rdfs:domain rdf:resource="http://www.semanticweb.org/marthinust/ontologies/2022/8/Gait_Ontology#Gait_Disturbance"/>
        <rdfs:range rdf:resource="http://www.semanticweb.org/marthinust/ontologies/2022/8/Gait_Ontology#Gait_expert"/>
        <rdfs:comment xml:lang="en">Gait disturbance isDiagnosedBy a Gait expert.</rdfs:comment>
        <rdfs:label xml:lang="en">isDiagnosedBy</rdfs:label>
    </owl:ObjectProperty>
    


    <!-- http://www.semanticweb.org/marthinust/ontologies/2022/8/Gait_Ontology#isEvaluatedIn -->

    <owl:ObjectProperty rdf:about="http://www.semanticweb.org/marthinust/ontologies/2022/8/Gait_Ontology#isEvaluatedIn">
        <rdf:type rdf:resource="http://www.w3.org/2002/07/owl#FunctionalProperty"/>
        <rdfs:domain rdf:resource="http://www.semanticweb.org/marthinust/ontologies/2022/8/Gait_Ontology#Gait_Parameter"/>
        <rdfs:range rdf:resource="http://www.semanticweb.org/marthinust/ontologies/2022/8/Gait_Ontology#Gait_Cycle"/>
        <rdfs:comment xml:lang="en">Gait Parameter isEvaluatedIn the Gait Cycle.</rdfs:comment>
        <rdfs:label xml:lang="en">isEvaluatedIn</rdfs:label>
    </owl:ObjectProperty>
    


    <!-- http://www.semanticweb.org/marthinust/ontologies/2022/8/Gait_Ontology#isExhibitedBy -->

    <owl:ObjectProperty rdf:about="http://www.semanticweb.org/marthinust/ontologies/2022/8/Gait_Ontology#isExhibitedBy">
        <rdf:type rdf:resource="http://www.w3.org/2002/07/owl#FunctionalProperty"/>
        <rdfs:domain rdf:resource="http://www.semanticweb.org/marthinust/ontologies/2022/8/Gait_Ontology#Type_of_Gait"/>
        <rdfs:range rdf:resource="http://www.semanticweb.org/marthinust/ontologies/2022/8/Gait_Ontology#Gait_patient"/>
        <rdfs:comment xml:lang="en">Type of Gait isExhibitedBy a Gait patient.</rdfs:comment>
        <rdfs:label xml:lang="en">isExhibitedBy</rdfs:label>
    </owl:ObjectProperty>
    


    <!-- http://www.semanticweb.org/marthinust/ontologies/2022/8/Gait_Ontology#isFacilitatedBy -->

    <owl:ObjectProperty rdf:about="http://www.semanticweb.org/marthinust/ontologies/2022/8/Gait_Ontology#isFacilitatedBy">
        <rdf:type rdf:resource="http://www.w3.org/2002/07/owl#FunctionalProperty"/>
        <rdfs:domain rdf:resource="http://www.semanticweb.org/marthinust/ontologies/2022/8/Gait_Ontology#Gait_analysis"/>
        <rdfs:range rdf:resource="http://www.semanticweb.org/marthinust/ontologies/2022/8/Gait_Ontology#Gait_expert"/>
        <rdfs:comment xml:lang="en">Gait analysis isFacilitatedBy a (gait) expert.</rdfs:comment>
        <rdfs:label xml:lang="en">isFacilitatedBy</rdfs:label>
    </owl:ObjectProperty>
    


    <!-- http://www.semanticweb.org/marthinust/ontologies/2022/8/Gait_Ontology#isGeneratedIn -->

    <owl:ObjectProperty rdf:about="http://www.semanticweb.org/marthinust/ontologies/2022/8/Gait_Ontology#isGeneratedIn">
        <rdf:type rdf:resource="http://www.w3.org/2002/07/owl#FunctionalProperty"/>
        <rdfs:domain rdf:resource="http://www.semanticweb.org/marthinust/ontologies/2022/8/Gait_Ontology#Gait_analysis"/>
        <rdfs:range rdf:resource="http://www.semanticweb.org/marthinust/ontologies/2022/8/Gait_Ontology#Gait-based_Process"/>
        <rdfs:comment xml:lang="en">Gait Analysis isGeneratedIn the Gait-based process</rdfs:comment>
        <rdfs:label xml:lang="en">isGeneratedIn</rdfs:label>
    </owl:ObjectProperty>
    


    <!-- http://www.semanticweb.org/marthinust/ontologies/2022/8/Gait_Ontology#isIdentifiedIn -->

    <owl:ObjectProperty rdf:about="http://www.semanticweb.org/marthinust/ontologies/2022/8/Gait_Ontology#isIdentifiedIn">
        <rdf:type rdf:resource="http://www.w3.org/2002/07/owl#FunctionalProperty"/>
        <rdfs:domain rdf:resource="http://www.semanticweb.org/marthinust/ontologies/2022/8/Gait_Ontology#Gait_Classification"/>
        <rdfs:range rdf:resource="http://www.semanticweb.org/marthinust/ontologies/2022/8/Gait_Ontology#Gait_Analysis_Method"/>
        <rdfs:comment xml:lang="en">Gait Classification isIdentifiedIn Gait Analysis Method</rdfs:comment>
        <rdfs:label xml:lang="en">isIdentifiedIn</rdfs:label>
    </owl:ObjectProperty>
    


    <!-- http://www.semanticweb.org/marthinust/ontologies/2022/8/Gait_Ontology#isInfluencedBy -->

    <owl:ObjectProperty rdf:about="http://www.semanticweb.org/marthinust/ontologies/2022/8/Gait_Ontology#isInfluencedBy">
        <rdf:type rdf:resource="http://www.w3.org/2002/07/owl#FunctionalProperty"/>
        <rdfs:domain rdf:resource="http://www.semanticweb.org/marthinust/ontologies/2022/8/Gait_Ontology#Type_of_Gait"/>
        <rdfs:range rdf:resource="http://www.semanticweb.org/marthinust/ontologies/2022/8/Gait_Ontology#Gait-related_Disease"/>
        <rdfs:comment xml:lang="en">The type of gait exhibited isInfluencedBy a gait-related disease.</rdfs:comment>
        <rdfs:label xml:lang="en">isInfluencedBy</rdfs:label>
    </owl:ObjectProperty>
    


    <!-- http://www.semanticweb.org/marthinust/ontologies/2022/8/Gait_Ontology#isInvolvedIn -->

    <owl:ObjectProperty rdf:about="http://www.semanticweb.org/marthinust/ontologies/2022/8/Gait_Ontology#isInvolvedIn">
        <rdf:type rdf:resource="http://www.w3.org/2002/07/owl#FunctionalProperty"/>
        <rdfs:domain rdf:resource="http://www.semanticweb.org/marthinust/ontologies/2022/8/Gait_Ontology#Gait_patient"/>
        <rdfs:range rdf:resource="http://www.semanticweb.org/marthinust/ontologies/2022/8/Gait_Ontology#Gait_acquisition"/>
        <rdfs:comment xml:lang="en">A gait patient isInvolvedIn the gait acquisition session</rdfs:comment>
        <rdfs:label xml:lang="en">isInvolvedIn</rdfs:label>
    </owl:ObjectProperty>
    


    <!-- http://www.semanticweb.org/marthinust/ontologies/2022/8/Gait_Ontology#isLinkedTo -->

    <owl:ObjectProperty rdf:about="http://www.semanticweb.org/marthinust/ontologies/2022/8/Gait_Ontology#isLinkedTo">
        <owl:inverseOf rdf:resource="http://www.semanticweb.org/marthinust/ontologies/2022/8/Gait_Ontology#isMonitoredBy"/>
        <rdf:type rdf:resource="http://www.w3.org/2002/07/owl#FunctionalProperty"/>
        <rdfs:domain rdf:resource="http://www.semanticweb.org/marthinust/ontologies/2022/8/Gait_Ontology#Gait_Analysis_Equipment"/>
        <rdfs:range rdf:resource="http://www.semanticweb.org/marthinust/ontologies/2022/8/Gait_Ontology#Gait_patient"/>
        <rdfs:comment xml:lang="en">Gait analysis equipment what isLinkedTo the (gait) patient</rdfs:comment>
        <rdfs:label xml:lang="en">isLinkedTo</rdfs:label>
    </owl:ObjectProperty>
    


    <!-- http://www.semanticweb.org/marthinust/ontologies/2022/8/Gait_Ontology#isLinkedWith -->

    <owl:ObjectProperty rdf:about="http://www.semanticweb.org/marthinust/ontologies/2022/8/Gait_Ontology#isLinkedWith">
        <rdf:type rdf:resource="http://www.w3.org/2002/07/owl#InverseFunctionalProperty"/>
        <rdfs:domain rdf:resource="http://www.semanticweb.org/marthinust/ontologies/2022/8/Gait_Ontology#Gait_patient"/>
        <rdfs:range rdf:resource="http://www.semanticweb.org/marthinust/ontologies/2022/8/Gait_Ontology#Gait-related_Disease"/>
        <rdfs:comment xml:lang="en">A gait patient isLinkedWith a (possible) gait-related disease.</rdfs:comment>
    </owl:ObjectProperty>
    


    <!-- http://www.semanticweb.org/marthinust/ontologies/2022/8/Gait_Ontology#isMilderThan -->

    <owl:ObjectProperty rdf:about="http://www.semanticweb.org/marthinust/ontologies/2022/8/Gait_Ontology#isMilderThan">
        <owl:inverseOf rdf:resource="http://www.semanticweb.org/marthinust/ontologies/2022/8/Gait_Ontology#isSevereThan"/>
        <rdfs:domain rdf:resource="http://www.semanticweb.org/marthinust/ontologies/2022/8/Gait_Ontology#Severity_Scale"/>
        <rdfs:range rdf:resource="http://www.semanticweb.org/marthinust/ontologies/2022/8/Gait_Ontology#Severity_Scale"/>
        <rdfs:comment xml:lang="en">The severity scale of the morbidity condition</rdfs:comment>
        <rdfs:label xml:lang="en">isMilderThan</rdfs:label>
    </owl:ObjectProperty>
    


    <!-- http://www.semanticweb.org/marthinust/ontologies/2022/8/Gait_Ontology#isMonitoredBy -->

    <owl:ObjectProperty rdf:about="http://www.semanticweb.org/marthinust/ontologies/2022/8/Gait_Ontology#isMonitoredBy">
        <rdf:type rdf:resource="http://www.w3.org/2002/07/owl#InverseFunctionalProperty"/>
        <rdfs:domain rdf:resource="http://www.semanticweb.org/marthinust/ontologies/2022/8/Gait_Ontology#Gait_patient"/>
        <rdfs:range rdf:resource="http://www.semanticweb.org/marthinust/ontologies/2022/8/Gait_Ontology#Gait_Analysis_Equipment"/>
        <rdfs:comment xml:lang="en">The patient isMonitoredBy gait analysis equipment</rdfs:comment>
        <rdfs:label xml:lang="en">isMonitoredBy</rdfs:label>
    </owl:ObjectProperty>
    


    <!-- http://www.semanticweb.org/marthinust/ontologies/2022/8/Gait_Ontology#isObservedBy -->

    <owl:ObjectProperty rdf:about="http://www.semanticweb.org/marthinust/ontologies/2022/8/Gait_Ontology#isObservedBy">
        <owl:inverseOf rdf:resource="http://www.semanticweb.org/marthinust/ontologies/2022/8/Gait_Ontology#observes"/>
        <rdf:type rdf:resource="http://www.w3.org/2002/07/owl#FunctionalProperty"/>
        <rdfs:domain rdf:resource="http://www.semanticweb.org/marthinust/ontologies/2022/8/Gait_Ontology#Gait_Cycle"/>
        <rdfs:range rdf:resource="http://www.semanticweb.org/marthinust/ontologies/2022/8/Gait_Ontology#Gait_expert"/>
        <rdfs:comment xml:lang="en">The gait cycle isObservedBy the gait expert</rdfs:comment>
        <rdfs:label xml:lang="en">isObservedBy</rdfs:label>
    </owl:ObjectProperty>
    


    <!-- http://www.semanticweb.org/marthinust/ontologies/2022/8/Gait_Ontology#isObservedIn -->

    <owl:ObjectProperty rdf:about="http://www.semanticweb.org/marthinust/ontologies/2022/8/Gait_Ontology#isObservedIn">
        <rdf:type rdf:resource="http://www.w3.org/2002/07/owl#FunctionalProperty"/>
        <rdfs:domain rdf:resource="http://www.semanticweb.org/marthinust/ontologies/2022/8/Gait_Ontology#Gait_Cycle"/>
        <rdfs:range rdf:resource="http://www.semanticweb.org/marthinust/ontologies/2022/8/Gait_Ontology#Gait-based_Process"/>
        <rdfs:comment xml:lang="en">Gait cycle pattern isObservedIn gait-based process</rdfs:comment>
        <rdfs:label xml:lang="en">isObservedIn</rdfs:label>
    </owl:ObjectProperty>
    


    <!-- http://www.semanticweb.org/marthinust/ontologies/2022/8/Gait_Ontology#isObtainedBy -->

    <owl:ObjectProperty rdf:about="http://www.semanticweb.org/marthinust/ontologies/2022/8/Gait_Ontology#isObtainedBy">
        <rdf:type rdf:resource="http://www.w3.org/2002/07/owl#FunctionalProperty"/>
        <rdfs:domain rdf:resource="http://www.semanticweb.org/marthinust/ontologies/2022/8/Gait_Ontology#Gait_data"/>
        <rdfs:range rdf:resource="http://www.semanticweb.org/marthinust/ontologies/2022/8/Gait_Ontology#Gait_Analysis_Equipment"/>
        <rdfs:comment xml:lang="en">Gait Data isObtainedBy Gait Analysis Equipment</rdfs:comment>
        <rdfs:label xml:lang="en">isObtainedBy</rdfs:label>
    </owl:ObjectProperty>
    


    <!-- http://www.semanticweb.org/marthinust/ontologies/2022/8/Gait_Ontology#isOlderThan -->

    <owl:ObjectProperty rdf:about="http://www.semanticweb.org/marthinust/ontologies/2022/8/Gait_Ontology#isOlderThan">
        <owl:inverseOf rdf:resource="http://www.semanticweb.org/marthinust/ontologies/2022/8/Gait_Ontology#isYoungerThan"/>
        <rdf:type rdf:resource="http://www.w3.org/2002/07/owl#TransitiveProperty"/>
        <rdfs:domain rdf:resource="http://www.semanticweb.org/marthinust/ontologies/2022/8/Gait_Ontology#Gait_patient"/>
        <rdfs:range rdf:resource="http://www.semanticweb.org/marthinust/ontologies/2022/8/Gait_Ontology#Gait_patient"/>
        <rdfs:label xml:lang="en">isOlderThan</rdfs:label>
    </owl:ObjectProperty>
    


    <!-- http://www.semanticweb.org/marthinust/ontologies/2022/8/Gait_Ontology#isPartOf -->

    <owl:ObjectProperty rdf:about="http://www.semanticweb.org/marthinust/ontologies/2022/8/Gait_Ontology#isPartOf">
        <rdf:type rdf:resource="http://www.w3.org/2002/07/owl#FunctionalProperty"/>
        <rdfs:domain rdf:resource="http://www.semanticweb.org/marthinust/ontologies/2022/8/Gait_Ontology#Gait_acquisition"/>
        <rdfs:range rdf:resource="http://www.semanticweb.org/marthinust/ontologies/2022/8/Gait_Ontology#Gait_analysis"/>
        <rdfs:comment xml:lang="en">Gait acquisition session isPartOf gait analysis.</rdfs:comment>
        <rdfs:label xml:lang="en">isPartOf</rdfs:label>
    </owl:ObjectProperty>
    


    <!-- http://www.semanticweb.org/marthinust/ontologies/2022/8/Gait_Ontology#isPrescribedBy -->

    <owl:ObjectProperty rdf:about="http://www.semanticweb.org/marthinust/ontologies/2022/8/Gait_Ontology#isPrescribedBy">
        <owl:inverseOf rdf:resource="http://www.semanticweb.org/marthinust/ontologies/2022/8/Gait_Ontology#prescribes"/>
        <rdf:type rdf:resource="http://www.w3.org/2002/07/owl#FunctionalProperty"/>
        <rdfs:domain rdf:resource="http://www.semanticweb.org/marthinust/ontologies/2022/8/Gait_Ontology#Gait_Assistive_Technology"/>
        <rdfs:range rdf:resource="http://www.semanticweb.org/marthinust/ontologies/2022/8/Gait_Ontology#Gait_expert"/>
        <rdfs:comment xml:lang="en">Gait assistive device solution isPrescribedBy the Gait expert</rdfs:comment>
        <rdfs:label xml:lang="en">isPrescribedBy</rdfs:label>
    </owl:ObjectProperty>
    


    <!-- http://www.semanticweb.org/marthinust/ontologies/2022/8/Gait_Ontology#isRecommendedTo -->

    <owl:ObjectProperty rdf:about="http://www.semanticweb.org/marthinust/ontologies/2022/8/Gait_Ontology#isRecommendedTo">
        <rdf:type rdf:resource="http://www.w3.org/2002/07/owl#FunctionalProperty"/>
        <rdfs:domain rdf:resource="http://www.semanticweb.org/marthinust/ontologies/2022/8/Gait_Ontology#Gait_Assistive_Technology"/>
        <rdfs:range rdf:resource="http://www.semanticweb.org/marthinust/ontologies/2022/8/Gait_Ontology#Gait_patient"/>
        <rdfs:comment xml:lang="en">Gait assistive devices are designed to help people with gait disorders or other mobility impairments to walk more easily and safely. The affected person is the individual who is using the gait assistive device to improve their mobility. The object property between these two concepts is that the gait assistive device is a tool or device that is used by the patient to improve their gait. This relationship is often described as a &quot;tool-user&quot; relationship, in which the gait assistive device is the tool and the affected person is the user of the tool.</rdfs:comment>
        <rdfs:label xml:lang="en">isRecommendedTo</rdfs:label>
    </owl:ObjectProperty>
    


    <!-- http://www.semanticweb.org/marthinust/ontologies/2022/8/Gait_Ontology#isRelatedTo -->

    <owl:ObjectProperty rdf:about="http://www.semanticweb.org/marthinust/ontologies/2022/8/Gait_Ontology#isRelatedTo">
        <rdf:type rdf:resource="http://www.w3.org/2002/07/owl#FunctionalProperty"/>
        <rdfs:domain rdf:resource="http://www.semanticweb.org/marthinust/ontologies/2022/8/Gait_Ontology#Type_of_Gait"/>
        <rdfs:range rdf:resource="http://www.semanticweb.org/marthinust/ontologies/2022/8/Gait_Ontology#Gait_Disturbance"/>
        <rdfs:comment xml:lang="en">Type of gait isRelatedTo the Gait disturbance diagnosed.</rdfs:comment>
        <rdfs:label xml:lang="en">isRelatedTo</rdfs:label>
    </owl:ObjectProperty>
    


    <!-- http://www.semanticweb.org/marthinust/ontologies/2022/8/Gait_Ontology#isSevereThan -->

    <owl:ObjectProperty rdf:about="http://www.semanticweb.org/marthinust/ontologies/2022/8/Gait_Ontology#isSevereThan">
        <rdf:type rdf:resource="http://www.w3.org/2002/07/owl#TransitiveProperty"/>
        <rdfs:domain rdf:resource="http://www.semanticweb.org/marthinust/ontologies/2022/8/Gait_Ontology#Severity_Scale"/>
        <rdfs:range rdf:resource="http://www.semanticweb.org/marthinust/ontologies/2022/8/Gait_Ontology#Severity_Scale"/>
        <rdfs:comment xml:lang="en">The severity scale of the morbidity condition.</rdfs:comment>
        <rdfs:label xml:lang="en">isSevereThan</rdfs:label>
    </owl:ObjectProperty>
    


    <!-- http://www.semanticweb.org/marthinust/ontologies/2022/8/Gait_Ontology#isTreatedBy -->

    <owl:ObjectProperty rdf:about="http://www.semanticweb.org/marthinust/ontologies/2022/8/Gait_Ontology#isTreatedBy">
        <owl:inverseOf rdf:resource="http://www.semanticweb.org/marthinust/ontologies/2022/8/Gait_Ontology#treats"/>
        <rdf:type rdf:resource="http://www.w3.org/2002/07/owl#FunctionalProperty"/>
        <rdfs:domain rdf:resource="http://www.semanticweb.org/marthinust/ontologies/2022/8/Gait_Ontology#Gait_patient"/>
        <rdfs:range rdf:resource="http://www.semanticweb.org/marthinust/ontologies/2022/8/Gait_Ontology#Gait_expert"/>
        <rdfs:comment xml:lang="en">A Gait patient isTreatedBy a Gait expert</rdfs:comment>
        <rdfs:label xml:lang="en">isTreatedBy</rdfs:label>
    </owl:ObjectProperty>
    


    <!-- http://www.semanticweb.org/marthinust/ontologies/2022/8/Gait_Ontology#isUsedFor -->

    <owl:ObjectProperty rdf:about="http://www.semanticweb.org/marthinust/ontologies/2022/8/Gait_Ontology#isUsedFor">
        <rdf:type rdf:resource="http://www.w3.org/2002/07/owl#TransitiveProperty"/>
        <rdfs:domain rdf:resource="http://www.semanticweb.org/marthinust/ontologies/2022/8/Gait_Ontology#Gait_Analysis_Equipment"/>
        <rdfs:range rdf:resource="http://www.semanticweb.org/marthinust/ontologies/2022/8/Gait_Ontology#Gait-based_Process"/>
        <rdfs:comment xml:lang="en">Gait analysis equipment isUsedFor gait-based process</rdfs:comment>
        <rdfs:label xml:lang="en">isUsedFor</rdfs:label>
    </owl:ObjectProperty>
    


    <!-- http://www.semanticweb.org/marthinust/ontologies/2022/8/Gait_Ontology#isUsedIn -->

    <owl:ObjectProperty rdf:about="http://www.semanticweb.org/marthinust/ontologies/2022/8/Gait_Ontology#isUsedIn">
        <rdf:type rdf:resource="http://www.w3.org/2002/07/owl#TransitiveProperty"/>
        <rdfs:domain rdf:resource="http://www.semanticweb.org/marthinust/ontologies/2022/8/Gait_Ontology#Gait_Analysis_Equipment"/>
        <rdfs:range rdf:resource="http://www.semanticweb.org/marthinust/ontologies/2022/8/Gait_Ontology#Gait_Analysis_Method"/>
        <rdfs:comment xml:lang="en">Gait analysis equipment isUsedIn the gait analysis method</rdfs:comment>
        <rdfs:label xml:lang="en">isUsedIn</rdfs:label>
    </owl:ObjectProperty>
    


    <!-- http://www.semanticweb.org/marthinust/ontologies/2022/8/Gait_Ontology#isVerifiedBy -->

    <owl:ObjectProperty rdf:about="http://www.semanticweb.org/marthinust/ontologies/2022/8/Gait_Ontology#isVerifiedBy">
        <rdf:type rdf:resource="http://www.w3.org/2002/07/owl#FunctionalProperty"/>
        <rdfs:domain rdf:resource="http://www.semanticweb.org/marthinust/ontologies/2022/8/Gait_Ontology#Gait_Disturbance"/>
        <rdfs:range rdf:resource="http://www.semanticweb.org/marthinust/ontologies/2022/8/Gait_Ontology#Gait_Analysis_Equipment"/>
        <rdfs:comment xml:lang="en">Gait disturbance isVerifiedBy gait analysis equipment</rdfs:comment>
        <rdfs:label xml:lang="en">isVerifiedBy</rdfs:label>
    </owl:ObjectProperty>
    


    <!-- http://www.semanticweb.org/marthinust/ontologies/2022/8/Gait_Ontology#isYoungerThan -->

    <owl:ObjectProperty rdf:about="http://www.semanticweb.org/marthinust/ontologies/2022/8/Gait_Ontology#isYoungerThan">
        <rdfs:domain rdf:resource="http://www.semanticweb.org/marthinust/ontologies/2022/8/Gait_Ontology#Gait_patient"/>
        <rdfs:range rdf:resource="http://www.semanticweb.org/marthinust/ontologies/2022/8/Gait_Ontology#Gait_patient"/>
        <rdfs:label xml:lang="en">isYoungerThan</rdfs:label>
    </owl:ObjectProperty>
    


    <!-- http://www.semanticweb.org/marthinust/ontologies/2022/8/Gait_Ontology#observes -->

    <owl:ObjectProperty rdf:about="http://www.semanticweb.org/marthinust/ontologies/2022/8/Gait_Ontology#observes">
        <rdf:type rdf:resource="http://www.w3.org/2002/07/owl#InverseFunctionalProperty"/>
        <rdfs:domain rdf:resource="http://www.semanticweb.org/marthinust/ontologies/2022/8/Gait_Ontology#Gait_expert"/>
        <rdfs:range rdf:resource="http://www.semanticweb.org/marthinust/ontologies/2022/8/Gait_Ontology#Gait_Cycle"/>
        <rdfs:comment xml:lang="en">The gait expert observes the gait cycle (stage)</rdfs:comment>
        <rdfs:label xml:lang="en">observes</rdfs:label>
    </owl:ObjectProperty>
    


    <!-- http://www.semanticweb.org/marthinust/ontologies/2022/8/Gait_Ontology#prescribes -->

    <owl:ObjectProperty rdf:about="http://www.semanticweb.org/marthinust/ontologies/2022/8/Gait_Ontology#prescribes">
        <rdf:type rdf:resource="http://www.w3.org/2002/07/owl#InverseFunctionalProperty"/>
        <rdfs:domain rdf:resource="http://www.semanticweb.org/marthinust/ontologies/2022/8/Gait_Ontology#Gait_expert"/>
        <rdfs:range rdf:resource="http://www.semanticweb.org/marthinust/ontologies/2022/8/Gait_Ontology#Gait_Assistive_Technology"/>
        <rdfs:comment xml:lang="en">Gait expert presribes gait assistive device solution</rdfs:comment>
        <rdfs:label xml:lang="en">prescribes</rdfs:label>
    </owl:ObjectProperty>
    


    <!-- http://www.semanticweb.org/marthinust/ontologies/2022/8/Gait_Ontology#treats -->

    <owl:ObjectProperty rdf:about="http://www.semanticweb.org/marthinust/ontologies/2022/8/Gait_Ontology#treats">
        <rdf:type rdf:resource="http://www.w3.org/2002/07/owl#InverseFunctionalProperty"/>
        <rdfs:domain rdf:resource="http://www.semanticweb.org/marthinust/ontologies/2022/8/Gait_Ontology#Gait_expert"/>
        <rdfs:range rdf:resource="http://www.semanticweb.org/marthinust/ontologies/2022/8/Gait_Ontology#Gait_patient"/>
        <rdfs:comment xml:lang="en">The gait expert treats a gait patient</rdfs:comment>
        <rdfs:label xml:lang="en">treats</rdfs:label>
    </owl:ObjectProperty>
    


    <!-- 
    ///////////////////////////////////////////////////////////////////////////////////////
    //
    // Data properties
    //
    ///////////////////////////////////////////////////////////////////////////////////////
     -->

    


    <!-- http://www.semanticweb.org/marthinust/ontologies/2022/8/Gait_Ontology#hasAffected_leg_side -->

    <owl:DatatypeProperty rdf:about="http://www.semanticweb.org/marthinust/ontologies/2022/8/Gait_Ontology#hasAffected_leg_side">
        <rdfs:domain rdf:resource="http://www.semanticweb.org/marthinust/ontologies/2022/8/Gait_Ontology#Gait_patient"/>
        <rdfs:range rdf:resource="http://www.w3.org/2001/XMLSchema#string"/>
        <rdfs:comment xml:lang="en">The affected side(s) of the body or leg that exhibits improper gait (Left, Right, Both or None).</rdfs:comment>
        <rdfs:label xml:lang="en">hasAffected_leg_side</rdfs:label>
    </owl:DatatypeProperty>
    


    <!-- http://www.semanticweb.org/marthinust/ontologies/2022/8/Gait_Ontology#hasAge_in_years -->

    <owl:DatatypeProperty rdf:about="http://www.semanticweb.org/marthinust/ontologies/2022/8/Gait_Ontology#hasAge_in_years">
        <rdfs:domain rdf:resource="http://www.semanticweb.org/marthinust/ontologies/2022/8/Gait_Ontology#Gait_Person"/>
        <rdfs:range rdf:resource="http://www.w3.org/2001/XMLSchema#integer"/>
        <rdfs:comment xml:lang="en">The length of time that a person has lived or a thing has existed.</rdfs:comment>
        <rdfs:label xml:lang="en">hasAge_in_years</rdfs:label>
    </owl:DatatypeProperty>
    


    <!-- http://www.semanticweb.org/marthinust/ontologies/2022/8/Gait_Ontology#hasAge_range -->

    <owl:DatatypeProperty rdf:about="http://www.semanticweb.org/marthinust/ontologies/2022/8/Gait_Ontology#hasAge_range">
        <rdfs:domain rdf:resource="http://www.semanticweb.org/marthinust/ontologies/2022/8/Gait_Ontology#Gait_patient"/>
        <rdfs:range rdf:resource="http://www.w3.org/2001/XMLSchema#string"/>
        <rdfs:comment xml:lang="en">The age group range where a Person slots in.</rdfs:comment>
        <rdfs:label xml:lang="en">hasAge_range</rdfs:label>
    </owl:DatatypeProperty>
    


    <!-- http://www.semanticweb.org/marthinust/ontologies/2022/8/Gait_Ontology#hasAnalysis_method -->

    <owl:DatatypeProperty rdf:about="http://www.semanticweb.org/marthinust/ontologies/2022/8/Gait_Ontology#hasAnalysis_method">
        <rdfs:domain rdf:resource="http://www.semanticweb.org/marthinust/ontologies/2022/8/Gait_Ontology#Gait_Analysis_Method"/>
        <rdfs:range rdf:resource="http://www.w3.org/2001/XMLSchema#string"/>
        <rdfs:comment xml:lang="en">Gait Analysis Method(s) is of great importance for the collection and correlation of valid (gait) data. These methods are used in recognition and analysis of the human gait from different approaches.</rdfs:comment>
        <rdfs:label xml:lang="en">hasAnalysis_method</rdfs:label>
    </owl:DatatypeProperty>
    


    <!-- http://www.semanticweb.org/marthinust/ontologies/2022/8/Gait_Ontology#hasClinical_term -->

    <owl:DatatypeProperty rdf:about="http://www.semanticweb.org/marthinust/ontologies/2022/8/Gait_Ontology#hasClinical_term">
        <rdfs:domain rdf:resource="http://www.semanticweb.org/marthinust/ontologies/2022/8/Gait_Ontology#Gait_Disturbance"/>
        <rdfs:range rdf:resource="http://www.w3.org/2001/XMLSchema#string"/>
        <rdfs:comment xml:lang="en">Gait Disturbance terminology can be determined through the clinical presentation, laboratory work and diagnostic testing.</rdfs:comment>
        <rdfs:label xml:lang="en">hasClinical_term</rdfs:label>
    </owl:DatatypeProperty>
    


    <!-- http://www.semanticweb.org/marthinust/ontologies/2022/8/Gait_Ontology#hasDisease_description -->

    <owl:DatatypeProperty rdf:about="http://www.semanticweb.org/marthinust/ontologies/2022/8/Gait_Ontology#hasDisease_description">
        <rdfs:domain rdf:resource="http://www.semanticweb.org/marthinust/ontologies/2022/8/Gait_Ontology#Gait-related_Disease"/>
        <rdfs:range rdf:resource="http://www.w3.org/2001/XMLSchema#string"/>
        <rdfs:comment xml:lang="en">Gait-related diseases can be differentiated and identified by the indicative symptom(s) and name.</rdfs:comment>
        <rdfs:label xml:lang="en">hasDisease_description</rdfs:label>
    </owl:DatatypeProperty>
    


    <!-- http://www.semanticweb.org/marthinust/ontologies/2022/8/Gait_Ontology#hasEquipment_type -->

    <owl:DatatypeProperty rdf:about="http://www.semanticweb.org/marthinust/ontologies/2022/8/Gait_Ontology#hasEquipment_type">
        <rdfs:domain rdf:resource="http://www.semanticweb.org/marthinust/ontologies/2022/8/Gait_Ontology#Gait_Analysis_Equipment"/>
        <rdfs:range rdf:resource="http://www.w3.org/2001/XMLSchema#string"/>
        <rdfs:comment xml:lang="en">The type of Gait Analysis equipment that is being used to collect gait data.</rdfs:comment>
        <rdfs:label xml:lang="en">hasEquipment_type</rdfs:label>
    </owl:DatatypeProperty>
    


    <!-- http://www.semanticweb.org/marthinust/ontologies/2022/8/Gait_Ontology#hasGait-based_process -->

    <owl:DatatypeProperty rdf:about="http://www.semanticweb.org/marthinust/ontologies/2022/8/Gait_Ontology#hasGait-based_process">
        <rdfs:domain rdf:resource="http://www.semanticweb.org/marthinust/ontologies/2022/8/Gait_Ontology#Gait-based_Process"/>
        <rdfs:range rdf:resource="http://www.w3.org/2001/XMLSchema#string"/>
        <rdfs:comment xml:lang="en">The Gait-based process will serve a purpose either in the Acquisition, (of) the gait Data, which then can be useful for Analysis in the gait Assessment by the domain Expert.</rdfs:comment>
        <rdfs:label xml:lang="en">hasGait-based_process</rdfs:label>
    </owl:DatatypeProperty>
    


    <!-- http://www.semanticweb.org/marthinust/ontologies/2022/8/Gait_Ontology#hasGait_acquisition -->

    <owl:DatatypeProperty rdf:about="http://www.semanticweb.org/marthinust/ontologies/2022/8/Gait_Ontology#hasGait_acquisition">
        <rdfs:subPropertyOf rdf:resource="http://www.semanticweb.org/marthinust/ontologies/2022/8/Gait_Ontology#hasGait-based_process"/>
        <rdfs:domain rdf:resource="http://www.semanticweb.org/marthinust/ontologies/2022/8/Gait_Ontology#Gait_acquisition"/>
        <rdfs:range rdf:resource="http://www.w3.org/2001/XMLSchema#string"/>
        <rdfs:comment xml:lang="en">Gait acquisition is the process of collecting and analyzing data on an individual&apos;s gait, or the way in which they walk.

Gait (data) acquisition is the process where a patient&apos;s gait assessment  or measurements are obtained in acquisition sessions and observations for quantitative recording and functional description.</rdfs:comment>
        <rdfs:label xml:lang="en">hasGait_acquisition</rdfs:label>
    </owl:DatatypeProperty>
    


    <!-- http://www.semanticweb.org/marthinust/ontologies/2022/8/Gait_Ontology#hasGait_analysis -->

    <owl:DatatypeProperty rdf:about="http://www.semanticweb.org/marthinust/ontologies/2022/8/Gait_Ontology#hasGait_analysis">
        <rdfs:subPropertyOf rdf:resource="http://www.semanticweb.org/marthinust/ontologies/2022/8/Gait_Ontology#hasGait-based_process"/>
        <rdfs:domain rdf:resource="http://www.semanticweb.org/marthinust/ontologies/2022/8/Gait_Ontology#Gait_analysis"/>
        <rdfs:range rdf:resource="http://www.w3.org/2001/XMLSchema#string"/>
        <rdfs:comment xml:lang="en">The term &quot;gait analysis&quot; encompasses a broad spectrum of potential assessment strategies used to evaluate normal and abnormal gait, both walking and running. Such assessments range from simple observation to sophisticated computer analysis of biomechanics. 

Gait analysis, though sometimes performed through simple observation, can now be performed with the help of advanced technology. By analysing the data provided by several devices, the patient&apos;s gait can be evaluated in terms of step length, stride length, cadence, cycle time and joint angles. 

Reasons for Gait Analysis:

Gait abnormalities involve unusual walking patterns that may be caused by disease or injury. Such irregularities can lead to pain in the hips, back, neck, feet, knees or ankles. Gait analysis, also known as walking or motion analysis, is a comprehensive evaluation of the way an individual stands and walks.</rdfs:comment>
        <rdfs:label xml:lang="en">hasGait_analysis</rdfs:label>
    </owl:DatatypeProperty>
    


    <!-- http://www.semanticweb.org/marthinust/ontologies/2022/8/Gait_Ontology#hasGait_assistive_solution -->

    <owl:DatatypeProperty rdf:about="http://www.semanticweb.org/marthinust/ontologies/2022/8/Gait_Ontology#hasGait_assistive_solution">
        <rdfs:domain rdf:resource="http://www.semanticweb.org/marthinust/ontologies/2022/8/Gait_Ontology#Gait_Assistive_Technology"/>
        <rdfs:range rdf:resource="http://www.w3.org/2001/XMLSchema#string"/>
        <rdfs:comment xml:lang="en">The type of assistive device recommendation such as; a walker, cane, exoskeleton, etc.</rdfs:comment>
        <rdfs:label xml:lang="en">hasGait_assistive_solution</rdfs:label>
    </owl:DatatypeProperty>
    


    <!-- http://www.semanticweb.org/marthinust/ontologies/2022/8/Gait_Ontology#hasGait_classification -->

    <owl:DatatypeProperty rdf:about="http://www.semanticweb.org/marthinust/ontologies/2022/8/Gait_Ontology#hasGait_classification">
        <rdfs:domain rdf:resource="http://www.semanticweb.org/marthinust/ontologies/2022/8/Gait_Ontology#Gait_Classification"/>
        <rdfs:range rdf:resource="http://www.w3.org/2001/XMLSchema#string"/>
        <rdfs:comment xml:lang="en">Gait classification allocates walking patterns into groups that can be identified and differentiated from one another.</rdfs:comment>
        <rdfs:label xml:lang="en">hasGait_classification</rdfs:label>
    </owl:DatatypeProperty>
    


    <!-- http://www.semanticweb.org/marthinust/ontologies/2022/8/Gait_Ontology#hasGait_data -->

    <owl:DatatypeProperty rdf:about="http://www.semanticweb.org/marthinust/ontologies/2022/8/Gait_Ontology#hasGait_data">
        <rdfs:subPropertyOf rdf:resource="http://www.semanticweb.org/marthinust/ontologies/2022/8/Gait_Ontology#hasGait-based_process"/>
        <rdfs:domain rdf:resource="http://www.semanticweb.org/marthinust/ontologies/2022/8/Gait_Ontology#Gait_data"/>
        <rdfs:range rdf:resource="http://www.w3.org/2001/XMLSchema#string"/>
        <rdfs:comment xml:lang="en">The collection of dynamical data during human walking has a long history beginning with the first motion pictures and now with modern marker(s) based motion capture techniques, wearable sensors, and high fidelity ground reaction load measurements. This data can likely be useful for validating or generating mathematical models that are capable of simulating normal periodic gait and non-periodic, perturbed gaits that results in clinical gait data for analysis.

Gait data is often used to evaluate various aspects of gait, such as efficiency, symmetry, and stability. It can also be used to diagnose and treat gait abnormalities, to evaluate the effectiveness of interventions such as orthotic devices or physical therapy, and to assess the impact of aging or diseases on gait. Gait data can be collected and analyzed both in the laboratory and in more naturalistic environments, such as the individual&apos;s home or community.</rdfs:comment>
        <rdfs:label xml:lang="en">hasGait_data</rdfs:label>
    </owl:DatatypeProperty>
    


    <!-- http://www.semanticweb.org/marthinust/ontologies/2022/8/Gait_Ontology#hasGait_expert -->

    <owl:DatatypeProperty rdf:about="http://www.semanticweb.org/marthinust/ontologies/2022/8/Gait_Ontology#hasGait_expert">
        <rdfs:domain rdf:resource="http://www.semanticweb.org/marthinust/ontologies/2022/8/Gait_Ontology#Gait_expert"/>
        <rdfs:range rdf:resource="http://www.w3.org/2001/XMLSchema#string"/>
        <rdfs:comment xml:lang="en">The occupational title of the gait (analysis) expert.</rdfs:comment>
        <rdfs:label xml:lang="en">hasGait_Expert</rdfs:label>
    </owl:DatatypeProperty>
    


    <!-- http://www.semanticweb.org/marthinust/ontologies/2022/8/Gait_Ontology#hasGait_phase_cycle -->

    <owl:DatatypeProperty rdf:about="http://www.semanticweb.org/marthinust/ontologies/2022/8/Gait_Ontology#hasGait_phase_cycle">
        <rdfs:domain rdf:resource="http://www.semanticweb.org/marthinust/ontologies/2022/8/Gait_Ontology#Gait_Cycle"/>
        <rdfs:range rdf:resource="http://www.w3.org/2001/XMLSchema#string"/>
        <rdfs:comment xml:lang="en">The Gait cycle is divided into gait phases/stages such as; stance, stride or swing</rdfs:comment>
        <rdfs:label xml:lang="en">hasGait_phase_cycle</rdfs:label>
    </owl:DatatypeProperty>
    


    <!-- http://www.semanticweb.org/marthinust/ontologies/2022/8/Gait_Ontology#hasGait_type -->

    <owl:DatatypeProperty rdf:about="http://www.semanticweb.org/marthinust/ontologies/2022/8/Gait_Ontology#hasGait_type">
        <rdfs:domain rdf:resource="http://www.semanticweb.org/marthinust/ontologies/2022/8/Gait_Ontology#Type_of_Gait"/>
        <rdfs:range rdf:resource="http://www.w3.org/2001/XMLSchema#string"/>
        <rdfs:comment xml:lang="en">Abnormal gait is categorised in different types of gait, based on the appearance of an individual&apos;s walk through assessment and observation.</rdfs:comment>
        <rdfs:label xml:lang="en">hasGait_type</rdfs:label>
    </owl:DatatypeProperty>
    


    <!-- http://www.semanticweb.org/marthinust/ontologies/2022/8/Gait_Ontology#hasGender -->

    <owl:DatatypeProperty rdf:about="http://www.semanticweb.org/marthinust/ontologies/2022/8/Gait_Ontology#hasGender">
        <rdfs:domain rdf:resource="http://www.semanticweb.org/marthinust/ontologies/2022/8/Gait_Ontology#Gait_Person"/>
        <rdfs:range rdf:resource="http://www.w3.org/2001/XMLSchema#string"/>
        <rdfs:comment xml:lang="en">A person entity&apos;s gender idenity (male, female, neutral, other, transgendered, etc.)</rdfs:comment>
        <rdfs:label xml:lang="en">hasGender</rdfs:label>
    </owl:DatatypeProperty>
    


    <!-- http://www.semanticweb.org/marthinust/ontologies/2022/8/Gait_Ontology#hasHeight_in_meters -->

    <owl:DatatypeProperty rdf:about="http://www.semanticweb.org/marthinust/ontologies/2022/8/Gait_Ontology#hasHeight_in_meters">
        <rdfs:domain rdf:resource="http://www.semanticweb.org/marthinust/ontologies/2022/8/Gait_Ontology#Gait_patient"/>
        <rdfs:range rdf:resource="http://www.w3.org/2001/XMLSchema#double"/>
        <rdfs:comment xml:lang="en">Body height of the affected person in centimeters.</rdfs:comment>
        <rdfs:label xml:lang="en">hasHeight_in_meters</rdfs:label>
    </owl:DatatypeProperty>
    


    <!-- http://www.semanticweb.org/marthinust/ontologies/2022/8/Gait_Ontology#hasMeasurement -->

    <owl:DatatypeProperty rdf:about="http://www.semanticweb.org/marthinust/ontologies/2022/8/Gait_Ontology#hasMeasurement">
        <rdfs:domain rdf:resource="http://www.semanticweb.org/marthinust/ontologies/2022/8/Gait_Ontology#Gait_Measurement_Point"/>
        <rdfs:range rdf:resource="http://www.w3.org/2001/XMLSchema#string"/>
        <rdfs:comment xml:lang="en">Observing the length of the stride, arm movement, heel placement and angle of the pelvis and foot.</rdfs:comment>
        <rdfs:label xml:lang="en">hasMeasurement</rdfs:label>
    </owl:DatatypeProperty>
    


    <!-- http://www.semanticweb.org/marthinust/ontologies/2022/8/Gait_Ontology#hasParameter -->

    <owl:DatatypeProperty rdf:about="http://www.semanticweb.org/marthinust/ontologies/2022/8/Gait_Ontology#hasParameter">
        <rdfs:domain rdf:resource="http://www.semanticweb.org/marthinust/ontologies/2022/8/Gait_Ontology#Gait_Parameter"/>
        <rdfs:range rdf:resource="http://www.w3.org/2001/XMLSchema#string"/>
        <rdfs:comment xml:lang="en">Parameters of gait include velocity, step length, swing and stance phase, double support time, ground reaction forces, impulse, and propulsion during habitual walking.

An objective approach is quantitative and parameters like time, distance, and muscle activity will be measured.</rdfs:comment>
        <rdfs:label xml:lang="en">hasParameter</rdfs:label>
    </owl:DatatypeProperty>
    


    <!-- http://www.semanticweb.org/marthinust/ontologies/2022/8/Gait_Ontology#hasPathology_trait -->

    <owl:DatatypeProperty rdf:about="http://www.semanticweb.org/marthinust/ontologies/2022/8/Gait_Ontology#hasPathology_trait">
        <rdfs:domain rdf:resource="http://www.semanticweb.org/marthinust/ontologies/2022/8/Gait_Ontology#Gait_Pathology"/>
        <rdfs:range rdf:resource="http://www.w3.org/2001/XMLSchema#string"/>
        <rdfs:comment xml:lang="en">The term &quot;gait pathologies&quot; refers to abnormalities or disorders that affect the way a person walks. These abnormalities can be caused by a wide range of factors, including neurological conditions, musculoskeletal disorders, injuries and age-related deterioration that are mainly divided into Pathological gait and Geriatric (Old Age) gait.</rdfs:comment>
        <rdfs:label xml:lang="en">hasPathology_trait</rdfs:label>
    </owl:DatatypeProperty>
    


    <!-- http://www.semanticweb.org/marthinust/ontologies/2022/8/Gait_Ontology#hasType_of_material -->

    <owl:DatatypeProperty rdf:about="http://www.semanticweb.org/marthinust/ontologies/2022/8/Gait_Ontology#hasType_of_material">
        <rdfs:subPropertyOf rdf:resource="http://www.semanticweb.org/marthinust/ontologies/2022/8/Gait_Ontology#hasGait_assistive_solution"/>
        <rdfs:domain rdf:resource="http://www.semanticweb.org/marthinust/ontologies/2022/8/Gait_Ontology#Gait_Assistive_Technology"/>
        <rdfs:range rdf:resource="http://www.w3.org/2001/XMLSchema#string"/>
        <rdfs:comment xml:lang="en">The materials used to construct the device, such as metal, plastic, rubber, wooden, or composite materials.</rdfs:comment>
        <rdfs:label xml:lang="en">hasType_of_material</rdfs:label>
    </owl:DatatypeProperty>
    


    <!-- http://www.semanticweb.org/marthinust/ontologies/2022/8/Gait_Ontology#hasWeight_in_kilograms -->

    <owl:DatatypeProperty rdf:about="http://www.semanticweb.org/marthinust/ontologies/2022/8/Gait_Ontology#hasWeight_in_kilograms">
        <rdfs:domain rdf:resource="http://www.semanticweb.org/marthinust/ontologies/2022/8/Gait_Ontology#Gait_patient"/>
        <rdfs:range rdf:resource="http://www.w3.org/2001/XMLSchema#double"/>
        <rdfs:comment xml:lang="en">Body weight of the affected person in kilograms</rdfs:comment>
        <rdfs:label xml:lang="en">hasWeight_in_kilograms</rdfs:label>
    </owl:DatatypeProperty>
    


    <!-- 
    ///////////////////////////////////////////////////////////////////////////////////////
    //
    // Classes
    //
    ///////////////////////////////////////////////////////////////////////////////////////
     -->

    


    <!-- http://www.semanticweb.org/marthinust/ontologies/2022/8/Gait_Ontology#AI-based -->

    <owl:Class rdf:about="http://www.semanticweb.org/marthinust/ontologies/2022/8/Gait_Ontology#AI-based">
        <rdfs:subClassOf rdf:resource="http://www.semanticweb.org/marthinust/ontologies/2022/8/Gait_Ontology#Gait_Analysis_Method"/>
        <opla-sd:entityPosition>
            <rdf:Description>
                <opla-sd:entityPositionX rdf:datatype="http://www.w3.org/2001/XMLSchema#double">61.479471062365235</opla-sd:entityPositionX>
                <opla-sd:entityPositionY rdf:datatype="http://www.w3.org/2001/XMLSchema#double">9.623284013264444</opla-sd:entityPositionY>
                <rdfs:comment xml:lang="en">This is an entity positioning annotation generated by CoModIDE (https://comodide.com/). Removing this annotation will break rendering the CoModIDE schema diagram view.</rdfs:comment>
            </rdf:Description>
        </opla-sd:entityPosition>
        <rdfs:comment xml:lang="en">AI algorithms, particularly machine learning and deep learning techniques, can be used to analyse and interpret data collected by gait analysis equipment, such as motion capture systems, force plates, and wearable sensors.

These AI algorithms can help in identifying and quantifying gait abnormalities, predicting the risk of falls or injuries, assessing the effectiveness of interventions, and even diagnosing specific movement disorders. AI-based gait analysis methods can improve the accuracy, efficiency, and clinical applicability of gait analysis by automating data processing, reducing human error, and providing insights that may not be easily discernible by human observers.

AI serves as a method or tool in gait analysis, enhancing the process by analysing and interpreting data generated by gait analysis equipment.</rdfs:comment>
        <rdfs:label xml:lang="en">AI-based</rdfs:label>
    </owl:Class>
    


    <!-- http://www.semanticweb.org/marthinust/ontologies/2022/8/Gait_Ontology#Abasia -->

    <owl:Class rdf:about="http://www.semanticweb.org/marthinust/ontologies/2022/8/Gait_Ontology#Abasia">
        <rdfs:subClassOf rdf:resource="http://www.semanticweb.org/marthinust/ontologies/2022/8/Gait_Ontology#Gait_ataxia"/>
        <opla-sd:entityPosition>
            <rdf:Description>
                <opla-sd:entityPositionX rdf:datatype="http://www.w3.org/2001/XMLSchema#double">234.60114521227146</opla-sd:entityPositionX>
                <opla-sd:entityPositionY rdf:datatype="http://www.w3.org/2001/XMLSchema#double">241.23282067829135</opla-sd:entityPositionY>
                <rdfs:comment xml:lang="en">This is an entity positioning annotation generated by CoModIDE (https://comodide.com/). Removing this annotation will break rendering the CoModIDE schema diagram view.</rdfs:comment>
            </rdf:Description>
        </opla-sd:entityPosition>
        <rdfs:comment>A severe form of gait ataxia such that an affected person cannot walk at all.</rdfs:comment>
        <rdfs:label xml:lang="en">Abasia</rdfs:label>
    </owl:Class>
    


    <!-- http://www.semanticweb.org/marthinust/ontologies/2022/8/Gait_Ontology#Accelerometer -->

    <owl:Class rdf:about="http://www.semanticweb.org/marthinust/ontologies/2022/8/Gait_Ontology#Accelerometer">
        <rdfs:subClassOf rdf:resource="http://www.semanticweb.org/marthinust/ontologies/2022/8/Gait_Ontology#Gait_Analysis_Equipment"/>
        <opla-sd:entityPosition>
            <rdf:Description>
                <opla-sd:entityPositionX rdf:datatype="http://www.w3.org/2001/XMLSchema#double">200.54761386010549</opla-sd:entityPositionX>
                <opla-sd:entityPositionY rdf:datatype="http://www.w3.org/2001/XMLSchema#double">83.1733017848135</opla-sd:entityPositionY>
                <rdfs:comment xml:lang="en">This is an entity positioning annotation generated by CoModIDE (https://comodide.com/). Removing this annotation will break rendering the CoModIDE schema diagram view.</rdfs:comment>
            </rdf:Description>
        </opla-sd:entityPosition>
        <rdfs:comment>An accelerometer is a type of inertial sensor that can measure acceleration along its sensitive axis. The common operation principle of accelerometers is based on a mechanical sensing element that comprises a proof mass attached to a mechanical suspension system, with respect to a reference frame. The mass proof can be forced to deflect by the inertial force because of acceleration or gravity according to Newtons second Law (force = mass  acceleration). Based on this principle, the acceleration can be measured electrically using the physical changes in the displacement of the proof mass, with respect to the reference frame.

Three common types of accelerometers are available, namely, piezoelectric, piezoresistive, and capacitive accelerometers. Piezoresistive and capacitive accelerometers can provide dual acceleration components and have higher stability. Thus, these types of accelerometers are suitable for measuring the motion status in the human gait. By attaching these accelerometers to the feet or legs, the acceleration/velocity of the feet or legs in the gait can be determined to perform the gait analysis.</rdfs:comment>
        <rdfs:label xml:lang="en">Accelerometer</rdfs:label>
    </owl:Class>
    


    <!-- http://www.semanticweb.org/marthinust/ontologies/2022/8/Gait_Ontology#Active_body_marker -->

    <owl:Class rdf:about="http://www.semanticweb.org/marthinust/ontologies/2022/8/Gait_Ontology#Active_body_marker">
        <rdfs:subClassOf rdf:resource="http://www.semanticweb.org/marthinust/ontologies/2022/8/Gait_Ontology#Gait_Analysis_Equipment"/>
        <opla-sd:entityPosition>
            <rdf:Description>
                <opla-sd:entityPositionX rdf:datatype="http://www.w3.org/2001/XMLSchema#double">256.88478492895496</opla-sd:entityPositionX>
                <opla-sd:entityPositionY rdf:datatype="http://www.w3.org/2001/XMLSchema#double">297.74033038168284</opla-sd:entityPositionY>
                <rdfs:comment xml:lang="en">This is an entity positioning annotation generated by CoModIDE (https://comodide.com/). Removing this annotation will break rendering the CoModIDE schema diagram view.</rdfs:comment>
            </rdf:Description>
        </opla-sd:entityPosition>
        <rdfs:comment>Active marker systems are similar to the passive marker system but use &quot;active&quot; markers. These markers are triggered by the incoming infra red signal and respond by sending out a corresponding signal of their own. This signal is then used to triangulate the location of the marker. The advantage of this system over the passive one is that individual markers work at predefined frequencies and therefore, have their own &quot;identity&quot;. This means that no post-processing of marker locations is required, however the systems tend to be less forgiving for out-of-view markers than the passive systems.

Therefore, a typical modern gait lab has several cameras (video or infra-red) placed around a walkway or treadmill, which are linked to a computer. The patient has markers applied to anatomical landmark points, which are mostly palpable bony landmarks such as the iliac spines of the pelvis, the malleoli of the ankle, and the condyles of the knee. The patient walks down the walkway or on the treadmill and the computer calculates the trajectory of each marker in three dimensions. A model is applied to compute the underlying motion of the bones. This gives a full breakdown of the motion at each joint.</rdfs:comment>
        <rdfs:label xml:lang="en">Active_body_marker</rdfs:label>
    </owl:Class>
    


    <!-- http://www.semanticweb.org/marthinust/ontologies/2022/8/Gait_Ontology#Actuator -->

    <owl:Class rdf:about="http://www.semanticweb.org/marthinust/ontologies/2022/8/Gait_Ontology#Actuator">
        <rdfs:subClassOf rdf:resource="http://www.semanticweb.org/marthinust/ontologies/2022/8/Gait_Ontology#Gait_Assistive_Technology"/>
        <opla-sd:entityPosition>
            <rdf:Description>
                <opla-sd:entityPositionX rdf:datatype="http://www.w3.org/2001/XMLSchema#double">295.21430828528537</opla-sd:entityPositionX>
                <opla-sd:entityPositionY rdf:datatype="http://www.w3.org/2001/XMLSchema#double">76.31463603473146</opla-sd:entityPositionY>
                <rdfs:comment xml:lang="en">This is an entity positioning annotation generated by CoModIDE (https://comodide.com/). Removing this annotation will break rendering the CoModIDE schema diagram view.</rdfs:comment>
            </rdf:Description>
        </opla-sd:entityPosition>
        <rdfs:comment>An actuator is a component of a machine that is responsible for moving and controlling a mechanism or system. An actuator is a device that produces a motion by converting energy and signals going into the system. The motion it produces can be either rotary or linear. In human gait the joint, muscle and ligament can be acutated by an actuator performing muscuskeletal functions.</rdfs:comment>
        <rdfs:label xml:lang="en">Actuator</rdfs:label>
    </owl:Class>
    


    <!-- http://www.semanticweb.org/marthinust/ontologies/2022/8/Gait_Ontology#Amputation -->

    <owl:Class rdf:about="http://www.semanticweb.org/marthinust/ontologies/2022/8/Gait_Ontology#Amputation">
        <rdfs:subClassOf rdf:resource="http://www.semanticweb.org/marthinust/ontologies/2022/8/Gait_Ontology#Disability"/>
        <opla-sd:entityPosition>
            <rdf:Description>
                <opla-sd:entityPositionX rdf:datatype="http://www.w3.org/2001/XMLSchema#double">234.2239766241546</opla-sd:entityPositionX>
                <opla-sd:entityPositionY rdf:datatype="http://www.w3.org/2001/XMLSchema#double">281.14641941759476</opla-sd:entityPositionY>
                <rdfs:comment xml:lang="en">This is an entity positioning annotation generated by CoModIDE (https://comodide.com/). Removing this annotation will break rendering the CoModIDE schema diagram view.</rdfs:comment>
            </rdf:Description>
        </opla-sd:entityPosition>
        <rdfs:comment xml:lang="en">There are a number of different causes of amputation in older adults, but the most common causes are peripheral artery disease (PAD) and diabetes.

Peripheral artery disease (PAD) is a condition in which the blood vessels in the legs become narrowed or blocked due to the buildup of plaque. This can lead to reduced blood flow to the legs, which can cause pain, cramping, and weakness in the legs. In severe cases, PAD can lead to the formation of sores or ulcers on the legs, and if these do not heal, amputation may be necessary.

Diabetes is another major cause of amputation in older adults. Diabetes can cause damage to the blood vessels and nerves in the legs, which can lead to poor circulation and a reduced ability to feel pain or other sensations in the feet. This can increase the risk of developing sores or ulcers on the feet, which can lead to infection if not properly treated. In some cases, amputation may be necessary to prevent the spread of infection or to prevent further damage to the leg or foot.

Amputation is the loss or removal of a body part such as a finger, toe, hand, foot, arm or leg. Amputation is the removal of a limb by trauma, medical illness, or surgery. As a surgical measure, it is used to control pain or a disease process in the affected limb, such as malignancy or gangrene. In some cases, it is carried out on individuals as a preventive surgery for such problems (usually) during old age.</rdfs:comment>
        <rdfs:label xml:lang="en">Amputation</rdfs:label>
    </owl:Class>
    


    <!-- http://www.semanticweb.org/marthinust/ontologies/2022/8/Gait_Ontology#Ankle -->

    <owl:Class rdf:about="http://www.semanticweb.org/marthinust/ontologies/2022/8/Gait_Ontology#Ankle">
        <rdfs:subClassOf rdf:resource="http://www.semanticweb.org/marthinust/ontologies/2022/8/Gait_Ontology#Musculoskeletal"/>
        <opla-sd:entityPosition>
            <rdf:Description>
                <opla-sd:entityPositionX rdf:datatype="http://www.w3.org/2001/XMLSchema#double">57.54930038443083</opla-sd:entityPositionX>
                <opla-sd:entityPositionY rdf:datatype="http://www.w3.org/2001/XMLSchema#double">233.17670089932093</opla-sd:entityPositionY>
                <rdfs:comment xml:lang="en">This is an entity positioning annotation generated by CoModIDE (https://comodide.com/). Removing this annotation will break rendering the CoModIDE schema diagram view.</rdfs:comment>
            </rdf:Description>
        </opla-sd:entityPosition>
        <rdfs:comment xml:lang="en">The ankle region is found at the junction of the leg and the foot. It extends downwards (distally) from the narrowest point of the lower leg and includes the parts of the foot closer to the body (proximal) to the heel and upper surface (dorsum) of the foot.

The ankle, or the talocrural region, or the jumping bone (informal) is the area where the foot and the leg meet. The ankle includes three joints: the ankle joint proper or talocrural joint, the subtalar joint, and the inferior tibiofibular joint.

The ankle is a large joint made up of three bones: The shin bone (tibia) The thinner bone running next to the shin bone (fibula) A foot bone that sits above the heel bone (talus).</rdfs:comment>
        <rdfs:label xml:lang="en">Ankle</rdfs:label>
    </owl:Class>
    


    <!-- http://www.semanticweb.org/marthinust/ontologies/2022/8/Gait_Ontology#Ankle_dorsiflexion_weakness -->

    <owl:Class rdf:about="http://www.semanticweb.org/marthinust/ontologies/2022/8/Gait_Ontology#Ankle_dorsiflexion_weakness">
        <rdfs:subClassOf rdf:resource="http://www.semanticweb.org/marthinust/ontologies/2022/8/Gait_Ontology#Ankle"/>
        <opla-sd:entityPosition>
            <rdf:Description>
                <opla-sd:entityPositionX rdf:datatype="http://www.w3.org/2001/XMLSchema#double">35.2226838472805</opla-sd:entityPositionX>
                <opla-sd:entityPositionY rdf:datatype="http://www.w3.org/2001/XMLSchema#double">285.41694761099416</opla-sd:entityPositionY>
                <rdfs:comment xml:lang="en">This is an entity positioning annotation generated by CoModIDE (https://comodide.com/). Removing this annotation will break rendering the CoModIDE schema diagram view.</rdfs:comment>
            </rdf:Description>
        </opla-sd:entityPosition>
        <rdfs:comment xml:lang="en">Ankle dorsiflexion weakness (Steppage gait and foot slap)
Pathomechanism: When there is severe weakness, the initial contact with the ground is made by the forefoot followed by the heel region. Mild weakness, the initial contact is made with the heel followed by a rapid ankle plantar flexion, causing a foot slap During the swing phase, toes may drag/catch. Compensatory is steppage gait with excessive hip and knee flexion or body shift to clear foot.

Ankle Dorsiflexion Weakness results in a lack of heel strike and decreased floor clearance. This leads to an increased step height and prolonged swing phase.</rdfs:comment>
        <rdfs:label xml:lang="en">Ankle_dorsiflexion_weakness</rdfs:label>
    </owl:Class>
    


    <!-- http://www.semanticweb.org/marthinust/ontologies/2022/8/Gait_Ontology#Ankle_plantor_flexor_weakness -->

    <owl:Class rdf:about="http://www.semanticweb.org/marthinust/ontologies/2022/8/Gait_Ontology#Ankle_plantor_flexor_weakness">
        <rdfs:subClassOf rdf:resource="http://www.semanticweb.org/marthinust/ontologies/2022/8/Gait_Ontology#Ankle"/>
        <opla-sd:entityPosition>
            <rdf:Description>
                <opla-sd:entityPositionX rdf:datatype="http://www.w3.org/2001/XMLSchema#double">165.42218795122298</opla-sd:entityPositionX>
                <opla-sd:entityPositionY rdf:datatype="http://www.w3.org/2001/XMLSchema#double">168.29750493687706</opla-sd:entityPositionY>
                <rdfs:comment xml:lang="en">This is an entity positioning annotation generated by CoModIDE (https://comodide.com/). Removing this annotation will break rendering the CoModIDE schema diagram view.</rdfs:comment>
            </rdf:Description>
        </opla-sd:entityPosition>
        <rdfs:comment xml:lang="en">Ankle Plantar Flexor Weakness (Calcaneal gait):
Pathomechanism: Heel remains in contact with the ground late in terminal stance. Lack of eccentric contraction of ankle plantar flexor causes GRF to pass behind knee, creating knee flexion moment with excess tibial motion over ankle during mid to late stance. Increased quadriceps contraction needed to prevent knee buckling. Contralateral leg step length (swing duration) reduced by unstable stance of affected limb. Heel off delayed and push off phase decreased.</rdfs:comment>
        <rdfs:label xml:lang="en">Ankle_plantor_flexor_weakness</rdfs:label>
    </owl:Class>
    


    <!-- http://www.semanticweb.org/marthinust/ontologies/2022/8/Gait_Ontology#Antalgic_gait -->

    <owl:Class rdf:about="http://www.semanticweb.org/marthinust/ontologies/2022/8/Gait_Ontology#Antalgic_gait">
        <rdfs:subClassOf rdf:resource="http://www.semanticweb.org/marthinust/ontologies/2022/8/Gait_Ontology#Gait_Disturbance"/>
        <opla-sd:entityPosition>
            <rdf:Description>
                <opla-sd:entityPositionX rdf:datatype="http://www.w3.org/2001/XMLSchema#double">94.10569091200283</opla-sd:entityPositionX>
                <opla-sd:entityPositionY rdf:datatype="http://www.w3.org/2001/XMLSchema#double">166.42493571821655</opla-sd:entityPositionY>
                <rdfs:comment xml:lang="en">This is an entity positioning annotation generated by CoModIDE (https://comodide.com/). Removing this annotation will break rendering the CoModIDE schema diagram view.</rdfs:comment>
            </rdf:Description>
        </opla-sd:entityPosition>
        <rdfs:comment>The patient appears to be walking as if there was a thorn in the sole of the foot. This is to avoid pain so the weight is put on the affected leg for as short a time as possible, resulting in a limp.</rdfs:comment>
        <rdfs:label xml:lang="en">Antalgic_gait</rdfs:label>
    </owl:Class>
    


    <!-- http://www.semanticweb.org/marthinust/ontologies/2022/8/Gait_Ontology#Apraxia -->

    <owl:Class rdf:about="http://www.semanticweb.org/marthinust/ontologies/2022/8/Gait_Ontology#Apraxia">
        <rdfs:subClassOf rdf:resource="http://www.semanticweb.org/marthinust/ontologies/2022/8/Gait_Ontology#Gait-related_Disease"/>
        <opla-sd:entityPosition>
            <rdf:Description>
                <opla-sd:entityPositionX rdf:datatype="http://www.w3.org/2001/XMLSchema#double">61.23889450859601</opla-sd:entityPositionX>
                <opla-sd:entityPositionY rdf:datatype="http://www.w3.org/2001/XMLSchema#double">239.21695067090178</opla-sd:entityPositionY>
                <rdfs:comment xml:lang="en">This is an entity positioning annotation generated by CoModIDE (https://comodide.com/). Removing this annotation will break rendering the CoModIDE schema diagram view.</rdfs:comment>
            </rdf:Description>
        </opla-sd:entityPosition>
        <rdfs:comment xml:lang="en">Apraxia is caused by a defect in the brain pathways that contain memory of learned patterns of movement. The lesion may be the result of certain metabolic, neurological or other disorders that involve the brain, particularly the frontal lobe (inferior parietal lobule) of the left hemisphere of the brain.

Difficulty with skilled movements even when a person has the ability and desire to do them. Apraxia is caused by brain disease or damage. The brain is unable to make and deliver correct movement instructions to the body. One type of apraxia affects speech. The brain struggles with lip, jaw and tongue movements. Other types affect the accuracy of limb movements, response to verbal commands and facial movements, such as winking.</rdfs:comment>
        <rdfs:label xml:lang="en">Apraxia</rdfs:label>
    </owl:Class>
    


    <!-- http://www.semanticweb.org/marthinust/ontologies/2022/8/Gait_Ontology#Arthritis -->

    <owl:Class rdf:about="http://www.semanticweb.org/marthinust/ontologies/2022/8/Gait_Ontology#Arthritis">
        <rdfs:subClassOf rdf:resource="http://www.semanticweb.org/marthinust/ontologies/2022/8/Gait_Ontology#Gait-related_Disease"/>
        <rdfs:subClassOf rdf:resource="http://www.semanticweb.org/marthinust/ontologies/2022/8/Gait_Ontology#Musculoskeletal"/>
        <opla-sd:entityPosition>
            <rdf:Description>
                <opla-sd:entityPositionX rdf:datatype="http://www.w3.org/2001/XMLSchema#double">136.15907496744524</opla-sd:entityPositionX>
                <opla-sd:entityPositionY rdf:datatype="http://www.w3.org/2001/XMLSchema#double">70.74951297573875</opla-sd:entityPositionY>
                <rdfs:comment xml:lang="en">This is an entity positioning annotation generated by CoModIDE (https://comodide.com/). Removing this annotation will break rendering the CoModIDE schema diagram view.</rdfs:comment>
            </rdf:Description>
        </opla-sd:entityPosition>
        <rdfs:comment xml:lang="en">Arthritis isnt a single disease; the term refers to joint pain or joint disease. People of all ages, races and sexes live with arthritis, and it is the leading cause of disability. Its most common among women, and although its not a disease of aging, some types of arthritis occur in older people more than younger people. Common arthritis symptoms include swelling, pain, stiffness and diminished range of motion in joints. Symptoms vary from mild to severe and may come and go. Some may stay about the same for years, but symptoms can also progress and get worse over time. Severe arthritis can result in chronic pain, difficulty performing daily activities and make walking and climbing stairs painful and grueling.

Arthritis is the swelling and tenderness of one or more joints. The main symptoms of arthritis are joint pain and stiffness, which typically worsen with age. The most common types of arthritis are osteoarthritis and rheumatoid arthritis.</rdfs:comment>
        <rdfs:label xml:lang="en">Arthritis</rdfs:label>
    </owl:Class>
    


    <!-- http://www.semanticweb.org/marthinust/ontologies/2022/8/Gait_Ontology#Ataxia -->

    <owl:Class rdf:about="http://www.semanticweb.org/marthinust/ontologies/2022/8/Gait_Ontology#Ataxia">
        <rdfs:subClassOf rdf:resource="http://www.semanticweb.org/marthinust/ontologies/2022/8/Gait_Ontology#Cerebellar_disease"/>
    </owl:Class>
    


    <!-- http://www.semanticweb.org/marthinust/ontologies/2022/8/Gait_Ontology#Ataxic_gait -->

    <owl:Class rdf:about="http://www.semanticweb.org/marthinust/ontologies/2022/8/Gait_Ontology#Ataxic_gait">
        <rdfs:subClassOf rdf:resource="http://www.semanticweb.org/marthinust/ontologies/2022/8/Gait_Ontology#Type_of_Gait"/>
    </owl:Class>
    


    <!-- http://www.semanticweb.org/marthinust/ontologies/2022/8/Gait_Ontology#Basal_ganglia_dysfunction -->

    <owl:Class rdf:about="http://www.semanticweb.org/marthinust/ontologies/2022/8/Gait_Ontology#Basal_ganglia_dysfunction">
        <rdfs:subClassOf rdf:resource="http://www.semanticweb.org/marthinust/ontologies/2022/8/Gait_Ontology#Neurological"/>
        <opla-sd:entityPosition>
            <rdf:Description>
                <opla-sd:entityPositionX rdf:datatype="http://www.w3.org/2001/XMLSchema#double">137.65520675186175</opla-sd:entityPositionX>
                <opla-sd:entityPositionY rdf:datatype="http://www.w3.org/2001/XMLSchema#double">4.211428618094208</opla-sd:entityPositionY>
                <rdfs:comment xml:lang="en">This is an entity positioning annotation generated by CoModIDE (https://comodide.com/). Removing this annotation will break rendering the CoModIDE schema diagram view.</rdfs:comment>
            </rdf:Description>
        </opla-sd:entityPosition>
        <rdfs:comment xml:lang="en">Basal ganglia dysfunction is a disorder that affects the function of the basal ganglia, a group of structures in the brain that are involved in motor control, cognition, and behavior. Symptoms of basal ganglia dysfunction can include problems with movement, such as tremors, muscle spasms, and difficulty initiating movements; cognitive problems, such as confusion, memory problems, and trouble paying attention; and behavioral problems, such as depression, anxiety, and impulsivity. The exact cause of basal ganglia dysfunction is unknown, but it is believed to be related to abnormal brain development or damage to the basal ganglia structures. Treatment typically includes medications and physical, speech, and occupational therapies.

The basal ganglia are particularly associated with movement disorders. Associated with damage to the BG are: tremors; involuntary muscle movements; abnormal increase in tone; difficulty initiating movements; abnormal posture.

Movement disorders comprise a variety of motor problems, not all of which are associated with dysfunction of the basal ganglia. Those that have a clearly established pathological basis and are caused by pathophysiological mechanisms directly involving the basal ganglia.</rdfs:comment>
        <rdfs:label xml:lang="en">Basal_ganglia_dysfunction</rdfs:label>
    </owl:Class>
    


    <!-- http://www.semanticweb.org/marthinust/ontologies/2022/8/Gait_Ontology#Broad-based_gait -->

    <owl:Class rdf:about="http://www.semanticweb.org/marthinust/ontologies/2022/8/Gait_Ontology#Broad-based_gait">
        <rdfs:subClassOf rdf:resource="http://www.semanticweb.org/marthinust/ontologies/2022/8/Gait_Ontology#Gait_Disturbance"/>
        <owl:disjointWith rdf:resource="http://www.semanticweb.org/marthinust/ontologies/2022/8/Gait_Ontology#Cautious_gait"/>
        <opla-sd:entityPosition>
            <rdf:Description>
                <opla-sd:entityPositionX rdf:datatype="http://www.w3.org/2001/XMLSchema#double">41.510374279291284</opla-sd:entityPositionX>
                <opla-sd:entityPositionY rdf:datatype="http://www.w3.org/2001/XMLSchema#double">123.08993663488815</opla-sd:entityPositionY>
                <rdfs:comment xml:lang="en">This is an entity positioning annotation generated by CoModIDE (https://comodide.com/). Removing this annotation will break rendering the CoModIDE schema diagram view.</rdfs:comment>
            </rdf:Description>
        </opla-sd:entityPosition>
        <rdfs:comment>An abnormal gait pattern in which persons stand and walk with their feet spaced widely apart. This is often a component of cerebellar ataxia.</rdfs:comment>
        <rdfs:label xml:lang="en">Broad-based_gait</rdfs:label>
    </owl:Class>
    


    <!-- http://www.semanticweb.org/marthinust/ontologies/2022/8/Gait_Ontology#Cadence -->

    <owl:Class rdf:about="http://www.semanticweb.org/marthinust/ontologies/2022/8/Gait_Ontology#Cadence">
        <rdfs:subClassOf rdf:resource="http://www.semanticweb.org/marthinust/ontologies/2022/8/Gait_Ontology#Gait_Parameter"/>
        <opla-sd:entityPosition>
            <rdf:Description>
                <opla-sd:entityPositionX rdf:datatype="http://www.w3.org/2001/XMLSchema#double">265.08740053383457</opla-sd:entityPositionX>
                <opla-sd:entityPositionY rdf:datatype="http://www.w3.org/2001/XMLSchema#double">79.9007831496035</opla-sd:entityPositionY>
                <rdfs:comment xml:lang="en">This is an entity positioning annotation generated by CoModIDE (https://comodide.com/). Removing this annotation will break rendering the CoModIDE schema diagram view.</rdfs:comment>
            </rdf:Description>
        </opla-sd:entityPosition>
        <rdfs:comment xml:lang="en">Cadence is walking rate in steps per minute, and is related to walking speed (speed = cadence x stride length) and intensity of activity. Cadence is one measure that can be used to check that adequate activity levels in daily living are being reached, since averaged cadences throughout a day will differ from the cadence of a pure walk.</rdfs:comment>
        <rdfs:label xml:lang="en">Cadence</rdfs:label>
    </owl:Class>
    


    <!-- http://www.semanticweb.org/marthinust/ontologies/2022/8/Gait_Ontology#Calcaneal_spur -->

    <owl:Class rdf:about="http://www.semanticweb.org/marthinust/ontologies/2022/8/Gait_Ontology#Calcaneal_spur">
        <rdfs:subClassOf rdf:resource="http://www.semanticweb.org/marthinust/ontologies/2022/8/Gait_Ontology#Calcaneus/Heel_bone"/>
        <opla-sd:entityPosition>
            <rdf:Description>
                <opla-sd:entityPositionX rdf:datatype="http://www.w3.org/2001/XMLSchema#double">259.24858299792226</opla-sd:entityPositionX>
                <opla-sd:entityPositionY rdf:datatype="http://www.w3.org/2001/XMLSchema#double">23.444645857923657</opla-sd:entityPositionY>
                <rdfs:comment xml:lang="en">This is an entity positioning annotation generated by CoModIDE (https://comodide.com/). Removing this annotation will break rendering the CoModIDE schema diagram view.</rdfs:comment>
            </rdf:Description>
        </opla-sd:entityPosition>
        <rdfs:comment xml:lang="en">This is a bony growth that develops on the heel bone, often as a result of strain or overuse. It can cause pain and discomfort in the heel and surrounding areas. 

A calcaneal spur, or commonly known as a heel spur, occurs when a bony outgrowth forms on the heel bone. Calcaneal spurs can be located at the back of the heel (dorsal heel spur) or under the sole (plantar heel spur).</rdfs:comment>
        <rdfs:label xml:lang="en">Calcaneal_spur</rdfs:label>
    </owl:Class>
    


    <!-- http://www.semanticweb.org/marthinust/ontologies/2022/8/Gait_Ontology#Calcification -->

    <owl:Class rdf:about="http://www.semanticweb.org/marthinust/ontologies/2022/8/Gait_Ontology#Calcification">
        <rdfs:subClassOf rdf:resource="http://www.semanticweb.org/marthinust/ontologies/2022/8/Gait_Ontology#Geriatric_gait"/>
        <opla-sd:entityPosition>
            <rdf:Description>
                <opla-sd:entityPositionX rdf:datatype="http://www.w3.org/2001/XMLSchema#double">292.8577615195123</opla-sd:entityPositionX>
                <opla-sd:entityPositionY rdf:datatype="http://www.w3.org/2001/XMLSchema#double">222.35490290828463</opla-sd:entityPositionY>
                <rdfs:comment xml:lang="en">This is an entity positioning annotation generated by CoModIDE (https://comodide.com/). Removing this annotation will break rendering the CoModIDE schema diagram view.</rdfs:comment>
            </rdf:Description>
        </opla-sd:entityPosition>
        <rdfs:comment xml:lang="en">Calcification occurs when you have a buildup of excess calcium in your body. Calcium deposits can form all over your body, including in your soft tissues, arteries and organs. Some calcium deposits are harmless, but others can be a sign of a serious health condition.</rdfs:comment>
        <rdfs:label xml:lang="en">Calcification</rdfs:label>
    </owl:Class>
    


    <!-- http://www.semanticweb.org/marthinust/ontologies/2022/8/Gait_Ontology#Cane -->

    <owl:Class rdf:about="http://www.semanticweb.org/marthinust/ontologies/2022/8/Gait_Ontology#Cane">
        <rdfs:subClassOf rdf:resource="http://www.semanticweb.org/marthinust/ontologies/2022/8/Gait_Ontology#Gait_Assistive_Technology"/>
        <opla-sd:entityPosition>
            <rdf:Description>
                <opla-sd:entityPositionX rdf:datatype="http://www.w3.org/2001/XMLSchema#double">16.57949641493052</opla-sd:entityPositionX>
                <opla-sd:entityPositionY rdf:datatype="http://www.w3.org/2001/XMLSchema#double">41.42428192978064</opla-sd:entityPositionY>
                <rdfs:comment xml:lang="en">This is an entity positioning annotation generated by CoModIDE (https://comodide.com/). Removing this annotation will break rendering the CoModIDE schema diagram view.</rdfs:comment>
            </rdf:Description>
        </opla-sd:entityPosition>
        <rdfs:comment xml:lang="en">A cane can be helpful if you have minor problems with balance or stability, some weakness in your leg or trunk, an injury, or a pain. If you are elderly, using a single point cane may help you to walk more comfortably and safely and, in some cases, may make it easier for you to continue living independently.</rdfs:comment>
        <rdfs:label xml:lang="en">Cane</rdfs:label>
    </owl:Class>
    


    <!-- http://www.semanticweb.org/marthinust/ontologies/2022/8/Gait_Ontology#Cautious_gait -->

    <owl:Class rdf:about="http://www.semanticweb.org/marthinust/ontologies/2022/8/Gait_Ontology#Cautious_gait">
        <rdfs:subClassOf rdf:resource="http://www.semanticweb.org/marthinust/ontologies/2022/8/Gait_Ontology#Gait_Disturbance"/>
        <opla-sd:entityPosition>
            <rdf:Description>
                <opla-sd:entityPositionX rdf:datatype="http://www.w3.org/2001/XMLSchema#double">180.951407618716</opla-sd:entityPositionX>
                <opla-sd:entityPositionY rdf:datatype="http://www.w3.org/2001/XMLSchema#double">95.11987398115417</opla-sd:entityPositionY>
                <rdfs:comment xml:lang="en">This is an entity positioning annotation generated by CoModIDE (https://comodide.com/). Removing this annotation will break rendering the CoModIDE schema diagram view.</rdfs:comment>
            </rdf:Description>
        </opla-sd:entityPosition>
        <rdfs:comment>Cautious gait refers to an excessive degree of age-related changes in walking and fear of falling. The walking difficulties seem out of proportion when considering the patient&apos;s actual sensory or motor deficits. The gait appears slow, with a wider base than normal, reduced arm swing bilaterally and a slightly stooped posture. This type of gait change often occurs after the first time a patient has fallen.</rdfs:comment>
        <rdfs:label xml:lang="en">Cautious_gait</rdfs:label>
    </owl:Class>
    


    <!-- http://www.semanticweb.org/marthinust/ontologies/2022/8/Gait_Ontology#Celerbellar_ataxia_associated_with_quadrupedal_gait -->

    <owl:Class rdf:about="http://www.semanticweb.org/marthinust/ontologies/2022/8/Gait_Ontology#Celerbellar_ataxia_associated_with_quadrupedal_gait">
        <rdfs:subClassOf rdf:resource="http://www.semanticweb.org/marthinust/ontologies/2022/8/Gait_Ontology#Gait_Disturbance"/>
        <opla-sd:entityPosition>
            <rdf:Description>
                <opla-sd:entityPositionX rdf:datatype="http://www.w3.org/2001/XMLSchema#double">240.5337278429067</opla-sd:entityPositionX>
                <opla-sd:entityPositionY rdf:datatype="http://www.w3.org/2001/XMLSchema#double">35.799968073855105</opla-sd:entityPositionY>
                <rdfs:comment xml:lang="en">This is an entity positioning annotation generated by CoModIDE (https://comodide.com/). Removing this annotation will break rendering the CoModIDE schema diagram view.</rdfs:comment>
            </rdf:Description>
        </opla-sd:entityPosition>
        <rdfs:comment>The presence of cerebellar signs and symptoms such as lack of balance associated with quadrupedal gait (locomotion on all four extremities with a &apos;bear-like&apos; gait with the legs held straight).</rdfs:comment>
        <rdfs:label xml:lang="en">Celerbellar_ataxia_associated_with_quadrupedal_gait</rdfs:label>
    </owl:Class>
    


    <!-- http://www.semanticweb.org/marthinust/ontologies/2022/8/Gait_Ontology#Cerebellar_disease -->

    <owl:Class rdf:about="http://www.semanticweb.org/marthinust/ontologies/2022/8/Gait_Ontology#Cerebellar_disease">
        <rdfs:subClassOf rdf:resource="http://www.semanticweb.org/marthinust/ontologies/2022/8/Gait_Ontology#Gait-related_Disease"/>
        <opla-sd:entityPosition>
            <rdf:Description>
                <opla-sd:entityPositionX rdf:datatype="http://www.w3.org/2001/XMLSchema#double">147.33698023138703</opla-sd:entityPositionX>
                <opla-sd:entityPositionY rdf:datatype="http://www.w3.org/2001/XMLSchema#double">107.6783226579448</opla-sd:entityPositionY>
                <rdfs:comment xml:lang="en">This is an entity positioning annotation generated by CoModIDE (https://comodide.com/). Removing this annotation will break rendering the CoModIDE schema diagram view.</rdfs:comment>
            </rdf:Description>
        </opla-sd:entityPosition>
        <rdfs:comment xml:lang="en">The cerebellum maintains our motor equilibrium and calibration of movements. It is an essential region of the brain playing a central role in maintaining our gait, stance, and balance, as well as the coordination of goal-directed movements and complex movements. Dysfunction manifests as clumsiness and &quot;drunken&quot; gait.

Damage to the cerebellum can lead to: 1) loss of coordination of motor movement (asynergia), 2) the inability to judge distance and when to stop (dysmetria), 3) the inability to perform rapid alternating movements (adiadochokinesia), 4) movement tremors (intention tremor), 5) staggering, wide based walking (ataxic gait), 6) tendency toward falling, 7) weak muscles (hypotonia), 8) slurred speech (ataxic dysarthria), and 9) abnormal eye movements (nystagmus).</rdfs:comment>
        <rdfs:label xml:lang="en">Cerebellar_disease</rdfs:label>
    </owl:Class>
    


    <!-- http://www.semanticweb.org/marthinust/ontologies/2022/8/Gait_Ontology#Cerebellar_gait -->

    <owl:Class rdf:about="http://www.semanticweb.org/marthinust/ontologies/2022/8/Gait_Ontology#Cerebellar_gait">
        <rdfs:subClassOf rdf:resource="http://www.semanticweb.org/marthinust/ontologies/2022/8/Gait_Ontology#Ataxic_gait"/>
        <opla-sd:entityPosition>
            <rdf:Description>
                <opla-sd:entityPositionX rdf:datatype="http://www.w3.org/2001/XMLSchema#double">195.05484556427956</opla-sd:entityPositionX>
                <opla-sd:entityPositionY rdf:datatype="http://www.w3.org/2001/XMLSchema#double">93.50605353369673</opla-sd:entityPositionY>
                <rdfs:comment xml:lang="en">This is an entity positioning annotation generated by CoModIDE (https://comodide.com/). Removing this annotation will break rendering the CoModIDE schema diagram view.</rdfs:comment>
            </rdf:Description>
        </opla-sd:entityPosition>
        <rdfs:comment xml:lang="en">The clinical features of cerebellar ataxic gait usually include a widened base, unsteadiness and irregularity of steps, and lateral veering. Locomotion in individuals with cerebellar ataxia is characterised by a significantly reduced step frequency with a prolonged stance and double limb support duration.</rdfs:comment>
        <rdfs:label xml:lang="en">Cerebellar_gait</rdfs:label>
    </owl:Class>
    


    <!-- http://www.semanticweb.org/marthinust/ontologies/2022/8/Gait_Ontology#Cerebral_palsy -->

    <owl:Class rdf:about="http://www.semanticweb.org/marthinust/ontologies/2022/8/Gait_Ontology#Cerebral_palsy">
        <rdfs:subClassOf rdf:resource="http://www.semanticweb.org/marthinust/ontologies/2022/8/Gait_Ontology#Cerebellar_disease"/>
        <rdfs:subClassOf rdf:resource="http://www.semanticweb.org/marthinust/ontologies/2022/8/Gait_Ontology#Neuromuscular"/>
        <opla-sd:entityPosition>
            <rdf:Description>
                <opla-sd:entityPositionX rdf:datatype="http://www.w3.org/2001/XMLSchema#double">36.06645106797495</opla-sd:entityPositionX>
                <opla-sd:entityPositionY rdf:datatype="http://www.w3.org/2001/XMLSchema#double">129.66846064801004</opla-sd:entityPositionY>
                <rdfs:comment xml:lang="en">This is an entity positioning annotation generated by CoModIDE (https://comodide.com/). Removing this annotation will break rendering the CoModIDE schema diagram view.</rdfs:comment>
            </rdf:Description>
        </opla-sd:entityPosition>
        <rdfs:comment>Cerebral Palsy is considered a neurological disorder caused by a non-progressive brain injury or malformation that occurs while the childs brain is under development. Cerebral Palsy primarily affects body movement and muscle coordination. Cerebral Palsy affects body movement, muscle control, muscle coordination, muscle tone, reflex, posture and balance. It can also impact fine motor skills, gross motor skills and oral motor functioning.</rdfs:comment>
        <rdfs:comment>Cerebral palsy (CP) is a group of disorders that affect a person&apos;s ability to move and maintain balance and posture. CP is the most common motor disability in childhood. Cerebral means having to do with the brain. Palsy means weakness or problems with using the muscles.</rdfs:comment>
        <rdfs:label xml:lang="en">Cerebral_palsy</rdfs:label>
    </owl:Class>
    


    <!-- http://www.semanticweb.org/marthinust/ontologies/2022/8/Gait_Ontology#Charcot-Marie-Tooth_disease -->

    <owl:Class rdf:about="http://www.semanticweb.org/marthinust/ontologies/2022/8/Gait_Ontology#Charcot-Marie-Tooth_disease">
        <rdfs:subClassOf rdf:resource="http://www.semanticweb.org/marthinust/ontologies/2022/8/Gait_Ontology#Gait-related_Disease"/>
        <opla-sd:entityPosition>
            <rdf:Description>
                <opla-sd:entityPositionX rdf:datatype="http://www.w3.org/2001/XMLSchema#double">80.85073196946914</opla-sd:entityPositionX>
                <opla-sd:entityPositionY rdf:datatype="http://www.w3.org/2001/XMLSchema#double">122.90664350119991</opla-sd:entityPositionY>
                <rdfs:comment xml:lang="en">This is an entity positioning annotation generated by CoModIDE (https://comodide.com/). Removing this annotation will break rendering the CoModIDE schema diagram view.</rdfs:comment>
            </rdf:Description>
        </opla-sd:entityPosition>
        <rdfs:comment xml:lang="en">Charcot-Marie-Tooth disease (CMT) is one of a group of disorders that cause damage to the peripheral nervesthe nerves that transmit information and signals from the brain and spinal cord to and from the rest of the body, as well as sensory information such as touch, back to the spinal cord and brain.  CMT also can directly affect the nerves that control the muscles. 

Progressive muscle weakness typically becomes noticeable in adolescence or early adulthood, but the onset of disease can occur at any age. Because longer nerves are affected first, symptoms usually begin in the feet and lower legs and then can affect the fingers, hands, and arms. Most individuals with CMT have some amount of physical disability, although some people may never know they have the disease.

Nearly all cases are inherited. It is possible to have two or more types of CMT, which happens when the person has mutations in two or more genes, each of which causes a form of the disease. CMT is a heterogenous genetic disease, meaning mutations in different genes can produce similar clinical symptoms. CMT is named for the three physicians who described it in 1886.

Symptoms

CMT affects both sensory and motor nerves (nerves that trigger an impulse for a muscle to contract) in the arms, hands, legs, and feet. The affected nerves slowly degenerate and lose the ability to communicate with their distant targets, resulting in muscle weakness and atrophy in the arms, legs, hands, or feet.

Symptoms may include:

Weakness or paralysis of the foot and lower leg muscles, which can cause difficulty lifting the foot (foot drop)
A high-stepped gait with frequent tripping or falling
Balance problems
Foot deformities, such as high arches and curled toes (hammertoes)
Lower legs may take on an &quot;inverted champagne bottle&quot; shape due to the loss of muscle bulk
Reduced ability to feel heat, cold, and touch
Weakness and atrophy may occur in the hands, causing difficulty with fine motor skills
Decreased sense of vibration and position (proprioception)
Curvature of the spine (scoliosis)
Hip displacement
Contractures (chronic shortening of muscles or tendons around joints)
Muscle cramping
Nerve pain
Some individuals may need to rely on foot or leg braces or other orthopedic devices to maintain mobility. Some people living with CMT experience tremor, and vision and hearing can also be affected. In rare cases, breathing difficulties may occur if the nerves that control the muscles of the diaphragm are affected.</rdfs:comment>
        <rdfs:label xml:lang="en">Charcot-Marie-Tooth disease</rdfs:label>
    </owl:Class>
    


    <!-- http://www.semanticweb.org/marthinust/ontologies/2022/8/Gait_Ontology#Choreiform_gait -->

    <owl:Class rdf:about="http://www.semanticweb.org/marthinust/ontologies/2022/8/Gait_Ontology#Choreiform_gait">
        <rdfs:subClassOf rdf:resource="http://www.semanticweb.org/marthinust/ontologies/2022/8/Gait_Ontology#Type_of_Gait"/>
        <opla-sd:entityPosition>
            <rdf:Description>
                <opla-sd:entityPositionX rdf:datatype="http://www.w3.org/2001/XMLSchema#double">55.31329363873925</opla-sd:entityPositionX>
                <opla-sd:entityPositionY rdf:datatype="http://www.w3.org/2001/XMLSchema#double">296.83854035649586</opla-sd:entityPositionY>
                <rdfs:comment xml:lang="en">This is an entity positioning annotation generated by CoModIDE (https://comodide.com/). Removing this annotation will break rendering the CoModIDE schema diagram view.</rdfs:comment>
            </rdf:Description>
        </opla-sd:entityPosition>
        <rdfs:comment xml:lang="en">This gait is seen with certain basal ganglia disorders including Sydenham&apos;s chorea, Huntington&apos;s Disease and other forms of chorea, athetosis or dystonia. The patient will display irregular, jerky, involuntary movements in all extremities. Walking may accentuate their baseline movement disorder.

(Hyperkinetic Gait)</rdfs:comment>
        <rdfs:label xml:lang="en">Choreiform_gait</rdfs:label>
    </owl:Class>
    


    <!-- http://www.semanticweb.org/marthinust/ontologies/2022/8/Gait_Ontology#Clubfoot -->

    <owl:Class rdf:about="http://www.semanticweb.org/marthinust/ontologies/2022/8/Gait_Ontology#Clubfoot">
        <rdfs:subClassOf rdf:resource="http://www.semanticweb.org/marthinust/ontologies/2022/8/Gait_Ontology#Foot"/>
        <opla-sd:entityPosition>
            <rdf:Description>
                <opla-sd:entityPositionX rdf:datatype="http://www.w3.org/2001/XMLSchema#double">56.685108904468144</opla-sd:entityPositionX>
                <opla-sd:entityPositionY rdf:datatype="http://www.w3.org/2001/XMLSchema#double">57.25430495523235</opla-sd:entityPositionY>
                <rdfs:comment xml:lang="en">This is an entity positioning annotation generated by CoModIDE (https://comodide.com/). Removing this annotation will break rendering the CoModIDE schema diagram view.</rdfs:comment>
            </rdf:Description>
        </opla-sd:entityPosition>
        <rdfs:comment xml:lang="en">Clubfoot describes a range of foot abnormalities usually present at birth (congenital) in which your baby&apos;s foot is twisted out of shape or position. In clubfoot, the tissues connecting the muscles to the bone (tendons) are shorter than usual. An idiopathic clubfoot has a very high arch and turns inward toward the other leg, with the toes pointed down and backward</rdfs:comment>
        <rdfs:label xml:lang="en">Clubfoot</rdfs:label>
    </owl:Class>
    


    <!-- http://www.semanticweb.org/marthinust/ontologies/2022/8/Gait_Ontology#Cock-walk_gait -->

    <owl:Class rdf:about="http://www.semanticweb.org/marthinust/ontologies/2022/8/Gait_Ontology#Cock-walk_gait">
        <rdfs:subClassOf rdf:resource="http://www.semanticweb.org/marthinust/ontologies/2022/8/Gait_Ontology#Dystonic_gait"/>
        <opla-sd:entityPosition>
            <rdf:Description>
                <opla-sd:entityPositionX rdf:datatype="http://www.w3.org/2001/XMLSchema#double">79.4090298535581</opla-sd:entityPositionX>
                <opla-sd:entityPositionY rdf:datatype="http://www.w3.org/2001/XMLSchema#double">43.52275363930453</opla-sd:entityPositionY>
                <rdfs:comment xml:lang="en">This is an entity positioning annotation generated by CoModIDE (https://comodide.com/). Removing this annotation will break rendering the CoModIDE schema diagram view.</rdfs:comment>
            </rdf:Description>
        </opla-sd:entityPosition>
        <rdfs:comment xml:lang="en">An abnormality of gait that can be observed in individuals with dystonic posture in which the individual walks with an extended trunk and flexed arms, while strutting on the toes without the heels touching the floor.</rdfs:comment>
        <rdfs:label xml:lang="en">Cock-walk_gait</rdfs:label>
    </owl:Class>
    


    <!-- http://www.semanticweb.org/marthinust/ontologies/2022/8/Gait_Ontology#Cognitive_decline -->

    <owl:Class rdf:about="http://www.semanticweb.org/marthinust/ontologies/2022/8/Gait_Ontology#Cognitive_decline">
        <rdfs:subClassOf rdf:resource="http://www.semanticweb.org/marthinust/ontologies/2022/8/Gait_Ontology#Morbidity"/>
        <opla-sd:entityPosition>
            <rdf:Description>
                <opla-sd:entityPositionX rdf:datatype="http://www.w3.org/2001/XMLSchema#double">252.53961533587665</opla-sd:entityPositionX>
                <opla-sd:entityPositionY rdf:datatype="http://www.w3.org/2001/XMLSchema#double">165.85999904675154</opla-sd:entityPositionY>
                <rdfs:comment xml:lang="en">This is an entity positioning annotation generated by CoModIDE (https://comodide.com/). Removing this annotation will break rendering the CoModIDE schema diagram view.</rdfs:comment>
            </rdf:Description>
        </opla-sd:entityPosition>
        <rdfs:comment xml:lang="en">Cognitive decline can cause confusion, memory loss, temporary forgetfulness, and other symptoms that can affect a person&apos;s ability to walk.</rdfs:comment>
        <rdfs:label xml:lang="en">Cognitive_decline</rdfs:label>
    </owl:Class>
    


    <!-- http://www.semanticweb.org/marthinust/ontologies/2022/8/Gait_Ontology#Crouch_gait -->

    <owl:Class rdf:about="http://www.semanticweb.org/marthinust/ontologies/2022/8/Gait_Ontology#Crouch_gait">
        <rdfs:subClassOf rdf:resource="http://www.semanticweb.org/marthinust/ontologies/2022/8/Gait_Ontology#Gait_Disturbance"/>
        <opla-sd:entityPosition>
            <rdf:Description>
                <opla-sd:entityPositionX rdf:datatype="http://www.w3.org/2001/XMLSchema#double">234.1358733811486</opla-sd:entityPositionX>
                <opla-sd:entityPositionY rdf:datatype="http://www.w3.org/2001/XMLSchema#double">3.909702743057321</opla-sd:entityPositionY>
                <rdfs:comment xml:lang="en">This is an entity positioning annotation generated by CoModIDE (https://comodide.com/). Removing this annotation will break rendering the CoModIDE schema diagram view.</rdfs:comment>
            </rdf:Description>
        </opla-sd:entityPosition>
        <rdfs:comment xml:lang="en">A gait disturbance that is characterized by excessive ankle dorsiflexion, knee and hip flexion during the stance phase.</rdfs:comment>
        <rdfs:label xml:lang="en">Crouch_gait</rdfs:label>
    </owl:Class>
    


    <!-- http://www.semanticweb.org/marthinust/ontologies/2022/8/Gait_Ontology#Crutch -->

    <owl:Class rdf:about="http://www.semanticweb.org/marthinust/ontologies/2022/8/Gait_Ontology#Crutch">
        <rdfs:subClassOf rdf:resource="http://www.semanticweb.org/marthinust/ontologies/2022/8/Gait_Ontology#Gait_Assistive_Technology"/>
        <opla-sd:entityPosition>
            <rdf:Description>
                <opla-sd:entityPositionX rdf:datatype="http://www.w3.org/2001/XMLSchema#double">121.64229696422784</opla-sd:entityPositionX>
                <opla-sd:entityPositionY rdf:datatype="http://www.w3.org/2001/XMLSchema#double">188.61419686755212</opla-sd:entityPositionY>
                <rdfs:comment xml:lang="en">This is an entity positioning annotation generated by CoModIDE (https://comodide.com/). Removing this annotation will break rendering the CoModIDE schema diagram view.</rdfs:comment>
            </rdf:Description>
        </opla-sd:entityPosition>
        <rdfs:comment>Crutches provide temporary support if you&apos;re struggling to balance or need to take weight off of one, or both, of your legs. They can feel more stable and secure. Crutches are assistive devices used by patients for walking when they are not able to bear full or partial weight on an injured leg.</rdfs:comment>
        <rdfs:label xml:lang="en">Crutch</rdfs:label>
    </owl:Class>
    


    <!-- http://www.semanticweb.org/marthinust/ontologies/2022/8/Gait_Ontology#Dementia -->

    <owl:Class rdf:about="http://www.semanticweb.org/marthinust/ontologies/2022/8/Gait_Ontology#Dementia">
        <rdfs:subClassOf rdf:resource="http://www.semanticweb.org/marthinust/ontologies/2022/8/Gait_Ontology#Geriatric_gait"/>
        <opla-sd:entityPosition>
            <rdf:Description>
                <opla-sd:entityPositionX rdf:datatype="http://www.w3.org/2001/XMLSchema#double">278.46096231826334</opla-sd:entityPositionX>
                <opla-sd:entityPositionY rdf:datatype="http://www.w3.org/2001/XMLSchema#double">271.00105353237126</opla-sd:entityPositionY>
                <rdfs:comment xml:lang="en">This is an entity positioning annotation generated by CoModIDE (https://comodide.com/). Removing this annotation will break rendering the CoModIDE schema diagram view.</rdfs:comment>
            </rdf:Description>
        </opla-sd:entityPosition>
        <rdfs:comment xml:lang="en">Gait disorders are more prevalent in dementia than in normal aging and are related to the severity of cognitive decline. Dementia-related gait changes (DRGC) mainly include decrease in walking speed provoked by a decrease in stride length and an increase in support phase. 

The aging of populations worldwide with an attendant increase in geriatric syndromes such as dementias has spurred interest in developing clinical approaches to identifying cognitive decline early in order to improve management of older adults presenting with cognitive concerns. While effective dementia therapies have not yet resulted, there has been a recent explosion of knowledge regarding the nature and clinical course of dementias that has led to the identification of noncognitive markers of dementia. An extensive body of research demonstrates that gait performance is impaired early during dementia. Identifying gait markers of dementia in older individuals can be vital.

Dementia is not the same as age-related cognitive declinewhen certain areas of thinking, memory, and information processing slow with age, but intelligence remains unchanged. Unlike dementia, age-related memory loss isn&apos;t disabling. Occasional lapses of forgetfulness are normal in elderly adults. While dementia is more common with advanced age (as many as half of all people age 85 or older may have some form of dementia), it is not an inevitable part of aging. Many people live into their 90s and beyond without any signs of dementia.</rdfs:comment>
        <rdfs:label xml:lang="en">Dementia</rdfs:label>
    </owl:Class>
    


    <!-- http://www.semanticweb.org/marthinust/ontologies/2022/8/Gait_Ontology#Diabetes -->

    <owl:Class rdf:about="http://www.semanticweb.org/marthinust/ontologies/2022/8/Gait_Ontology#Diabetes">
        <rdfs:subClassOf rdf:resource="http://www.semanticweb.org/marthinust/ontologies/2022/8/Gait_Ontology#Gait-related_Disease"/>
        <rdfs:subClassOf rdf:resource="http://www.semanticweb.org/marthinust/ontologies/2022/8/Gait_Ontology#Morbidity"/>
        <opla-sd:entityPosition>
            <rdf:Description>
                <opla-sd:entityPositionX rdf:datatype="http://www.w3.org/2001/XMLSchema#double">50.76918736040968</opla-sd:entityPositionX>
                <opla-sd:entityPositionY rdf:datatype="http://www.w3.org/2001/XMLSchema#double">139.36966764810353</opla-sd:entityPositionY>
                <rdfs:comment xml:lang="en">This is an entity positioning annotation generated by CoModIDE (https://comodide.com/). Removing this annotation will break rendering the CoModIDE schema diagram view.</rdfs:comment>
            </rdf:Description>
        </opla-sd:entityPosition>
        <rdfs:comment xml:lang="en">Diabetes can cause nerve damage and other complications that can affect a person&apos;s ability to walk.</rdfs:comment>
        <rdfs:comment xml:lang="en">Diabetes mellitus refers to a group of diseases that affect how the body uses blood sugar (glucose). Glucose is an important source of energy for the cells that make up the muscles and tissues. It&apos;s also the brain&apos;s main source of fuel.

The main cause of diabetes varies by type. But no matter what type of diabetes you have, it can lead to excess sugar in the blood. Too much sugar in the blood can lead to serious health problems.</rdfs:comment>
        <rdfs:label xml:lang="en">Diabetes</rdfs:label>
    </owl:Class>
    


    <!-- http://www.semanticweb.org/marthinust/ontologies/2022/8/Gait_Ontology#Diabetic_neuropathy -->

    <owl:Class rdf:about="http://www.semanticweb.org/marthinust/ontologies/2022/8/Gait_Ontology#Diabetic_neuropathy">
        <rdfs:subClassOf rdf:resource="http://www.semanticweb.org/marthinust/ontologies/2022/8/Gait_Ontology#Diabetes"/>
        <rdfs:subClassOf rdf:resource="http://www.semanticweb.org/marthinust/ontologies/2022/8/Gait_Ontology#Neuropathy"/>
        <opla-sd:entityPosition>
            <rdf:Description>
                <opla-sd:entityPositionX rdf:datatype="http://www.w3.org/2001/XMLSchema#double">10.022375538173806</opla-sd:entityPositionX>
                <opla-sd:entityPositionY rdf:datatype="http://www.w3.org/2001/XMLSchema#double">51.97581130613299</opla-sd:entityPositionY>
                <rdfs:comment xml:lang="en">This is an entity positioning annotation generated by CoModIDE (https://comodide.com/). Removing this annotation will break rendering the CoModIDE schema diagram view.</rdfs:comment>
            </rdf:Description>
        </opla-sd:entityPosition>
        <rdfs:comment>A type of nerve damage that can occur with diabetes. The condition most often affects the legs and feet. For some people, symptoms are mild. For others, symptoms can be painful, debilitating and even fatal. Symptoms include pain and numbness in the legs. In more severe cases, symptoms include issues with digestion, the bladder and controlling heart rate. Treatment includes managing blood sugar and using medication to control symptoms.</rdfs:comment>
        <rdfs:comment xml:lang="en">Diabetic neuropathy is a type of neuropathy that is caused by diabetes. It is a complication of diabetes that occurs when high blood sugar levels damage the nerves over time. Diabetic neuropathy most commonly affects the nerves in the feet and legs, but it can also affect the nerves in the hands and arms.

Symptoms of diabetic neuropathy can vary depending on the type of neuropathy and which nerves are affected. Some common symptoms include numbness, tingling, and pain in the feet and legs; weakness; and difficulty walking.</rdfs:comment>
        <rdfs:label xml:lang="en">Diabetic_neuropathy</rdfs:label>
    </owl:Class>
    


    <!-- http://www.semanticweb.org/marthinust/ontologies/2022/8/Gait_Ontology#Difficulty_walking -->

    <owl:Class rdf:about="http://www.semanticweb.org/marthinust/ontologies/2022/8/Gait_Ontology#Difficulty_walking">
        <rdfs:subClassOf rdf:resource="http://www.semanticweb.org/marthinust/ontologies/2022/8/Gait_Ontology#Gait_Disturbance"/>
        <opla-sd:entityPosition>
            <rdf:Description>
                <opla-sd:entityPositionX rdf:datatype="http://www.w3.org/2001/XMLSchema#double">174.34668274250694</opla-sd:entityPositionX>
                <opla-sd:entityPositionY rdf:datatype="http://www.w3.org/2001/XMLSchema#double">216.53978817382333</opla-sd:entityPositionY>
                <rdfs:comment xml:lang="en">This is an entity positioning annotation generated by CoModIDE (https://comodide.com/). Removing this annotation will break rendering the CoModIDE schema diagram view.</rdfs:comment>
            </rdf:Description>
        </opla-sd:entityPosition>
        <rdfs:comment>Reduced ability to walk (ambulate). Walking disability.</rdfs:comment>
        <rdfs:label xml:lang="en">Difficulty_walking</rdfs:label>
    </owl:Class>
    


    <!-- http://www.semanticweb.org/marthinust/ontologies/2022/8/Gait_Ontology#Difficulty_walking_backward -->

    <owl:Class rdf:about="http://www.semanticweb.org/marthinust/ontologies/2022/8/Gait_Ontology#Difficulty_walking_backward">
        <rdfs:subClassOf rdf:resource="http://www.semanticweb.org/marthinust/ontologies/2022/8/Gait_Ontology#Gait_Disturbance"/>
        <opla-sd:entityPosition>
            <rdf:Description>
                <opla-sd:entityPositionX rdf:datatype="http://www.w3.org/2001/XMLSchema#double">132.24248061097418</opla-sd:entityPositionX>
                <opla-sd:entityPositionY rdf:datatype="http://www.w3.org/2001/XMLSchema#double">230.3087226962265</opla-sd:entityPositionY>
                <rdfs:comment xml:lang="en">This is an entity positioning annotation generated by CoModIDE (https://comodide.com/). Removing this annotation will break rendering the CoModIDE schema diagram view.</rdfs:comment>
            </rdf:Description>
        </opla-sd:entityPosition>
        <rdfs:comment>Reduced ability to walk (ambulate) in a backwards direction.

We walk backward on a daily basis, such as when backing away from the kitchen sink or stepping back from a curb as a swiftly moving bus passes. This task may be particularly difficult for some individuals who can fall as a result of moving or being perturbed in the backward direction. Some individuals with Parkinson disease exhibit this feature.</rdfs:comment>
        <rdfs:label xml:lang="en">Difficulty_walking_backward</rdfs:label>
    </owl:Class>
    


    <!-- http://www.semanticweb.org/marthinust/ontologies/2022/8/Gait_Ontology#Diplegic_gait -->

    <owl:Class rdf:about="http://www.semanticweb.org/marthinust/ontologies/2022/8/Gait_Ontology#Diplegic_gait">
        <rdfs:subClassOf rdf:resource="http://www.semanticweb.org/marthinust/ontologies/2022/8/Gait_Ontology#Type_of_Gait"/>
        <opla-sd:entityPosition>
            <rdf:Description>
                <opla-sd:entityPositionX rdf:datatype="http://www.w3.org/2001/XMLSchema#double">101.86608431375163</opla-sd:entityPositionX>
                <opla-sd:entityPositionY rdf:datatype="http://www.w3.org/2001/XMLSchema#double">177.73990678202117</opla-sd:entityPositionY>
                <rdfs:comment xml:lang="en">This is an entity positioning annotation generated by CoModIDE (https://comodide.com/). Removing this annotation will break rendering the CoModIDE schema diagram view.</rdfs:comment>
            </rdf:Description>
        </opla-sd:entityPosition>
        <rdfs:comment xml:lang="en">Patients have involvement on both sides with spasticity in lower extremities worse than upper extremities. The patient walks with an abnormally narrow base, dragging both legs and scraping the toes. This gait is seen in bilateral periventricular lesions, such as those seen in cerebral palsy. There is also characteristic extreme tightness of hip adductors which can cause legs to cross the midline referred to as a scissors gait. In countries with adequate medical care, patients with cerebral palsy may have hip adductor release surgery to minimise scissoring.</rdfs:comment>
        <rdfs:label xml:lang="en">Diplegic_gait</rdfs:label>
    </owl:Class>
    


    <!-- http://www.semanticweb.org/marthinust/ontologies/2022/8/Gait_Ontology#Disability -->

    <owl:Class rdf:about="http://www.semanticweb.org/marthinust/ontologies/2022/8/Gait_Ontology#Disability">
        <rdfs:subClassOf rdf:resource="http://www.semanticweb.org/marthinust/ontologies/2022/8/Gait_Ontology#Geriatric_gait"/>
        <opla-sd:entityPosition>
            <rdf:Description>
                <opla-sd:entityPositionX rdf:datatype="http://www.w3.org/2001/XMLSchema#double">137.2571037271739</opla-sd:entityPositionX>
                <opla-sd:entityPositionY rdf:datatype="http://www.w3.org/2001/XMLSchema#double">163.08628614110924</opla-sd:entityPositionY>
                <rdfs:comment xml:lang="en">This is an entity positioning annotation generated by CoModIDE (https://comodide.com/). Removing this annotation will break rendering the CoModIDE schema diagram view.</rdfs:comment>
            </rdf:Description>
        </opla-sd:entityPosition>
        <rdfs:comment xml:lang="en">Diseases, particularly multiple chronic illnesses, are the main cause of old age disability. Disability in old age is frequent and lowers quality of life.

Additionally, older individuals often adopt a cautious gait pattern characterised by slower walking speed, reduced step length and increased variability in step timing. This gait adaptation is more apparent on irregular than level surfaces and may be a mechanism to increase head and pelvis stability in older adults due to aging muscles, impairment, cognitive decline and neural motor skills.</rdfs:comment>
        <rdfs:label xml:lang="en">Disability</rdfs:label>
    </owl:Class>
    


    <!-- http://www.semanticweb.org/marthinust/ontologies/2022/8/Gait_Ontology#Double_support -->

    <owl:Class rdf:about="http://www.semanticweb.org/marthinust/ontologies/2022/8/Gait_Ontology#Double_support">
        <rdfs:subClassOf rdf:resource="http://www.semanticweb.org/marthinust/ontologies/2022/8/Gait_Ontology#Gait_Parameter"/>
        <opla-sd:entityPosition>
            <rdf:Description>
                <opla-sd:entityPositionX rdf:datatype="http://www.w3.org/2001/XMLSchema#double">148.72387370338893</opla-sd:entityPositionX>
                <opla-sd:entityPositionY rdf:datatype="http://www.w3.org/2001/XMLSchema#double">279.08776131728473</opla-sd:entityPositionY>
                <rdfs:comment xml:lang="en">This is an entity positioning annotation generated by CoModIDE (https://comodide.com/). Removing this annotation will break rendering the CoModIDE schema diagram view.</rdfs:comment>
            </rdf:Description>
        </opla-sd:entityPosition>
        <rdfs:comment xml:lang="en">Double support is the percentage of time spent with both feet on the ground during one gait cycle. Double support is a reflection of balance ability and confidence in balance ability, as someone who is unstable on their feet would try to maximise their base of support. For the general adult population, 20% double support is the norm.</rdfs:comment>
        <rdfs:label xml:lang="en">Double_support</rdfs:label>
    </owl:Class>
    


    <!-- http://www.semanticweb.org/marthinust/ontologies/2022/8/Gait_Ontology#Dystonia -->

    <owl:Class rdf:about="http://www.semanticweb.org/marthinust/ontologies/2022/8/Gait_Ontology#Dystonia">
        <rdfs:subClassOf rdf:resource="http://www.semanticweb.org/marthinust/ontologies/2022/8/Gait_Ontology#Gait-related_Disease"/>
    </owl:Class>
    


    <!-- http://www.semanticweb.org/marthinust/ontologies/2022/8/Gait_Ontology#Dystonic_gait -->

    <owl:Class rdf:about="http://www.semanticweb.org/marthinust/ontologies/2022/8/Gait_Ontology#Dystonic_gait">
        <rdfs:subClassOf rdf:resource="http://www.semanticweb.org/marthinust/ontologies/2022/8/Gait_Ontology#Gait_Disturbance"/>
    </owl:Class>
    


    <!-- http://www.semanticweb.org/marthinust/ontologies/2022/8/Gait_Ontology#Electromagnetic_tracking_system -->

    <owl:Class rdf:about="http://www.semanticweb.org/marthinust/ontologies/2022/8/Gait_Ontology#Electromagnetic_tracking_system">
        <rdfs:subClassOf rdf:resource="http://www.semanticweb.org/marthinust/ontologies/2022/8/Gait_Ontology#Gait_Analysis_Equipment"/>
        <opla-sd:entityPosition>
            <rdf:Description>
                <opla-sd:entityPositionX rdf:datatype="http://www.w3.org/2001/XMLSchema#double">170.92718384174754</opla-sd:entityPositionX>
                <opla-sd:entityPositionY rdf:datatype="http://www.w3.org/2001/XMLSchema#double">218.47411877155244</opla-sd:entityPositionY>
                <rdfs:comment xml:lang="en">This is an entity positioning annotation generated by CoModIDE (https://comodide.com/). Removing this annotation will break rendering the CoModIDE schema diagram view.</rdfs:comment>
            </rdf:Description>
        </opla-sd:entityPosition>
        <rdfs:comment xml:lang="en">The electromagnetic tracking system is a kind of 3D measurement device based on Faradays law of magnetic induction. When an object carrying sensor coils performs a motion inside controlled magnetic fields, the induced voltages in the sensor coils will change, with respect to the change of the objects position and orientation, relative to the source of controlled magnetic fields. In the ETS, the controlled magnetic fields are generated by a fixed transmitter and detected by the receivers fixed on the object in motion. Therefore, the positions and orientations of the object in relation to the transmitter can be calculated. Based on this working principle, some developed commercialised ETSs have been applied in bioengineering, including gait analysis and the kinematic study of body segments.</rdfs:comment>
        <rdfs:label xml:lang="en">Electromagnetic_tracking_system</rdfs:label>
    </owl:Class>
    


    <!-- http://www.semanticweb.org/marthinust/ontologies/2022/8/Gait_Ontology#Electromyography -->

    <owl:Class rdf:about="http://www.semanticweb.org/marthinust/ontologies/2022/8/Gait_Ontology#Electromyography">
        <rdfs:subClassOf rdf:resource="http://www.semanticweb.org/marthinust/ontologies/2022/8/Gait_Ontology#Gait_Analysis_Equipment"/>
    </owl:Class>
    


    <!-- http://www.semanticweb.org/marthinust/ontologies/2022/8/Gait_Ontology#Equine_gait -->

    <owl:Class rdf:about="http://www.semanticweb.org/marthinust/ontologies/2022/8/Gait_Ontology#Equine_gait">
        <rdfs:subClassOf rdf:resource="http://www.semanticweb.org/marthinust/ontologies/2022/8/Gait_Ontology#Neuropathic_gait"/>
        <opla-sd:entityPosition>
            <rdf:Description>
                <opla-sd:entityPositionX rdf:datatype="http://www.w3.org/2001/XMLSchema#double">159.73393421722602</opla-sd:entityPositionX>
                <opla-sd:entityPositionY rdf:datatype="http://www.w3.org/2001/XMLSchema#double">26.828511266219852</opla-sd:entityPositionY>
                <rdfs:comment xml:lang="en">This is an entity positioning annotation generated by CoModIDE (https://comodide.com/). Removing this annotation will break rendering the CoModIDE schema diagram view.</rdfs:comment>
            </rdf:Description>
        </opla-sd:entityPosition>
        <rdfs:comment xml:lang="en">An equine gait, or steppage gait, occurs when a person has bilateral foot drop, making it difficult to raise the feet and toes off the floor while walking. To compensate, the patient has to raise the leg higher to clear the foot from the floor, and the foot hangs downward while walking.</rdfs:comment>
        <rdfs:label xml:lang="en">Equine_gait</rdfs:label>
    </owl:Class>
    


    <!-- http://www.semanticweb.org/marthinust/ontologies/2022/8/Gait_Ontology#Exoskeleton -->

    <owl:Class rdf:about="http://www.semanticweb.org/marthinust/ontologies/2022/8/Gait_Ontology#Exoskeleton">
        <rdfs:subClassOf rdf:resource="http://www.semanticweb.org/marthinust/ontologies/2022/8/Gait_Ontology#Gait_Assistive_Technology"/>
        <opla-sd:entityPosition>
            <rdf:Description>
                <opla-sd:entityPositionX rdf:datatype="http://www.w3.org/2001/XMLSchema#double">55.71965710241819</opla-sd:entityPositionX>
                <opla-sd:entityPositionY rdf:datatype="http://www.w3.org/2001/XMLSchema#double">267.8985622527693</opla-sd:entityPositionY>
                <rdfs:comment xml:lang="en">This is an entity positioning annotation generated by CoModIDE (https://comodide.com/). Removing this annotation will break rendering the CoModIDE schema diagram view.</rdfs:comment>
            </rdf:Description>
        </opla-sd:entityPosition>
        <rdfs:comment xml:lang="en">An exoskeleton is a wearable device that helps to support a person&apos;s body and assist with movement. Exoskeletons can be used to help people with gait disorders or other mobility impairments to walk more easily and safely.</rdfs:comment>
        <rdfs:label xml:lang="en">Exoskeleton</rdfs:label>
    </owl:Class>
    


    <!-- http://www.semanticweb.org/marthinust/ontologies/2022/8/Gait_Ontology#Extensometer -->

    <owl:Class rdf:about="http://www.semanticweb.org/marthinust/ontologies/2022/8/Gait_Ontology#Extensometer">
        <rdfs:subClassOf rdf:resource="http://www.semanticweb.org/marthinust/ontologies/2022/8/Gait_Ontology#Gait_Analysis_Equipment"/>
        <opla-sd:entityPosition>
            <rdf:Description>
                <opla-sd:entityPositionX rdf:datatype="http://www.w3.org/2001/XMLSchema#double">39.40699735185387</opla-sd:entityPositionX>
                <opla-sd:entityPositionY rdf:datatype="http://www.w3.org/2001/XMLSchema#double">282.13917542836424</opla-sd:entityPositionY>
                <rdfs:comment xml:lang="en">This is an entity positioning annotation generated by CoModIDE (https://comodide.com/). Removing this annotation will break rendering the CoModIDE schema diagram view.</rdfs:comment>
            </rdf:Description>
        </opla-sd:entityPosition>
        <rdfs:comment xml:lang="en">It is possible that an extensometer could be used in a research setting to measure small changes in the length of certain body tissues, such as skin or muscle, in response to various stimuli. In this case, the extensometer would be used as a tool to collect data, rather than as a diagnostic or treatment tool.

Extensometers measure strain (or displacement) directly on the test specimen. As a result, they provide far more accurate and repeatable measurements than measurements based on the motion of the testing machines grips, which include errors from the compliance of the testing machine. They come in a great variety of shapes, sizes, measuring capacities, and temperature ratings, and they may contact the specimen directly or make measurements optically without contacting the specimen. Extensometers are reusable and last for years, and they are very cost-effective compared to adhesively bonded strain gages or digital imaging measurements.</rdfs:comment>
        <rdfs:label xml:lang="en">Extensometer</rdfs:label>
    </owl:Class>
    


    <!-- http://www.semanticweb.org/marthinust/ontologies/2022/8/Gait_Ontology#Falls -->

    <owl:Class rdf:about="http://www.semanticweb.org/marthinust/ontologies/2022/8/Gait_Ontology#Falls">
        <rdfs:subClassOf rdf:resource="http://www.semanticweb.org/marthinust/ontologies/2022/8/Gait_Ontology#Gait_Disturbance"/>
        <opla-sd:entityPosition>
            <rdf:Description>
                <opla-sd:entityPositionX rdf:datatype="http://www.w3.org/2001/XMLSchema#double">157.8560752330048</opla-sd:entityPositionX>
                <opla-sd:entityPositionY rdf:datatype="http://www.w3.org/2001/XMLSchema#double">237.6397609550408</opla-sd:entityPositionY>
                <rdfs:comment xml:lang="en">This is an entity positioning annotation generated by CoModIDE (https://comodide.com/). Removing this annotation will break rendering the CoModIDE schema diagram view.</rdfs:comment>
            </rdf:Description>
        </opla-sd:entityPosition>
        <rdfs:comment>Falls has to be attributed due to neurodegenerative diseases, dementia, delirium, or psychotropic medication. From a pragmatic point of view falls can be classified according to loss or preservation of consciousness.</rdfs:comment>
        <rdfs:label xml:lang="en">Falls</rdfs:label>
    </owl:Class>
    


    <!-- http://www.semanticweb.org/marthinust/ontologies/2022/8/Gait_Ontology#Festinating_gait -->

    <owl:Class rdf:about="http://www.semanticweb.org/marthinust/ontologies/2022/8/Gait_Ontology#Festinating_gait">
        <rdfs:subClassOf rdf:resource="http://www.semanticweb.org/marthinust/ontologies/2022/8/Gait_Ontology#Parkinsonian_gait"/>
        <opla-sd:entityPosition>
            <rdf:Description>
                <opla-sd:entityPositionX rdf:datatype="http://www.w3.org/2001/XMLSchema#double">59.644780049976184</opla-sd:entityPositionX>
                <opla-sd:entityPositionY rdf:datatype="http://www.w3.org/2001/XMLSchema#double">189.75282083594905</opla-sd:entityPositionY>
                <rdfs:comment xml:lang="en">This is an entity positioning annotation generated by CoModIDE (https://comodide.com/). Removing this annotation will break rendering the CoModIDE schema diagram view.</rdfs:comment>
            </rdf:Description>
        </opla-sd:entityPosition>
        <rdfs:comment xml:lang="en">Festinating gait (FSG) is one of the most typical and unique disturbance of locomotion associated with parkinsonism. FSG is described as; rapid, small steps, done in an attempt to keep the center of gravity (COG) in between the feet while the trunk leans forward involuntarily and shift the COG forward.

Festinating gait is described as rapid small steps done in an attempt to keep the centre of gravity in between the feet while the trunk is leaning forward involuntarily.</rdfs:comment>
        <rdfs:label xml:lang="en">Festinating_gait</rdfs:label>
    </owl:Class>
    


    <!-- http://www.semanticweb.org/marthinust/ontologies/2022/8/Gait_Ontology#Foot -->

    <owl:Class rdf:about="http://www.semanticweb.org/marthinust/ontologies/2022/8/Gait_Ontology#Foot">
        <rdfs:subClassOf rdf:resource="http://www.semanticweb.org/marthinust/ontologies/2022/8/Gait_Ontology#Musculoskeletal"/>
        <opla-sd:entityPosition>
            <rdf:Description>
                <opla-sd:entityPositionX rdf:datatype="http://www.w3.org/2001/XMLSchema#double">86.16026794249629</opla-sd:entityPositionX>
                <opla-sd:entityPositionY rdf:datatype="http://www.w3.org/2001/XMLSchema#double">274.858027450599</opla-sd:entityPositionY>
                <rdfs:comment xml:lang="en">This is an entity positioning annotation generated by CoModIDE (https://comodide.com/). Removing this annotation will break rendering the CoModIDE schema diagram view.</rdfs:comment>
            </rdf:Description>
        </opla-sd:entityPosition>
        <rdfs:comment xml:lang="en">The foot is one of the most complex parts of the body. It is made up of 26 bones connected by many joints, muscles, tendons, and ligaments. 

It&apos;s an anatomical structure found in many vertebrates (which humans are part of). It is the terminal portion of a limb which bears weight and allows locomotion.</rdfs:comment>
        <rdfs:label xml:lang="en">Foot</rdfs:label>
    </owl:Class>
    


    <!-- http://www.semanticweb.org/marthinust/ontologies/2022/8/Gait_Ontology#Foot_progession_angle -->

    <owl:Class rdf:about="http://www.semanticweb.org/marthinust/ontologies/2022/8/Gait_Ontology#Foot_progession_angle">
        <rdfs:subClassOf rdf:resource="http://www.semanticweb.org/marthinust/ontologies/2022/8/Gait_Ontology#Gait_Measurement_Point"/>
        <opla-sd:entityPosition>
            <rdf:Description>
                <opla-sd:entityPositionX rdf:datatype="http://www.w3.org/2001/XMLSchema#double">260.01391747144544</opla-sd:entityPositionX>
                <opla-sd:entityPositionY rdf:datatype="http://www.w3.org/2001/XMLSchema#double">135.2513155304341</opla-sd:entityPositionY>
                <rdfs:comment xml:lang="en">This is an entity positioning annotation generated by CoModIDE (https://comodide.com/). Removing this annotation will break rendering the CoModIDE schema diagram view.</rdfs:comment>
            </rdf:Description>
        </opla-sd:entityPosition>
        <rdfs:comment xml:lang="en">The foot progression angle (FPA) is defined as the angle between the line from the calcaneous to the second metatarsal and the line of progression averaged from heel strike to toe off during the stance phase of walking for each step (toe-in angle is positive and toe-out angle is negative). 

Assessing the foot progression angle (FPA) during gait is an important part of a clinician&apos;s examination. The FPA is defined as the angle made by the long axis of the foot from the heel to 2nd metatarsal and the line of progression of gait. A negative FPA indicates in-toeing and a positive FPA out-toeing. Knowing the FPA may help clinicians recognize and manage a number of different lower extremity conditions.</rdfs:comment>
        <rdfs:label xml:lang="en">Foot_progression_angle</rdfs:label>
    </owl:Class>
    


    <!-- http://www.semanticweb.org/marthinust/ontologies/2022/8/Gait_Ontology#Force_sensor -->

    <owl:Class rdf:about="http://www.semanticweb.org/marthinust/ontologies/2022/8/Gait_Ontology#Force_sensor">
        <rdfs:subClassOf rdf:resource="http://www.semanticweb.org/marthinust/ontologies/2022/8/Gait_Ontology#Gait_Analysis_Equipment"/>
        <opla-sd:entityPosition>
            <rdf:Description>
                <opla-sd:entityPositionX rdf:datatype="http://www.w3.org/2001/XMLSchema#double">29.00148392926447</opla-sd:entityPositionX>
                <opla-sd:entityPositionY rdf:datatype="http://www.w3.org/2001/XMLSchema#double">292.54108327391174</opla-sd:entityPositionY>
                <rdfs:comment xml:lang="en">This is an entity positioning annotation generated by CoModIDE (https://comodide.com/). Removing this annotation will break rendering the CoModIDE schema diagram view.</rdfs:comment>
            </rdf:Description>
        </opla-sd:entityPosition>
        <rdfs:comment xml:lang="en">Force sensors can be embedded into footwear to realize ambulatory measurements of Ground Reaction Force (GRF) during the gait. This GRF is a 3D vector, with the actual direction depending on the nature of the interface between the foot and the ground.

In the development of wearable force sensors, various implementations of the force transducer, including piezoelectrics, strain gauged and capacitive transducerd , are feasible. In addition, Hessert et al. designed a type of wearable force sensor based on a photoelastic triaxial force transducer to measure GRF in gait analysis. Force sensors based on the optical fiber matrix were developed to detect the shear and compressive force during human walking.

There are several different types of force sensors, including load cells, strain gauges, and piezoelectric sensors. Load cells are sensors that are used to measure force by converting it into an electrical signal. They are commonly used in force platforms, which are devices that measure the forces acting on a body or object. Strain gauges are sensors that are used to measure the deformation or strain of an object when it is subjected to a force.</rdfs:comment>
        <rdfs:label xml:lang="en">Force_sensor</rdfs:label>
    </owl:Class>
    


    <!-- http://www.semanticweb.org/marthinust/ontologies/2022/8/Gait_Ontology#Freezing_of_gait -->

    <owl:Class rdf:about="http://www.semanticweb.org/marthinust/ontologies/2022/8/Gait_Ontology#Freezing_of_gait">
        <rdfs:subClassOf rdf:resource="http://www.semanticweb.org/marthinust/ontologies/2022/8/Gait_Ontology#Gait_Disturbance"/>
    </owl:Class>
    


    <!-- http://www.semanticweb.org/marthinust/ontologies/2022/8/Gait_Ontology#Frontal_gait_ataxia -->

    <owl:Class rdf:about="http://www.semanticweb.org/marthinust/ontologies/2022/8/Gait_Ontology#Frontal_gait_ataxia">
        <rdfs:subClassOf rdf:resource="http://www.semanticweb.org/marthinust/ontologies/2022/8/Gait_Ontology#Neurological"/>
        <opla-sd:entityPosition>
            <rdf:Description>
                <opla-sd:entityPositionX rdf:datatype="http://www.w3.org/2001/XMLSchema#double">37.40137923573878</opla-sd:entityPositionX>
                <opla-sd:entityPositionY rdf:datatype="http://www.w3.org/2001/XMLSchema#double">157.25470927858868</opla-sd:entityPositionY>
                <rdfs:comment xml:lang="en">This is an entity positioning annotation generated by CoModIDE (https://comodide.com/). Removing this annotation will break rendering the CoModIDE schema diagram view.</rdfs:comment>
            </rdf:Description>
        </opla-sd:entityPosition>
        <rdfs:comment xml:lang="en">Usually secondary to injury to frontal lobe and connecting networks. May be secondary to vascular disease or hydrocephalus. May involve other lobes of brain and associated with Alzheimers disease. Difficult to classify condition. Not Parkinsons disease or any neurologic tremor. Patients have lost the ability to walk, change positions from sit to stand, and have a broad base gait with short stride length and are unable to initiate gait on own. Will also have en bloc gait, freezing episodes, and retropulsion.</rdfs:comment>
        <rdfs:label xml:lang="en">Frontal_gait_ataxia</rdfs:label>
    </owl:Class>
    


    <!-- http://www.semanticweb.org/marthinust/ontologies/2022/8/Gait_Ontology#Gait-based_Process -->

    <owl:Class rdf:about="http://www.semanticweb.org/marthinust/ontologies/2022/8/Gait_Ontology#Gait-based_Process">
        <rdfs:subClassOf>
            <owl:Restriction>
                <owl:onProperty rdf:resource="http://www.semanticweb.org/marthinust/ontologies/2022/8/Gait_Ontology#isAdministeredBy"/>
                <owl:someValuesFrom rdf:resource="http://www.semanticweb.org/marthinust/ontologies/2022/8/Gait_Ontology#Gait_expert"/>
            </owl:Restriction>
        </rdfs:subClassOf>
        <rdfs:subClassOf>
            <owl:Restriction>
                <owl:onProperty rdf:resource="http://www.semanticweb.org/marthinust/ontologies/2022/8/Gait_Ontology#isCapturedIn"/>
                <owl:someValuesFrom rdf:resource="http://www.semanticweb.org/marthinust/ontologies/2022/8/Gait_Ontology#Gait_Analysis_Method"/>
            </owl:Restriction>
        </rdfs:subClassOf>
        <owl:disjointWith rdf:resource="http://www.semanticweb.org/marthinust/ontologies/2022/8/Gait_Ontology#Gait-related_Disease"/>
        <owl:disjointWith rdf:resource="http://www.semanticweb.org/marthinust/ontologies/2022/8/Gait_Ontology#Gait_Analysis_Method"/>
        <opla-sd:entityPosition>
            <rdf:Description>
                <opla-sd:entityPositionX rdf:datatype="http://www.w3.org/2001/XMLSchema#double">48.653454824669254</opla-sd:entityPositionX>
                <opla-sd:entityPositionY rdf:datatype="http://www.w3.org/2001/XMLSchema#double">77.15663912920925</opla-sd:entityPositionY>
                <rdfs:comment xml:lang="en">This is an entity positioning annotation generated by CoModIDE (https://comodide.com/). Removing this annotation will break rendering the CoModIDE schema diagram view.</rdfs:comment>
            </rdf:Description>
        </opla-sd:entityPosition>
        <rdfs:comment xml:lang="en">It&apos;s an assessment process of the way the body moves, usually by walking or running, from one point to another by collecting gait data through observation or system-based. The purpose is to detect any abnormalities in locomotion to gain information about lower limb dysfunction in dynamic movement and loading.

The process typically begins with a thorough evaluation of the individual&apos;s gait and mobility. This may involve a physical examination, gait analysis, and functional assessments to determine the underlying causes of the gait and mobility problems. The healthcare team will then develop a treatment plan that is tailored to the individual&apos;s needs and goals.</rdfs:comment>
        <rdfs:label xml:lang="en">Gait-based_Process</rdfs:label>
    </owl:Class>
    


    <!-- http://www.semanticweb.org/marthinust/ontologies/2022/8/Gait_Ontology#Gait-related_Disease -->

    <owl:Class rdf:about="http://www.semanticweb.org/marthinust/ontologies/2022/8/Gait_Ontology#Gait-related_Disease">
        <rdfs:subClassOf>
            <owl:Restriction>
                <owl:onProperty rdf:resource="http://www.semanticweb.org/marthinust/ontologies/2022/8/Gait_Ontology#isAssociatedTo"/>
                <owl:someValuesFrom rdf:resource="http://www.semanticweb.org/marthinust/ontologies/2022/8/Gait_Ontology#Gait_patient"/>
            </owl:Restriction>
        </rdfs:subClassOf>
        <owl:disjointWith rdf:resource="http://www.semanticweb.org/marthinust/ontologies/2022/8/Gait_Ontology#Gait_Analysis_Equipment"/>
        <owl:disjointWith rdf:resource="http://www.semanticweb.org/marthinust/ontologies/2022/8/Gait_Ontology#Gait_Measurement_Point"/>
        <owl:disjointWith rdf:resource="http://www.semanticweb.org/marthinust/ontologies/2022/8/Gait_Ontology#Type_of_Gait"/>
        <opla-sd:entityPosition>
            <rdf:Description>
                <opla-sd:entityPositionX rdf:datatype="http://www.w3.org/2001/XMLSchema#double">30.798215479530192</opla-sd:entityPositionX>
                <opla-sd:entityPositionY rdf:datatype="http://www.w3.org/2001/XMLSchema#double">47.83188154997808</opla-sd:entityPositionY>
                <rdfs:comment xml:lang="en">This is an entity positioning annotation generated by CoModIDE (https://comodide.com/). Removing this annotation will break rendering the CoModIDE schema diagram view.</rdfs:comment>
            </rdf:Description>
        </opla-sd:entityPosition>
        <rdfs:comment xml:lang="en">Gait-related diseases are conditions that can affect an individual&apos;s gait, or the way in which they walk. Gait abnormalities can be caused by a variety of factors, including neurological conditions, musculoskeletal abnormalities, trauma, and degenerative diseases.

Causes of walking/gait disorders that can range from arthritis to a neurological condition to orthopedic issues and neuromuscular.</rdfs:comment>
        <rdfs:label xml:lang="en">Gait-related_Disease</rdfs:label>
    </owl:Class>
    


    <!-- http://www.semanticweb.org/marthinust/ontologies/2022/8/Gait_Ontology#Gait_Analysis_Equipment -->

    <owl:Class rdf:about="http://www.semanticweb.org/marthinust/ontologies/2022/8/Gait_Ontology#Gait_Analysis_Equipment">
        <rdfs:subClassOf>
            <owl:Restriction>
                <owl:onProperty rdf:resource="http://www.semanticweb.org/marthinust/ontologies/2022/8/Gait_Ontology#isLinkedTo"/>
                <owl:someValuesFrom rdf:resource="http://www.semanticweb.org/marthinust/ontologies/2022/8/Gait_Ontology#Gait_patient"/>
            </owl:Restriction>
        </rdfs:subClassOf>
        <rdfs:subClassOf>
            <owl:Restriction>
                <owl:onProperty rdf:resource="http://www.semanticweb.org/marthinust/ontologies/2022/8/Gait_Ontology#isUsedFor"/>
                <owl:someValuesFrom rdf:resource="http://www.semanticweb.org/marthinust/ontologies/2022/8/Gait_Ontology#Gait-based_Process"/>
            </owl:Restriction>
        </rdfs:subClassOf>
        <rdfs:subClassOf>
            <owl:Restriction>
                <owl:onProperty rdf:resource="http://www.semanticweb.org/marthinust/ontologies/2022/8/Gait_Ontology#isUsedIn"/>
                <owl:someValuesFrom rdf:resource="http://www.semanticweb.org/marthinust/ontologies/2022/8/Gait_Ontology#Gait_Analysis_Method"/>
            </owl:Restriction>
        </rdfs:subClassOf>
        <owl:disjointWith rdf:resource="http://www.semanticweb.org/marthinust/ontologies/2022/8/Gait_Ontology#Gait_Classification"/>
        <owl:disjointWith rdf:resource="http://www.semanticweb.org/marthinust/ontologies/2022/8/Gait_Ontology#Gait_Cycle"/>
        <owl:disjointWith rdf:resource="http://www.semanticweb.org/marthinust/ontologies/2022/8/Gait_Ontology#Gait_Parameter"/>
        <opla-sd:entityPosition>
            <rdf:Description>
                <opla-sd:entityPositionX rdf:datatype="http://www.w3.org/2001/XMLSchema#double">152.38641905605903</opla-sd:entityPositionX>
                <opla-sd:entityPositionY rdf:datatype="http://www.w3.org/2001/XMLSchema#double">171.67607047064863</opla-sd:entityPositionY>
                <rdfs:comment xml:lang="en">This is an entity positioning annotation generated by CoModIDE (https://comodide.com/). Removing this annotation will break rendering the CoModIDE schema diagram view.</rdfs:comment>
            </rdf:Description>
        </opla-sd:entityPosition>
        <rdfs:comment xml:lang="en">Gait analysis equipment is used to study and assess a person&apos;s gait, or the manner in which they walk. This equipment can provide detailed information about a person&apos;s gait patterns, including their stride length, foot placement, and body movements. Gait analysis equipment can be used to identify any abnormalities or disorders that may be affecting a person&apos;s gait, and can help to diagnose and treat gait-related conditions.

Gait analysis commonly involves the measurement of the movement of the body in space (kinematics) and the forces involved in producing these movements (kinetics) which can be quantified by gait analysis equipment.</rdfs:comment>
        <rdfs:label xml:lang="en">Gait_Analysis_Equipment</rdfs:label>
    </owl:Class>
    


    <!-- http://www.semanticweb.org/marthinust/ontologies/2022/8/Gait_Ontology#Gait_Analysis_Method -->

    <owl:Class rdf:about="http://www.semanticweb.org/marthinust/ontologies/2022/8/Gait_Ontology#Gait_Analysis_Method">
        <rdfs:subClassOf>
            <owl:Restriction>
                <owl:onProperty rdf:resource="http://www.semanticweb.org/marthinust/ontologies/2022/8/Gait_Ontology#isBasedOn"/>
                <owl:someValuesFrom rdf:resource="http://www.semanticweb.org/marthinust/ontologies/2022/8/Gait_Ontology#Gait_Analysis_Equipment"/>
            </owl:Restriction>
        </rdfs:subClassOf>
        <owl:disjointWith rdf:resource="http://www.semanticweb.org/marthinust/ontologies/2022/8/Gait_Ontology#Gait_Assistive_Technology"/>
        <owl:disjointWith rdf:resource="http://www.semanticweb.org/marthinust/ontologies/2022/8/Gait_Ontology#Gait_Disturbance"/>
        <owl:disjointWith rdf:resource="http://www.semanticweb.org/marthinust/ontologies/2022/8/Gait_Ontology#Gait_Pathology"/>
        <opla-sd:entityPosition>
            <rdf:Description>
                <opla-sd:entityPositionX rdf:datatype="http://www.w3.org/2001/XMLSchema#double">101.46272241937267</opla-sd:entityPositionX>
                <opla-sd:entityPositionY rdf:datatype="http://www.w3.org/2001/XMLSchema#double">81.84672572875863</opla-sd:entityPositionY>
                <rdfs:comment xml:lang="en">This is an entity positioning annotation generated by CoModIDE (https://comodide.com/). Removing this annotation will break rendering the CoModIDE schema diagram view.</rdfs:comment>
            </rdf:Description>
        </opla-sd:entityPosition>
        <rdfs:comment xml:lang="en">Gait analysis often requires the quantification of motion of individual body segments in two- or three-dimensional space. The most common method for collecting this information is through the use of motion capture technology, in which markers are affixed to the subject and tracked throughout the motion of interest.

This information can be used to identify any abnormalities or disorders that may be affecting a person&apos;s gait, and can help to diagnose and treat gait-related conditions. Gait analysis methods can also be used to assess the effectiveness of different treatments for gait disorders, and to monitor a person&apos;s progress over time. Some common gait analysis methods include observing a person walking, using video cameras or sensors to capture a person&apos;s gait patterns, and analysing the data collected to identify specific gait characteristics.</rdfs:comment>
        <rdfs:label xml:lang="en">Gait _Analysis_Method</rdfs:label>
    </owl:Class>
    


    <!-- http://www.semanticweb.org/marthinust/ontologies/2022/8/Gait_Ontology#Gait_Assistive_Technology -->

    <owl:Class rdf:about="http://www.semanticweb.org/marthinust/ontologies/2022/8/Gait_Ontology#Gait_Assistive_Technology">
        <rdfs:subClassOf>
            <owl:Restriction>
                <owl:onProperty rdf:resource="http://www.semanticweb.org/marthinust/ontologies/2022/8/Gait_Ontology#isAscertainedIn"/>
                <owl:someValuesFrom rdf:resource="http://www.semanticweb.org/marthinust/ontologies/2022/8/Gait_Ontology#Gait-based_Process"/>
            </owl:Restriction>
        </rdfs:subClassOf>
        <rdfs:subClassOf>
            <owl:Restriction>
                <owl:onProperty rdf:resource="http://www.semanticweb.org/marthinust/ontologies/2022/8/Gait_Ontology#isPrescribedBy"/>
                <owl:someValuesFrom rdf:resource="http://www.semanticweb.org/marthinust/ontologies/2022/8/Gait_Ontology#Gait_expert"/>
            </owl:Restriction>
        </rdfs:subClassOf>
        <rdfs:subClassOf>
            <owl:Restriction>
                <owl:onProperty rdf:resource="http://www.semanticweb.org/marthinust/ontologies/2022/8/Gait_Ontology#isRecommendedTo"/>
                <owl:someValuesFrom rdf:resource="http://www.semanticweb.org/marthinust/ontologies/2022/8/Gait_Ontology#Gait_patient"/>
            </owl:Restriction>
        </rdfs:subClassOf>
        <rdfs:subClassOf>
            <owl:Restriction>
                <owl:onProperty rdf:resource="http://www.semanticweb.org/marthinust/ontologies/2022/8/Gait_Ontology#hasType_of_material"/>
                <owl:someValuesFrom rdf:resource="http://www.w3.org/2001/XMLSchema#string"/>
            </owl:Restriction>
        </rdfs:subClassOf>
        <owl:disjointWith rdf:resource="http://www.semanticweb.org/marthinust/ontologies/2022/8/Gait_Ontology#Gait_Measurement_Point"/>
        <owl:disjointWith rdf:resource="http://www.semanticweb.org/marthinust/ontologies/2022/8/Gait_Ontology#Gait_Pathology"/>
        <opla-sd:entityPosition>
            <rdf:Description>
                <opla-sd:entityPositionX rdf:datatype="http://www.w3.org/2001/XMLSchema#double">217.58935578269643</opla-sd:entityPositionX>
                <opla-sd:entityPositionY rdf:datatype="http://www.w3.org/2001/XMLSchema#double">290.0978638990234</opla-sd:entityPositionY>
                <rdfs:comment xml:lang="en">This is an entity positioning annotation generated by CoModIDE (https://comodide.com/). Removing this annotation will break rendering the CoModIDE schema diagram view.</rdfs:comment>
            </rdf:Description>
        </opla-sd:entityPosition>
        <rdfs:comment xml:lang="en">These are devices a patient may be issued with in order to improve their walking pattern, balance or safety while mobilising independently. They can also be a means of transferring weight from the upper limb to the ground, in cases where reducing weight bearing through the lower limb is desired. 

They assist with ambulation by enhancing the patient&apos;s balance and ability to bear weight. An assistive device is an object or piece of equipment designed to help a patient with activities of daily living.</rdfs:comment>
        <rdfs:label xml:lang="en">Gait_Assistive_Technology</rdfs:label>
    </owl:Class>
    


    <!-- http://www.semanticweb.org/marthinust/ontologies/2022/8/Gait_Ontology#Gait_Classification -->

    <owl:Class rdf:about="http://www.semanticweb.org/marthinust/ontologies/2022/8/Gait_Ontology#Gait_Classification">
        <rdfs:subClassOf>
            <owl:Restriction>
                <owl:onProperty rdf:resource="http://www.semanticweb.org/marthinust/ontologies/2022/8/Gait_Ontology#isIdentifiedIn"/>
                <owl:someValuesFrom rdf:resource="http://www.semanticweb.org/marthinust/ontologies/2022/8/Gait_Ontology#Gait_Analysis_Method"/>
            </owl:Restriction>
        </rdfs:subClassOf>
        <owl:disjointWith rdf:resource="http://www.semanticweb.org/marthinust/ontologies/2022/8/Gait_Ontology#Gait_Cycle"/>
        <owl:disjointWith rdf:resource="http://www.semanticweb.org/marthinust/ontologies/2022/8/Gait_Ontology#Gait_Person"/>
        <opla-sd:entityPosition>
            <rdf:Description>
                <opla-sd:entityPositionX rdf:datatype="http://www.w3.org/2001/XMLSchema#double">58.07012698846076</opla-sd:entityPositionX>
                <opla-sd:entityPositionY rdf:datatype="http://www.w3.org/2001/XMLSchema#double">37.93093411028254</opla-sd:entityPositionY>
                <rdfs:comment xml:lang="en">This is an entity positioning annotation generated by CoModIDE (https://comodide.com/). Removing this annotation will break rendering the CoModIDE schema diagram view.</rdfs:comment>
            </rdf:Description>
        </opla-sd:entityPosition>
        <rdfs:comment xml:lang="en">Gait classification allocates walking patterns into groups that can be identified and differentiated from one another based on a set of defined variables. It involves analysing and understanding the different characteristics of a person&apos;s gait to identify and classify abnormalities or pathologies.</rdfs:comment>
        <rdfs:label xml:lang="en">Gait_Classification</rdfs:label>
    </owl:Class>
    


    <!-- http://www.semanticweb.org/marthinust/ontologies/2022/8/Gait_Ontology#Gait_Cycle -->

    <owl:Class rdf:about="http://www.semanticweb.org/marthinust/ontologies/2022/8/Gait_Ontology#Gait_Cycle">
        <rdfs:subClassOf>
            <owl:Restriction>
                <owl:onProperty rdf:resource="http://www.semanticweb.org/marthinust/ontologies/2022/8/Gait_Ontology#isDemonstratedBy"/>
                <owl:someValuesFrom rdf:resource="http://www.semanticweb.org/marthinust/ontologies/2022/8/Gait_Ontology#Gait_patient"/>
            </owl:Restriction>
        </rdfs:subClassOf>
        <rdfs:subClassOf>
            <owl:Restriction>
                <owl:onProperty rdf:resource="http://www.semanticweb.org/marthinust/ontologies/2022/8/Gait_Ontology#isObservedBy"/>
                <owl:someValuesFrom rdf:resource="http://www.semanticweb.org/marthinust/ontologies/2022/8/Gait_Ontology#Gait_expert"/>
            </owl:Restriction>
        </rdfs:subClassOf>
        <rdfs:subClassOf>
            <owl:Restriction>
                <owl:onProperty rdf:resource="http://www.semanticweb.org/marthinust/ontologies/2022/8/Gait_Ontology#isObservedIn"/>
                <owl:someValuesFrom rdf:resource="http://www.semanticweb.org/marthinust/ontologies/2022/8/Gait_Ontology#Gait-based_Process"/>
            </owl:Restriction>
        </rdfs:subClassOf>
        <opla-sd:entityPosition>
            <rdf:Description>
                <opla-sd:entityPositionX rdf:datatype="http://www.w3.org/2001/XMLSchema#double">188.29517851119326</opla-sd:entityPositionX>
                <opla-sd:entityPositionY rdf:datatype="http://www.w3.org/2001/XMLSchema#double">276.09834028517923</opla-sd:entityPositionY>
                <rdfs:comment xml:lang="en">This is an entity positioning annotation generated by CoModIDE (https://comodide.com/). Removing this annotation will break rendering the CoModIDE schema diagram view.</rdfs:comment>
            </rdf:Description>
        </opla-sd:entityPosition>
        <rdfs:comment xml:lang="en">The gait cycle describes the cyclic pattern of movement that occurs while walking. A single cycle of gait starts when the heel of one foot strikes the ground and ends when that same heel touches the ground again.</rdfs:comment>
        <rdfs:label xml:lang="en">Gait_Cycle</rdfs:label>
    </owl:Class>
    


    <!-- http://www.semanticweb.org/marthinust/ontologies/2022/8/Gait_Ontology#Gait_Disturbance -->

    <owl:Class rdf:about="http://www.semanticweb.org/marthinust/ontologies/2022/8/Gait_Ontology#Gait_Disturbance">
        <rdfs:subClassOf>
            <owl:Restriction>
                <owl:onProperty rdf:resource="http://www.semanticweb.org/marthinust/ontologies/2022/8/Gait_Ontology#affects"/>
                <owl:someValuesFrom rdf:resource="http://www.semanticweb.org/marthinust/ontologies/2022/8/Gait_Ontology#Gait_patient"/>
            </owl:Restriction>
        </rdfs:subClassOf>
        <rdfs:subClassOf>
            <owl:Restriction>
                <owl:onProperty rdf:resource="http://www.semanticweb.org/marthinust/ontologies/2022/8/Gait_Ontology#isDiagnosedBy"/>
                <owl:someValuesFrom rdf:resource="http://www.semanticweb.org/marthinust/ontologies/2022/8/Gait_Ontology#Gait_expert"/>
            </owl:Restriction>
        </rdfs:subClassOf>
        <rdfs:subClassOf>
            <owl:Restriction>
                <owl:onProperty rdf:resource="http://www.semanticweb.org/marthinust/ontologies/2022/8/Gait_Ontology#isVerifiedBy"/>
                <owl:someValuesFrom rdf:resource="http://www.semanticweb.org/marthinust/ontologies/2022/8/Gait_Ontology#Gait_Analysis_Equipment"/>
            </owl:Restriction>
        </rdfs:subClassOf>
        <opla-sd:entityPosition>
            <rdf:Description>
                <opla-sd:entityPositionX rdf:datatype="http://www.w3.org/2001/XMLSchema#double">100.84787700578089</opla-sd:entityPositionX>
                <opla-sd:entityPositionY rdf:datatype="http://www.w3.org/2001/XMLSchema#double">36.588635173753644</opla-sd:entityPositionY>
                <rdfs:comment xml:lang="en">This is an entity positioning annotation generated by CoModIDE (https://comodide.com/). Removing this annotation will break rendering the CoModIDE schema diagram view.</rdfs:comment>
            </rdf:Description>
        </opla-sd:entityPosition>
        <rdfs:comment xml:lang="en">Gait disturbances are described as any deviations from normal walking or gait. Numerous etiologies cause these disturbances. Due to their different clinical presentations, a high index of suspicion is required. The etiology can be determined through the clinical presentation, laboratory work, and diagnostic testing.

The causes of gait disorders include neurological conditions (e.g. sensory or motor impairments), orthopedic problems (e.g. osteoarthritis and skeletal deformities) and medical conditions (e.g. heart failure, respiratory insufficiency, peripheral arterial occlusive disease and obesity).</rdfs:comment>
        <rdfs:label xml:lang="en">Gait_Disturbance</rdfs:label>
    </owl:Class>
    


    <!-- http://www.semanticweb.org/marthinust/ontologies/2022/8/Gait_Ontology#Gait_Measurement_Point -->

    <owl:Class rdf:about="http://www.semanticweb.org/marthinust/ontologies/2022/8/Gait_Ontology#Gait_Measurement_Point">
        <rdfs:subClassOf>
            <owl:Restriction>
                <owl:onProperty rdf:resource="http://www.semanticweb.org/marthinust/ontologies/2022/8/Gait_Ontology#isAnalysedIn"/>
                <owl:someValuesFrom rdf:resource="http://www.semanticweb.org/marthinust/ontologies/2022/8/Gait_Ontology#Gait_Cycle"/>
            </owl:Restriction>
        </rdfs:subClassOf>
        <opla-sd:entityPosition>
            <rdf:Description>
                <opla-sd:entityPositionX rdf:datatype="http://www.w3.org/2001/XMLSchema#double">109.97744961743291</opla-sd:entityPositionX>
                <opla-sd:entityPositionY rdf:datatype="http://www.w3.org/2001/XMLSchema#double">201.82077174936492</opla-sd:entityPositionY>
                <rdfs:comment xml:lang="en">This is an entity positioning annotation generated by CoModIDE (https://comodide.com/). Removing this annotation will break rendering the CoModIDE schema diagram view.</rdfs:comment>
            </rdf:Description>
        </opla-sd:entityPosition>
        <rdfs:comment xml:lang="en">It usually involved watching a person walk towards and away from you, observing the length of the stride, arm movement, heel placement and angle of the pelvis.

Gait measurement points are specific locations on the body that are used to analyse and measure the way a person walks or moves. These points are typically defined by specific landmarks on the body, such as the joints or the center of mass. Gait measurement points are used in a variety of settings, including in research studies, in clinical settings to assess mobility and balance, and in sports performance analysis. The specific points that are measured can vary depending on the specific purpose of the analysis and the equipment being used. Some common gait measurement points include the pelvis, hip, knee, and ankle.</rdfs:comment>
        <rdfs:label xml:lang="en">Gait_Measurement_Point</rdfs:label>
    </owl:Class>
    


    <!-- http://www.semanticweb.org/marthinust/ontologies/2022/8/Gait_Ontology#Gait_Parameter -->

    <owl:Class rdf:about="http://www.semanticweb.org/marthinust/ontologies/2022/8/Gait_Ontology#Gait_Parameter">
        <rdfs:subClassOf>
            <owl:Restriction>
                <owl:onProperty rdf:resource="http://www.semanticweb.org/marthinust/ontologies/2022/8/Gait_Ontology#isDeterminedBy"/>
                <owl:someValuesFrom rdf:resource="http://www.semanticweb.org/marthinust/ontologies/2022/8/Gait_Ontology#Gait_Measurement_Point"/>
            </owl:Restriction>
        </rdfs:subClassOf>
        <rdfs:subClassOf>
            <owl:Restriction>
                <owl:onProperty rdf:resource="http://www.semanticweb.org/marthinust/ontologies/2022/8/Gait_Ontology#isEvaluatedIn"/>
                <owl:someValuesFrom rdf:resource="http://www.semanticweb.org/marthinust/ontologies/2022/8/Gait_Ontology#Gait_Cycle"/>
            </owl:Restriction>
        </rdfs:subClassOf>
        <owl:disjointWith rdf:resource="http://www.semanticweb.org/marthinust/ontologies/2022/8/Gait_Ontology#Type_of_Gait"/>
        <opla-sd:entityPosition>
            <rdf:Description>
                <opla-sd:entityPositionX rdf:datatype="http://www.w3.org/2001/XMLSchema#double">101.10977855557579</opla-sd:entityPositionX>
                <opla-sd:entityPositionY rdf:datatype="http://www.w3.org/2001/XMLSchema#double">193.95943677564725</opla-sd:entityPositionY>
                <rdfs:comment xml:lang="en">This is an entity positioning annotation generated by CoModIDE (https://comodide.com/). Removing this annotation will break rendering the CoModIDE schema diagram view.</rdfs:comment>
            </rdf:Description>
        </opla-sd:entityPosition>
        <rdfs:comment xml:lang="en">Parameters of gait include velocity, step length, swing and stance phase, double support time, ground reaction forces, impulse, and propulsion during habitual walking.

An objective approach is quantitative and parameters like time, distance, and muscle activity will be measured.</rdfs:comment>
        <rdfs:label xml:lang="en">Gait_Parameter</rdfs:label>
    </owl:Class>
    


    <!-- http://www.semanticweb.org/marthinust/ontologies/2022/8/Gait_Ontology#Gait_Pathology -->

    <owl:Class rdf:about="http://www.semanticweb.org/marthinust/ontologies/2022/8/Gait_Ontology#Gait_Pathology">
        <rdfs:subClassOf>
            <owl:Restriction>
                <owl:onProperty rdf:resource="http://www.semanticweb.org/marthinust/ontologies/2022/8/Gait_Ontology#isCategorisedIn"/>
                <owl:someValuesFrom rdf:resource="http://www.semanticweb.org/marthinust/ontologies/2022/8/Gait_Ontology#Gait_Classification"/>
            </owl:Restriction>
        </rdfs:subClassOf>
        <opla-sd:entityPosition>
            <rdf:Description>
                <opla-sd:entityPositionX rdf:datatype="http://www.w3.org/2001/XMLSchema#double">5.243940907771614</opla-sd:entityPositionX>
                <opla-sd:entityPositionY rdf:datatype="http://www.w3.org/2001/XMLSchema#double">297.4100537880053</opla-sd:entityPositionY>
                <rdfs:comment xml:lang="en">This is an entity positioning annotation generated by CoModIDE (https://comodide.com/). Removing this annotation will break rendering the CoModIDE schema diagram view.</rdfs:comment>
            </rdf:Description>
        </opla-sd:entityPosition>
        <rdfs:comment xml:lang="en">The term &quot;gait pathologies&quot; refers to abnormalities or disorders that affect the way a person walks. These abnormalities can be caused by a wide range of factors, including neurological conditions, musculoskeletal disorders, injuries and age-related deterioration.

Gait pathology involves, but not limited to infections, injuries, such as; fractures (broken bones), sprains, and tendinitis. Movement disorders, such as Parkinson&apos;s disease. Neurologic diseases, including multiple sclerosis and peripheral nerve disorders. Various underlying issues and abnormalities that have an impact on gait-related conditions.

Gait pathology is a specialized area of study within the field of movement disorders, and is often performed by doctors or other healthcare providers who have expertise in this area. Gait disorders can be caused by a wide range of factors, including medical conditions, injuries, or simply the natural aging process.</rdfs:comment>
        <rdfs:label xml:lang="en">Gait_Pathology</rdfs:label>
    </owl:Class>
    


    <!-- http://www.semanticweb.org/marthinust/ontologies/2022/8/Gait_Ontology#Gait_Person -->

    <owl:Class rdf:about="http://www.semanticweb.org/marthinust/ontologies/2022/8/Gait_Ontology#Gait_Person">
        <rdfs:subClassOf>
            <owl:Restriction>
                <owl:onProperty rdf:resource="http://www.semanticweb.org/marthinust/ontologies/2022/8/Gait_Ontology#hasAge_in_years"/>
                <owl:someValuesFrom rdf:resource="http://www.w3.org/2001/XMLSchema#integer"/>
            </owl:Restriction>
        </rdfs:subClassOf>
        <rdfs:subClassOf>
            <owl:Restriction>
                <owl:onProperty rdf:resource="http://www.semanticweb.org/marthinust/ontologies/2022/8/Gait_Ontology#hasGender"/>
                <owl:someValuesFrom rdf:resource="http://www.w3.org/2001/XMLSchema#string"/>
            </owl:Restriction>
        </rdfs:subClassOf>
        <opla-sd:entityPosition>
            <rdf:Description>
                <opla-sd:entityPositionX rdf:datatype="http://www.w3.org/2001/XMLSchema#double">293.8972320394836</opla-sd:entityPositionX>
                <opla-sd:entityPositionY rdf:datatype="http://www.w3.org/2001/XMLSchema#double">151.0510306964911</opla-sd:entityPositionY>
                <rdfs:comment xml:lang="en">This is an entity positioning annotation generated by CoModIDE (https://comodide.com/). Removing this annotation will break rendering the CoModIDE schema diagram view.</rdfs:comment>
            </rdf:Description>
        </opla-sd:entityPosition>
        <rdfs:comment xml:lang="en">A person (PL: people) is a being that has certain capacities or attributes such as reason, morality, consciousness or self-consciousness, and being a part of a culturally established form of social relations such as kinship, ownership of property, or legal responsibility.

Person, individual, personage are terms applied to human beings. Person is the most general and common word: the average person. Individual views a person as standing alone or as a single member of a group.</rdfs:comment>
        <rdfs:label xml:lang="en">Gait_Person</rdfs:label>
    </owl:Class>
    


    <!-- http://www.semanticweb.org/marthinust/ontologies/2022/8/Gait_Ontology#Gait_acquisition -->

    <owl:Class rdf:about="http://www.semanticweb.org/marthinust/ontologies/2022/8/Gait_Ontology#Gait_acquisition">
        <rdfs:subClassOf rdf:resource="http://www.semanticweb.org/marthinust/ontologies/2022/8/Gait_Ontology#Gait-based_Process"/>
        <rdfs:subClassOf>
            <owl:Restriction>
                <owl:onProperty rdf:resource="http://www.semanticweb.org/marthinust/ontologies/2022/8/Gait_Ontology#collects"/>
                <owl:someValuesFrom rdf:resource="http://www.semanticweb.org/marthinust/ontologies/2022/8/Gait_Ontology#Gait_data"/>
            </owl:Restriction>
        </rdfs:subClassOf>
        <rdfs:subClassOf>
            <owl:Restriction>
                <owl:onProperty rdf:resource="http://www.semanticweb.org/marthinust/ontologies/2022/8/Gait_Ontology#involves"/>
                <owl:someValuesFrom rdf:resource="http://www.semanticweb.org/marthinust/ontologies/2022/8/Gait_Ontology#Gait_patient"/>
            </owl:Restriction>
        </rdfs:subClassOf>
        <rdfs:subClassOf>
            <owl:Restriction>
                <owl:onProperty rdf:resource="http://www.semanticweb.org/marthinust/ontologies/2022/8/Gait_Ontology#isPartOf"/>
                <owl:someValuesFrom rdf:resource="http://www.semanticweb.org/marthinust/ontologies/2022/8/Gait_Ontology#Gait_analysis"/>
            </owl:Restriction>
        </rdfs:subClassOf>
        <opla-sd:entityPosition>
            <rdf:Description>
                <opla-sd:entityPositionX rdf:datatype="http://www.w3.org/2001/XMLSchema#double">168.92544278498195</opla-sd:entityPositionX>
                <opla-sd:entityPositionY rdf:datatype="http://www.w3.org/2001/XMLSchema#double">284.26671640078024</opla-sd:entityPositionY>
                <rdfs:comment xml:lang="en">This is an entity positioning annotation generated by CoModIDE (https://comodide.com/). Removing this annotation will break rendering the CoModIDE schema diagram view.</rdfs:comment>
            </rdf:Description>
        </opla-sd:entityPosition>
        <rdfs:comment xml:lang="en">Gait acquisition is the process of collecting and analyzing data on an individual&apos;s gait, or the way in which they walk.

Gait (data) acquisition is the process where a patient&apos;s gait assessment  or measurements are obtained in acquisition sessions and observations for quantitative recording and functional description.</rdfs:comment>
        <rdfs:label xml:lang="en">Gait_acquisition</rdfs:label>
    </owl:Class>
    


    <!-- http://www.semanticweb.org/marthinust/ontologies/2022/8/Gait_Ontology#Gait_analysis -->

    <owl:Class rdf:about="http://www.semanticweb.org/marthinust/ontologies/2022/8/Gait_Ontology#Gait_analysis">
        <rdfs:subClassOf rdf:resource="http://www.semanticweb.org/marthinust/ontologies/2022/8/Gait_Ontology#Gait-based_Process"/>
        <rdfs:subClassOf>
            <owl:Restriction>
                <owl:onProperty rdf:resource="http://www.semanticweb.org/marthinust/ontologies/2022/8/Gait_Ontology#isFacilitatedBy"/>
                <owl:someValuesFrom rdf:resource="http://www.semanticweb.org/marthinust/ontologies/2022/8/Gait_Ontology#Gait_expert"/>
            </owl:Restriction>
        </rdfs:subClassOf>
        <rdfs:subClassOf>
            <owl:Restriction>
                <owl:onProperty rdf:resource="http://www.semanticweb.org/marthinust/ontologies/2022/8/Gait_Ontology#isGeneratedIn"/>
                <owl:someValuesFrom rdf:resource="http://www.semanticweb.org/marthinust/ontologies/2022/8/Gait_Ontology#Gait-based_Process"/>
            </owl:Restriction>
        </rdfs:subClassOf>
        <rdfs:subClassOf>
            <owl:Restriction>
                <owl:onProperty rdf:resource="http://www.semanticweb.org/marthinust/ontologies/2022/8/Gait_Ontology#hasGait_analysis"/>
                <owl:someValuesFrom rdf:resource="http://www.w3.org/2001/XMLSchema#string"/>
            </owl:Restriction>
        </rdfs:subClassOf>
        <opla-sd:entityPosition>
            <rdf:Description>
                <opla-sd:entityPositionX rdf:datatype="http://www.w3.org/2001/XMLSchema#double">187.18541646404984</opla-sd:entityPositionX>
                <opla-sd:entityPositionY rdf:datatype="http://www.w3.org/2001/XMLSchema#double">44.051154237917906</opla-sd:entityPositionY>
                <rdfs:comment xml:lang="en">This is an entity positioning annotation generated by CoModIDE (https://comodide.com/). Removing this annotation will break rendering the CoModIDE schema diagram view.</rdfs:comment>
            </rdf:Description>
        </opla-sd:entityPosition>
        <rdfs:comment xml:lang="en">The term &quot;gait analysis&quot; encompasses a broad spectrum of potential assessment strategies used to evaluate normal and abnormal gait, both walking and running. Such assessments range from simple observation to sophisticated computer analysis of biomechanics. 

Gait analysis, though sometimes performed through simple observation, can now be performed with the help of advanced technology. By analysing the data provided by several devices, the patient&apos;s gait can be evaluated in terms of step length, stride length, cadence, cycle time and joint angles. 

Reasons for Gait Analysis:

Gait abnormalities involve unusual walking patterns that may be caused by disease or injury. Such irregularities can lead to pain in the hips, back, neck, feet, knees or ankles. Gait analysis, also known as walking or motion analysis, is a comprehensive evaluation of the way an individual stands and walks. 

This analysis can help:

Identify the source of muscle, nerve or skeletal problems
Discover the source of a patient&apos;s pain while standing or walking
Help to diagnose bone deformities or skeletal misalignments
Assist in discovering muscle or nerve dysfunction
Check the progression of diseases like arthritis or muscular dystrophy</rdfs:comment>
        <rdfs:label xml:lang="en">Gait_analysis</rdfs:label>
    </owl:Class>
    


    <!-- http://www.semanticweb.org/marthinust/ontologies/2022/8/Gait_Ontology#Gait_apraxia -->

    <owl:Class rdf:about="http://www.semanticweb.org/marthinust/ontologies/2022/8/Gait_Ontology#Gait_apraxia">
        <rdfs:subClassOf rdf:resource="http://www.semanticweb.org/marthinust/ontologies/2022/8/Gait_Ontology#Gait_Disturbance"/>
        <opla-sd:entityPosition>
            <rdf:Description>
                <opla-sd:entityPositionX rdf:datatype="http://www.w3.org/2001/XMLSchema#double">28.162361345475432</opla-sd:entityPositionX>
                <opla-sd:entityPositionY rdf:datatype="http://www.w3.org/2001/XMLSchema#double">258.03105005740014</opla-sd:entityPositionY>
                <rdfs:comment xml:lang="en">This is an entity positioning annotation generated by CoModIDE (https://comodide.com/). Removing this annotation will break rendering the CoModIDE schema diagram view.</rdfs:comment>
            </rdf:Description>
        </opla-sd:entityPosition>
        <rdfs:comment>Gait apraxia affecting the ability to make walking movements with the legs.</rdfs:comment>
        <rdfs:label xml:lang="en">Gait_apraxia</rdfs:label>
    </owl:Class>
    


    <!-- http://www.semanticweb.org/marthinust/ontologies/2022/8/Gait_Ontology#Gait_ataxia -->

    <owl:Class rdf:about="http://www.semanticweb.org/marthinust/ontologies/2022/8/Gait_Ontology#Gait_ataxia">
        <rdfs:subClassOf rdf:resource="http://www.semanticweb.org/marthinust/ontologies/2022/8/Gait_Ontology#Gait_Disturbance"/>
        <opla-sd:entityPosition>
            <rdf:Description>
                <opla-sd:entityPositionX rdf:datatype="http://www.w3.org/2001/XMLSchema#double">275.942610227576</opla-sd:entityPositionX>
                <opla-sd:entityPositionY rdf:datatype="http://www.w3.org/2001/XMLSchema#double">20.445906674176648</opla-sd:entityPositionY>
                <rdfs:comment xml:lang="en">This is an entity positioning annotation generated by CoModIDE (https://comodide.com/). Removing this annotation will break rendering the CoModIDE schema diagram view.</rdfs:comment>
            </rdf:Description>
        </opla-sd:entityPosition>
        <rdfs:comment xml:lang="en">A type of ataxia characterised by the impairment of the ability to coordinate the movements required for normal walking. Gait ataxia is characterized by a wide-based staggering gait with a tendency to fall.</rdfs:comment>
        <rdfs:label xml:lang="en">Gait_ataxia</rdfs:label>
    </owl:Class>
    


    <!-- http://www.semanticweb.org/marthinust/ontologies/2022/8/Gait_Ontology#Gait_data -->

    <owl:Class rdf:about="http://www.semanticweb.org/marthinust/ontologies/2022/8/Gait_Ontology#Gait_data">
        <rdfs:subClassOf rdf:resource="http://www.semanticweb.org/marthinust/ontologies/2022/8/Gait_Ontology#Gait-based_Process"/>
        <rdfs:subClassOf>
            <owl:Restriction>
                <owl:onProperty rdf:resource="http://www.semanticweb.org/marthinust/ontologies/2022/8/Gait_Ontology#isAcquiredFrom"/>
                <owl:someValuesFrom rdf:resource="http://www.semanticweb.org/marthinust/ontologies/2022/8/Gait_Ontology#Gait_patient"/>
            </owl:Restriction>
        </rdfs:subClassOf>
        <rdfs:subClassOf>
            <owl:Restriction>
                <owl:onProperty rdf:resource="http://www.semanticweb.org/marthinust/ontologies/2022/8/Gait_Ontology#isAnalysedBy"/>
                <owl:someValuesFrom rdf:resource="http://www.semanticweb.org/marthinust/ontologies/2022/8/Gait_Ontology#Gait_expert"/>
            </owl:Restriction>
        </rdfs:subClassOf>
        <rdfs:subClassOf>
            <owl:Restriction>
                <owl:onProperty rdf:resource="http://www.semanticweb.org/marthinust/ontologies/2022/8/Gait_Ontology#isCollectedBy"/>
                <owl:someValuesFrom rdf:resource="http://www.semanticweb.org/marthinust/ontologies/2022/8/Gait_Ontology#Gait_acquisition"/>
            </owl:Restriction>
        </rdfs:subClassOf>
        <rdfs:subClassOf>
            <owl:Restriction>
                <owl:onProperty rdf:resource="http://www.semanticweb.org/marthinust/ontologies/2022/8/Gait_Ontology#isObtainedBy"/>
                <owl:someValuesFrom rdf:resource="http://www.semanticweb.org/marthinust/ontologies/2022/8/Gait_Ontology#Gait_Analysis_Equipment"/>
            </owl:Restriction>
        </rdfs:subClassOf>
        <opla-sd:entityPosition>
            <rdf:Description>
                <opla-sd:entityPositionX rdf:datatype="http://www.w3.org/2001/XMLSchema#double">39.33626365275739</opla-sd:entityPositionX>
                <opla-sd:entityPositionY rdf:datatype="http://www.w3.org/2001/XMLSchema#double">150.24721357835355</opla-sd:entityPositionY>
                <rdfs:comment xml:lang="en">This is an entity positioning annotation generated by CoModIDE (https://comodide.com/). Removing this annotation will break rendering the CoModIDE schema diagram view.</rdfs:comment>
            </rdf:Description>
        </opla-sd:entityPosition>
        <rdfs:comment xml:lang="en">The collection of dynamical data during human walking has a long history beginning with the first motion pictures and now with modern marker(s) based motion capture techniques, wearable sensors, and high fidelity ground reaction load measurements. This data can likely be useful for validating or generating mathematical models that are capable of simulating normal periodic gait and non-periodic, perturbed gaits that results in clinical gait data for analysis.

Gait data is often used to evaluate various aspects of gait, such as efficiency, symmetry, and stability. It can also be used to diagnose and treat gait abnormalities, to evaluate the effectiveness of interventions such as orthotic devices or physical therapy, and to assess the impact of aging or diseases on gait. Gait data can be collected and analyzed both in the laboratory and in more naturalistic environments, such as the individual&apos;s home or community.</rdfs:comment>
        <rdfs:label xml:lang="en">Gait_data</rdfs:label>
    </owl:Class>
    


    <!-- http://www.semanticweb.org/marthinust/ontologies/2022/8/Gait_Ontology#Gait_expert -->

    <owl:Class rdf:about="http://www.semanticweb.org/marthinust/ontologies/2022/8/Gait_Ontology#Gait_expert">
        <owl:equivalentClass>
            <owl:Class>
                <owl:oneOf rdf:parseType="Collection">
                    <rdf:Description rdf:about="http://www.semanticweb.org/marthinust/ontologies/2022/8/Gait_Ontology#Biomechanist"/>
                    <rdf:Description rdf:about="http://www.semanticweb.org/marthinust/ontologies/2022/8/Gait_Ontology#Healthcare_practitioner"/>
                    <rdf:Description rdf:about="http://www.semanticweb.org/marthinust/ontologies/2022/8/Gait_Ontology#Orthopedist"/>
                    <rdf:Description rdf:about="http://www.semanticweb.org/marthinust/ontologies/2022/8/Gait_Ontology#Physical_therapist"/>
                    <rdf:Description rdf:about="http://www.semanticweb.org/marthinust/ontologies/2022/8/Gait_Ontology#Podiatrist"/>
                </owl:oneOf>
            </owl:Class>
        </owl:equivalentClass>
        <rdfs:subClassOf rdf:resource="http://www.semanticweb.org/marthinust/ontologies/2022/8/Gait_Ontology#Gait-based_Process"/>
        <rdfs:subClassOf rdf:resource="http://www.semanticweb.org/marthinust/ontologies/2022/8/Gait_Ontology#Gait_Person"/>
        <rdfs:subClassOf>
            <owl:Restriction>
                <owl:onProperty rdf:resource="http://www.semanticweb.org/marthinust/ontologies/2022/8/Gait_Ontology#administers"/>
                <owl:someValuesFrom rdf:resource="http://www.semanticweb.org/marthinust/ontologies/2022/8/Gait_Ontology#Gait-based_Process"/>
            </owl:Restriction>
        </rdfs:subClassOf>
        <rdfs:subClassOf>
            <owl:Restriction>
                <owl:onProperty rdf:resource="http://www.semanticweb.org/marthinust/ontologies/2022/8/Gait_Ontology#analyzes"/>
                <owl:someValuesFrom rdf:resource="http://www.semanticweb.org/marthinust/ontologies/2022/8/Gait_Ontology#Gait_data"/>
            </owl:Restriction>
        </rdfs:subClassOf>
        <rdfs:subClassOf>
            <owl:Restriction>
                <owl:onProperty rdf:resource="http://www.semanticweb.org/marthinust/ontologies/2022/8/Gait_Ontology#facilitates"/>
                <owl:someValuesFrom rdf:resource="http://www.semanticweb.org/marthinust/ontologies/2022/8/Gait_Ontology#Gait_analysis"/>
            </owl:Restriction>
        </rdfs:subClassOf>
        <rdfs:subClassOf>
            <owl:Restriction>
                <owl:onProperty rdf:resource="http://www.semanticweb.org/marthinust/ontologies/2022/8/Gait_Ontology#observes"/>
                <owl:someValuesFrom rdf:resource="http://www.semanticweb.org/marthinust/ontologies/2022/8/Gait_Ontology#Gait_Cycle"/>
            </owl:Restriction>
        </rdfs:subClassOf>
        <rdfs:subClassOf>
            <owl:Restriction>
                <owl:onProperty rdf:resource="http://www.semanticweb.org/marthinust/ontologies/2022/8/Gait_Ontology#prescribes"/>
                <owl:someValuesFrom rdf:resource="http://www.semanticweb.org/marthinust/ontologies/2022/8/Gait_Ontology#Gait_Assistive_Technology"/>
            </owl:Restriction>
        </rdfs:subClassOf>
        <rdfs:subClassOf>
            <owl:Restriction>
                <owl:onProperty rdf:resource="http://www.semanticweb.org/marthinust/ontologies/2022/8/Gait_Ontology#treats"/>
                <owl:someValuesFrom rdf:resource="http://www.semanticweb.org/marthinust/ontologies/2022/8/Gait_Ontology#Gait_patient"/>
            </owl:Restriction>
        </rdfs:subClassOf>
        <opla-sd:entityPosition>
            <rdf:Description>
                <opla-sd:entityPositionX rdf:datatype="http://www.w3.org/2001/XMLSchema#double">135.8830287946281</opla-sd:entityPositionX>
                <opla-sd:entityPositionY rdf:datatype="http://www.w3.org/2001/XMLSchema#double">198.40739235793347</opla-sd:entityPositionY>
                <rdfs:comment xml:lang="en">This is an entity positioning annotation generated by CoModIDE (https://comodide.com/). Removing this annotation will break rendering the CoModIDE schema diagram view.</rdfs:comment>
            </rdf:Description>
        </opla-sd:entityPosition>
        <rdfs:comment xml:lang="en">An expert who specialises in the musculoskeletal system including bones, joints, ligaments, tendons and muscles that use gait assessments to help diagnose injuries that affect or inhibit everyday movements like walking or running.

Gait experts may work in a variety of settings, including hospitals, clinics, and research institutions. They may be involved in the diagnosis and treatment of gait abnormalities, the evaluation of interventions such as orthotic devices or physical therapy, and the assessment of the impact of aging or diseases on gait.

Gait experts may also be involved in the development and validation of new methods and technologies for gait analysis. Gait experts may have a background in fields such as physical therapy, kinesiology, biomechanics, or engineering.</rdfs:comment>
        <rdfs:label xml:lang="en">Gait_expert</rdfs:label>
    </owl:Class>
    


    <!-- http://www.semanticweb.org/marthinust/ontologies/2022/8/Gait_Ontology#Gait_imbalance -->

    <owl:Class rdf:about="http://www.semanticweb.org/marthinust/ontologies/2022/8/Gait_Ontology#Gait_imbalance">
        <rdfs:subClassOf rdf:resource="http://www.semanticweb.org/marthinust/ontologies/2022/8/Gait_Ontology#Gait_Disturbance"/>
    </owl:Class>
    


    <!-- http://www.semanticweb.org/marthinust/ontologies/2022/8/Gait_Ontology#Gait_instability_worse_in_the_dark -->

    <owl:Class rdf:about="http://www.semanticweb.org/marthinust/ontologies/2022/8/Gait_Ontology#Gait_instability_worse_in_the_dark">
        <rdfs:subClassOf rdf:resource="http://www.semanticweb.org/marthinust/ontologies/2022/8/Gait_Ontology#Unsteady_gait"/>
        <opla-sd:entityPosition>
            <rdf:Description>
                <opla-sd:entityPositionX rdf:datatype="http://www.w3.org/2001/XMLSchema#double">200.09219140401194</opla-sd:entityPositionX>
                <opla-sd:entityPositionY rdf:datatype="http://www.w3.org/2001/XMLSchema#double">47.114430375300465</opla-sd:entityPositionY>
                <rdfs:comment xml:lang="en">This is an entity positioning annotation generated by CoModIDE (https://comodide.com/). Removing this annotation will break rendering the CoModIDE schema diagram view.</rdfs:comment>
            </rdf:Description>
        </opla-sd:entityPosition>
        <rdfs:comment xml:lang="en">Unstable walking, worse in the dark.</rdfs:comment>
        <rdfs:label xml:lang="en">Gait_instability_worse_in_the_dark</rdfs:label>
    </owl:Class>
    


    <!-- http://www.semanticweb.org/marthinust/ontologies/2022/8/Gait_Ontology#Gait_observations -->

    <owl:Class rdf:about="http://www.semanticweb.org/marthinust/ontologies/2022/8/Gait_Ontology#Gait_observations">
        <rdfs:subClassOf rdf:resource="http://www.semanticweb.org/marthinust/ontologies/2022/8/Gait_Ontology#Gait_Analysis_Method"/>
        <opla-sd:entityPosition>
            <rdf:Description>
                <opla-sd:entityPositionX rdf:datatype="http://www.w3.org/2001/XMLSchema#double">241.71157114168335</opla-sd:entityPositionX>
                <opla-sd:entityPositionY rdf:datatype="http://www.w3.org/2001/XMLSchema#double">27.905408441349355</opla-sd:entityPositionY>
                <rdfs:comment xml:lang="en">This is an entity positioning annotation generated by CoModIDE (https://comodide.com/). Removing this annotation will break rendering the CoModIDE schema diagram view.</rdfs:comment>
            </rdf:Description>
        </opla-sd:entityPosition>
        <rdfs:comment xml:lang="en">Gait (analysis) process assessment is administered by the gait expert.

By simply observing the gait and noting abnormalities is of little value by itself. It needs to be followed by gait assessment, which is the synthesis of these observations with other information about the subject, obtained from the history and physical examination, combined with the intelligence and experience of the observer. Visual gait analysis is entirely subjective and the quality of the analysis depends on the skill of the person performing it. It can be an interesting exercise to perform visual gait analysis on people walking past in the street, but without knowing their clinical details it is easy to misinterpret what is wrong with them. When performing any type of gait analysis, one thing that must be constantly borne in mind is that you are observing effects and not causes.</rdfs:comment>
        <rdfs:label xml:lang="en">Gait_observations</rdfs:label>
    </owl:Class>
    


    <!-- http://www.semanticweb.org/marthinust/ontologies/2022/8/Gait_Ontology#Gait_patient -->

    <owl:Class rdf:about="http://www.semanticweb.org/marthinust/ontologies/2022/8/Gait_Ontology#Gait_patient">
        <owl:equivalentClass>
            <owl:Class>
                <owl:oneOf rdf:parseType="Collection">
                    <rdf:Description rdf:about="http://www.semanticweb.org/marthinust/ontologies/2022/8/Gait_Ontology#Adolescent"/>
                    <rdf:Description rdf:about="http://www.semanticweb.org/marthinust/ontologies/2022/8/Gait_Ontology#Adult"/>
                    <rdf:Description rdf:about="http://www.semanticweb.org/marthinust/ontologies/2022/8/Gait_Ontology#Athlete"/>
                    <rdf:Description rdf:about="http://www.semanticweb.org/marthinust/ontologies/2022/8/Gait_Ontology#Child"/>
                    <rdf:Description rdf:about="http://www.semanticweb.org/marthinust/ontologies/2022/8/Gait_Ontology#Elderly"/>
                </owl:oneOf>
            </owl:Class>
        </owl:equivalentClass>
        <rdfs:subClassOf rdf:resource="http://www.semanticweb.org/marthinust/ontologies/2022/8/Gait_Ontology#Gait-based_Process"/>
        <rdfs:subClassOf rdf:resource="http://www.semanticweb.org/marthinust/ontologies/2022/8/Gait_Ontology#Gait_Person"/>
        <rdfs:subClassOf>
            <owl:Restriction>
                <owl:onProperty rdf:resource="http://www.semanticweb.org/marthinust/ontologies/2022/8/Gait_Ontology#demonstrates"/>
                <owl:someValuesFrom rdf:resource="http://www.semanticweb.org/marthinust/ontologies/2022/8/Gait_Ontology#Gait_Cycle"/>
            </owl:Restriction>
        </rdfs:subClassOf>
        <rdfs:subClassOf>
            <owl:Restriction>
                <owl:onProperty rdf:resource="http://www.semanticweb.org/marthinust/ontologies/2022/8/Gait_Ontology#exhibits"/>
                <owl:someValuesFrom rdf:resource="http://www.semanticweb.org/marthinust/ontologies/2022/8/Gait_Ontology#Type_of_Gait"/>
            </owl:Restriction>
        </rdfs:subClassOf>
        <rdfs:subClassOf>
            <owl:Restriction>
                <owl:onProperty rdf:resource="http://www.semanticweb.org/marthinust/ontologies/2022/8/Gait_Ontology#isAffectedBy"/>
                <owl:someValuesFrom rdf:resource="http://www.semanticweb.org/marthinust/ontologies/2022/8/Gait_Ontology#Gait_Disturbance"/>
            </owl:Restriction>
        </rdfs:subClassOf>
        <rdfs:subClassOf>
            <owl:Restriction>
                <owl:onProperty rdf:resource="http://www.semanticweb.org/marthinust/ontologies/2022/8/Gait_Ontology#isAssessedIn"/>
                <owl:someValuesFrom rdf:resource="http://www.semanticweb.org/marthinust/ontologies/2022/8/Gait_Ontology#Gait-based_Process"/>
            </owl:Restriction>
        </rdfs:subClassOf>
        <rdfs:subClassOf>
            <owl:Restriction>
                <owl:onProperty rdf:resource="http://www.semanticweb.org/marthinust/ontologies/2022/8/Gait_Ontology#isAssignedWith"/>
                <owl:someValuesFrom rdf:resource="http://www.semanticweb.org/marthinust/ontologies/2022/8/Gait_Ontology#Gait_Assistive_Technology"/>
            </owl:Restriction>
        </rdfs:subClassOf>
        <rdfs:subClassOf>
            <owl:Restriction>
                <owl:onProperty rdf:resource="http://www.semanticweb.org/marthinust/ontologies/2022/8/Gait_Ontology#isClassedIn"/>
                <owl:someValuesFrom rdf:resource="http://www.semanticweb.org/marthinust/ontologies/2022/8/Gait_Ontology#Gait_Classification"/>
            </owl:Restriction>
        </rdfs:subClassOf>
        <rdfs:subClassOf>
            <owl:Restriction>
                <owl:onProperty rdf:resource="http://www.semanticweb.org/marthinust/ontologies/2022/8/Gait_Ontology#isInvolvedIn"/>
                <owl:someValuesFrom rdf:resource="http://www.semanticweb.org/marthinust/ontologies/2022/8/Gait_Ontology#Gait_acquisition"/>
            </owl:Restriction>
        </rdfs:subClassOf>
        <rdfs:subClassOf>
            <owl:Restriction>
                <owl:onProperty rdf:resource="http://www.semanticweb.org/marthinust/ontologies/2022/8/Gait_Ontology#isLinkedWith"/>
                <owl:someValuesFrom rdf:resource="http://www.semanticweb.org/marthinust/ontologies/2022/8/Gait_Ontology#Gait-related_Disease"/>
            </owl:Restriction>
        </rdfs:subClassOf>
        <rdfs:subClassOf>
            <owl:Restriction>
                <owl:onProperty rdf:resource="http://www.semanticweb.org/marthinust/ontologies/2022/8/Gait_Ontology#isMonitoredBy"/>
                <owl:someValuesFrom rdf:resource="http://www.semanticweb.org/marthinust/ontologies/2022/8/Gait_Ontology#Gait_Analysis_Equipment"/>
            </owl:Restriction>
        </rdfs:subClassOf>
        <rdfs:subClassOf>
            <owl:Restriction>
                <owl:onProperty rdf:resource="http://www.semanticweb.org/marthinust/ontologies/2022/8/Gait_Ontology#isTreatedBy"/>
                <owl:someValuesFrom rdf:resource="http://www.semanticweb.org/marthinust/ontologies/2022/8/Gait_Ontology#Gait_expert"/>
            </owl:Restriction>
        </rdfs:subClassOf>
        <opla-sd:entityPosition>
            <rdf:Description>
                <opla-sd:entityPositionX rdf:datatype="http://www.w3.org/2001/XMLSchema#double">284.69865093902456</opla-sd:entityPositionX>
                <opla-sd:entityPositionY rdf:datatype="http://www.w3.org/2001/XMLSchema#double">111.852221480122</opla-sd:entityPositionY>
                <rdfs:comment xml:lang="en">This is an entity positioning annotation generated by CoModIDE (https://comodide.com/). Removing this annotation will break rendering the CoModIDE schema diagram view.</rdfs:comment>
            </rdf:Description>
        </opla-sd:entityPosition>
        <rdfs:comment xml:lang="en">A person who suffers from any harm, impairment or situation. 
A person who is impacted by a harmful situation or disease.</rdfs:comment>
        <rdfs:label xml:lang="en">Gait_patient</rdfs:label>
    </owl:Class>
    


    <!-- http://www.semanticweb.org/marthinust/ontologies/2022/8/Gait_Ontology#Gait_training -->

    <owl:Class rdf:about="http://www.semanticweb.org/marthinust/ontologies/2022/8/Gait_Ontology#Gait_training">
        <rdfs:subClassOf rdf:resource="http://www.semanticweb.org/marthinust/ontologies/2022/8/Gait_Ontology#Physical_therapy"/>
        <opla-sd:entityPosition>
            <rdf:Description>
                <opla-sd:entityPositionX rdf:datatype="http://www.w3.org/2001/XMLSchema#double">59.5115103511289</opla-sd:entityPositionX>
                <opla-sd:entityPositionY rdf:datatype="http://www.w3.org/2001/XMLSchema#double">21.929443264245307</opla-sd:entityPositionY>
                <rdfs:comment xml:lang="en">This is an entity positioning annotation generated by CoModIDE (https://comodide.com/). Removing this annotation will break rendering the CoModIDE schema diagram view.</rdfs:comment>
            </rdf:Description>
        </opla-sd:entityPosition>
        <rdfs:comment xml:lang="en">Gait training is physical therapy to improve walking. It may be part of an overall physical therapy program to treat an injury or a physical condition that limits or prohibits the ability to walk or walking correctly.

Gait training is a set of exercises that are specifically implemented by your physical therapist to help you walk better. It can help improve your ability to stand and walk. Your doctor may recommend gait training if youve had an illness or injury that affects your ability to get around. It may help you gain independence in walking, even if you need an assistive device.</rdfs:comment>
        <rdfs:label xml:lang="en">Gait_training</rdfs:label>
    </owl:Class>
    


    <!-- http://www.semanticweb.org/marthinust/ontologies/2022/8/Gait_Ontology#Genu_recurvatum -->

    <owl:Class rdf:about="http://www.semanticweb.org/marthinust/ontologies/2022/8/Gait_Ontology#Genu_recurvatum">
        <rdfs:subClassOf rdf:resource="http://www.semanticweb.org/marthinust/ontologies/2022/8/Gait_Ontology#Knee"/>
        <opla-sd:entityPosition>
            <rdf:Description>
                <opla-sd:entityPositionX rdf:datatype="http://www.w3.org/2001/XMLSchema#double">151.63543885732562</opla-sd:entityPositionX>
                <opla-sd:entityPositionY rdf:datatype="http://www.w3.org/2001/XMLSchema#double">33.8517538479403</opla-sd:entityPositionY>
                <rdfs:comment xml:lang="en">This is an entity positioning annotation generated by CoModIDE (https://comodide.com/). Removing this annotation will break rendering the CoModIDE schema diagram view.</rdfs:comment>
            </rdf:Description>
        </opla-sd:entityPosition>
        <rdfs:comment xml:lang="en">Genu recurvatum is a deformity in the knee joint, so that the knee bends backwards. In this deformity, excessive extension occurs in the tibiofemoral joint. Genu recurvatum is also called knee hyperextension and back knee. This deformity is more common in women and people with familial ligamentous laxity. 

Individuals with genu recurvatum may experience knee pain, display an extension gait pattern, and have poor proprioceptive control of terminal knee extension.</rdfs:comment>
        <rdfs:label xml:lang="en">Genu_recurvatum</rdfs:label>
    </owl:Class>
    


    <!-- http://www.semanticweb.org/marthinust/ontologies/2022/8/Gait_Ontology#Genu_recurvatum_gait -->

    <owl:Class rdf:about="http://www.semanticweb.org/marthinust/ontologies/2022/8/Gait_Ontology#Genu_recurvatum_gait">
        <rdfs:subClassOf rdf:resource="http://www.semanticweb.org/marthinust/ontologies/2022/8/Gait_Ontology#Gait_Disturbance"/>
        <opla-sd:entityPosition>
            <rdf:Description>
                <opla-sd:entityPositionX rdf:datatype="http://www.w3.org/2001/XMLSchema#double">214.157745946056</opla-sd:entityPositionX>
                <opla-sd:entityPositionY rdf:datatype="http://www.w3.org/2001/XMLSchema#double">299.40026078116165</opla-sd:entityPositionY>
                <rdfs:comment xml:lang="en">This is an entity positioning annotation generated by CoModIDE (https://comodide.com/). Removing this annotation will break rendering the CoModIDE schema diagram view.</rdfs:comment>
            </rdf:Description>
        </opla-sd:entityPosition>
        <rdfs:comment xml:lang="en">Genu recurvatum is a gait pattern characterized by hyperextension of the knee joint during the stance phase of gait. It is caused by a weakness in the quadriceps and hamstring muscles, which are responsible for knee flexion and extension, respectively. This gait pattern can lead to pain and fatigue in the legs and lower back, as well as an increased risk of falls. Treatment includes exercises to strengthen the quadriceps and hamstrings, as well as physical therapy to improve balance and gait patterns.</rdfs:comment>
        <rdfs:label xml:lang="en">Genu_recurvatum_gait (Hamstring gait)</rdfs:label>
    </owl:Class>
    


    <!-- http://www.semanticweb.org/marthinust/ontologies/2022/8/Gait_Ontology#Geriatric_gait -->

    <owl:Class rdf:about="http://www.semanticweb.org/marthinust/ontologies/2022/8/Gait_Ontology#Geriatric_gait">
        <rdfs:subClassOf rdf:resource="http://www.semanticweb.org/marthinust/ontologies/2022/8/Gait_Ontology#Gait_Pathology"/>
        <rdfs:subClassOf>
            <owl:Restriction>
                <owl:onProperty rdf:resource="http://www.semanticweb.org/marthinust/ontologies/2022/8/Gait_Ontology#hasAgeGroup"/>
                <owl:hasValue rdf:resource="http://www.semanticweb.org/marthinust/ontologies/2022/8/Gait_Ontology#Elderly"/>
            </owl:Restriction>
        </rdfs:subClassOf>
        <opla-sd:entityPosition>
            <rdf:Description>
                <opla-sd:entityPositionX rdf:datatype="http://www.w3.org/2001/XMLSchema#double">151.40194577001066</opla-sd:entityPositionX>
                <opla-sd:entityPositionY rdf:datatype="http://www.w3.org/2001/XMLSchema#double">5.324045666656274</opla-sd:entityPositionY>
                <rdfs:comment xml:lang="en">This is an entity positioning annotation generated by CoModIDE (https://comodide.com/). Removing this annotation will break rendering the CoModIDE schema diagram view.</rdfs:comment>
            </rdf:Description>
        </opla-sd:entityPosition>
        <rdfs:comment xml:lang="en">Geriatric, also known as old age-related gait pathology is a term used to describe the changes in walking pattern and mobility that can occur in older adults as a result of age-related changes in the body. As people age, they may experience changes in their musculoskeletal system, nervous system, and overall health that can affect their gait and mobility. These changes can be caused by a variety of factors, including a decrease in muscle strength, flexibility, and coordination; changes in balance and sensory perception; and the development of chronic medical conditions such as arthritis or Parkinson&apos;s disease.

Ageing is associated with a decline in gait speed, shorter step length and slower cadence. These changes provide greater stability because both feet are on the ground simultaneously for a greater percentage of the cycle. This factors interplay to results in increase in prevalence of gait disorders among older adults. Common gait disorders in older adults under neurological causes are sensory ataxia, Parkinsonism &amp; frontal gait disorders. While non-neurological ( includes hip and knee osteoarthritis).</rdfs:comment>
        <rdfs:label xml:lang="en">Geriatric_gait</rdfs:label>
    </owl:Class>
    


    <!-- http://www.semanticweb.org/marthinust/ontologies/2022/8/Gait_Ontology#Glutues_maximus_gait -->

    <owl:Class rdf:about="http://www.semanticweb.org/marthinust/ontologies/2022/8/Gait_Ontology#Glutues_maximus_gait">
        <rdfs:subClassOf rdf:resource="http://www.semanticweb.org/marthinust/ontologies/2022/8/Gait_Ontology#Gait_Disturbance"/>
        <opla-sd:entityPosition>
            <rdf:Description>
                <opla-sd:entityPositionX rdf:datatype="http://www.w3.org/2001/XMLSchema#double">290.7992257886882</opla-sd:entityPositionX>
                <opla-sd:entityPositionY rdf:datatype="http://www.w3.org/2001/XMLSchema#double">201.09615582663844</opla-sd:entityPositionY>
                <rdfs:comment xml:lang="en">This is an entity positioning annotation generated by CoModIDE (https://comodide.com/). Removing this annotation will break rendering the CoModIDE schema diagram view.</rdfs:comment>
            </rdf:Description>
        </opla-sd:entityPosition>
        <rdfs:comment xml:lang="en">Gluteus maximus gait is a walking pattern characterized by an inability to extend the hip during the stance phase of gait. It is caused by a weakness in the gluteus maximus muscle, which is the largest of the gluteal muscles and is responsible for hip extension. This weakness can lead to an abnormal gait pattern, with the person leaning their body backwards to maintain balance. This gait can lead to pain and fatigue in the legs and lower back, as well as an increased risk of falls. Treatment includes exercises to strengthen the gluteal muscles, as well as physical therapy to improve balance and gait patterns.

Normally the gluteus maximus contracts at the point of heel strike during gait, arresting hip flexion, and thereby slowing forward motion of the trunk. A weakened gluteus maximus causes a backwards lurch (trunk extension) at heel strike on the weakened side, interrupting the forward motion of the trunk.</rdfs:comment>
        <rdfs:label xml:lang="en">Gluteus_maximus_gait</rdfs:label>
    </owl:Class>
    


    <!-- http://www.semanticweb.org/marthinust/ontologies/2022/8/Gait_Ontology#Goniometers -->

    <owl:Class rdf:about="http://www.semanticweb.org/marthinust/ontologies/2022/8/Gait_Ontology#Goniometers">
        <rdfs:subClassOf rdf:resource="http://www.semanticweb.org/marthinust/ontologies/2022/8/Gait_Ontology#Gait_Analysis_Equipment"/>
        <opla-sd:entityPosition>
            <rdf:Description>
                <opla-sd:entityPositionX rdf:datatype="http://www.w3.org/2001/XMLSchema#double">209.83819440328267</opla-sd:entityPositionX>
                <opla-sd:entityPositionY rdf:datatype="http://www.w3.org/2001/XMLSchema#double">202.9515231163919</opla-sd:entityPositionY>
                <rdfs:comment xml:lang="en">This is an entity positioning annotation generated by CoModIDE (https://comodide.com/). Removing this annotation will break rendering the CoModIDE schema diagram view.</rdfs:comment>
            </rdf:Description>
        </opla-sd:entityPosition>
        <rdfs:comment xml:lang="en">Unlike the inertial sensor, the flexible goniometer is operated by measuring the change in the physical signal resulting from the angular change. A flexible goniometer can be used to measure the relative rotation between two human body segments.

The flexible goniometers used in gait analysis can be divided into strain gauges, mechanical flexible, inductive, and optical fiber goniometers. A number of flexible electrogoniometers based on a strain gauge have been developed and used for angle measurement in gait analysis since the 1980s. At present, numerous commercialised flexible electrogoniometers are available for the measurement of human posture and spinal motion. A mechanical flexible goniometer is designed to obtain angular change by measuring the longitudinal displacement of two parallel wires bent in the plane of rotation, which is demonstrated by measuring the knee joint during human walking.</rdfs:comment>
        <rdfs:label xml:lang="en">Goniometer</rdfs:label>
    </owl:Class>
    


    <!-- http://www.semanticweb.org/marthinust/ontologies/2022/8/Gait_Ontology#Guillain-Barr_syndrome -->

    <owl:Class rdf:about="http://www.semanticweb.org/marthinust/ontologies/2022/8/Gait_Ontology#Guillain-Barr_syndrome">
        <rdfs:subClassOf rdf:resource="http://www.semanticweb.org/marthinust/ontologies/2022/8/Gait_Ontology#Gait-related_Disease"/>
        <opla-sd:entityPosition>
            <rdf:Description>
                <opla-sd:entityPositionX rdf:datatype="http://www.w3.org/2001/XMLSchema#double">144.7824413993102</opla-sd:entityPositionX>
                <opla-sd:entityPositionY rdf:datatype="http://www.w3.org/2001/XMLSchema#double">276.29398318026404</opla-sd:entityPositionY>
                <rdfs:comment xml:lang="en">This is an entity positioning annotation generated by CoModIDE (https://comodide.com/). Removing this annotation will break rendering the CoModIDE schema diagram view.</rdfs:comment>
            </rdf:Description>
        </opla-sd:entityPosition>
        <rdfs:comment xml:lang="en">Guillain-Barre Syndrome is a problem with your nervous system. It can cause muscle weakness, reflex loss, and numbness or tingling in parts of your body. It can lead to paralysis, which is usually temporary. It mainly affects the feet, hands and limbs, causing problems such as numbness, weakness and pain. It can be treated and most people will eventually make a full recovery, although it can occasionally be life-threatening and some people are left with long-term problems.</rdfs:comment>
        <rdfs:label xml:lang="en">Guillain-Barr_syndrome</rdfs:label>
    </owl:Class>
    


    <!-- http://www.semanticweb.org/marthinust/ontologies/2022/8/Gait_Ontology#Gyroscopic_sensors -->

    <owl:Class rdf:about="http://www.semanticweb.org/marthinust/ontologies/2022/8/Gait_Ontology#Gyroscopic_sensors">
        <rdfs:subClassOf rdf:resource="http://www.semanticweb.org/marthinust/ontologies/2022/8/Gait_Ontology#Gait_Analysis_Equipment"/>
        <opla-sd:entityPosition>
            <rdf:Description>
                <opla-sd:entityPositionX rdf:datatype="http://www.w3.org/2001/XMLSchema#double">96.43195000145425</opla-sd:entityPositionX>
                <opla-sd:entityPositionY rdf:datatype="http://www.w3.org/2001/XMLSchema#double">15.662032467286746</opla-sd:entityPositionY>
                <rdfs:comment xml:lang="en">This is an entity positioning annotation generated by CoModIDE (https://comodide.com/). Removing this annotation will break rendering the CoModIDE schema diagram view.</rdfs:comment>
            </rdf:Description>
        </opla-sd:entityPosition>
        <rdfs:comment xml:lang="en">A gyroscope is an angular velocity sensor. The micromachined gyroscope is based on the concept of measuring the Coriolis force, which is an apparent force proportional to the angular rate of rotation in a rotating reference frame. By detecting the linear motion from the Coriolis effort and performing an integration of the gyroscopic signal, the angular rate can be obtained. In addition, gyroscopes based on other operating principles also exist, such as the electronic, microchip-packaged MEMS gyroscope devices found in consumer electronic devices, solid-state ring lasers, fiber optic gyroscopes, and the extremely sensitive quantum gyroscope. A gyroscope can be applied for the measurement of the motion and posture of the human segment in gait analysis by measuring the angular rate. For example, by attaching a gyroscope to human feet or legs, the angular velocity and angle of feet or legs during the gait can be determined to realise the reorganisation of the various gait phases. In the gait analysis, a gyroscope is usually combined with an accelerometer to construct a complete initial sensing system.</rdfs:comment>
        <rdfs:label xml:lang="en">Gyroscopic_sensor</rdfs:label>
    </owl:Class>
    


    <!-- http://www.semanticweb.org/marthinust/ontologies/2022/8/Gait_Ontology#HIp_extensor_weakness -->

    <owl:Class rdf:about="http://www.semanticweb.org/marthinust/ontologies/2022/8/Gait_Ontology#HIp_extensor_weakness">
        <rdfs:subClassOf rdf:resource="http://www.semanticweb.org/marthinust/ontologies/2022/8/Gait_Ontology#Hip"/>
        <opla-sd:entityPosition>
            <rdf:Description>
                <opla-sd:entityPositionX rdf:datatype="http://www.w3.org/2001/XMLSchema#double">270.26302279373573</opla-sd:entityPositionX>
                <opla-sd:entityPositionY rdf:datatype="http://www.w3.org/2001/XMLSchema#double">130.15781487594012</opla-sd:entityPositionY>
                <rdfs:comment xml:lang="en">This is an entity positioning annotation generated by CoModIDE (https://comodide.com/). Removing this annotation will break rendering the CoModIDE schema diagram view.</rdfs:comment>
            </rdf:Description>
        </opla-sd:entityPosition>
        <rdfs:comment xml:lang="en">Hip extensor weakness (Posterior lurch gait): Backward trunk lean with hyperextended hip during stance phase of affected limb. This action moves the line of gravity of the trunk behind the hip and reduces the need for hip extension torque.
Pathomechanism: Use of iliofemoral ligament to lock hip in extension to prevent trunk falling forward.

Weak Hip Extensors will cause a person to take a smaller step to lessen the hip flexion required for initial contact, resulting in a lesser force of contraction required from the extensors. Overall gait will be slower to allow time for limb stabilisation. Compensation is increased posterior trunk positioning to maintain alignment of the pelvis in relation to the trunk</rdfs:comment>
        <rdfs:label xml:lang="en">Hip_extensor_weakness</rdfs:label>
    </owl:Class>
    


    <!-- http://www.semanticweb.org/marthinust/ontologies/2022/8/Gait_Ontology#Hallux_rigidus -->

    <owl:Class rdf:about="http://www.semanticweb.org/marthinust/ontologies/2022/8/Gait_Ontology#Hallux_rigidus">
        <rdfs:subClassOf rdf:resource="http://www.semanticweb.org/marthinust/ontologies/2022/8/Gait_Ontology#Foot"/>
    </owl:Class>
    


    <!-- http://www.semanticweb.org/marthinust/ontologies/2022/8/Gait_Ontology#Heart_disease -->

    <owl:Class rdf:about="http://www.semanticweb.org/marthinust/ontologies/2022/8/Gait_Ontology#Heart_disease">
        <rdfs:subClassOf rdf:resource="http://www.semanticweb.org/marthinust/ontologies/2022/8/Gait_Ontology#Morbidity"/>
        <opla-sd:entityPosition>
            <rdf:Description>
                <opla-sd:entityPositionX rdf:datatype="http://www.w3.org/2001/XMLSchema#double">35.76128874339597</opla-sd:entityPositionX>
                <opla-sd:entityPositionY rdf:datatype="http://www.w3.org/2001/XMLSchema#double">208.28104567646164</opla-sd:entityPositionY>
                <rdfs:comment xml:lang="en">This is an entity positioning annotation generated by CoModIDE (https://comodide.com/). Removing this annotation will break rendering the CoModIDE schema diagram view.</rdfs:comment>
            </rdf:Description>
        </opla-sd:entityPosition>
        <rdfs:comment xml:lang="en">Heart disease (developed over time) can cause a person to experience fatigue, shortness of breath, and other symptoms that can make it difficult to walk.</rdfs:comment>
        <rdfs:label xml:lang="en">Heart_disease</rdfs:label>
    </owl:Class>
    


    <!-- http://www.semanticweb.org/marthinust/ontologies/2022/8/Gait_Ontology#Hemiparetic -->

    <owl:Class rdf:about="http://www.semanticweb.org/marthinust/ontologies/2022/8/Gait_Ontology#Hemiparetic">
        <rdfs:subClassOf rdf:resource="http://www.semanticweb.org/marthinust/ontologies/2022/8/Gait_Ontology#Neurological"/>
        <opla-sd:entityPosition>
            <rdf:Description>
                <opla-sd:entityPositionX rdf:datatype="http://www.w3.org/2001/XMLSchema#double">206.3119868096125</opla-sd:entityPositionX>
                <opla-sd:entityPositionY rdf:datatype="http://www.w3.org/2001/XMLSchema#double">120.87838767782331</opla-sd:entityPositionY>
                <rdfs:comment xml:lang="en">This is an entity positioning annotation generated by CoModIDE (https://comodide.com/). Removing this annotation will break rendering the CoModIDE schema diagram view.</rdfs:comment>
            </rdf:Description>
        </opla-sd:entityPosition>
        <rdfs:comment xml:lang="en">Hemiparetic: Paretic side with flexor muscle synergy noted. Typical features are as follows for the affected side: Upper arm is adducted and internally rotated with flexion at the shoulder, elbow, and wrist. Hip and knee flexed. Foot inverted and plantarflexed. Lower leg circumducts during swing phase, also known as Wernicke-Mann gait.. It involves the brain hemispheres or injury.</rdfs:comment>
        <rdfs:label xml:lang="en">Hemiparetic</rdfs:label>
    </owl:Class>
    


    <!-- http://www.semanticweb.org/marthinust/ontologies/2022/8/Gait_Ontology#Hemiplegia -->

    <owl:Class rdf:about="http://www.semanticweb.org/marthinust/ontologies/2022/8/Gait_Ontology#Hemiplegia">
        <rdfs:subClassOf rdf:resource="http://www.semanticweb.org/marthinust/ontologies/2022/8/Gait_Ontology#Gait-related_Disease"/>
        <opla-sd:entityPosition>
            <rdf:Description>
                <opla-sd:entityPositionX rdf:datatype="http://www.w3.org/2001/XMLSchema#double">123.76840614184603</opla-sd:entityPositionX>
                <opla-sd:entityPositionY rdf:datatype="http://www.w3.org/2001/XMLSchema#double">87.68141308318903</opla-sd:entityPositionY>
                <rdfs:comment xml:lang="en">This is an entity positioning annotation generated by CoModIDE (https://comodide.com/). Removing this annotation will break rendering the CoModIDE schema diagram view.</rdfs:comment>
            </rdf:Description>
        </opla-sd:entityPosition>
        <rdfs:comment xml:lang="en">Hemiplegia is a symptom that involves one-sided paralysis. Hemiplegia affects either the right or left side of your body. It happens because of brain or spinal cord injuries and conditions. Depending on the cause, hemiplegia can be temporary or permanent.</rdfs:comment>
        <rdfs:label xml:lang="en">Hemiplegia</rdfs:label>
    </owl:Class>
    


    <!-- http://www.semanticweb.org/marthinust/ontologies/2022/8/Gait_Ontology#Hemiplegic_gait -->

    <owl:Class rdf:about="http://www.semanticweb.org/marthinust/ontologies/2022/8/Gait_Ontology#Hemiplegic_gait">
        <rdfs:subClassOf rdf:resource="http://www.semanticweb.org/marthinust/ontologies/2022/8/Gait_Ontology#Type_of_Gait"/>
        <opla-sd:entityPosition>
            <rdf:Description>
                <opla-sd:entityPositionX rdf:datatype="http://www.w3.org/2001/XMLSchema#double">165.36606038794903</opla-sd:entityPositionX>
                <opla-sd:entityPositionY rdf:datatype="http://www.w3.org/2001/XMLSchema#double">253.43448471848788</opla-sd:entityPositionY>
                <rdfs:comment xml:lang="en">This is an entity positioning annotation generated by CoModIDE (https://comodide.com/). Removing this annotation will break rendering the CoModIDE schema diagram view.</rdfs:comment>
            </rdf:Description>
        </opla-sd:entityPosition>
        <rdfs:comment xml:lang="en">Hemiplegic gait is a type of abnormal gait that occurs in individuals who have experienced hemiplegia, a condition characterised by weakness or paralysis on one side of the body, often resulting from a stroke, brain injury, or other neurological disorders. Hemiplegic gait is marked by distinctive features that stem from the affected side&apos;s muscle weakness, lack of coordination, and impaired motor function.

In a hemiplegic gait, the affected leg is often stiff and extended, with the foot dragging or scuffing the ground during the swing phase of walking. The person may circumduct their leg, meaning they swing it outward in a semi-circular motion to clear the ground due to weakness in the hip and knee flexors. Additionally, the affected arm may be flexed and held close to the body, with little to no movement during the walking process.

Hemiplegic gait can significantly impact an individual&apos;s mobility, balance, and independence. Treatment options for hemiplegic gait may include physical therapy, gait training, orthotics, and assistive devices such as canes or walkers to improve walking ability and safety.</rdfs:comment>
        <rdfs:label xml:lang="en">Hemiplegic_gait</rdfs:label>
    </owl:Class>
    


    <!-- http://www.semanticweb.org/marthinust/ontologies/2022/8/Gait_Ontology#Hip -->

    <owl:Class rdf:about="http://www.semanticweb.org/marthinust/ontologies/2022/8/Gait_Ontology#Hip">
        <rdfs:subClassOf rdf:resource="http://www.semanticweb.org/marthinust/ontologies/2022/8/Gait_Ontology#Musculoskeletal"/>
        <opla-sd:entityPosition>
            <rdf:Description>
                <opla-sd:entityPositionX rdf:datatype="http://www.w3.org/2001/XMLSchema#double">176.89933671509633</opla-sd:entityPositionX>
                <opla-sd:entityPositionY rdf:datatype="http://www.w3.org/2001/XMLSchema#double">284.37207870785153</opla-sd:entityPositionY>
                <rdfs:comment xml:lang="en">This is an entity positioning annotation generated by CoModIDE (https://comodide.com/). Removing this annotation will break rendering the CoModIDE schema diagram view.</rdfs:comment>
            </rdf:Description>
        </opla-sd:entityPosition>
        <rdfs:comment xml:lang="en">The hip is one of the body&apos;s largest joints. It is a ball-and-socket joint. The socket is formed by the acetabulum, which is part of the pelvis bone. The ball is the femoral head, which is the upper end of the femur (thighbone).

The hip joint is the junction where the hip joins the leg to the trunk of the body. It is comprised of two bones: the thighbone or femur, and the pelvis, which is made up of three bones called ilium, ischium and pubis. The ball of the hip joint is made by the femoral head while the socket is formed by the acetabulum.</rdfs:comment>
        <rdfs:label xml:lang="en">Hip</rdfs:label>
    </owl:Class>
    


    <!-- http://www.semanticweb.org/marthinust/ontologies/2022/8/Gait_Ontology#Hip_abductor_weakness -->

    <owl:Class rdf:about="http://www.semanticweb.org/marthinust/ontologies/2022/8/Gait_Ontology#Hip_abductor_weakness">
        <rdfs:subClassOf rdf:resource="http://www.semanticweb.org/marthinust/ontologies/2022/8/Gait_Ontology#Hip"/>
    </owl:Class>
    


    <!-- http://www.semanticweb.org/marthinust/ontologies/2022/8/Gait_Ontology#Hip_dislocation -->

    <owl:Class rdf:about="http://www.semanticweb.org/marthinust/ontologies/2022/8/Gait_Ontology#Hip_dislocation">
        <rdfs:subClassOf rdf:resource="http://www.semanticweb.org/marthinust/ontologies/2022/8/Gait_Ontology#Hip"/>
        <opla-sd:entityPosition>
            <rdf:Description>
                <opla-sd:entityPositionX rdf:datatype="http://www.w3.org/2001/XMLSchema#double">258.88081364114237</opla-sd:entityPositionX>
                <opla-sd:entityPositionY rdf:datatype="http://www.w3.org/2001/XMLSchema#double">29.416994852208216</opla-sd:entityPositionY>
                <rdfs:comment xml:lang="en">This is an entity positioning annotation generated by CoModIDE (https://comodide.com/). Removing this annotation will break rendering the CoModIDE schema diagram view.</rdfs:comment>
            </rdf:Description>
        </opla-sd:entityPosition>
        <rdfs:comment xml:lang="en">Hip dislocation is a condition in which the ball-shaped head of the femur (thigh bone) is forced out of its socket in the pelvis. This can occur due to a traumatic injury, such as a car accident or a fall, or as a result of a medical condition that affects the stability of the hip joint, such as arthritis or hip dysplasia.

Hip dislocation is a serious injury that can cause significant pain, swelling, and difficulty with mobility. In some cases, the injury can also damage the surrounding tissues, nerves, and blood vessels, leading to further complications.

Treatment for hip dislocation typically involves emergency medical care to put the joint back into its proper position and stabilize the injury. This may involve a surgical procedure called a reduction, in which the doctor manipulates the hip joint to realign the bones. In some cases, surgery may be required to repair any damaged tissues or address underlying medical conditions that contributed to the dislocation. Rehabilitation and physical therapy may also be necessary to help the patient regain mobility and strength in the affected hip.</rdfs:comment>
        <rdfs:label xml:lang="en">Hip_dislocation</rdfs:label>
    </owl:Class>
    


    <!-- http://www.semanticweb.org/marthinust/ontologies/2022/8/Gait_Ontology#Hip_dysplasia -->

    <owl:Class rdf:about="http://www.semanticweb.org/marthinust/ontologies/2022/8/Gait_Ontology#Hip_dysplasia">
        <rdfs:subClassOf rdf:resource="http://www.semanticweb.org/marthinust/ontologies/2022/8/Gait_Ontology#Spina_bifida"/>
        <opla-sd:entityPosition>
            <rdf:Description>
                <opla-sd:entityPositionX rdf:datatype="http://www.w3.org/2001/XMLSchema#double">37.40950640235435</opla-sd:entityPositionX>
                <opla-sd:entityPositionY rdf:datatype="http://www.w3.org/2001/XMLSchema#double">142.59688396751181</opla-sd:entityPositionY>
                <rdfs:comment xml:lang="en">This is an entity positioning annotation generated by CoModIDE (https://comodide.com/). Removing this annotation will break rendering the CoModIDE schema diagram view.</rdfs:comment>
            </rdf:Description>
        </opla-sd:entityPosition>
        <rdfs:comment xml:lang="en">Hip dysplasia is a condition where the hip joint does not form correctly and is loose in the hip socket. This can lead to pain and difficulty in movement, as well as an increased risk of hip arthritis in later life. It can be caused by genetics, or due to environmental factors such as exposure to certain hormones or drugs during pregnancy. Treatment may involve physical therapy, bracing, or surgery.</rdfs:comment>
        <rdfs:label xml:lang="en">Hip_dysplasia</rdfs:label>
    </owl:Class>
    


    <!-- http://www.semanticweb.org/marthinust/ontologies/2022/8/Gait_Ontology#Hip_excessive_flexion -->

    <owl:Class rdf:about="http://www.semanticweb.org/marthinust/ontologies/2022/8/Gait_Ontology#Hip_excessive_flexion">
        <rdfs:subClassOf rdf:resource="http://www.semanticweb.org/marthinust/ontologies/2022/8/Gait_Ontology#Hip"/>
        <opla-sd:entityPosition>
            <rdf:Description>
                <opla-sd:entityPositionX rdf:datatype="http://www.w3.org/2001/XMLSchema#double">176.49439670482587</opla-sd:entityPositionX>
                <opla-sd:entityPositionY rdf:datatype="http://www.w3.org/2001/XMLSchema#double">4.533346963088603</opla-sd:entityPositionY>
                <rdfs:comment xml:lang="en">This is an entity positioning annotation generated by CoModIDE (https://comodide.com/). Removing this annotation will break rendering the CoModIDE schema diagram view.</rdfs:comment>
            </rdf:Description>
        </opla-sd:entityPosition>
        <rdfs:comment xml:lang="en">Excessive Hip Flexion can significantly alter gait pattern most commonly due to;  Hip flexion contractures  IT band contractures,  Hip flexor spasticity,  Compensation for excessive knee flexion and ankle DF,  Hip pain  Compensation for excess ankle plantar flexion in mid swing. The deviation of stance phase will occur mainly on the affected side. The result is forward tilt of the trunk and increased demand on the hip extensors or increased lordosis of the spine with anterior pelvic tilt. A person with reduced spinal mobility will adopt a forward flexion position in order to alter their centre of gravity permanently during gait.</rdfs:comment>
        <rdfs:label xml:lang="en">Hip_excessive_flexion</rdfs:label>
    </owl:Class>
    


    <!-- http://www.semanticweb.org/marthinust/ontologies/2022/8/Gait_Ontology#Hobby_horse_gait -->

    <owl:Class rdf:about="http://www.semanticweb.org/marthinust/ontologies/2022/8/Gait_Ontology#Hobby_horse_gait">
        <rdfs:subClassOf rdf:resource="http://www.semanticweb.org/marthinust/ontologies/2022/8/Gait_Ontology#Dystonic_gait"/>
        <opla-sd:entityPosition>
            <rdf:Description>
                <opla-sd:entityPositionX rdf:datatype="http://www.w3.org/2001/XMLSchema#double">240.92510322163497</opla-sd:entityPositionX>
                <opla-sd:entityPositionY rdf:datatype="http://www.w3.org/2001/XMLSchema#double">69.75627352670996</opla-sd:entityPositionY>
                <rdfs:comment xml:lang="en">This is an entity positioning annotation generated by CoModIDE (https://comodide.com/). Removing this annotation will break rendering the CoModIDE schema diagram view.</rdfs:comment>
            </rdf:Description>
        </opla-sd:entityPosition>
        <rdfs:comment xml:lang="en">An abnormal gait characterised by toe walking, stiff legs, and skipping. The gait pattern has some resemblance to cock-walk gait, but affected individuals are able to improve their dystonic gait by walking backward.</rdfs:comment>
        <rdfs:label xml:lang="en">Hobby_horse_gait</rdfs:label>
    </owl:Class>
    


    <!-- http://www.semanticweb.org/marthinust/ontologies/2022/8/Gait_Ontology#Hyperkinetic_gait -->

    <owl:Class rdf:about="http://www.semanticweb.org/marthinust/ontologies/2022/8/Gait_Ontology#Hyperkinetic_gait">
        <rdfs:subClassOf rdf:resource="http://www.semanticweb.org/marthinust/ontologies/2022/8/Gait_Ontology#Choreiform_gait"/>
        <opla-sd:entityPosition>
            <rdf:Description>
                <opla-sd:entityPositionX rdf:datatype="http://www.w3.org/2001/XMLSchema#double">288.5767254901958</opla-sd:entityPositionX>
                <opla-sd:entityPositionY rdf:datatype="http://www.w3.org/2001/XMLSchema#double">210.12214366114839</opla-sd:entityPositionY>
                <rdfs:comment xml:lang="en">This is an entity positioning annotation generated by CoModIDE (https://comodide.com/). Removing this annotation will break rendering the CoModIDE schema diagram view.</rdfs:comment>
            </rdf:Description>
        </opla-sd:entityPosition>
        <rdfs:comment xml:lang="en">This gait is seen with certain basal ganglia disorders including Sydenham&apos;s chorea, Huntington&apos;s Disease and other forms of chorea, athetosis or dystonia. The patient will display irregular, jerky, involuntary movements in all extremities. Walking may accentuate their baseline movement disorder.</rdfs:comment>
        <rdfs:label xml:lang="en">Hyperkinetic_gait</rdfs:label>
    </owl:Class>
    


    <!-- http://www.semanticweb.org/marthinust/ontologies/2022/8/Gait_Ontology#Hypertension -->

    <owl:Class rdf:about="http://www.semanticweb.org/marthinust/ontologies/2022/8/Gait_Ontology#Hypertension">
        <rdfs:subClassOf rdf:resource="http://www.semanticweb.org/marthinust/ontologies/2022/8/Gait_Ontology#Morbidity"/>
        <opla-sd:entityPosition>
            <rdf:Description>
                <opla-sd:entityPositionX rdf:datatype="http://www.w3.org/2001/XMLSchema#double">277.94778580829006</opla-sd:entityPositionX>
                <opla-sd:entityPositionY rdf:datatype="http://www.w3.org/2001/XMLSchema#double">155.35302482695175</opla-sd:entityPositionY>
                <rdfs:comment xml:lang="en">This is an entity positioning annotation generated by CoModIDE (https://comodide.com/). Removing this annotation will break rendering the CoModIDE schema diagram view.</rdfs:comment>
            </rdf:Description>
        </opla-sd:entityPosition>
        <rdfs:comment xml:lang="en">Hypertension can cause dizziness, fainting, and other symptoms that can make it difficult to walk.</rdfs:comment>
        <rdfs:label xml:lang="en">Hypertension</rdfs:label>
    </owl:Class>
    


    <!-- http://www.semanticweb.org/marthinust/ontologies/2022/8/Gait_Ontology#Image_sensing -->

    <owl:Class rdf:about="http://www.semanticweb.org/marthinust/ontologies/2022/8/Gait_Ontology#Image_sensing">
        <rdfs:subClassOf rdf:resource="http://www.semanticweb.org/marthinust/ontologies/2022/8/Gait_Ontology#Gait_Analysis_Method"/>
    </owl:Class>
    


    <!-- http://www.semanticweb.org/marthinust/ontologies/2022/8/Gait_Ontology#Impaired_tandem_gait -->

    <owl:Class rdf:about="http://www.semanticweb.org/marthinust/ontologies/2022/8/Gait_Ontology#Impaired_tandem_gait">
        <rdfs:subClassOf rdf:resource="http://www.semanticweb.org/marthinust/ontologies/2022/8/Gait_Ontology#Gait_Disturbance"/>
        <opla-sd:entityPosition>
            <rdf:Description>
                <opla-sd:entityPositionX rdf:datatype="http://www.w3.org/2001/XMLSchema#double">143.85927439093234</opla-sd:entityPositionX>
                <opla-sd:entityPositionY rdf:datatype="http://www.w3.org/2001/XMLSchema#double">32.99595443499821</opla-sd:entityPositionY>
                <rdfs:comment xml:lang="en">This is an entity positioning annotation generated by CoModIDE (https://comodide.com/). Removing this annotation will break rendering the CoModIDE schema diagram view.</rdfs:comment>
            </rdf:Description>
        </opla-sd:entityPosition>
        <rdfs:comment>Reduced ability to walk in a straight line while placing the feet heel to toe.</rdfs:comment>
        <rdfs:label xml:lang="en">Impaired_tandem_gait</rdfs:label>
    </owl:Class>
    


    <!-- http://www.semanticweb.org/marthinust/ontologies/2022/8/Gait_Ontology#Impaired_toe-walking_ability -->

    <owl:Class rdf:about="http://www.semanticweb.org/marthinust/ontologies/2022/8/Gait_Ontology#Impaired_toe-walking_ability">
        <rdfs:subClassOf rdf:resource="http://www.semanticweb.org/marthinust/ontologies/2022/8/Gait_Ontology#Gait_Disturbance"/>
        <opla-sd:entityPosition>
            <rdf:Description>
                <opla-sd:entityPositionX rdf:datatype="http://www.w3.org/2001/XMLSchema#double">193.1913198130383</opla-sd:entityPositionX>
                <opla-sd:entityPositionY rdf:datatype="http://www.w3.org/2001/XMLSchema#double">152.91057364872205</opla-sd:entityPositionY>
                <rdfs:comment xml:lang="en">This is an entity positioning annotation generated by CoModIDE (https://comodide.com/). Removing this annotation will break rendering the CoModIDE schema diagram view.</rdfs:comment>
            </rdf:Description>
        </opla-sd:entityPosition>
        <rdfs:comment>Difficulty or reduced ability to walk on toes. Toe-walking can be tested as a part of the neurological examination. Foot plantar flexion weakness leads to difficulties in walking on toes.</rdfs:comment>
        <rdfs:label xml:lang="en">Impaired_toe-walking_ability</rdfs:label>
    </owl:Class>
    


    <!-- http://www.semanticweb.org/marthinust/ontologies/2022/8/Gait_Ontology#Inability_to_walk -->

    <owl:Class rdf:about="http://www.semanticweb.org/marthinust/ontologies/2022/8/Gait_Ontology#Inability_to_walk">
        <rdfs:subClassOf rdf:resource="http://www.semanticweb.org/marthinust/ontologies/2022/8/Gait_Ontology#Gait_Disturbance"/>
        <opla-sd:entityPosition>
            <rdf:Description>
                <opla-sd:entityPositionX rdf:datatype="http://www.w3.org/2001/XMLSchema#double">115.9458618322944</opla-sd:entityPositionX>
                <opla-sd:entityPositionY rdf:datatype="http://www.w3.org/2001/XMLSchema#double">260.9253064870516</opla-sd:entityPositionY>
                <rdfs:comment xml:lang="en">This is an entity positioning annotation generated by CoModIDE (https://comodide.com/). Removing this annotation will break rendering the CoModIDE schema diagram view.</rdfs:comment>
            </rdf:Description>
        </opla-sd:entityPosition>
        <rdfs:comment>Incapability to ambulate.</rdfs:comment>
        <rdfs:label xml:lang="en">Inability_to_walk</rdfs:label>
    </owl:Class>
    


    <!-- http://www.semanticweb.org/marthinust/ontologies/2022/8/Gait_Ontology#Initial_contact -->

    <owl:Class rdf:about="http://www.semanticweb.org/marthinust/ontologies/2022/8/Gait_Ontology#Initial_contact">
        <rdfs:subClassOf rdf:resource="http://www.semanticweb.org/marthinust/ontologies/2022/8/Gait_Ontology#Stance_phase"/>
        <opla-sd:entityPosition>
            <rdf:Description>
                <opla-sd:entityPositionX rdf:datatype="http://www.w3.org/2001/XMLSchema#double">224.96166910077176</opla-sd:entityPositionX>
                <opla-sd:entityPositionY rdf:datatype="http://www.w3.org/2001/XMLSchema#double">209.8564890387111</opla-sd:entityPositionY>
                <rdfs:comment xml:lang="en">This is an entity positioning annotation generated by CoModIDE (https://comodide.com/). Removing this annotation will break rendering the CoModIDE schema diagram view.</rdfs:comment>
            </rdf:Description>
        </opla-sd:entityPosition>
        <rdfs:comment xml:lang="en">Initial contact consists of the first 3% of the gait cycle. In typical gait, the heel strikes the ground and initiates the rotation over the heel to foot flat to preserve progression. This motion is the first rocker of the gait cycle.</rdfs:comment>
        <rdfs:label xml:lang="en">Initial_contact</rdfs:label>
    </owl:Class>
    


    <!-- http://www.semanticweb.org/marthinust/ontologies/2022/8/Gait_Ontology#Initial_swing -->

    <owl:Class rdf:about="http://www.semanticweb.org/marthinust/ontologies/2022/8/Gait_Ontology#Initial_swing">
        <rdfs:subClassOf rdf:resource="http://www.semanticweb.org/marthinust/ontologies/2022/8/Gait_Ontology#Swing_phase"/>
        <opla-sd:entityPosition>
            <rdf:Description>
                <opla-sd:entityPositionX rdf:datatype="http://www.w3.org/2001/XMLSchema#double">45.640463006856415</opla-sd:entityPositionX>
                <opla-sd:entityPositionY rdf:datatype="http://www.w3.org/2001/XMLSchema#double">193.7712383094014</opla-sd:entityPositionY>
                <rdfs:comment xml:lang="en">This is an entity positioning annotation generated by CoModIDE (https://comodide.com/). Removing this annotation will break rendering the CoModIDE schema diagram view.</rdfs:comment>
            </rdf:Description>
        </opla-sd:entityPosition>
        <rdfs:comment xml:lang="en">The initial swing phase is the phase of the gait cycle in which the foot is in the air and not in contact with the ground. It begins when the foot leaves the ground at the end of the stance phase and ends when the foot makes contact with the ground again at the beginning of the next stance phase.

During the initial swing phase, the hip, knee, and ankle joints all undergo flexion (bending) as the leg swings forward. This helps to propel the body forward and prepare the leg for the next stance phase. The initial swing phase is an important part of the gait cycle as it helps to maintain balance and stability while walking.

Initial swing goes from 62-75% of the gait cycle. During initial swing, the hip, knee, and ankle are flexed to begin advancement of the limb forward and create clearance of the foot over the ground.</rdfs:comment>
        <rdfs:label xml:lang="en">Initial_swing</rdfs:label>
    </owl:Class>
    


    <!-- http://www.semanticweb.org/marthinust/ontologies/2022/8/Gait_Ontology#Joints -->

    <owl:Class rdf:about="http://www.semanticweb.org/marthinust/ontologies/2022/8/Gait_Ontology#Joints">
        <rdfs:subClassOf rdf:resource="http://www.semanticweb.org/marthinust/ontologies/2022/8/Gait_Ontology#Calcification"/>
        <opla-sd:entityPosition>
            <rdf:Description>
                <opla-sd:entityPositionX rdf:datatype="http://www.w3.org/2001/XMLSchema#double">74.26351077698939</opla-sd:entityPositionX>
                <opla-sd:entityPositionY rdf:datatype="http://www.w3.org/2001/XMLSchema#double">267.88562877568154</opla-sd:entityPositionY>
                <rdfs:comment xml:lang="en">This is an entity positioning annotation generated by CoModIDE (https://comodide.com/). Removing this annotation will break rendering the CoModIDE schema diagram view.</rdfs:comment>
            </rdf:Description>
        </opla-sd:entityPosition>
        <rdfs:comment xml:lang="en">The joints become stiffer and less flexible. Fluid in the joints may decrease. The cartilage may begin to rub together and wear away. Minerals may deposit in and around some joints (calcification). Age-related changes in joints can cause joint pain in old age and is a significant concern that should not be ignored.

As you age, joint movement becomes stiffer and less flexible because the amount of lubricating fluid inside your joints decreases and the cartilage becomes thinner. Ligaments also tend to shorten and lose some flexibility, making joints feel stiff.</rdfs:comment>
        <rdfs:label xml:lang="en">Joints</rdfs:label>
    </owl:Class>
    


    <!-- http://www.semanticweb.org/marthinust/ontologies/2022/8/Gait_Ontology#Kinematics -->

    <owl:Class rdf:about="http://www.semanticweb.org/marthinust/ontologies/2022/8/Gait_Ontology#Kinematics">
        <rdfs:subClassOf rdf:resource="http://www.semanticweb.org/marthinust/ontologies/2022/8/Gait_Ontology#Gait_Analysis_Method"/>
        <opla-sd:entityPosition>
            <rdf:Description>
                <opla-sd:entityPositionX rdf:datatype="http://www.w3.org/2001/XMLSchema#double">229.62002949543376</opla-sd:entityPositionX>
                <opla-sd:entityPositionY rdf:datatype="http://www.w3.org/2001/XMLSchema#double">60.09588575394827</opla-sd:entityPositionY>
                <rdfs:comment xml:lang="en">This is an entity positioning annotation generated by CoModIDE (https://comodide.com/). Removing this annotation will break rendering the CoModIDE schema diagram view.</rdfs:comment>
            </rdf:Description>
        </opla-sd:entityPosition>
        <rdfs:comment>Kinematics is the measurement of movement or, more specifically, the geometric description of motion, in terms of displacements, velocities and accelerations. Kinematic systems are used in gait analysis to record the position and orientation of the body segments, the angles of the joints and the corresponding linear and angular velocities and accelerations. Kinematic measurement may be made in either two dimensions or three. Three-dimensional measurements normally require the use of two or more cameras, although methods have been devised in which a single camera can be used to make limited three-dimensional measurements.</rdfs:comment>
        <rdfs:label xml:lang="en">Kinematics</rdfs:label>
    </owl:Class>
    


    <!-- http://www.semanticweb.org/marthinust/ontologies/2022/8/Gait_Ontology#Knee -->

    <owl:Class rdf:about="http://www.semanticweb.org/marthinust/ontologies/2022/8/Gait_Ontology#Knee">
        <rdfs:subClassOf rdf:resource="http://www.semanticweb.org/marthinust/ontologies/2022/8/Gait_Ontology#Musculoskeletal"/>
        <opla-sd:entityPosition>
            <rdf:Description>
                <opla-sd:entityPositionX rdf:datatype="http://www.w3.org/2001/XMLSchema#double">129.98424106251767</opla-sd:entityPositionX>
                <opla-sd:entityPositionY rdf:datatype="http://www.w3.org/2001/XMLSchema#double">80.83116347747931</opla-sd:entityPositionY>
                <rdfs:comment xml:lang="en">This is an entity positioning annotation generated by CoModIDE (https://comodide.com/). Removing this annotation will break rendering the CoModIDE schema diagram view.</rdfs:comment>
            </rdf:Description>
        </opla-sd:entityPosition>
        <rdfs:comment xml:lang="en">The knee is the joint where the bones of the lower and upper legs meet. The largest joint in the body, the knee moves like a hinge, allowing you to sit, squat, walk or jump. The knee consists of three bones: femur  the upper leg bone, or thigh bone. tibia  the bone at the front of the lower leg, or shin bone.

The knee is one of the largest and most complex joints in the body. The knee joins the thigh bone (femur) to the shin bone (tibia). The smaller bone that runs alongside the tibia (fibula) and the kneecap (patella) are the other bones that make the knee joint.</rdfs:comment>
        <rdfs:label xml:lang="en">Knee</rdfs:label>
    </owl:Class>
    


    <!-- http://www.semanticweb.org/marthinust/ontologies/2022/8/Gait_Ontology#Knee_extensor_weakness -->

    <owl:Class rdf:about="http://www.semanticweb.org/marthinust/ontologies/2022/8/Gait_Ontology#Knee_extensor_weakness">
        <rdfs:subClassOf rdf:resource="http://www.semanticweb.org/marthinust/ontologies/2022/8/Gait_Ontology#Knee"/>
        <opla-sd:entityPosition>
            <rdf:Description>
                <opla-sd:entityPositionX rdf:datatype="http://www.w3.org/2001/XMLSchema#double">94.28905652578489</opla-sd:entityPositionX>
                <opla-sd:entityPositionY rdf:datatype="http://www.w3.org/2001/XMLSchema#double">289.27267527792117</opla-sd:entityPositionY>
                <rdfs:comment xml:lang="en">This is an entity positioning annotation generated by CoModIDE (https://comodide.com/). Removing this annotation will break rendering the CoModIDE schema diagram view.</rdfs:comment>
            </rdf:Description>
        </opla-sd:entityPosition>
        <rdfs:comment xml:lang="en">Knee extensor weakness: Knee buckling (uncompensated), genu recurvatum (compensated).
Pathomechanism: Knee remains fully extended throughout the stance. An associated anterior trunk lean in the early part of stance moves the line of gravity of the trunk slightly anterior to the axis of rotation of the knee. This keeps the knee extended without action of the knee extensors. This gait deviation may lead to an excessive stretching of the posterior capsule of the knee.</rdfs:comment>
        <rdfs:label xml:lang="en">Knee_extensor_weakness</rdfs:label>
    </owl:Class>
    


    <!-- http://www.semanticweb.org/marthinust/ontologies/2022/8/Gait_Ontology#Knee_flexion_contraction -->

    <owl:Class rdf:about="http://www.semanticweb.org/marthinust/ontologies/2022/8/Gait_Ontology#Knee_flexion_contraction">
        <rdfs:subClassOf rdf:resource="http://www.semanticweb.org/marthinust/ontologies/2022/8/Gait_Ontology#Knee"/>
        <opla-sd:entityPosition>
            <rdf:Description>
                <opla-sd:entityPositionX rdf:datatype="http://www.w3.org/2001/XMLSchema#double">171.4162531379328</opla-sd:entityPositionX>
                <opla-sd:entityPositionY rdf:datatype="http://www.w3.org/2001/XMLSchema#double">156.82662013615413</opla-sd:entityPositionY>
                <rdfs:comment xml:lang="en">This is an entity positioning annotation generated by CoModIDE (https://comodide.com/). Removing this annotation will break rendering the CoModIDE schema diagram view.</rdfs:comment>
            </rdf:Description>
        </opla-sd:entityPosition>
        <rdfs:comment xml:lang="en">Knee Flexion Contraction will cause a limping type gait pattern. The knee is restricted in extension, meaning heel strike is limited and step length reduced. To compensate the person is likely to toe walk during stance phase. Knee flexion contractures of more than 30 degrees will be obvious during normal paced gait. Contractures less then this will be more evident with increased speeds.</rdfs:comment>
        <rdfs:label xml:lang="en">Knee_flexion_contraction</rdfs:label>
    </owl:Class>
    


    <!-- http://www.semanticweb.org/marthinust/ontologies/2022/8/Gait_Ontology#Leg -->

    <owl:Class rdf:about="http://www.semanticweb.org/marthinust/ontologies/2022/8/Gait_Ontology#Leg">
        <rdfs:subClassOf rdf:resource="http://www.semanticweb.org/marthinust/ontologies/2022/8/Gait_Ontology#Musculoskeletal"/>
        <opla-sd:entityPosition>
            <rdf:Description>
                <opla-sd:entityPositionX rdf:datatype="http://www.w3.org/2001/XMLSchema#double">124.31126595426534</opla-sd:entityPositionX>
                <opla-sd:entityPositionY rdf:datatype="http://www.w3.org/2001/XMLSchema#double">210.64527780894718</opla-sd:entityPositionY>
                <rdfs:comment xml:lang="en">This is an entity positioning annotation generated by CoModIDE (https://comodide.com/). Removing this annotation will break rendering the CoModIDE schema diagram view.</rdfs:comment>
            </rdf:Description>
        </opla-sd:entityPosition>
        <rdfs:comment xml:lang="en">The human leg, in the general word sense, is the entire lower limb of the human body, including the foot, thigh or sometimes even the hip or gluteal region.

The leg provides support and a range of movements.</rdfs:comment>
        <rdfs:label xml:lang="en">Leg</rdfs:label>
    </owl:Class>
    


    <!-- http://www.semanticweb.org/marthinust/ontologies/2022/8/Gait_Ontology#Leg_length_discrepancy -->

    <owl:Class rdf:about="http://www.semanticweb.org/marthinust/ontologies/2022/8/Gait_Ontology#Leg_length_discrepancy">
        <rdfs:subClassOf rdf:resource="http://www.semanticweb.org/marthinust/ontologies/2022/8/Gait_Ontology#Leg"/>
        <opla-sd:entityPosition>
            <rdf:Description>
                <opla-sd:entityPositionX rdf:datatype="http://www.w3.org/2001/XMLSchema#double">12.723523842616617</opla-sd:entityPositionX>
                <opla-sd:entityPositionY rdf:datatype="http://www.w3.org/2001/XMLSchema#double">106.65663281084898</opla-sd:entityPositionY>
                <rdfs:comment xml:lang="en">This is an entity positioning annotation generated by CoModIDE (https://comodide.com/). Removing this annotation will break rendering the CoModIDE schema diagram view.</rdfs:comment>
            </rdf:Description>
        </opla-sd:entityPosition>
        <rdfs:comment xml:lang="en">Leg length discrepancy (LLD) refers to a condition in which the length of one leg is significantly different from the length of the other leg. This can be due to a number of factors, including congenital differences (present at birth), developmental conditions, injuries, or diseases. The difference in leg length can be measured in millimeters or centimeters and is usually determined by a physical examination, x-ray, or other imaging modality.

LLD can lead to a number of symptoms, such as pain in the back, hips, knees, or ankles, as well as problems with walking or standing. In some cases, LLD can be treated with the use of shoe lifts or orthotic devices, while in other cases, surgical intervention may be necessary.

Leg length discrepancy can be as a result of an asymmetrical pelvic, tibia, or femur length or for other reasons such as scoliosis or contractures. The gait pattern will present as a pelvic dip to the shortened side during the stance phase with possible toe walking on that limb. The opposite leg is likely to increase its knee and hip flexion to reduce its length.</rdfs:comment>
        <rdfs:label xml:lang="en">Leg_length_discrepancy</rdfs:label>
    </owl:Class>
    


    <!-- http://www.semanticweb.org/marthinust/ontologies/2022/8/Gait_Ontology#Leg_limping -->

    <owl:Class rdf:about="http://www.semanticweb.org/marthinust/ontologies/2022/8/Gait_Ontology#Leg_limping">
        <rdfs:subClassOf rdf:resource="http://www.semanticweb.org/marthinust/ontologies/2022/8/Gait_Ontology#Leg"/>
        <opla-sd:entityPosition>
            <rdf:Description>
                <opla-sd:entityPositionX rdf:datatype="http://www.w3.org/2001/XMLSchema#double">118.09947511523278</opla-sd:entityPositionX>
                <opla-sd:entityPositionY rdf:datatype="http://www.w3.org/2001/XMLSchema#double">11.700610491725206</opla-sd:entityPositionY>
                <rdfs:comment xml:lang="en">This is an entity positioning annotation generated by CoModIDE (https://comodide.com/). Removing this annotation will break rendering the CoModIDE schema diagram view.</rdfs:comment>
            </rdf:Description>
        </opla-sd:entityPosition>
        <rdfs:comment xml:lang="en">Limping may be caused by pain, weakness, neuromuscular imbalance, or a skeletal deformity. The most common underlying cause of a painful limp is physical trauma; however, in the absence of trauma, other serious causes, such as septic arthritis or slipped capital femoral epiphysis, may be present.</rdfs:comment>
        <rdfs:label xml:lang="en">Leg_limping</rdfs:label>
    </owl:Class>
    


    <!-- http://www.semanticweb.org/marthinust/ontologies/2022/8/Gait_Ontology#Limp_gait -->

    <owl:Class rdf:about="http://www.semanticweb.org/marthinust/ontologies/2022/8/Gait_Ontology#Limp_gait">
        <rdfs:subClassOf rdf:resource="http://www.semanticweb.org/marthinust/ontologies/2022/8/Gait_Ontology#Type_of_Gait"/>
    </owl:Class>
    


    <!-- http://www.semanticweb.org/marthinust/ontologies/2022/8/Gait_Ontology#Loading_rate -->

    <owl:Class rdf:about="http://www.semanticweb.org/marthinust/ontologies/2022/8/Gait_Ontology#Loading_rate">
        <rdfs:subClassOf rdf:resource="http://www.semanticweb.org/marthinust/ontologies/2022/8/Gait_Ontology#Gait_Parameter"/>
        <opla-sd:entityPosition>
            <rdf:Description>
                <opla-sd:entityPositionX rdf:datatype="http://www.w3.org/2001/XMLSchema#double">226.65820978866492</opla-sd:entityPositionX>
                <opla-sd:entityPositionY rdf:datatype="http://www.w3.org/2001/XMLSchema#double">156.08099818291876</opla-sd:entityPositionY>
                <rdfs:comment xml:lang="en">This is an entity positioning annotation generated by CoModIDE (https://comodide.com/). Removing this annotation will break rendering the CoModIDE schema diagram view.</rdfs:comment>
            </rdf:Description>
        </opla-sd:entityPosition>
        <rdfs:comment xml:lang="en">Loading rate is an important gait parameter because it can affect the mechanical efficiency of gait and can also be used to assess the impact of various interventions on gait. For example, changes in loading rate may be used to evaluate the effectiveness of orthotic devices or other treatments for conditions such as osteoarthritis or gait abnormalities.</rdfs:comment>
        <rdfs:label xml:lang="en">Loading_rate</rdfs:label>
    </owl:Class>
    


    <!-- http://www.semanticweb.org/marthinust/ontologies/2022/8/Gait_Ontology#Loading_response -->

    <owl:Class rdf:about="http://www.semanticweb.org/marthinust/ontologies/2022/8/Gait_Ontology#Loading_response">
        <rdfs:subClassOf rdf:resource="http://www.semanticweb.org/marthinust/ontologies/2022/8/Gait_Ontology#Stance_phase"/>
        <opla-sd:entityPosition>
            <rdf:Description>
                <opla-sd:entityPositionX rdf:datatype="http://www.w3.org/2001/XMLSchema#double">277.92733952189326</opla-sd:entityPositionX>
                <opla-sd:entityPositionY rdf:datatype="http://www.w3.org/2001/XMLSchema#double">142.5678158796421</opla-sd:entityPositionY>
                <rdfs:comment xml:lang="en">This is an entity positioning annotation generated by CoModIDE (https://comodide.com/). Removing this annotation will break rendering the CoModIDE schema diagram view.</rdfs:comment>
            </rdf:Description>
        </opla-sd:entityPosition>
        <rdfs:comment xml:lang="en">In this portion, the knee flexes slightly in order to absorb shock as the foot falls flat on the ground, stabilizing in advance of single limb support. Loading response goes from 3-12% of the gait cycle.</rdfs:comment>
        <rdfs:label xml:lang="en">Loading_response</rdfs:label>
    </owl:Class>
    


    <!-- http://www.semanticweb.org/marthinust/ontologies/2022/8/Gait_Ontology#Loss_of_ability_to_walk -->

    <owl:Class rdf:about="http://www.semanticweb.org/marthinust/ontologies/2022/8/Gait_Ontology#Loss_of_ability_to_walk">
        <rdfs:subClassOf rdf:resource="http://www.semanticweb.org/marthinust/ontologies/2022/8/Gait_Ontology#Loss_of_ambulation"/>
        <opla-sd:entityPosition>
            <rdf:Description>
                <opla-sd:entityPositionX rdf:datatype="http://www.w3.org/2001/XMLSchema#double">144.18365963489987</opla-sd:entityPositionX>
                <opla-sd:entityPositionY rdf:datatype="http://www.w3.org/2001/XMLSchema#double">184.79515131878958</opla-sd:entityPositionY>
                <rdfs:comment xml:lang="en">This is an entity positioning annotation generated by CoModIDE (https://comodide.com/). Removing this annotation will break rendering the CoModIDE schema diagram view.</rdfs:comment>
            </rdf:Description>
        </opla-sd:entityPosition>
        <rdfs:comment>Loss of ability to walk</rdfs:comment>
        <rdfs:label xml:lang="en">Loss_of_ability_to_walk</rdfs:label>
    </owl:Class>
    


    <!-- http://www.semanticweb.org/marthinust/ontologies/2022/8/Gait_Ontology#Loss_of_ability_to_walk_in_early_childhood -->

    <owl:Class rdf:about="http://www.semanticweb.org/marthinust/ontologies/2022/8/Gait_Ontology#Loss_of_ability_to_walk_in_early_childhood">
        <rdfs:subClassOf rdf:resource="http://www.semanticweb.org/marthinust/ontologies/2022/8/Gait_Ontology#Loss_of_ambulation"/>
        <opla-sd:entityPosition>
            <rdf:Description>
                <opla-sd:entityPositionX rdf:datatype="http://www.w3.org/2001/XMLSchema#double">45.19757403229073</opla-sd:entityPositionX>
                <opla-sd:entityPositionY rdf:datatype="http://www.w3.org/2001/XMLSchema#double">111.64509506596991</opla-sd:entityPositionY>
                <rdfs:comment xml:lang="en">This is an entity positioning annotation generated by CoModIDE (https://comodide.com/). Removing this annotation will break rendering the CoModIDE schema diagram view.</rdfs:comment>
            </rdf:Description>
        </opla-sd:entityPosition>
        <rdfs:comment>Loss of ability to walk in early childhood</rdfs:comment>
        <rdfs:label xml:lang="en">Loss_of_ability_to_walk_in_early_childhood</rdfs:label>
    </owl:Class>
    


    <!-- http://www.semanticweb.org/marthinust/ontologies/2022/8/Gait_Ontology#Loss_of_ability_to_walk_in_first_decade -->

    <owl:Class rdf:about="http://www.semanticweb.org/marthinust/ontologies/2022/8/Gait_Ontology#Loss_of_ability_to_walk_in_first_decade">
        <rdfs:subClassOf rdf:resource="http://www.semanticweb.org/marthinust/ontologies/2022/8/Gait_Ontology#Loss_of_ambulation"/>
        <opla-sd:entityPosition>
            <rdf:Description>
                <opla-sd:entityPositionX rdf:datatype="http://www.w3.org/2001/XMLSchema#double">207.9182498925505</opla-sd:entityPositionX>
                <opla-sd:entityPositionY rdf:datatype="http://www.w3.org/2001/XMLSchema#double">238.36081660787076</opla-sd:entityPositionY>
                <rdfs:comment xml:lang="en">This is an entity positioning annotation generated by CoModIDE (https://comodide.com/). Removing this annotation will break rendering the CoModIDE schema diagram view.</rdfs:comment>
            </rdf:Description>
        </opla-sd:entityPosition>
        <rdfs:comment>Loss of ability to walk in first decade</rdfs:comment>
        <rdfs:label xml:lang="en">Loss_of_ability_to_walk_in_first_decade</rdfs:label>
    </owl:Class>
    


    <!-- http://www.semanticweb.org/marthinust/ontologies/2022/8/Gait_Ontology#Loss_of_ambulation -->

    <owl:Class rdf:about="http://www.semanticweb.org/marthinust/ontologies/2022/8/Gait_Ontology#Loss_of_ambulation">
        <rdfs:subClassOf rdf:resource="http://www.semanticweb.org/marthinust/ontologies/2022/8/Gait_Ontology#Inability_to_walk"/>
        <opla-sd:entityPosition>
            <rdf:Description>
                <opla-sd:entityPositionX rdf:datatype="http://www.w3.org/2001/XMLSchema#double">48.61043307654897</opla-sd:entityPositionX>
                <opla-sd:entityPositionY rdf:datatype="http://www.w3.org/2001/XMLSchema#double">181.68796125749677</opla-sd:entityPositionY>
                <rdfs:comment xml:lang="en">This is an entity positioning annotation generated by CoModIDE (https://comodide.com/). Removing this annotation will break rendering the CoModIDE schema diagram view.</rdfs:comment>
            </rdf:Description>
        </opla-sd:entityPosition>
        <rdfs:comment>Progressive inability to walk in a person who previous had the ability to walk.</rdfs:comment>
        <rdfs:label xml:lang="en">Loss_of_ambulation</rdfs:label>
    </owl:Class>
    


    <!-- http://www.semanticweb.org/marthinust/ontologies/2022/8/Gait_Ontology#Magnometer -->

    <owl:Class rdf:about="http://www.semanticweb.org/marthinust/ontologies/2022/8/Gait_Ontology#Magnometer">
        <rdfs:subClassOf rdf:resource="http://www.semanticweb.org/marthinust/ontologies/2022/8/Gait_Ontology#Gait_Analysis_Equipment"/>
        <opla-sd:entityPosition>
            <rdf:Description>
                <opla-sd:entityPositionX rdf:datatype="http://www.w3.org/2001/XMLSchema#double">179.9138515059333</opla-sd:entityPositionX>
                <opla-sd:entityPositionY rdf:datatype="http://www.w3.org/2001/XMLSchema#double">252.0757321895833</opla-sd:entityPositionY>
                <rdfs:comment xml:lang="en">This is an entity positioning annotation generated by CoModIDE (https://comodide.com/). Removing this annotation will break rendering the CoModIDE schema diagram view.</rdfs:comment>
            </rdf:Description>
        </opla-sd:entityPosition>
        <rdfs:comment xml:lang="en">A magnetometer is a component of an Inertial and Magnetic Measurement System (MMS) that measures the orientation of body segments in three-dimensional space by detecting the Earth&apos;s magnetic field. When combined with other sensors like accelerometers and gyroscopes, magnetometers contribute to a comprehensive system for monitoring and analyzing body movement during walking, running, or other activities. This data can help identify abnormalities in gait patterns, assess rehabilitation progress, and optimise sports performance.</rdfs:comment>
        <rdfs:label xml:lang="en">Magnometer</rdfs:label>
    </owl:Class>
    


    <!-- http://www.semanticweb.org/marthinust/ontologies/2022/8/Gait_Ontology#Mid_stance -->

    <owl:Class rdf:about="http://www.semanticweb.org/marthinust/ontologies/2022/8/Gait_Ontology#Mid_stance">
        <rdfs:subClassOf rdf:resource="http://www.semanticweb.org/marthinust/ontologies/2022/8/Gait_Ontology#Stance_phase"/>
        <opla-sd:entityPosition>
            <rdf:Description>
                <opla-sd:entityPositionX rdf:datatype="http://www.w3.org/2001/XMLSchema#double">48.21442879557506</opla-sd:entityPositionX>
                <opla-sd:entityPositionY rdf:datatype="http://www.w3.org/2001/XMLSchema#double">86.9575525506143</opla-sd:entityPositionY>
                <rdfs:comment xml:lang="en">This is an entity positioning annotation generated by CoModIDE (https://comodide.com/). Removing this annotation will break rendering the CoModIDE schema diagram view.</rdfs:comment>
            </rdf:Description>
        </opla-sd:entityPosition>
        <rdfs:comment xml:lang="en">The mid-stance phase is the point where the support limb moves from shock absorption to more of a stability function. This phase is defined from the toe-off point of the contralateral leg to the first point the heel comes off the ground of the lead leg. The mid-stance phase makes up 29-37% of the stance phase.</rdfs:comment>
        <rdfs:label xml:lang="en">Mid_stance</rdfs:label>
    </owl:Class>
    


    <!-- http://www.semanticweb.org/marthinust/ontologies/2022/8/Gait_Ontology#Mid_swing -->

    <owl:Class rdf:about="http://www.semanticweb.org/marthinust/ontologies/2022/8/Gait_Ontology#Mid_swing">
        <rdfs:subClassOf rdf:resource="http://www.semanticweb.org/marthinust/ontologies/2022/8/Gait_Ontology#Swing_phase"/>
        <opla-sd:entityPosition>
            <rdf:Description>
                <opla-sd:entityPositionX rdf:datatype="http://www.w3.org/2001/XMLSchema#double">141.4015409659916</opla-sd:entityPositionX>
                <opla-sd:entityPositionY rdf:datatype="http://www.w3.org/2001/XMLSchema#double">1.7624887356974823</opla-sd:entityPositionY>
                <rdfs:comment xml:lang="en">This is an entity positioning annotation generated by CoModIDE (https://comodide.com/). Removing this annotation will break rendering the CoModIDE schema diagram view.</rdfs:comment>
            </rdf:Description>
        </opla-sd:entityPosition>
        <rdfs:comment xml:lang="en">The mid swing phase is the phase of the gait cycle that occurs halfway through the initial swing phase. During mid swing, the hip, knee, and ankle joints continue to undergo flexion (bending) as the leg swings forward. At this point in the gait cycle, the toes of the swinging leg may be pointed downward in preparation for foot strike.

The mid swing phase is a transitional phase in the gait cycle and it helps to prepare the leg for the next stance phase. It is important for maintaining balance and stability while walking.

Mid-swing goes from 75-87% of the gait cycle. During mid-swing, limb advancement continues and the thigh reaches its peak advancement.</rdfs:comment>
        <rdfs:label xml:lang="en">Mid_swing</rdfs:label>
    </owl:Class>
    


    <!-- http://www.semanticweb.org/marthinust/ontologies/2022/8/Gait_Ontology#Mobility_scooter -->

    <owl:Class rdf:about="http://www.semanticweb.org/marthinust/ontologies/2022/8/Gait_Ontology#Mobility_scooter">
        <rdfs:subClassOf rdf:resource="http://www.semanticweb.org/marthinust/ontologies/2022/8/Gait_Ontology#Gait_Assistive_Technology"/>
        <opla-sd:entityPosition>
            <rdf:Description>
                <opla-sd:entityPositionX rdf:datatype="http://www.w3.org/2001/XMLSchema#double">22.675389202974557</opla-sd:entityPositionX>
                <opla-sd:entityPositionY rdf:datatype="http://www.w3.org/2001/XMLSchema#double">168.3443832734724</opla-sd:entityPositionY>
                <rdfs:comment xml:lang="en">This is an entity positioning annotation generated by CoModIDE (https://comodide.com/). Removing this annotation will break rendering the CoModIDE schema diagram view.</rdfs:comment>
            </rdf:Description>
        </opla-sd:entityPosition>
        <rdfs:comment xml:lang="en">A mobility scooter is a type of electric vehicle designed to assist people with limited mobility in their daily activities. It is typically used by individuals who have difficulty walking long distances, standing for extended periods of time, or who have a medical condition that affects their mobility. Mobility scooters provide users with increased independence and mobility, allowing them to move around more easily and participate in daily activities such as shopping, socializing, and traveling. They are commonly used by older adults, people with disabilities, and individuals recovering from injuries or surgeries that affect their mobility.</rdfs:comment>
        <rdfs:label xml:lang="en">Mobility_scooter</rdfs:label>
    </owl:Class>
    


    <!-- http://www.semanticweb.org/marthinust/ontologies/2022/8/Gait_Ontology#Morbidity -->

    <owl:Class rdf:about="http://www.semanticweb.org/marthinust/ontologies/2022/8/Gait_Ontology#Morbidity">
        <rdfs:subClassOf rdf:resource="http://www.semanticweb.org/marthinust/ontologies/2022/8/Gait_Ontology#Geriatric_gait"/>
        <opla-sd:entityPosition>
            <rdf:Description>
                <opla-sd:entityPositionX rdf:datatype="http://www.w3.org/2001/XMLSchema#double">67.11791100337085</opla-sd:entityPositionX>
                <opla-sd:entityPositionY rdf:datatype="http://www.w3.org/2001/XMLSchema#double">30.313859036564136</opla-sd:entityPositionY>
                <rdfs:comment xml:lang="en">This is an entity positioning annotation generated by CoModIDE (https://comodide.com/). Removing this annotation will break rendering the CoModIDE schema diagram view.</rdfs:comment>
            </rdf:Description>
        </opla-sd:entityPosition>
        <rdfs:comment xml:lang="en">Morbidity can be used to assess the overall health of a population and to identify trends in the prevalence of different diseases. Geriatric assessment should include detailed medical history and physical examination, with particular focus on problems specific to the elderly such as vision, hearing, mobility, nutrition, fall prevention, urinary incontinence, osteoporosis, and preventative health conditions (hypertension, diabetes, etc.).

Refers to having a disease or a symptom of disease, or to the amount of disease within a population resulting in a higher morbidity for the elderly cohort. Morbidity also refers to medical problems caused by a treatment.</rdfs:comment>
        <rdfs:label xml:lang="en">Morbidity</rdfs:label>
    </owl:Class>
    


    <!-- http://www.semanticweb.org/marthinust/ontologies/2022/8/Gait_Ontology#Motion_systems -->

    <owl:Class rdf:about="http://www.semanticweb.org/marthinust/ontologies/2022/8/Gait_Ontology#Motion_systems">
        <rdfs:subClassOf rdf:resource="http://www.semanticweb.org/marthinust/ontologies/2022/8/Gait_Ontology#Gait_Analysis_Method"/>
        <opla-sd:entityPosition>
            <rdf:Description>
                <opla-sd:entityPositionX rdf:datatype="http://www.w3.org/2001/XMLSchema#double">101.92987052287364</opla-sd:entityPositionX>
                <opla-sd:entityPositionY rdf:datatype="http://www.w3.org/2001/XMLSchema#double">172.03029969229956</opla-sd:entityPositionY>
                <rdfs:comment xml:lang="en">This is an entity positioning annotation generated by CoModIDE (https://comodide.com/). Removing this annotation will break rendering the CoModIDE schema diagram view.</rdfs:comment>
            </rdf:Description>
        </opla-sd:entityPosition>
        <rdfs:comment xml:lang="en">Gait analysis has used different types of motion sensors and systems, such as the accelerometer, gyroscope, magnetoresistive sensors, flexible goniometer, electromagnetic tracking system (ETS), sensing fabric, force sensor, and sensors for electromyography (EMG). Based on these sensors, a single type or a combined sensor system of multiple types of sensors may be used for various gait analysis applications.</rdfs:comment>
        <rdfs:label xml:lang="en">Motion_systems</rdfs:label>
    </owl:Class>
    


    <!-- http://www.semanticweb.org/marthinust/ontologies/2022/8/Gait_Ontology#Multiple_sclerosis -->

    <owl:Class rdf:about="http://www.semanticweb.org/marthinust/ontologies/2022/8/Gait_Ontology#Multiple_sclerosis">
        <rdfs:subClassOf rdf:resource="http://www.semanticweb.org/marthinust/ontologies/2022/8/Gait_Ontology#Gait-related_Disease"/>
        <rdfs:subClassOf rdf:resource="http://www.semanticweb.org/marthinust/ontologies/2022/8/Gait_Ontology#Neurological"/>
        <opla-sd:entityPosition>
            <rdf:Description>
                <opla-sd:entityPositionX rdf:datatype="http://www.w3.org/2001/XMLSchema#double">287.97398148708413</opla-sd:entityPositionX>
                <opla-sd:entityPositionY rdf:datatype="http://www.w3.org/2001/XMLSchema#double">81.79121624696457</opla-sd:entityPositionY>
                <rdfs:comment xml:lang="en">This is an entity positioning annotation generated by CoModIDE (https://comodide.com/). Removing this annotation will break rendering the CoModIDE schema diagram view.</rdfs:comment>
            </rdf:Description>
        </opla-sd:entityPosition>
        <rdfs:comment xml:lang="en">A disease in which the immune system eats away at the protective covering of nerves. In Multiple sclerosis, resulting nerve damage disrupts communication between the brain and the body. Multiple sclerosis causes many different symptoms, including vision loss, pain, fatigue and impaired coordination. The symptoms, severity, and duration can vary from person to person. Some people may be symptom free for most of their lives, while others can have severe, chronic symptoms that never go away.</rdfs:comment>
        <rdfs:comment>Multiple sclerosis is a disease that impacts the brain, spinal cord and optic nerves, which make up the central nervous system and controls everything we do. The exact cause of MS is unknown, but we do know that something triggers the immune system to attack the CNS. The resulting damage to myelin, the protective layer insulating wire-like nerve fibers, disrupts signals to and from the brain. This interruption of communication signals causes unpredictable symptoms such as numbness, tingling, mood changes, memory problems, pain, fatigue, blindness and/or paralysis.

Most people experience their first symptoms of MS between the ages of 20 and 40; the initial symptom of MS is often blurred or double vision, red-green color distortion, or even blindness in one eye.  Most MS patients experience muscle weakness in their extremities and difficulty with coordination and balance.  These symptoms may be severe enough to impair walking or even standing. In the worst cases, MS can produce partial or complete paralysis.</rdfs:comment>
        <rdfs:label xml:lang="en">Multiple_sclerosis</rdfs:label>
    </owl:Class>
    


    <!-- http://www.semanticweb.org/marthinust/ontologies/2022/8/Gait_Ontology#Muscle_atrophy -->

    <owl:Class rdf:about="http://www.semanticweb.org/marthinust/ontologies/2022/8/Gait_Ontology#Muscle_atrophy">
        <rdfs:subClassOf rdf:resource="http://www.semanticweb.org/marthinust/ontologies/2022/8/Gait_Ontology#Morbidity"/>
        <opla-sd:entityPosition>
            <rdf:Description>
                <opla-sd:entityPositionX rdf:datatype="http://www.w3.org/2001/XMLSchema#double">229.63223133265612</opla-sd:entityPositionX>
                <opla-sd:entityPositionY rdf:datatype="http://www.w3.org/2001/XMLSchema#double">296.6436382425407</opla-sd:entityPositionY>
                <rdfs:comment xml:lang="en">This is an entity positioning annotation generated by CoModIDE (https://comodide.com/). Removing this annotation will break rendering the CoModIDE schema diagram view.</rdfs:comment>
            </rdf:Description>
        </opla-sd:entityPosition>
        <rdfs:comment xml:lang="en">Muscle atrophy is the wasting (thinning) or loss of muscle mass tissue. Muscle atrophy can occur due to malnutrition, age, genetics, a lack of physical activity or certain medical conditions. Disuse (physiologic) atrophy occurs when you don&apos;t use your muscles enough.</rdfs:comment>
        <rdfs:label xml:lang="en">Muscle_atrophy</rdfs:label>
    </owl:Class>
    


    <!-- http://www.semanticweb.org/marthinust/ontologies/2022/8/Gait_Ontology#Muscular_dystrophy -->

    <owl:Class rdf:about="http://www.semanticweb.org/marthinust/ontologies/2022/8/Gait_Ontology#Muscular_dystrophy">
        <rdfs:subClassOf rdf:resource="http://www.semanticweb.org/marthinust/ontologies/2022/8/Gait_Ontology#Gait-related_Disease"/>
        <rdfs:subClassOf rdf:resource="http://www.semanticweb.org/marthinust/ontologies/2022/8/Gait_Ontology#Neuromuscular"/>
        <opla-sd:entityPosition>
            <rdf:Description>
                <opla-sd:entityPositionX rdf:datatype="http://www.w3.org/2001/XMLSchema#double">118.26261556220814</opla-sd:entityPositionX>
                <opla-sd:entityPositionY rdf:datatype="http://www.w3.org/2001/XMLSchema#double">169.2863460807486</opla-sd:entityPositionY>
                <rdfs:comment xml:lang="en">This is an entity positioning annotation generated by CoModIDE (https://comodide.com/). Removing this annotation will break rendering the CoModIDE schema diagram view.</rdfs:comment>
            </rdf:Description>
        </opla-sd:entityPosition>
        <rdfs:comment xml:lang="en">In muscular dystrophy, abnormal genes (mutations) interfere with the production of proteins needed to form healthy muscle. Damaged muscles become progressively weaker.</rdfs:comment>
        <rdfs:comment>Muscular dystrophy is a group of diseases that make muscles weaker and less flexible over time. It is caused by a problem in the genes that control how the body keeps muscles healthy. For some people, the disease starts early in childhood. Others dont have any symptoms until they are teenagers or middle-aged adults. Most peoples condition will get worse over time, and some people may lose the ability to walk, talk, or care for themselves. But that doesnt happen to everyone. Other people can live for many years with mild symptoms.</rdfs:comment>
        <rdfs:label xml:lang="en">Muscular_dystrophy</rdfs:label>
    </owl:Class>
    


    <!-- http://www.semanticweb.org/marthinust/ontologies/2022/8/Gait_Ontology#Musculoskeletal -->

    <owl:Class rdf:about="http://www.semanticweb.org/marthinust/ontologies/2022/8/Gait_Ontology#Musculoskeletal">
        <rdfs:subClassOf rdf:resource="http://www.semanticweb.org/marthinust/ontologies/2022/8/Gait_Ontology#Gait_Classification"/>
        <rdfs:subClassOf rdf:resource="http://www.semanticweb.org/marthinust/ontologies/2022/8/Gait_Ontology#Pathological_gait"/>
    </owl:Class>
    


    <!-- http://www.semanticweb.org/marthinust/ontologies/2022/8/Gait_Ontology#Myasthenia_gravis -->

    <owl:Class rdf:about="http://www.semanticweb.org/marthinust/ontologies/2022/8/Gait_Ontology#Myasthenia_gravis">
        <rdfs:subClassOf rdf:resource="http://www.semanticweb.org/marthinust/ontologies/2022/8/Gait_Ontology#Gait-related_Disease"/>
        <opla-sd:entityPosition>
            <rdf:Description>
                <opla-sd:entityPositionX rdf:datatype="http://www.w3.org/2001/XMLSchema#double">114.68970750525085</opla-sd:entityPositionX>
                <opla-sd:entityPositionY rdf:datatype="http://www.w3.org/2001/XMLSchema#double">109.10386994248665</opla-sd:entityPositionY>
                <rdfs:comment xml:lang="en">This is an entity positioning annotation generated by CoModIDE (https://comodide.com/). Removing this annotation will break rendering the CoModIDE schema diagram view.</rdfs:comment>
            </rdf:Description>
        </opla-sd:entityPosition>
        <rdfs:comment xml:lang="en">Myasthenia gravis (MG) is a neuromuscular disorder that causes weakness in the skeletal muscles, which are the muscles your body uses for movement. MG happens when communication between nerve cells and muscles becomes impaired. This impairment prevents crucial muscle contractions from occurring, causing muscle weakness.

Myasthenia gravis (MG) is a neuromuscular disorder that causes weakness in your voluntary skeletal muscles. It can affect people of any age, but is more common in women under the age of 40 and men older than 60. 

Symptoms include:

muscle weakness in the arms, hands, legs, or feet
drooping eyelids
double vision
trouble speaking
difficulty swallowing or chewing</rdfs:comment>
        <rdfs:label xml:lang="en">Myasthenia_gravis</rdfs:label>
    </owl:Class>
    


    <!-- http://www.semanticweb.org/marthinust/ontologies/2022/8/Gait_Ontology#Myoclonus_tremor -->

    <owl:Class rdf:about="http://www.semanticweb.org/marthinust/ontologies/2022/8/Gait_Ontology#Myoclonus_tremor">
        <rdfs:subClassOf rdf:resource="http://www.semanticweb.org/marthinust/ontologies/2022/8/Gait_Ontology#Gait_Disturbance"/>
        <rdfs:subClassOf rdf:resource="http://www.semanticweb.org/marthinust/ontologies/2022/8/Gait_Ontology#Neurological"/>
        <opla-sd:entityPosition>
            <rdf:Description>
                <opla-sd:entityPositionX rdf:datatype="http://www.w3.org/2001/XMLSchema#double">175.56656561734056</opla-sd:entityPositionX>
                <opla-sd:entityPositionY rdf:datatype="http://www.w3.org/2001/XMLSchema#double">32.70026881289731</opla-sd:entityPositionY>
                <rdfs:comment xml:lang="en">This is an entity positioning annotation generated by CoModIDE (https://comodide.com/). Removing this annotation will break rendering the CoModIDE schema diagram view.</rdfs:comment>
            </rdf:Description>
        </opla-sd:entityPosition>
        <rdfs:comment xml:lang="en">Tremor and myoclonus are both common jerky, hyperkinetic, movement disorders. The classic tremor phenotype consists of a regular alternating movement of muscles, while myoclonus is normally characterised by irregular jerks.

The tremulous movements are in fact small, high-frequency myoclonic jerks, induced by posture or action. They can be mild, but can also be more incapacitating. When present in the lower limbs, these may lead to gait disorders and even drop attacks. These tremor-like movements during action can be mistaken for essential tremor or epileptic seizures.</rdfs:comment>
        <rdfs:label xml:lang="en">Myoclonus_tremor</rdfs:label>
    </owl:Class>
    


    <!-- http://www.semanticweb.org/marthinust/ontologies/2022/8/Gait_Ontology#Myopathic_gait -->

    <owl:Class rdf:about="http://www.semanticweb.org/marthinust/ontologies/2022/8/Gait_Ontology#Myopathic_gait">
        <rdfs:subClassOf rdf:resource="http://www.semanticweb.org/marthinust/ontologies/2022/8/Gait_Ontology#Type_of_Gait"/>
        <opla-sd:entityPosition>
            <rdf:Description>
                <opla-sd:entityPositionX rdf:datatype="http://www.w3.org/2001/XMLSchema#double">75.9614565321209</opla-sd:entityPositionX>
                <opla-sd:entityPositionY rdf:datatype="http://www.w3.org/2001/XMLSchema#double">213.95480943504882</opla-sd:entityPositionY>
                <rdfs:comment xml:lang="en">This is an entity positioning annotation generated by CoModIDE (https://comodide.com/). Removing this annotation will break rendering the CoModIDE schema diagram view.</rdfs:comment>
            </rdf:Description>
        </opla-sd:entityPosition>
        <rdfs:comment xml:lang="en">Hip girdle muscles are responsible for keeping the pelvis level when walking. If you have weakness on one side, this will lead to a drop in the pelvis on the contralateral side of the pelvis while walking (Trendelenburg sign). With bilateral weakness, you will have dropping of the pelvis on both sides during walking leading to waddling. This gait is seen in patient with myopathies, such as muscular dystrophy.

(Waddling Gait)</rdfs:comment>
        <rdfs:label xml:lang="en">Myopathic_gait</rdfs:label>
    </owl:Class>
    


    <!-- http://www.semanticweb.org/marthinust/ontologies/2022/8/Gait_Ontology#Myotonia_congenita -->

    <owl:Class rdf:about="http://www.semanticweb.org/marthinust/ontologies/2022/8/Gait_Ontology#Myotonia_congenita">
        <rdfs:subClassOf rdf:resource="http://www.semanticweb.org/marthinust/ontologies/2022/8/Gait_Ontology#Gait-related_Disease"/>
        <opla-sd:entityPosition>
            <rdf:Description>
                <opla-sd:entityPositionX rdf:datatype="http://www.w3.org/2001/XMLSchema#double">30.940097398999526</opla-sd:entityPositionX>
                <opla-sd:entityPositionY rdf:datatype="http://www.w3.org/2001/XMLSchema#double">100.87121580416536</opla-sd:entityPositionY>
                <rdfs:comment xml:lang="en">This is an entity positioning annotation generated by CoModIDE (https://comodide.com/). Removing this annotation will break rendering the CoModIDE schema diagram view.</rdfs:comment>
            </rdf:Description>
        </opla-sd:entityPosition>
        <rdfs:comment xml:lang="en">Myotonia congenita (or, congenital myotonia) is a rare genetic disease that affects skeletal muscles. It prevents skeletal muscles from quickly relaxing after movement or contraction. Myotonia congenita symptoms usually appear in early childhood and can vary among individuals.

Beginning in childhood, people with this condition experience bouts of sustained muscle tensing (myotonia) that prevent muscles from relaxing normally. Although myotonia can affect any skeletal muscles, including muscles of the face and tongue, it occurs most often in the legs. Myotonia causes muscle stiffness that can interfere with movement. In some people the stiffness is very mild, while in other cases it may be severe enough to interfere with walking, running, and other activities of daily life. These muscle problems are particularly noticeable during movement following a period of rest. Many affected individuals find that repeated movements can temporarily alleviate their muscle stiffness, a phenomenon known as the warm-up effect.

The two major types of myotonia congenita are known as Thomsen disease and Becker disease. These conditions are distinguished by the severity of their symptoms and their patterns of inheritance. Becker disease usually appears later in childhood than Thomsen disease and causes more severe muscle stiffness, particularly in males. People with Becker disease often experience temporary attacks of muscle weakness, particularly in the arms and hands, brought on by movement after periods of rest. They may also develop mild, permanent muscle weakness over time. This muscle weakness is not seen in people with Thomsen disease.

This disease is caused by mutations in the gene for a chloride channel thats necessary for shutting off the electrical excitation that causes muscle contraction.

The Becker type is inherited in an autosomal recessive pattern, meaning it is produced by defective genes contributed by both parents.

The Thomsen type is autosomal dominant, meaning it is produced by a defective gene contributed by one parent. 

Myotonia congenita can be detected in children ages 2 and 3 if they have muscle stiffness in their legs during sudden movement after rest.</rdfs:comment>
        <rdfs:label xml:lang="en">Myotonia_congenita</rdfs:label>
    </owl:Class>
    


    <!-- http://www.semanticweb.org/marthinust/ontologies/2022/8/Gait_Ontology#Neurogenic_claudication -->

    <owl:Class rdf:about="http://www.semanticweb.org/marthinust/ontologies/2022/8/Gait_Ontology#Neurogenic_claudication">
        <rdfs:subClassOf rdf:resource="http://www.semanticweb.org/marthinust/ontologies/2022/8/Gait_Ontology#Gait_Disturbance"/>
        <opla-sd:entityPosition>
            <rdf:Description>
                <opla-sd:entityPositionX rdf:datatype="http://www.w3.org/2001/XMLSchema#double">64.93608253218419</opla-sd:entityPositionX>
                <opla-sd:entityPositionY rdf:datatype="http://www.w3.org/2001/XMLSchema#double">264.60988610726577</opla-sd:entityPositionY>
                <rdfs:comment xml:lang="en">This is an entity positioning annotation generated by CoModIDE (https://comodide.com/). Removing this annotation will break rendering the CoModIDE schema diagram view.</rdfs:comment>
            </rdf:Description>
        </opla-sd:entityPosition>
        <rdfs:comment>Lumbar spinal stenoses may induce symptoms following an individually typical latency on standing or when walking due to swelling of the cauda equina, which leads to compression. This is referred to as neurogenic claudication. The symptoms of lumbar spinal stenosis can be explained by an increase in lumbar lordosis and spinal canal stenosis in an upright position compared to the sitting position or if spondylolisthesis is present by a shift of the vertebrae while standing and walking. Following an individually characteristic distance, walking becomes associated with deep muscular pain and with neurological deficits, such as sensory deficits and paresis in the lower limbs, which resolve within minutes when the affected person sits or lies down. Activities performed in a flexed posture, such as cycling often cause less problems than walking. For the same reason, walking uphill may be tolerated better than walking downhill. Clinical neurological examination at rest may be entirely normal but there is usually pain on hyperextension of the lumbar spine.</rdfs:comment>
        <rdfs:label xml:lang="en">Neurogenic_claudication</rdfs:label>
    </owl:Class>
    


    <!-- http://www.semanticweb.org/marthinust/ontologies/2022/8/Gait_Ontology#Neurologic_gait_dysfunction -->

    <owl:Class rdf:about="http://www.semanticweb.org/marthinust/ontologies/2022/8/Gait_Ontology#Neurologic_gait_dysfunction">
        <rdfs:subClassOf rdf:resource="http://www.semanticweb.org/marthinust/ontologies/2022/8/Gait_Ontology#Neurological"/>
        <opla-sd:entityPosition>
            <rdf:Description>
                <opla-sd:entityPositionX rdf:datatype="http://www.w3.org/2001/XMLSchema#double">286.73198510218356</opla-sd:entityPositionX>
                <opla-sd:entityPositionY rdf:datatype="http://www.w3.org/2001/XMLSchema#double">215.46873663574644</opla-sd:entityPositionY>
                <rdfs:comment xml:lang="en">This is an entity positioning annotation generated by CoModIDE (https://comodide.com/). Removing this annotation will break rendering the CoModIDE schema diagram view.</rdfs:comment>
            </rdf:Description>
        </opla-sd:entityPosition>
        <rdfs:comment xml:lang="en">Gait abnormalities that are a manifestation of nervous system dysfunction. These conditions may be caused by a wide variety of disorders which affect motor control, sensory feedback, and muscle strength including: CENTRAL NERVOUS SYSTEM DISEASES; PERIPHERAL NERVOUS SYSTEM DISEASES; NEUROMUSCULAR DISEASES; or MUSCULAR DISEASES.</rdfs:comment>
        <rdfs:label xml:lang="en">Neurologic_gait_dysfunction</rdfs:label>
    </owl:Class>
    


    <!-- http://www.semanticweb.org/marthinust/ontologies/2022/8/Gait_Ontology#Neurological -->

    <owl:Class rdf:about="http://www.semanticweb.org/marthinust/ontologies/2022/8/Gait_Ontology#Neurological">
        <rdfs:subClassOf rdf:resource="http://www.semanticweb.org/marthinust/ontologies/2022/8/Gait_Ontology#Gait_Classification"/>
        <rdfs:subClassOf rdf:resource="http://www.semanticweb.org/marthinust/ontologies/2022/8/Gait_Ontology#Pathological_gait"/>
    </owl:Class>
    


    <!-- http://www.semanticweb.org/marthinust/ontologies/2022/8/Gait_Ontology#Neuromuscular -->

    <owl:Class rdf:about="http://www.semanticweb.org/marthinust/ontologies/2022/8/Gait_Ontology#Neuromuscular">
        <rdfs:subClassOf rdf:resource="http://www.semanticweb.org/marthinust/ontologies/2022/8/Gait_Ontology#Gait_Classification"/>
    </owl:Class>
    


    <!-- http://www.semanticweb.org/marthinust/ontologies/2022/8/Gait_Ontology#Neuropathic_gait -->

    <owl:Class rdf:about="http://www.semanticweb.org/marthinust/ontologies/2022/8/Gait_Ontology#Neuropathic_gait">
        <rdfs:subClassOf rdf:resource="http://www.semanticweb.org/marthinust/ontologies/2022/8/Gait_Ontology#Type_of_Gait"/>
        <opla-sd:entityPosition>
            <rdf:Description>
                <opla-sd:entityPositionX rdf:datatype="http://www.w3.org/2001/XMLSchema#double">138.32587513845695</opla-sd:entityPositionX>
                <opla-sd:entityPositionY rdf:datatype="http://www.w3.org/2001/XMLSchema#double">160.24255108897867</opla-sd:entityPositionY>
                <rdfs:comment xml:lang="en">This is an entity positioning annotation generated by CoModIDE (https://comodide.com/). Removing this annotation will break rendering the CoModIDE schema diagram view.</rdfs:comment>
            </rdf:Description>
        </opla-sd:entityPosition>
        <rdfs:comment xml:lang="en">Seen in patients with foot drop (weakness of foot dorsiflexion), the cause of this gait is due to an attempt to lift the leg high enough during walking so that the foot does not drag on the floor. If unilateral, causes include peroneal nerve palsy and L5 radiculopathy. If bilateral, causes include amyotrophic lateral sclerosis, Charcot-Marie-Tooth disease and other peripheral neuropathies including those associated with uncontrolled diabetes.

(Steppage Gait, Equine Gait)</rdfs:comment>
        <rdfs:label xml:lang="en">Neuropathic_gait</rdfs:label>
    </owl:Class>
    


    <!-- http://www.semanticweb.org/marthinust/ontologies/2022/8/Gait_Ontology#Neuropathy -->

    <owl:Class rdf:about="http://www.semanticweb.org/marthinust/ontologies/2022/8/Gait_Ontology#Neuropathy">
        <rdfs:subClassOf rdf:resource="http://www.semanticweb.org/marthinust/ontologies/2022/8/Gait_Ontology#Gait-related_Disease"/>
        <opla-sd:entityPosition>
            <rdf:Description>
                <opla-sd:entityPositionX rdf:datatype="http://www.w3.org/2001/XMLSchema#double">89.76942108830204</opla-sd:entityPositionX>
                <opla-sd:entityPositionY rdf:datatype="http://www.w3.org/2001/XMLSchema#double">65.88740217955453</opla-sd:entityPositionY>
                <rdfs:comment xml:lang="en">This is an entity positioning annotation generated by CoModIDE (https://comodide.com/). Removing this annotation will break rendering the CoModIDE schema diagram view.</rdfs:comment>
            </rdf:Description>
        </opla-sd:entityPosition>
        <rdfs:comment xml:lang="en">Neuropathy is a general term used to describe a problem with the nerves, typically in the peripheral nervous system. Neuropathy can cause a range of symptoms, depending on which nerves are affected and to what extent. Some common symptoms of neuropathy include numbness and tingling in the hands and feet, weakness, and pain. Neuropathy can be caused by a variety of factors, including diabetes, alcoholism, autoimmune diseases, and certain medications. It can also be a complication of other medical conditions, such as cancer or HIV/AIDS.

Treatment of neuropathy may involve medications to manage pain and other symptoms, as well as lifestyle changes such as improving nutrition and avoiding alcohol. In some cases, treating the underlying cause of the neuropathy can help to improve symptoms. Neuropathy can sometimes be severe and debilitating, and it can have a significant impact on an individual&apos;s mobility and quality of life.</rdfs:comment>
        <rdfs:label xml:lang="en">Neuropathy</rdfs:label>
    </owl:Class>
    


    <!-- http://www.semanticweb.org/marthinust/ontologies/2022/8/Gait_Ontology#Normal_gait -->

    <owl:Class rdf:about="http://www.semanticweb.org/marthinust/ontologies/2022/8/Gait_Ontology#Normal_gait">
        <rdfs:subClassOf rdf:resource="http://www.semanticweb.org/marthinust/ontologies/2022/8/Gait_Ontology#Type_of_Gait"/>
    </owl:Class>
    


    <!-- http://www.semanticweb.org/marthinust/ontologies/2022/8/Gait_Ontology#Obesity -->

    <owl:Class rdf:about="http://www.semanticweb.org/marthinust/ontologies/2022/8/Gait_Ontology#Obesity">
        <rdfs:subClassOf rdf:resource="http://www.semanticweb.org/marthinust/ontologies/2022/8/Gait_Ontology#Gait-related_Disease"/>
        <opla-sd:entityPosition>
            <rdf:Description>
                <opla-sd:entityPositionX rdf:datatype="http://www.w3.org/2001/XMLSchema#double">52.88544566963024</opla-sd:entityPositionX>
                <opla-sd:entityPositionY rdf:datatype="http://www.w3.org/2001/XMLSchema#double">249.26592256831432</opla-sd:entityPositionY>
                <rdfs:comment xml:lang="en">This is an entity positioning annotation generated by CoModIDE (https://comodide.com/). Removing this annotation will break rendering the CoModIDE schema diagram view.</rdfs:comment>
            </rdf:Description>
        </opla-sd:entityPosition>
        <rdfs:comment xml:lang="en">Obesity is a complex disease involving an excessive amount of body fat. It&apos;s a disorder involving excessive body fat that increases the risk of health problems. Obesity often results from taking in more calories than are burned by exercise and normal daily activities. Moreover, obesity affects gait mechanics during walking. Adults with obesity have slower gait velocity, greater absolute ground reaction forces, and altered lower-limb joint loading patterns compared to normal-weight adults.</rdfs:comment>
        <rdfs:label xml:lang="en">Obesity</rdfs:label>
    </owl:Class>
    


    <!-- http://www.semanticweb.org/marthinust/ontologies/2022/8/Gait_Ontology#Orthotic_device -->

    <owl:Class rdf:about="http://www.semanticweb.org/marthinust/ontologies/2022/8/Gait_Ontology#Orthotic_device">
        <rdfs:subClassOf rdf:resource="http://www.semanticweb.org/marthinust/ontologies/2022/8/Gait_Ontology#Gait_Assistive_Technology"/>
        <opla-sd:entityPosition>
            <rdf:Description>
                <opla-sd:entityPositionX rdf:datatype="http://www.w3.org/2001/XMLSchema#double">30.74230139627279</opla-sd:entityPositionX>
                <opla-sd:entityPositionY rdf:datatype="http://www.w3.org/2001/XMLSchema#double">197.3192943552579</opla-sd:entityPositionY>
                <rdfs:comment xml:lang="en">This is an entity positioning annotation generated by CoModIDE (https://comodide.com/). Removing this annotation will break rendering the CoModIDE schema diagram view.</rdfs:comment>
            </rdf:Description>
        </opla-sd:entityPosition>
        <rdfs:comment xml:lang="en">Orthotic devices are specially designed devices that are worn on the feet or legs to provide support, alignment, and stability. They can be used to treat a variety of conditions, including foot and ankle injuries, flat feet, and plantar fasciitis. 

For example, ankle braces that allow a person to stand straight are orthotics. Also, wrist braces, arm braces, spinal orthotics, and heel casts are orthotic devices. They all work to help those who have pain or difficulty with basic movements to be able to perform these activities again.

An orthosis is a device designed to improve biomechanical function, encourage proper joint alignment or to protect an existing limb.</rdfs:comment>
        <rdfs:label xml:lang="en">Orthotic_device</rdfs:label>
    </owl:Class>
    


    <!-- http://www.semanticweb.org/marthinust/ontologies/2022/8/Gait_Ontology#Osteoarthritis -->

    <owl:Class rdf:about="http://www.semanticweb.org/marthinust/ontologies/2022/8/Gait_Ontology#Osteoarthritis">
        <rdfs:subClassOf rdf:resource="http://www.semanticweb.org/marthinust/ontologies/2022/8/Gait_Ontology#Arthritis"/>
        <opla-sd:entityPosition>
            <rdf:Description>
                <opla-sd:entityPositionX rdf:datatype="http://www.w3.org/2001/XMLSchema#double">82.36723537512646</opla-sd:entityPositionX>
                <opla-sd:entityPositionY rdf:datatype="http://www.w3.org/2001/XMLSchema#double">22.847404781057335</opla-sd:entityPositionY>
                <rdfs:comment xml:lang="en">This is an entity positioning annotation generated by CoModIDE (https://comodide.com/). Removing this annotation will break rendering the CoModIDE schema diagram view.</rdfs:comment>
            </rdf:Description>
        </opla-sd:entityPosition>
        <rdfs:comment xml:lang="en">Osteoarthritis (OA) is a degenerative joint disorder that affects the cartilage in joints. Cartilage is the smooth, rubbery tissue that cushions the ends of bones in a joint. In OA, the cartilage wears away, causing the bones to rub together. This can lead to pain, stiffness, and loss of motion in the affected joint. OA is often referred as a &quot;wear-and-tear&quot; arthritis, because it is caused by mechanical stress on the joints over time.</rdfs:comment>
        <rdfs:comment>Osteoarthritis, also known as degenerative joint disease (DJD), is the most common type of arthritis. Osteoarthritis is more likely to develop as people age. The changes in osteoarthritis usually occur slowly over many years, though there are occasional exceptions. Inflammation and injury to the joint cause bony changes, deterioration of tendons and ligaments and a breakdown of cartilage, resulting in pain, swelling, and deformity of the joint.  Often it increases with activities that put stress on the joint, such as running or prolonged walking. Other changes cause the joint to lose mobility and function, resulting in joint pain with activity.</rdfs:comment>
        <rdfs:label xml:lang="en">Osteoarthritis</rdfs:label>
    </owl:Class>
    


    <!-- http://www.semanticweb.org/marthinust/ontologies/2022/8/Gait_Ontology#Osteoporosis -->

    <owl:Class rdf:about="http://www.semanticweb.org/marthinust/ontologies/2022/8/Gait_Ontology#Osteoporosis">
        <rdfs:subClassOf rdf:resource="http://www.semanticweb.org/marthinust/ontologies/2022/8/Gait_Ontology#Morbidity"/>
        <opla-sd:entityPosition>
            <rdf:Description>
                <opla-sd:entityPositionX rdf:datatype="http://www.w3.org/2001/XMLSchema#double">60.016624524140816</opla-sd:entityPositionX>
                <opla-sd:entityPositionY rdf:datatype="http://www.w3.org/2001/XMLSchema#double">212.4449367642764</opla-sd:entityPositionY>
                <rdfs:comment xml:lang="en">This is an entity positioning annotation generated by CoModIDE (https://comodide.com/). Removing this annotation will break rendering the CoModIDE schema diagram view.</rdfs:comment>
            </rdf:Description>
        </opla-sd:entityPosition>
        <rdfs:comment xml:lang="en">Osteoporosis is a health condition that weakens bones, making them fragile and more likely to break. It develops slowly over several years and is often only diagnosed when a fall or sudden impact causes a bone to break (fracture).

Bones become more brittle and may break more easily. Overall height decreases, mainly because the trunk and spine shorten. Breakdown of the joints may lead to inflammation, pain, stiffness, and deformity. Joint changes affect almost all older people.</rdfs:comment>
        <rdfs:label xml:lang="en">Osteoporosis</rdfs:label>
    </owl:Class>
    


    <!-- http://www.semanticweb.org/marthinust/ontologies/2022/8/Gait_Ontology#Paraparesis -->

    <owl:Class rdf:about="http://www.semanticweb.org/marthinust/ontologies/2022/8/Gait_Ontology#Paraparesis">
        <rdfs:subClassOf rdf:resource="http://www.semanticweb.org/marthinust/ontologies/2022/8/Gait_Ontology#Neurological"/>
        <opla-sd:entityPosition>
            <rdf:Description>
                <opla-sd:entityPositionX rdf:datatype="http://www.w3.org/2001/XMLSchema#double">2.1033399182829213</opla-sd:entityPositionX>
                <opla-sd:entityPositionY rdf:datatype="http://www.w3.org/2001/XMLSchema#double">277.9793171054099</opla-sd:entityPositionY>
                <rdfs:comment xml:lang="en">This is an entity positioning annotation generated by CoModIDE (https://comodide.com/). Removing this annotation will break rendering the CoModIDE schema diagram view.</rdfs:comment>
            </rdf:Description>
        </opla-sd:entityPosition>
        <rdfs:comment xml:lang="en">Paraparesis occurs when you&apos;re partially unable to move your legs. The condition can also refer to weakness in your hips and legs. Paraparesis is different from paraplegia, which refers to a complete inability to move your legs. This partial loss of function can be caused by: (pathological) injury.

Paraparesis is the partial paralysis of both legs due to disrupted nerve signals from the brain to the muscles.</rdfs:comment>
        <rdfs:label xml:lang="en">Paraparesis</rdfs:label>
    </owl:Class>
    


    <!-- http://www.semanticweb.org/marthinust/ontologies/2022/8/Gait_Ontology#Parkinsonian_gait -->

    <owl:Class rdf:about="http://www.semanticweb.org/marthinust/ontologies/2022/8/Gait_Ontology#Parkinsonian_gait">
        <rdfs:subClassOf rdf:resource="http://www.semanticweb.org/marthinust/ontologies/2022/8/Gait_Ontology#Type_of_Gait"/>
    </owl:Class>
    


    <!-- http://www.semanticweb.org/marthinust/ontologies/2022/8/Gait_Ontology#Parkinsonism -->

    <owl:Class rdf:about="http://www.semanticweb.org/marthinust/ontologies/2022/8/Gait_Ontology#Parkinsonism">
        <rdfs:subClassOf rdf:resource="http://www.semanticweb.org/marthinust/ontologies/2022/8/Gait_Ontology#Neurological"/>
        <rdfs:subClassOf rdf:resource="http://www.semanticweb.org/marthinust/ontologies/2022/8/Gait_Ontology#Parkinson&apos;s_disease"/>
        <opla-sd:entityPosition>
            <rdf:Description>
                <opla-sd:entityPositionX rdf:datatype="http://www.w3.org/2001/XMLSchema#double">74.93198403094851</opla-sd:entityPositionX>
                <opla-sd:entityPositionY rdf:datatype="http://www.w3.org/2001/XMLSchema#double">126.27907672910669</opla-sd:entityPositionY>
                <rdfs:comment xml:lang="en">This is an entity positioning annotation generated by CoModIDE (https://comodide.com/). Removing this annotation will break rendering the CoModIDE schema diagram view.</rdfs:comment>
            </rdf:Description>
        </opla-sd:entityPosition>
        <rdfs:comment xml:lang="en">Parkinsonism comprises a clinical syndrome that presents with a varying degree of rigidity, and a variety of symptoms that include bradykinesia, tremor, and unstable posture, all of which can cause a profound gait impairment. Parkinsonism is an umbrella term that refers to conditions with similar, movement-related effects. These conditions involve slowed movements, and other symptoms are possible depending on the condition.</rdfs:comment>
        <rdfs:comment>Parkinsonism is a general term that refers to a group of neurological disorders that cause movement problems similar to those seen in Parkinson&apos;s disease. A progressive disorder that affects the nervous system and the parts of the body controlled by the nerves. Symptoms start slowly. The first symptom may be a barely noticeable tremor in just one hand. Tremors are common, but the disorder may also cause stiffness or slowing of movement.</rdfs:comment>
        <rdfs:label xml:lang="en">Parkinsonism</rdfs:label>
    </owl:Class>
    


    <!-- http://www.semanticweb.org/marthinust/ontologies/2022/8/Gait_Ontology#Pathological_gait -->

    <owl:Class rdf:about="http://www.semanticweb.org/marthinust/ontologies/2022/8/Gait_Ontology#Pathological_gait">
        <rdfs:subClassOf rdf:resource="http://www.semanticweb.org/marthinust/ontologies/2022/8/Gait_Ontology#Gait_Pathology"/>
        <opla-sd:entityPosition>
            <rdf:Description>
                <opla-sd:entityPositionX rdf:datatype="http://www.w3.org/2001/XMLSchema#double">224.58396608039405</opla-sd:entityPositionX>
                <opla-sd:entityPositionY rdf:datatype="http://www.w3.org/2001/XMLSchema#double">206.690811090442</opla-sd:entityPositionY>
                <rdfs:comment xml:lang="en">This is an entity positioning annotation generated by CoModIDE (https://comodide.com/). Removing this annotation will break rendering the CoModIDE schema diagram view.</rdfs:comment>
            </rdf:Description>
        </opla-sd:entityPosition>
        <rdfs:comment xml:lang="en">Pathological gait patterns resulting from musculoskeletal are often caused by soft tissue imbalance, joint alignment or bony abnormalities affect the gait pattern as a result. It is an altered gait pattern due to deformities, weakness, or other impairments.

Pathological gait can be caused by a variety of factors, including neurological disorders, musculoskeletal problems, and certain medical conditions such as arthritis or stroke. It can also be caused by injuries to the feet, legs, or ankles.

Pathologic gait results from impaired strength range of motion, proprioception, pain, or balance combined with mechanical compensations, and can have musculoskeletal and neuromuscular etiologies.</rdfs:comment>
        <rdfs:label xml:lang="en">Pathological_gait</rdfs:label>
    </owl:Class>
    


    <!-- http://www.semanticweb.org/marthinust/ontologies/2022/8/Gait_Ontology#Peripheral_neuropathy -->

    <owl:Class rdf:about="http://www.semanticweb.org/marthinust/ontologies/2022/8/Gait_Ontology#Peripheral_neuropathy">
        <rdfs:subClassOf rdf:resource="http://www.semanticweb.org/marthinust/ontologies/2022/8/Gait_Ontology#Neuropathy"/>
        <opla-sd:entityPosition>
            <rdf:Description>
                <opla-sd:entityPositionX rdf:datatype="http://www.w3.org/2001/XMLSchema#double">125.91578620513481</opla-sd:entityPositionX>
                <opla-sd:entityPositionY rdf:datatype="http://www.w3.org/2001/XMLSchema#double">60.57276231916206</opla-sd:entityPositionY>
                <rdfs:comment xml:lang="en">This is an entity positioning annotation generated by CoModIDE (https://comodide.com/). Removing this annotation will break rendering the CoModIDE schema diagram view.</rdfs:comment>
            </rdf:Description>
        </opla-sd:entityPosition>
        <rdfs:comment xml:lang="en">Peripheral neuropathy, a result of damage to the nerves located outside of the brain and spinal cord (peripheral nerves), often causes weakness, numbness and pain, usually in the hands and feet.</rdfs:comment>
        <rdfs:label xml:lang="en">Peripheral_neuropathy</rdfs:label>
    </owl:Class>
    


    <!-- http://www.semanticweb.org/marthinust/ontologies/2022/8/Gait_Ontology#Pharmacotherapy -->

    <owl:Class rdf:about="http://www.semanticweb.org/marthinust/ontologies/2022/8/Gait_Ontology#Pharmacotherapy">
        <rdfs:subClassOf rdf:resource="http://www.semanticweb.org/marthinust/ontologies/2022/8/Gait_Ontology#Treatment"/>
        <opla-sd:entityPosition>
            <rdf:Description>
                <opla-sd:entityPositionX rdf:datatype="http://www.w3.org/2001/XMLSchema#double">179.09484336904515</opla-sd:entityPositionX>
                <opla-sd:entityPositionY rdf:datatype="http://www.w3.org/2001/XMLSchema#double">74.62570035418058</opla-sd:entityPositionY>
                <rdfs:comment xml:lang="en">This is an entity positioning annotation generated by CoModIDE (https://comodide.com/). Removing this annotation will break rendering the CoModIDE schema diagram view.</rdfs:comment>
            </rdf:Description>
        </opla-sd:entityPosition>
        <rdfs:comment xml:lang="en">Pharmacotherapy (pharmacology) is the treatment of a disorder or disease with medication.

Pharmacotherapy is the treatment of health conditions by using pharmaceutical products (drugs) as medication.</rdfs:comment>
        <rdfs:label xml:lang="en">Pharmacotherapy</rdfs:label>
    </owl:Class>
    


    <!-- http://www.semanticweb.org/marthinust/ontologies/2022/8/Gait_Ontology#Physical_therapy -->

    <owl:Class rdf:about="http://www.semanticweb.org/marthinust/ontologies/2022/8/Gait_Ontology#Physical_therapy">
        <rdfs:subClassOf rdf:resource="http://www.semanticweb.org/marthinust/ontologies/2022/8/Gait_Ontology#Treatment"/>
        <opla-sd:entityPosition>
            <rdf:Description>
                <opla-sd:entityPositionX rdf:datatype="http://www.w3.org/2001/XMLSchema#double">270.40059419471936</opla-sd:entityPositionX>
                <opla-sd:entityPositionY rdf:datatype="http://www.w3.org/2001/XMLSchema#double">242.31436900922324</opla-sd:entityPositionY>
                <rdfs:comment xml:lang="en">This is an entity positioning annotation generated by CoModIDE (https://comodide.com/). Removing this annotation will break rendering the CoModIDE schema diagram view.</rdfs:comment>
            </rdf:Description>
        </opla-sd:entityPosition>
        <rdfs:comment xml:lang="en">The most popular physical therapy specialty is orthopedic physical therapy, which involves treating conditions of the bones, muscles, ligaments, tendons and joints.

Physical therapy is care that aims to ease pain and help you function, move, and live better. This is in an effort to relieve pain. Improve movement or ability. Prevent or recover from a (sports) injury.</rdfs:comment>
        <rdfs:label xml:lang="en">Physical_therapy</rdfs:label>
    </owl:Class>
    


    <!-- http://www.semanticweb.org/marthinust/ontologies/2022/8/Gait_Ontology#Pre_swing -->

    <owl:Class rdf:about="http://www.semanticweb.org/marthinust/ontologies/2022/8/Gait_Ontology#Pre_swing">
        <rdfs:subClassOf rdf:resource="http://www.semanticweb.org/marthinust/ontologies/2022/8/Gait_Ontology#Swing_phase"/>
        <opla-sd:entityPosition>
            <rdf:Description>
                <opla-sd:entityPositionX rdf:datatype="http://www.w3.org/2001/XMLSchema#double">13.734045246276006</opla-sd:entityPositionX>
                <opla-sd:entityPositionY rdf:datatype="http://www.w3.org/2001/XMLSchema#double">154.30598895601244</opla-sd:entityPositionY>
                <rdfs:comment xml:lang="en">This is an entity positioning annotation generated by CoModIDE (https://comodide.com/). Removing this annotation will break rendering the CoModIDE schema diagram view.</rdfs:comment>
            </rdf:Description>
        </opla-sd:entityPosition>
        <rdfs:comment xml:lang="en">The pre-swing phase is the phase of the gait cycle that occurs immediately before the initial swing phase. It begins when the heel of the supporting foot makes contact with the ground at the end of the stance phase and ends when the foot leaves the ground at the beginning of the initial swing phase.

During the pre swing phase, the hip, knee, and ankle joints undergo a rapid series of movements as the body shifts weight from the supporting leg to the swinging leg. This helps to propel the body forward and prepare the leg for the initial swing phase

Pre-swing takes place during 50-62% of the gait cycle. Pre-swing is the transition phase between stance and swing, in which the foot is pushed and lifted off of the ground.</rdfs:comment>
        <rdfs:label xml:lang="en">Pre_swing</rdfs:label>
    </owl:Class>
    


    <!-- http://www.semanticweb.org/marthinust/ontologies/2022/8/Gait_Ontology#Pressure_sensors -->

    <owl:Class rdf:about="http://www.semanticweb.org/marthinust/ontologies/2022/8/Gait_Ontology#Pressure_sensors">
        <rdfs:subClassOf rdf:resource="http://www.semanticweb.org/marthinust/ontologies/2022/8/Gait_Ontology#Gait_Analysis_Equipment"/>
        <opla-sd:entityPosition>
            <rdf:Description>
                <opla-sd:entityPositionX rdf:datatype="http://www.w3.org/2001/XMLSchema#double">188.83824031914543</opla-sd:entityPositionX>
                <opla-sd:entityPositionY rdf:datatype="http://www.w3.org/2001/XMLSchema#double">292.69727859640966</opla-sd:entityPositionY>
                <rdfs:comment xml:lang="en">This is an entity positioning annotation generated by CoModIDE (https://comodide.com/). Removing this annotation will break rendering the CoModIDE schema diagram view.</rdfs:comment>
            </rdf:Description>
        </opla-sd:entityPosition>
        <rdfs:comment xml:lang="en">Pressure sensors have been widely used to measure gait and the distributed vertical component of GRF, as well as to analyse the loading pattern on the plantar soft tissue during the stance phase of gait. However, in these systems, the transverse components of GRF (friction forces), which are some of the primary factors resulting in falling, have been neglected. By fixing two externally mounted sensors beneath the front and rear boards of a special shoe, an instrumented shoe for ambulatory measurements of center of pressure (CoP) and triaxial GRF in successive walking trials has been developed.</rdfs:comment>
        <rdfs:label xml:lang="en">Pressure_sensor</rdfs:label>
    </owl:Class>
    


    <!-- http://www.semanticweb.org/marthinust/ontologies/2022/8/Gait_Ontology#Progressive_gait_ataxia -->

    <owl:Class rdf:about="http://www.semanticweb.org/marthinust/ontologies/2022/8/Gait_Ontology#Progressive_gait_ataxia">
        <rdfs:subClassOf rdf:resource="http://www.semanticweb.org/marthinust/ontologies/2022/8/Gait_Ontology#Gait_ataxia"/>
        <opla-sd:entityPosition>
            <rdf:Description>
                <opla-sd:entityPositionX rdf:datatype="http://www.w3.org/2001/XMLSchema#double">131.38963633409514</opla-sd:entityPositionX>
                <opla-sd:entityPositionY rdf:datatype="http://www.w3.org/2001/XMLSchema#double">123.61875745956273</opla-sd:entityPositionY>
                <rdfs:comment xml:lang="en">This is an entity positioning annotation generated by CoModIDE (https://comodide.com/). Removing this annotation will break rendering the CoModIDE schema diagram view.</rdfs:comment>
            </rdf:Description>
        </opla-sd:entityPosition>
        <rdfs:comment xml:lang="en">A type of gait ataxia displaying progression of clinical severity. Progressive ataxia describes a group of uncommon neurological disorders, characterised by problems with balance and coordination.

Progressive cerebellar ataxia is a degenerative neurological condition that affects the nervous system. It occurs when the cerebellum is damaged due to exposure to certain medications, autoimmune disorders, genetics, or other factors.</rdfs:comment>
        <rdfs:label xml:lang="en">Progressive_gait_ataxia</rdfs:label>
    </owl:Class>
    


    <!-- http://www.semanticweb.org/marthinust/ontologies/2022/8/Gait_Ontology#Progressive_supranuclear_palsy -->

    <owl:Class rdf:about="http://www.semanticweb.org/marthinust/ontologies/2022/8/Gait_Ontology#Progressive_supranuclear_palsy">
        <rdfs:subClassOf rdf:resource="http://www.semanticweb.org/marthinust/ontologies/2022/8/Gait_Ontology#Cerebellar_disease"/>
        <opla-sd:entityPosition>
            <rdf:Description>
                <opla-sd:entityPositionX rdf:datatype="http://www.w3.org/2001/XMLSchema#double">178.13353257050258</opla-sd:entityPositionX>
                <opla-sd:entityPositionY rdf:datatype="http://www.w3.org/2001/XMLSchema#double">228.03149596334637</opla-sd:entityPositionY>
                <rdfs:comment xml:lang="en">This is an entity positioning annotation generated by CoModIDE (https://comodide.com/). Removing this annotation will break rendering the CoModIDE schema diagram view.</rdfs:comment>
            </rdf:Description>
        </opla-sd:entityPosition>
        <rdfs:comment xml:lang="en">Progressive supranuclear palsy (PSP) is a rare neurological disorder that affects your body movements, walking and balance, and eye movement. It results from damage to nerve cells in areas of the brain that control thinking and body movement.

PSP is different than Parkinson&apos;s diseaseanother movement disorderalthough they share some symptoms (see section, How is PSP different from Parkinson&apos;s Disease?). PSP typically begins in late middle age and worsens over time, with severe disability occurring within three to five years of onset. The disease can lead to serious complications such as pneumonia, choking, head injury, and fractures.

Currently there is no effective treatment for PSP, but some symptoms can be managed with medication or other interventions.

Symptoms

PSP affects your movement, control of walking (gait) and balance, speech, swallowing, eye movements and vision, mood and behavior, and thinking. The most frequent first symptom of PSP is a loss of balance while walking. You may also have abrupt and unexplained falls without loss of consciousness, a stiff and awkward gait, or slow movement.

Progressive supranuclear palsy is also called Steele-Richardson-Olszewski syndrome.</rdfs:comment>
        <rdfs:label xml:lang="en">Progressive_supranuclear_palsy</rdfs:label>
    </owl:Class>
    


    <!-- http://www.semanticweb.org/marthinust/ontologies/2022/8/Gait_Ontology#Propulsive_gait -->

    <owl:Class rdf:about="http://www.semanticweb.org/marthinust/ontologies/2022/8/Gait_Ontology#Propulsive_gait">
        <rdfs:subClassOf rdf:resource="http://www.semanticweb.org/marthinust/ontologies/2022/8/Gait_Ontology#Parkinsonian_gait"/>
        <opla-sd:entityPosition>
            <rdf:Description>
                <opla-sd:entityPositionX rdf:datatype="http://www.w3.org/2001/XMLSchema#double">203.51719691615085</opla-sd:entityPositionX>
                <opla-sd:entityPositionY rdf:datatype="http://www.w3.org/2001/XMLSchema#double">208.77176089292462</opla-sd:entityPositionY>
                <rdfs:comment xml:lang="en">This is an entity positioning annotation generated by CoModIDE (https://comodide.com/). Removing this annotation will break rendering the CoModIDE schema diagram view.</rdfs:comment>
            </rdf:Description>
        </opla-sd:entityPosition>
        <rdfs:comment xml:lang="en">A propulsive gait is a stooped, stiff posture with the head and neck bent forward. It may be caused by toxins (like carbon monoxide poisoning), Parkinson&apos;s disease or certain medications (like haloperidol).

This type of gait is seen in patients with parkinsonism. It is characterized by a stooping, rigid posture, and the head and neck are bent forward. Steps tend to become faster and shorter.</rdfs:comment>
        <rdfs:label xml:lang="en">Propulsive_gait</rdfs:label>
    </owl:Class>
    


    <!-- http://www.semanticweb.org/marthinust/ontologies/2022/8/Gait_Ontology#Prosthetic_leg -->

    <owl:Class rdf:about="http://www.semanticweb.org/marthinust/ontologies/2022/8/Gait_Ontology#Prosthetic_leg">
        <rdfs:subClassOf rdf:resource="http://www.semanticweb.org/marthinust/ontologies/2022/8/Gait_Ontology#Gait_Assistive_Technology"/>
        <opla-sd:entityPosition>
            <rdf:Description>
                <opla-sd:entityPositionX rdf:datatype="http://www.w3.org/2001/XMLSchema#double">32.73613189711577</opla-sd:entityPositionX>
                <opla-sd:entityPositionY rdf:datatype="http://www.w3.org/2001/XMLSchema#double">158.17766257070969</opla-sd:entityPositionY>
                <rdfs:comment xml:lang="en">This is an entity positioning annotation generated by CoModIDE (https://comodide.com/). Removing this annotation will break rendering the CoModIDE schema diagram view.</rdfs:comment>
            </rdf:Description>
        </opla-sd:entityPosition>
        <rdfs:comment xml:lang="en">Prosthetic legs, or prostheses, can help people with leg amputations get around more easily. They mimic the function and, sometimes, even the appearance of a real leg. Some people still need a cane, walker or crutches to walk with a prosthetic leg, while others can walk freely.</rdfs:comment>
        <rdfs:label xml:lang="en">Prosthetic_leg</rdfs:label>
    </owl:Class>
    


    <!-- http://www.semanticweb.org/marthinust/ontologies/2022/8/Gait_Ontology#Proximal_neuropathy -->

    <owl:Class rdf:about="http://www.semanticweb.org/marthinust/ontologies/2022/8/Gait_Ontology#Proximal_neuropathy">
        <rdfs:subClassOf rdf:resource="http://www.semanticweb.org/marthinust/ontologies/2022/8/Gait_Ontology#Neuropathy"/>
        <opla-sd:entityPosition>
            <rdf:Description>
                <opla-sd:entityPositionX rdf:datatype="http://www.w3.org/2001/XMLSchema#double">280.1632869044896</opla-sd:entityPositionX>
                <opla-sd:entityPositionY rdf:datatype="http://www.w3.org/2001/XMLSchema#double">148.29747299031845</opla-sd:entityPositionY>
                <rdfs:comment xml:lang="en">This is an entity positioning annotation generated by CoModIDE (https://comodide.com/). Removing this annotation will break rendering the CoModIDE schema diagram view.</rdfs:comment>
            </rdf:Description>
        </opla-sd:entityPosition>
        <rdfs:comment xml:lang="en">Proximal neuropathy is a rare and disabling type of nerve damage in your hip, buttock, or thigh. This type of nerve damage typically affects one side of your body and may rarely spread to the other side. Proximal neuropathy is more common in men than in women and more common in people older than age 50.</rdfs:comment>
        <rdfs:label xml:lang="en">Proximal_neuropathy</rdfs:label>
    </owl:Class>
    


    <!-- http://www.semanticweb.org/marthinust/ontologies/2022/8/Gait_Ontology#Rehabilitation_therapy -->

    <owl:Class rdf:about="http://www.semanticweb.org/marthinust/ontologies/2022/8/Gait_Ontology#Rehabilitation_therapy">
        <rdfs:subClassOf rdf:resource="http://www.semanticweb.org/marthinust/ontologies/2022/8/Gait_Ontology#Treatment"/>
        <opla-sd:entityPosition>
            <rdf:Description>
                <opla-sd:entityPositionX rdf:datatype="http://www.w3.org/2001/XMLSchema#double">87.76312326610068</opla-sd:entityPositionX>
                <opla-sd:entityPositionY rdf:datatype="http://www.w3.org/2001/XMLSchema#double">119.9978555465059</opla-sd:entityPositionY>
                <rdfs:comment xml:lang="en">This is an entity positioning annotation generated by CoModIDE (https://comodide.com/). Removing this annotation will break rendering the CoModIDE schema diagram view.</rdfs:comment>
            </rdf:Description>
        </opla-sd:entityPosition>
        <rdfs:comment xml:lang="en">Rehabilitation is defined as a set of interventions designed to optimise functioning and reduce disability in individuals with health conditions in interaction with their environment.

A rehabilitation process brings about improvements to function and environment for the injured, post surgery, stroke recovery, or physically impaired person.</rdfs:comment>
        <rdfs:label xml:lang="en">Rehabilitation_therapy</rdfs:label>
    </owl:Class>
    


    <!-- http://www.semanticweb.org/marthinust/ontologies/2022/8/Gait_Ontology#Rheumatoid_arthritis -->

    <owl:Class rdf:about="http://www.semanticweb.org/marthinust/ontologies/2022/8/Gait_Ontology#Rheumatoid_arthritis">
        <rdfs:subClassOf rdf:resource="http://www.semanticweb.org/marthinust/ontologies/2022/8/Gait_Ontology#Arthritis"/>
        <opla-sd:entityPosition>
            <rdf:Description>
                <opla-sd:entityPositionX rdf:datatype="http://www.w3.org/2001/XMLSchema#double">231.1975678797878</opla-sd:entityPositionX>
                <opla-sd:entityPositionY rdf:datatype="http://www.w3.org/2001/XMLSchema#double">147.49604777372585</opla-sd:entityPositionY>
                <rdfs:comment xml:lang="en">This is an entity positioning annotation generated by CoModIDE (https://comodide.com/). Removing this annotation will break rendering the CoModIDE schema diagram view.</rdfs:comment>
            </rdf:Description>
        </opla-sd:entityPosition>
        <rdfs:comment>A chronic inflammatory disorder affecting many joints, including those in the hands and feet. In rheumatoid arthritis, the body&apos;s immune system attacks its own tissue, including joints. In severe cases, it attacks internal organs. Rheumatoid arthritis affects joint linings, causing painful swelling. Over long periods of time, the inflammation associated with rheumatoid arthritis can cause bone erosion and joint deformity.</rdfs:comment>
        <rdfs:comment>Rheumatoid arthritis (RA) has many physical and social consequences and can lower quality of life. It can cause pain, disability, and premature death. Premature heart disease. RA usually affects the hands and feet first, but it can occur in any joint. It usually involves the same joints on both sides of the body. People with RA are also at a higher risk for developing other chronic diseases such as heart disease and diabetes</rdfs:comment>
        <rdfs:label xml:lang="en">Rheumatiod_arthritis</rdfs:label>
    </owl:Class>
    


    <!-- http://www.semanticweb.org/marthinust/ontologies/2022/8/Gait_Ontology#Scissor_gait -->

    <owl:Class rdf:about="http://www.semanticweb.org/marthinust/ontologies/2022/8/Gait_Ontology#Scissor_gait">
        <rdfs:subClassOf rdf:resource="http://www.semanticweb.org/marthinust/ontologies/2022/8/Gait_Ontology#Spastic_paraparetic_gait"/>
        <opla-sd:entityPosition>
            <rdf:Description>
                <opla-sd:entityPositionX rdf:datatype="http://www.w3.org/2001/XMLSchema#double">269.25767460432894</opla-sd:entityPositionX>
                <opla-sd:entityPositionY rdf:datatype="http://www.w3.org/2001/XMLSchema#double">165.37382648613516</opla-sd:entityPositionY>
                <rdfs:comment xml:lang="en">This is an entity positioning annotation generated by CoModIDE (https://comodide.com/). Removing this annotation will break rendering the CoModIDE schema diagram view.</rdfs:comment>
            </rdf:Description>
        </opla-sd:entityPosition>
        <rdfs:comment>A type of spastic paraparetic gait in which the muscle tone in the adductors is marked. It is characterized by hypertonia and flexion in the legs, hips and pelvis accompanied by extreme adduction leading to the knees and thighs hitting, or sometimes even crossing, in a scissors-like movement. The opposing muscles (abductors) become comparatively weak from lack of use.

Scissor gait is a form of gait abnormality primarily associated with spastic cerebral palsy.</rdfs:comment>
        <rdfs:label xml:lang="en">Scissor_gait</rdfs:label>
    </owl:Class>
    


    <!-- http://www.semanticweb.org/marthinust/ontologies/2022/8/Gait_Ontology#Scoliosis -->

    <owl:Class rdf:about="http://www.semanticweb.org/marthinust/ontologies/2022/8/Gait_Ontology#Scoliosis">
        <rdfs:subClassOf rdf:resource="http://www.semanticweb.org/marthinust/ontologies/2022/8/Gait_Ontology#Gait-related_Disease"/>
    </owl:Class>
    


    <!-- http://www.semanticweb.org/marthinust/ontologies/2022/8/Gait_Ontology#Sensors -->

    <owl:Class rdf:about="http://www.semanticweb.org/marthinust/ontologies/2022/8/Gait_Ontology#Sensors">
        <rdfs:subClassOf rdf:resource="http://www.semanticweb.org/marthinust/ontologies/2022/8/Gait_Ontology#Gait_Analysis_Method"/>
        <opla-sd:entityPosition>
            <rdf:Description>
                <opla-sd:entityPositionX rdf:datatype="http://www.w3.org/2001/XMLSchema#double">167.9709857784413</opla-sd:entityPositionX>
                <opla-sd:entityPositionY rdf:datatype="http://www.w3.org/2001/XMLSchema#double">9.326579043390725</opla-sd:entityPositionY>
                <rdfs:comment xml:lang="en">This is an entity positioning annotation generated by CoModIDE (https://comodide.com/). Removing this annotation will break rendering the CoModIDE schema diagram view.</rdfs:comment>
            </rdf:Description>
        </opla-sd:entityPosition>
        <rdfs:comment xml:lang="en">In gait analysis using wearable sensors, motion sensors are worn or attached to various parts of the patients body, such as the foot and waist. These sensors, which may be accelerometers, gyrosensors, force sensors, strain gauges, inclinometers, goniometers, and so on, can measure various characteristics of the human gait. The temporal characteristics of gait are collected and estimated from body-worn accelerometers and pressure sensors inside footwear, on leg sections such as the knee, ankle or foot.</rdfs:comment>
        <rdfs:label xml:lang="en">Sensors</rdfs:label>
    </owl:Class>
    


    <!-- http://www.semanticweb.org/marthinust/ontologies/2022/8/Gait_Ontology#Sensory_gait -->

    <owl:Class rdf:about="http://www.semanticweb.org/marthinust/ontologies/2022/8/Gait_Ontology#Sensory_gait">
        <rdfs:subClassOf rdf:resource="http://www.semanticweb.org/marthinust/ontologies/2022/8/Gait_Ontology#Type_of_Gait"/>
        <opla-sd:entityPosition>
            <rdf:Description>
                <opla-sd:entityPositionX rdf:datatype="http://www.w3.org/2001/XMLSchema#double">175.72503282561797</opla-sd:entityPositionX>
                <opla-sd:entityPositionY rdf:datatype="http://www.w3.org/2001/XMLSchema#double">53.64284552941387</opla-sd:entityPositionY>
                <rdfs:comment xml:lang="en">This is an entity positioning annotation generated by CoModIDE (https://comodide.com/). Removing this annotation will break rendering the CoModIDE schema diagram view.</rdfs:comment>
            </rdf:Description>
        </opla-sd:entityPosition>
        <rdfs:comment xml:lang="en">As our feet touch the ground, we receive propioreceptive information to tell us their location. The sensory ataxic gait occurs when there is loss of this propioreceptive input. In an effort to know when the feet land and their location, the patient will slam the foot hard onto the ground in order to sense it. A key to this gait involves its exacerbation when patients cannot see their feet (i.e. in the dark). This gait is also sometimes referred to as a stomping gait since patients may lift their legs very high to hit the ground hard. This gait can be seen in disorders of the dorsal columns (B12 deficiency or tabes dorsalis) or in diseases affecting the peripheral nerves (uncontrolled diabetes). In its severe form, this gait can cause an ataxia that resembles the cerebellar ataxic gait.</rdfs:comment>
        <rdfs:label xml:lang="en">Sensory_gait</rdfs:label>
    </owl:Class>
    


    <!-- http://www.semanticweb.org/marthinust/ontologies/2022/8/Gait_Ontology#Severe_weak_quadriceps -->

    <owl:Class rdf:about="http://www.semanticweb.org/marthinust/ontologies/2022/8/Gait_Ontology#Severe_weak_quadriceps">
        <rdfs:subClassOf rdf:resource="http://www.semanticweb.org/marthinust/ontologies/2022/8/Gait_Ontology#Knee"/>
        <opla-sd:entityPosition>
            <rdf:Description>
                <opla-sd:entityPositionX rdf:datatype="http://www.w3.org/2001/XMLSchema#double">172.2241252841535</opla-sd:entityPositionX>
                <opla-sd:entityPositionY rdf:datatype="http://www.w3.org/2001/XMLSchema#double">27.781502555113427</opla-sd:entityPositionY>
                <rdfs:comment xml:lang="en">This is an entity positioning annotation generated by CoModIDE (https://comodide.com/). Removing this annotation will break rendering the CoModIDE schema diagram view.</rdfs:comment>
            </rdf:Description>
        </opla-sd:entityPosition>
        <rdfs:comment xml:lang="en">Severe Quadriceps Weakness or instability at the knee joint will present in hyperextension during the initial contact to stance phase. The knee joint will snap back into hyperextension as the bodyweight moves forwards over the limb</rdfs:comment>
        <rdfs:label xml:lang="en">Severe_quadriceps_weakness</rdfs:label>
    </owl:Class>
    


    <!-- http://www.semanticweb.org/marthinust/ontologies/2022/8/Gait_Ontology#Severity_Scale -->

    <owl:Class rdf:about="http://www.semanticweb.org/marthinust/ontologies/2022/8/Gait_Ontology#Severity_Scale">
        <owl:equivalentClass>
            <owl:Class>
                <owl:oneOf rdf:parseType="Collection">
                    <rdf:Description rdf:about="http://www.semanticweb.org/marthinust/ontologies/2022/8/Gait_Ontology#Acute"/>
                    <rdf:Description rdf:about="http://www.semanticweb.org/marthinust/ontologies/2022/8/Gait_Ontology#Mild"/>
                    <rdf:Description rdf:about="http://www.semanticweb.org/marthinust/ontologies/2022/8/Gait_Ontology#Severe"/>
                </owl:oneOf>
            </owl:Class>
        </owl:equivalentClass>
        <rdfs:subClassOf rdf:resource="http://www.semanticweb.org/marthinust/ontologies/2022/8/Gait_Ontology#Gait_Pathology"/>
        <opla-sd:entityPosition>
            <rdf:Description>
                <opla-sd:entityPositionX rdf:datatype="http://www.w3.org/2001/XMLSchema#double">27.12748925194704</opla-sd:entityPositionX>
                <opla-sd:entityPositionY rdf:datatype="http://www.w3.org/2001/XMLSchema#double">17.34820184208155</opla-sd:entityPositionY>
                <rdfs:comment xml:lang="en">This is an entity positioning annotation generated by CoModIDE (https://comodide.com/). Removing this annotation will break rendering the CoModIDE schema diagram view.</rdfs:comment>
            </rdf:Description>
        </opla-sd:entityPosition>
        <rdfs:comment xml:lang="en">The tolerance severity level of a morbidity or impairment i.e: &apos;mild&apos;, &apos;acute&apos; or &apos;severe&apos;.</rdfs:comment>
        <rdfs:label xml:lang="en">Severity_Scale</rdfs:label>
    </owl:Class>
    


    <!-- http://www.semanticweb.org/marthinust/ontologies/2022/8/Gait_Ontology#Short_stepped_shuffling_gait -->

    <owl:Class rdf:about="http://www.semanticweb.org/marthinust/ontologies/2022/8/Gait_Ontology#Short_stepped_shuffling_gait">
        <rdfs:subClassOf rdf:resource="http://www.semanticweb.org/marthinust/ontologies/2022/8/Gait_Ontology#Shuffling_gait"/>
        <opla-sd:entityPosition>
            <rdf:Description>
                <opla-sd:entityPositionX rdf:datatype="http://www.w3.org/2001/XMLSchema#double">287.48817423974543</opla-sd:entityPositionX>
                <opla-sd:entityPositionY rdf:datatype="http://www.w3.org/2001/XMLSchema#double">220.80682848337446</opla-sd:entityPositionY>
                <rdfs:comment xml:lang="en">This is an entity positioning annotation generated by CoModIDE (https://comodide.com/). Removing this annotation will break rendering the CoModIDE schema diagram view.</rdfs:comment>
            </rdf:Description>
        </opla-sd:entityPosition>
        <rdfs:comment xml:lang="en">Short stepped shuffling walk</rdfs:comment>
        <rdfs:label xml:lang="en">Short_stepped_shuffling_gait</rdfs:label>
    </owl:Class>
    


    <!-- http://www.semanticweb.org/marthinust/ontologies/2022/8/Gait_Ontology#Shuffling_gait -->

    <owl:Class rdf:about="http://www.semanticweb.org/marthinust/ontologies/2022/8/Gait_Ontology#Shuffling_gait">
        <rdfs:subClassOf rdf:resource="http://www.semanticweb.org/marthinust/ontologies/2022/8/Gait_Ontology#Gait_Disturbance"/>
        <opla-sd:entityPosition>
            <rdf:Description>
                <opla-sd:entityPositionX rdf:datatype="http://www.w3.org/2001/XMLSchema#double">57.65008406101198</opla-sd:entityPositionX>
                <opla-sd:entityPositionY rdf:datatype="http://www.w3.org/2001/XMLSchema#double">194.33411145608952</opla-sd:entityPositionY>
                <rdfs:comment xml:lang="en">This is an entity positioning annotation generated by CoModIDE (https://comodide.com/). Removing this annotation will break rendering the CoModIDE schema diagram view.</rdfs:comment>
            </rdf:Description>
        </opla-sd:entityPosition>
        <rdfs:comment xml:lang="en">A type of gait (walking) characterized by by dragging one&apos;s feet along or without lifting the feet fully from the ground.</rdfs:comment>
        <rdfs:label xml:lang="en">Shuffling_gait</rdfs:label>
    </owl:Class>
    


    <!-- http://www.semanticweb.org/marthinust/ontologies/2022/8/Gait_Ontology#Single_support -->

    <owl:Class rdf:about="http://www.semanticweb.org/marthinust/ontologies/2022/8/Gait_Ontology#Single_support">
        <rdfs:subClassOf rdf:resource="http://www.semanticweb.org/marthinust/ontologies/2022/8/Gait_Ontology#Gait_Parameter"/>
        <opla-sd:entityPosition>
            <rdf:Description>
                <opla-sd:entityPositionX rdf:datatype="http://www.w3.org/2001/XMLSchema#double">64.64818146196747</opla-sd:entityPositionX>
                <opla-sd:entityPositionY rdf:datatype="http://www.w3.org/2001/XMLSchema#double">62.0128022727969</opla-sd:entityPositionY>
                <rdfs:comment xml:lang="en">This is an entity positioning annotation generated by CoModIDE (https://comodide.com/). Removing this annotation will break rendering the CoModIDE schema diagram view.</rdfs:comment>
            </rdf:Description>
        </opla-sd:entityPosition>
        <rdfs:comment xml:lang="en">Single support is the inverse of double support, as a walking motion consists of having at least one foot on the ground at all times.Therefore the normative values of single support would be 100% - double support%. For the general adult population, 80% single support is the norm.</rdfs:comment>
        <rdfs:label xml:lang="en">Single_support</rdfs:label>
    </owl:Class>
    


    <!-- http://www.semanticweb.org/marthinust/ontologies/2022/8/Gait_Ontology#Spastic_gait -->

    <owl:Class rdf:about="http://www.semanticweb.org/marthinust/ontologies/2022/8/Gait_Ontology#Spastic_gait">
        <rdfs:subClassOf rdf:resource="http://www.semanticweb.org/marthinust/ontologies/2022/8/Gait_Ontology#Gait_Disturbance"/>
        <opla-sd:entityPosition>
            <rdf:Description>
                <opla-sd:entityPositionX rdf:datatype="http://www.w3.org/2001/XMLSchema#double">175.63147339453698</opla-sd:entityPositionX>
                <opla-sd:entityPositionY rdf:datatype="http://www.w3.org/2001/XMLSchema#double">200.20668308823758</opla-sd:entityPositionY>
                <rdfs:comment xml:lang="en">This is an entity positioning annotation generated by CoModIDE (https://comodide.com/). Removing this annotation will break rendering the CoModIDE schema diagram view.</rdfs:comment>
            </rdf:Description>
        </opla-sd:entityPosition>
        <rdfs:comment xml:lang="en">Spasticity is manifested by increased stretch reflex which is intensified with movement velocity. This results in excessive and inappropriate muscle activation which can contribute to muscle hypertonia. Spastic gait is characterized by manifestations such as muscle hypertonia, stiff knee, and circumduction of the leg.</rdfs:comment>
        <rdfs:label xml:lang="en">Spastic_gait</rdfs:label>
    </owl:Class>
    


    <!-- http://www.semanticweb.org/marthinust/ontologies/2022/8/Gait_Ontology#Spastic_hemiparetic_gait -->

    <owl:Class rdf:about="http://www.semanticweb.org/marthinust/ontologies/2022/8/Gait_Ontology#Spastic_hemiparetic_gait">
        <rdfs:subClassOf rdf:resource="http://www.semanticweb.org/marthinust/ontologies/2022/8/Gait_Ontology#Spastic_gait"/>
        <opla-sd:entityPosition>
            <rdf:Description>
                <opla-sd:entityPositionX rdf:datatype="http://www.w3.org/2001/XMLSchema#double">25.592872243952336</opla-sd:entityPositionX>
                <opla-sd:entityPositionY rdf:datatype="http://www.w3.org/2001/XMLSchema#double">165.90472334586346</opla-sd:entityPositionY>
                <rdfs:comment xml:lang="en">This is an entity positioning annotation generated by CoModIDE (https://comodide.com/). Removing this annotation will break rendering the CoModIDE schema diagram view.</rdfs:comment>
            </rdf:Description>
        </opla-sd:entityPosition>
        <rdfs:comment xml:lang="en">Spastic hemiparesis is characterized by a dominance of the tonus in the upper limb flexor muscles: the arm is held in an adducted posture and is bent and rotated inwards, the forearm is pronated and the hand and the fingers are flexed. The leg is slightly bent at the hip, the knee cannot be extended fully at the end of the stance phase and the foot is inverted and in a plantar flexed position. Gait is slow, with a wide base and asymmetrical with a shortened weight-bearing phase on the paretic side. During the swing phase, the paretic leg performs a lateral movement (circumduction) which is characteristic of this gait disorder, also termed Wernicke-Mann gait. Spastic gait problems typically worsen on attempts to walk faster.</rdfs:comment>
        <rdfs:label xml:lang="en">Spastic_hemiparetic_gait</rdfs:label>
    </owl:Class>
    


    <!-- http://www.semanticweb.org/marthinust/ontologies/2022/8/Gait_Ontology#Spastic_paraparetic_gait -->

    <owl:Class rdf:about="http://www.semanticweb.org/marthinust/ontologies/2022/8/Gait_Ontology#Spastic_paraparetic_gait">
        <rdfs:subClassOf rdf:resource="http://www.semanticweb.org/marthinust/ontologies/2022/8/Gait_Ontology#Spastic_gait"/>
        <opla-sd:entityPosition>
            <rdf:Description>
                <opla-sd:entityPositionX rdf:datatype="http://www.w3.org/2001/XMLSchema#double">5.884091833597093</opla-sd:entityPositionX>
                <opla-sd:entityPositionY rdf:datatype="http://www.w3.org/2001/XMLSchema#double">264.8571331718689</opla-sd:entityPositionY>
                <rdfs:comment xml:lang="en">This is an entity positioning annotation generated by CoModIDE (https://comodide.com/). Removing this annotation will break rendering the CoModIDE schema diagram view.</rdfs:comment>
            </rdf:Description>
        </opla-sd:entityPosition>
        <rdfs:comment xml:lang="en">A type of spastic gait in which the legs are usually slightly bent at the hip and in an adducted position. The knees are extended or slightly bent and the feet are in a plantar flexion position. This posture requires circumduction of the legs during walking. The gait may appear stiff (spastic gait disorder) or stiff as well as insecure (spastic ataxic gait disorder). In spastic paraparetic gait, each leg appears to be dragged forward. If the muscle tone in the adductors is marked, the resulting gait disorder is referred to as scissor gait.

Early in the disease, there may be mild trouble walking and stiffness. These symptoms typically get worse slowly until a cane, walker, or wheelchair is needed.</rdfs:comment>
        <rdfs:label xml:lang="en">Spastic_paraparetic_gait</rdfs:label>
    </owl:Class>
    


    <!-- http://www.semanticweb.org/marthinust/ontologies/2022/8/Gait_Ontology#Spatiotemporal -->

    <owl:Class rdf:about="http://www.semanticweb.org/marthinust/ontologies/2022/8/Gait_Ontology#Spatiotemporal">
        <rdfs:subClassOf rdf:resource="http://www.semanticweb.org/marthinust/ontologies/2022/8/Gait_Ontology#Gait_Parameter"/>
        <opla-sd:entityPosition>
            <rdf:Description>
                <opla-sd:entityPositionX rdf:datatype="http://www.w3.org/2001/XMLSchema#double">174.94326748141458</opla-sd:entityPositionX>
                <opla-sd:entityPositionY rdf:datatype="http://www.w3.org/2001/XMLSchema#double">88.90524348536137</opla-sd:entityPositionY>
                <rdfs:comment xml:lang="en">This is an entity positioning annotation generated by CoModIDE (https://comodide.com/). Removing this annotation will break rendering the CoModIDE schema diagram view.</rdfs:comment>
            </rdf:Description>
        </opla-sd:entityPosition>
        <rdfs:comment xml:lang="en">Spatiotemporal Gait Parameters are the measures obtained from a comprehensive gait analysis using the walk or run tests. Gait analyses are used for clinical identification of deviations from normal gait. Spatiotemporal gait parameters concern spatial (distance) parameters along with temporal (time) parameters. They can also be separated into temporophasic parameters which reflect time-based percentages of these parameters in reference to the gait cycle as a whole.</rdfs:comment>
        <rdfs:label xml:lang="en">Spatiotemporal</rdfs:label>
    </owl:Class>
    


    <!-- http://www.semanticweb.org/marthinust/ontologies/2022/8/Gait_Ontology#Specialised_footwear -->

    <owl:Class rdf:about="http://www.semanticweb.org/marthinust/ontologies/2022/8/Gait_Ontology#Specialised_footwear">
        <rdfs:subClassOf rdf:resource="http://www.semanticweb.org/marthinust/ontologies/2022/8/Gait_Ontology#Gait_Assistive_Technology"/>
        <opla-sd:entityPosition>
            <rdf:Description>
                <opla-sd:entityPositionX rdf:datatype="http://www.w3.org/2001/XMLSchema#double">40.97200915576761</opla-sd:entityPositionX>
                <opla-sd:entityPositionY rdf:datatype="http://www.w3.org/2001/XMLSchema#double">23.774725583714844</opla-sd:entityPositionY>
                <rdfs:comment xml:lang="en">This is an entity positioning annotation generated by CoModIDE (https://comodide.com/). Removing this annotation will break rendering the CoModIDE schema diagram view.</rdfs:comment>
            </rdf:Description>
        </opla-sd:entityPosition>
        <rdfs:comment xml:lang="en">Foot specialists, among other treatments, apply corrective measures, including specialized footwear, orthotics, and braces, to address these pathologies. However, this often based on the physical assessment and visual observations of a patients gait. In-shoe pressure measurement technology becomes a useful tool for analyzing how footwear materials influence a patients gait pattern. Having the ability to position pressure sensors within the subject or patients shoe helps tell the complete story as to whether the intervention is correcting a problem, or causing more challenges.

Specialised footwear can effectively reduce joint ligament loads and is a flexible, lightweight shoe specifically engineered to improve gait-related issues.</rdfs:comment>
        <rdfs:label xml:lang="en">Specialised_footwear</rdfs:label>
    </owl:Class>
    


    <!-- http://www.semanticweb.org/marthinust/ontologies/2022/8/Gait_Ontology#Speed -->

    <owl:Class rdf:about="http://www.semanticweb.org/marthinust/ontologies/2022/8/Gait_Ontology#Speed">
        <rdfs:subClassOf rdf:resource="http://www.semanticweb.org/marthinust/ontologies/2022/8/Gait_Ontology#Gait_Parameter"/>
        <opla-sd:entityPosition>
            <rdf:Description>
                <opla-sd:entityPositionX rdf:datatype="http://www.w3.org/2001/XMLSchema#double">297.521758345144</opla-sd:entityPositionX>
                <opla-sd:entityPositionY rdf:datatype="http://www.w3.org/2001/XMLSchema#double">222.67397705647485</opla-sd:entityPositionY>
                <rdfs:comment xml:lang="en">This is an entity positioning annotation generated by CoModIDE (https://comodide.com/). Removing this annotation will break rendering the CoModIDE schema diagram view.</rdfs:comment>
            </rdf:Description>
        </opla-sd:entityPosition>
        <rdfs:comment xml:lang="en">Measurement for walking and running speed over the entirety of an activity.
Individual foot speeds can be used to get a sense of how fast each foot is moving compared to the other.

Average walking speed is often used clinically as an overall measure of walking capacity and preparedness for safe community mobility. Changes in walking speed reflect a compensation for impaired control, so slowing of gait is a proxy for challenges to control of gait.</rdfs:comment>
        <rdfs:label xml:lang="en">Speed</rdfs:label>
    </owl:Class>
    


    <!-- http://www.semanticweb.org/marthinust/ontologies/2022/8/Gait_Ontology#Spina_bifida -->

    <owl:Class rdf:about="http://www.semanticweb.org/marthinust/ontologies/2022/8/Gait_Ontology#Spina_bifida">
        <rdfs:subClassOf rdf:resource="http://www.semanticweb.org/marthinust/ontologies/2022/8/Gait_Ontology#Gait-related_Disease"/>
        <opla-sd:entityPosition>
            <rdf:Description>
                <opla-sd:entityPositionX rdf:datatype="http://www.w3.org/2001/XMLSchema#double">219.75709260298763</opla-sd:entityPositionX>
                <opla-sd:entityPositionY rdf:datatype="http://www.w3.org/2001/XMLSchema#double">140.32503540375876</opla-sd:entityPositionY>
                <rdfs:comment xml:lang="en">This is an entity positioning annotation generated by CoModIDE (https://comodide.com/). Removing this annotation will break rendering the CoModIDE schema diagram view.</rdfs:comment>
            </rdf:Description>
        </opla-sd:entityPosition>
        <rdfs:comment xml:lang="en">Spina bifida is a gait-related disease, meaning that it can cause gait disturbances. Individuals with spina bifida often experience gait impairments due to the neurological deficits associated with the condition. These impairments can include reduced muscle strength and coordination, as well as decreased sensation, which can all lead to impaired gait patterns.

Spina bifida is a congenital birth defect that affects the spinal column and spinal cord. It occurs when the neural tube, which forms during the early stages of fetal development, does not close properly, resulting in a gap or opening in the spinal column. This can lead to damage or malformation of the spinal cord and nerves, which can cause a range of physical and neurological problems.

The condition can cause weakness or paralysis in the legs, as well as other neurological problems that can affect an individual&apos;s ability to walk and maintain balance. Some individuals with spina bifida may require assistive devices such as braces, crutches, or wheelchairs to help with mobility, while others may be able to walk independently. Treatment for spina bifida often involves physical therapy and other interventions to improve gait and mobility, as well as manage other symptoms of the condition.</rdfs:comment>
        <rdfs:label xml:lang="en">Spina_bifida</rdfs:label>
    </owl:Class>
    


    <!-- http://www.semanticweb.org/marthinust/ontologies/2022/8/Gait_Ontology#Spinocerebellar_ataxia -->

    <owl:Class rdf:about="http://www.semanticweb.org/marthinust/ontologies/2022/8/Gait_Ontology#Spinocerebellar_ataxia">
        <rdfs:subClassOf rdf:resource="http://www.semanticweb.org/marthinust/ontologies/2022/8/Gait_Ontology#Gait_ataxia"/>
        <opla-sd:entityPosition>
            <rdf:Description>
                <opla-sd:entityPositionX rdf:datatype="http://www.w3.org/2001/XMLSchema#double">75.50089450007737</opla-sd:entityPositionX>
                <opla-sd:entityPositionY rdf:datatype="http://www.w3.org/2001/XMLSchema#double">218.13817884386216</opla-sd:entityPositionY>
                <rdfs:comment xml:lang="en">This is an entity positioning annotation generated by CoModIDE (https://comodide.com/). Removing this annotation will break rendering the CoModIDE schema diagram view.</rdfs:comment>
            </rdf:Description>
        </opla-sd:entityPosition>
        <rdfs:comment xml:lang="en">Spinocerebellar ataxia-6 (SCA6) is caused by heterozygous mutation in the CACNA1A gene (601011) on chromosome.

Spinocerebellar ataxia (SCA) is consisting predominantly of mild but slowly progressive cerebellar ataxia of the limbs and gait, dysarthria, nystagmus, and mild vibratory and proprioceptive sensory loss. The disease is insidious and most patients do not realize they are affected initially but do describe a sense of momentary imbalance and &apos;wooziness&apos; when they make a quick turn or a rapid movement. Typically, it is years after this initial sensation when the patients realize they have developed balance and coordination difficulties. The disease usually progresses over 20 to 30 years, leading to impairment of gait and causing the patient to become wheelchair-bound. In a few older patients, choking has been observed, suggesting involvement of the brainstem.

The age of onset of ataxia ranged from 24 to 63 years among affected individuals. Radiographically and pathologically, there was selective atrophy of the cerebellum and extensive loss of Purkinje cells in the cerebellar cortex. In addition, clinical and quantitative measurement of extraocular movements demonstrated a characteristic pattern of oculomotor and vestibular abnormalities, including horizontal and vertical nystagmus and an abnormal vestibuloocular reflex.

Symptoms of SCA

Depending on the type of SCA, symptoms will most often appear in adulthood but can appear in childhood. Several SCAs may have their own clinical signs, but most include:

Progressive loss of coordination and balance
Progressive lack of coordination in the arms and legs, including tremor
Slowness of movement
Problems with walking (gait)
Decreased muscle tone
Vision problems, particularly with focusing the eyes and unwanted eye movements
Difficulty speaking (dysarthria) and swallowing (dysphagia)
Cognitive problems (thinking, remembering, and concentration)</rdfs:comment>
        <rdfs:label xml:lang="en">Spinocerebellar_ataxia</rdfs:label>
    </owl:Class>
    


    <!-- http://www.semanticweb.org/marthinust/ontologies/2022/8/Gait_Ontology#Stance_phase -->

    <owl:Class rdf:about="http://www.semanticweb.org/marthinust/ontologies/2022/8/Gait_Ontology#Stance_phase">
        <rdfs:subClassOf rdf:resource="http://www.semanticweb.org/marthinust/ontologies/2022/8/Gait_Ontology#Gait_Cycle"/>
        <opla-sd:entityPosition>
            <rdf:Description>
                <opla-sd:entityPositionX rdf:datatype="http://www.w3.org/2001/XMLSchema#double">212.25960714129462</opla-sd:entityPositionX>
                <opla-sd:entityPositionY rdf:datatype="http://www.w3.org/2001/XMLSchema#double">283.11227623510837</opla-sd:entityPositionY>
                <rdfs:comment xml:lang="en">This is an entity positioning annotation generated by CoModIDE (https://comodide.com/). Removing this annotation will break rendering the CoModIDE schema diagram view.</rdfs:comment>
            </rdf:Description>
        </opla-sd:entityPosition>
        <rdfs:comment xml:lang="en">The stance phase of gait begins when the foot first touches the ground and ends when the same foot leaves the ground. The stance phase makes up approximately 60% of the gait cycle.

During the stance phase, the foot contacts the ground, the mass of the body is supported, and then the body is propelled forward during the later stages of stance. During stance phase, the foot of the corresponding limb is on the ground, whereas in swing, the foot is no longer in contact with the ground, i.e., it is swinging through to move the body forward.</rdfs:comment>
        <rdfs:label xml:lang="en">Stance_phase</rdfs:label>
    </owl:Class>
    


    <!-- http://www.semanticweb.org/marthinust/ontologies/2022/8/Gait_Ontology#Step_length -->

    <owl:Class rdf:about="http://www.semanticweb.org/marthinust/ontologies/2022/8/Gait_Ontology#Step_length">
        <rdfs:subClassOf rdf:resource="http://www.semanticweb.org/marthinust/ontologies/2022/8/Gait_Ontology#Gait_Measurement_Point"/>
        <opla-sd:entityPosition>
            <rdf:Description>
                <opla-sd:entityPositionX rdf:datatype="http://www.w3.org/2001/XMLSchema#double">56.387549850299365</opla-sd:entityPositionX>
                <opla-sd:entityPositionY rdf:datatype="http://www.w3.org/2001/XMLSchema#double">166.18639218920637</opla-sd:entityPositionY>
                <rdfs:comment xml:lang="en">This is an entity positioning annotation generated by CoModIDE (https://comodide.com/). Removing this annotation will break rendering the CoModIDE schema diagram view.</rdfs:comment>
            </rdf:Description>
        </opla-sd:entityPosition>
        <rdfs:comment xml:lang="en">Step length is the distance between the point of initial contact of one foot and the point of initial contact of the opposite foot. In normal gait, right and left step lengths are similar.

A step length is the distance covered when you take one step. Start with your two feet together and start walking. You can start with either foot, but lets say you start with your left:

Lift your left foot up and step forward.

Now both feet are on the ground with your left foot ahead of your right one.
The distance your left foot traveled (from the toe of your right foot to the toe of your left foot, or from the heel of your right foot to the heel of your left foot) is your step length. There might be a difference between your left step length and your right step length.</rdfs:comment>
        <rdfs:label xml:lang="en">Step_length</rdfs:label>
    </owl:Class>
    


    <!-- http://www.semanticweb.org/marthinust/ontologies/2022/8/Gait_Ontology#Step_width -->

    <owl:Class rdf:about="http://www.semanticweb.org/marthinust/ontologies/2022/8/Gait_Ontology#Step_width">
        <rdfs:subClassOf rdf:resource="http://www.semanticweb.org/marthinust/ontologies/2022/8/Gait_Ontology#Gait_Measurement_Point"/>
        <opla-sd:entityPosition>
            <rdf:Description>
                <opla-sd:entityPositionX rdf:datatype="http://www.w3.org/2001/XMLSchema#double">215.22079458505664</opla-sd:entityPositionX>
                <opla-sd:entityPositionY rdf:datatype="http://www.w3.org/2001/XMLSchema#double">193.07415947734373</opla-sd:entityPositionY>
                <rdfs:comment xml:lang="en">This is an entity positioning annotation generated by CoModIDE (https://comodide.com/). Removing this annotation will break rendering the CoModIDE schema diagram view.</rdfs:comment>
            </rdf:Description>
        </opla-sd:entityPosition>
        <rdfs:comment xml:lang="en">Step width was determined as the distance between the outer most borders of two consecutive footprints also defined as the distance between the centre lines of the two feet, perpendicular to the plane of walking.</rdfs:comment>
        <rdfs:label xml:lang="en">Step_width</rdfs:label>
    </owl:Class>
    


    <!-- http://www.semanticweb.org/marthinust/ontologies/2022/8/Gait_Ontology#Steppage_gait -->

    <owl:Class rdf:about="http://www.semanticweb.org/marthinust/ontologies/2022/8/Gait_Ontology#Steppage_gait">
        <rdfs:subClassOf rdf:resource="http://www.semanticweb.org/marthinust/ontologies/2022/8/Gait_Ontology#Gait_Disturbance"/>
        <opla-sd:entityPosition>
            <rdf:Description>
                <opla-sd:entityPositionX rdf:datatype="http://www.w3.org/2001/XMLSchema#double">203.58759453746782</opla-sd:entityPositionX>
                <opla-sd:entityPositionY rdf:datatype="http://www.w3.org/2001/XMLSchema#double">72.32256049611925</opla-sd:entityPositionY>
                <rdfs:comment xml:lang="en">This is an entity positioning annotation generated by CoModIDE (https://comodide.com/). Removing this annotation will break rendering the CoModIDE schema diagram view.</rdfs:comment>
            </rdf:Description>
        </opla-sd:entityPosition>
        <rdfs:comment>An abnormal gait pattern that arises from weakness of the pretibial and peroneal muscles due to a lower motor neuron lesion. Affected patients have footdrop and are unable to dorsiflex and evert the foot. The leg is lifted high on walking so that the toes clear the ground, and there may be a slapping noise when the foot strikes the ground again.</rdfs:comment>
        <rdfs:label xml:lang="en">Steppage_gait</rdfs:label>
    </owl:Class>
    


    <!-- http://www.semanticweb.org/marthinust/ontologies/2022/8/Gait_Ontology#Steps -->

    <owl:Class rdf:about="http://www.semanticweb.org/marthinust/ontologies/2022/8/Gait_Ontology#Steps">
        <rdfs:subClassOf rdf:resource="http://www.semanticweb.org/marthinust/ontologies/2022/8/Gait_Ontology#Gait_Parameter"/>
        <rdfs:subClassOf rdf:resource="http://www.semanticweb.org/marthinust/ontologies/2022/8/Gait_Ontology#Stride"/>
        <opla-sd:entityPosition>
            <rdf:Description>
                <opla-sd:entityPositionX rdf:datatype="http://www.w3.org/2001/XMLSchema#double">26.31690888322603</opla-sd:entityPositionX>
                <opla-sd:entityPositionY rdf:datatype="http://www.w3.org/2001/XMLSchema#double">131.58259449315258</opla-sd:entityPositionY>
                <rdfs:comment xml:lang="en">This is an entity positioning annotation generated by CoModIDE (https://comodide.com/). Removing this annotation will break rendering the CoModIDE schema diagram view.</rdfs:comment>
            </rdf:Description>
        </opla-sd:entityPosition>
        <rdfs:comment xml:lang="en">One gait cycle, or stride, is defined as two consecutive heel strikes of the same limb. Each gait cycle is composed of two steps.

Step count is the number of steps taken over the duration of the activity.</rdfs:comment>
        <rdfs:label xml:lang="en">Steps</rdfs:label>
    </owl:Class>
    


    <!-- http://www.semanticweb.org/marthinust/ontologies/2022/8/Gait_Ontology#Stride -->

    <owl:Class rdf:about="http://www.semanticweb.org/marthinust/ontologies/2022/8/Gait_Ontology#Stride">
        <rdfs:subClassOf rdf:resource="http://www.semanticweb.org/marthinust/ontologies/2022/8/Gait_Ontology#Gait_Cycle"/>
        <opla-sd:entityPosition>
            <rdf:Description>
                <opla-sd:entityPositionX rdf:datatype="http://www.w3.org/2001/XMLSchema#double">172.37020951917066</opla-sd:entityPositionX>
                <opla-sd:entityPositionY rdf:datatype="http://www.w3.org/2001/XMLSchema#double">175.51949776538132</opla-sd:entityPositionY>
                <rdfs:comment xml:lang="en">This is an entity positioning annotation generated by CoModIDE (https://comodide.com/). Removing this annotation will break rendering the CoModIDE schema diagram view.</rdfs:comment>
            </rdf:Description>
        </opla-sd:entityPosition>
        <rdfs:comment xml:lang="en">A stride is one whole/complete gait cycle.</rdfs:comment>
        <rdfs:label xml:lang="en">Stride</rdfs:label>
    </owl:Class>
    


    <!-- http://www.semanticweb.org/marthinust/ontologies/2022/8/Gait_Ontology#Stride_length -->

    <owl:Class rdf:about="http://www.semanticweb.org/marthinust/ontologies/2022/8/Gait_Ontology#Stride_length">
        <rdfs:subClassOf rdf:resource="http://www.semanticweb.org/marthinust/ontologies/2022/8/Gait_Ontology#Gait_Measurement_Point"/>
        <opla-sd:entityPosition>
            <rdf:Description>
                <opla-sd:entityPositionX rdf:datatype="http://www.w3.org/2001/XMLSchema#double">52.11403772760838</opla-sd:entityPositionX>
                <opla-sd:entityPositionY rdf:datatype="http://www.w3.org/2001/XMLSchema#double">216.3283376022293</opla-sd:entityPositionY>
                <rdfs:comment xml:lang="en">This is an entity positioning annotation generated by CoModIDE (https://comodide.com/). Removing this annotation will break rendering the CoModIDE schema diagram view.</rdfs:comment>
            </rdf:Description>
        </opla-sd:entityPosition>
        <rdfs:comment xml:lang="en">Stride length is the distance between successive points of initial contact of the same foot. Stride length is the distance covered when you take two steps, one with each foot. Start with your two feet together and start walking. You can start with either foot, but lets say you start with your left:

Lift your left foot up and step forward.
Now both feet are on the ground with the left foot ahead of the right one.
Lift your right foot and swing it forward past your left foot, and place it on the ground.

Now both feet are on the ground with the right foot ahead of the left one.
The distance traveled during that motion is your stride length. In other words, your stride length is the distance from the toe of your right foot (starting position) to the toe of your right foot (ending position), or the heel of your right foot (starting position) to the heel of your right foot (ending position).</rdfs:comment>
        <rdfs:label xml:lang="en">Stride_length</rdfs:label>
    </owl:Class>
    


    <!-- http://www.semanticweb.org/marthinust/ontologies/2022/8/Gait_Ontology#Stride_width -->

    <owl:Class rdf:about="http://www.semanticweb.org/marthinust/ontologies/2022/8/Gait_Ontology#Stride_width">
        <rdfs:subClassOf rdf:resource="http://www.semanticweb.org/marthinust/ontologies/2022/8/Gait_Ontology#Gait_Measurement_Point"/>
        <opla-sd:entityPosition>
            <rdf:Description>
                <opla-sd:entityPositionX rdf:datatype="http://www.w3.org/2001/XMLSchema#double">33.52413231370153</opla-sd:entityPositionX>
                <opla-sd:entityPositionY rdf:datatype="http://www.w3.org/2001/XMLSchema#double">256.75047089496286</opla-sd:entityPositionY>
                <rdfs:comment xml:lang="en">This is an entity positioning annotation generated by CoModIDE (https://comodide.com/). Removing this annotation will break rendering the CoModIDE schema diagram view.</rdfs:comment>
            </rdf:Description>
        </opla-sd:entityPosition>
        <rdfs:comment xml:lang="en">Stride width, also called base of support, is the distance between the heels of the two feet during double stance. Stride width is measured either between the medial-most borders of the two heels or between lines through the midline of the two heels. Normal stride width for adults is between 1-3 inches (3-8 cm).

The walking base (also known as the stride width or base of support) is the side-to-side distance between the line of the two feet, usually measured at the midpoint of the back of the heel but sometimes below the center of the ankle joint. The preferred units for stride length and step length are meters and for the walking base, millimeters. The pattern of walking known as tandem gait involves walking with the heel of one foot placed directly in front of the toes of the other, i.e. with a walking base close to zero. Although this pattern is not typically seen, even as a pathological gait, it requires good balance and coordination and it is often used by the police as a test for intoxication!</rdfs:comment>
        <rdfs:label xml:lang="en">Stride_width</rdfs:label>
    </owl:Class>
    


    <!-- http://www.semanticweb.org/marthinust/ontologies/2022/8/Gait_Ontology#Stroke -->

    <owl:Class rdf:about="http://www.semanticweb.org/marthinust/ontologies/2022/8/Gait_Ontology#Stroke">
        <rdfs:subClassOf rdf:resource="http://www.semanticweb.org/marthinust/ontologies/2022/8/Gait_Ontology#Hemiplegia"/>
        <rdfs:subClassOf rdf:resource="http://www.semanticweb.org/marthinust/ontologies/2022/8/Gait_Ontology#Neurological"/>
        <opla-sd:entityPosition>
            <rdf:Description>
                <opla-sd:entityPositionX rdf:datatype="http://www.w3.org/2001/XMLSchema#double">138.28805797138108</opla-sd:entityPositionX>
                <opla-sd:entityPositionY rdf:datatype="http://www.w3.org/2001/XMLSchema#double">156.2504105256744</opla-sd:entityPositionY>
                <rdfs:comment xml:lang="en">This is an entity positioning annotation generated by CoModIDE (https://comodide.com/). Removing this annotation will break rendering the CoModIDE schema diagram view.</rdfs:comment>
            </rdf:Description>
        </opla-sd:entityPosition>
        <rdfs:comment xml:lang="en">A medical condition where the blood supply to a part of the brain is interrupted or reduced, leading to brain damage. Depending on the area of the brain affected, stroke survivors may experience hemiplegia (paralysis on one side of the body), which can cause gait disturbances such as dragging the affected leg or foot, limping, or reduced arm swing.</rdfs:comment>
        <rdfs:label xml:lang="en">Stroke</rdfs:label>
    </owl:Class>
    


    <!-- http://www.semanticweb.org/marthinust/ontologies/2022/8/Gait_Ontology#Surgery -->

    <owl:Class rdf:about="http://www.semanticweb.org/marthinust/ontologies/2022/8/Gait_Ontology#Surgery">
        <rdfs:subClassOf rdf:resource="http://www.semanticweb.org/marthinust/ontologies/2022/8/Gait_Ontology#Treatment"/>
        <opla-sd:entityPosition>
            <rdf:Description>
                <opla-sd:entityPositionX rdf:datatype="http://www.w3.org/2001/XMLSchema#double">229.41937836318618</opla-sd:entityPositionX>
                <opla-sd:entityPositionY rdf:datatype="http://www.w3.org/2001/XMLSchema#double">213.44811093285372</opla-sd:entityPositionY>
                <rdfs:comment xml:lang="en">This is an entity positioning annotation generated by CoModIDE (https://comodide.com/). Removing this annotation will break rendering the CoModIDE schema diagram view.</rdfs:comment>
            </rdf:Description>
        </opla-sd:entityPosition>
        <rdfs:comment xml:lang="en">Surgery, medical branch that is concerned with the treatment of injuries, diseases, and other disorders by manual and instrumental means.

Surgery or prostheses may be recommended, such as hip and knee replacement for persons with osteoarthritis.</rdfs:comment>
        <rdfs:label xml:lang="en">Surgery</rdfs:label>
    </owl:Class>
    


    <!-- http://www.semanticweb.org/marthinust/ontologies/2022/8/Gait_Ontology#Swing_phase -->

    <owl:Class rdf:about="http://www.semanticweb.org/marthinust/ontologies/2022/8/Gait_Ontology#Swing_phase">
        <rdfs:subClassOf rdf:resource="http://www.semanticweb.org/marthinust/ontologies/2022/8/Gait_Ontology#Gait_Cycle"/>
        <opla-sd:entityPosition>
            <rdf:Description>
                <opla-sd:entityPositionX rdf:datatype="http://www.w3.org/2001/XMLSchema#double">137.90768900174973</opla-sd:entityPositionX>
                <opla-sd:entityPositionY rdf:datatype="http://www.w3.org/2001/XMLSchema#double">137.8715988526785</opla-sd:entityPositionY>
                <rdfs:comment xml:lang="en">This is an entity positioning annotation generated by CoModIDE (https://comodide.com/). Removing this annotation will break rendering the CoModIDE schema diagram view.</rdfs:comment>
            </rdf:Description>
        </opla-sd:entityPosition>
        <rdfs:comment xml:lang="en">The swing phase of gait begins when the foot first leaves the ground and ends when the same foot touches the ground again. The swing phase makes up the other 40% of the gait cycle.

The swing phase is the period of time when the foot under consideration is not in contact with the floor. The stance phase is the period of time when the foot under consideration is in contact with the floor.</rdfs:comment>
        <rdfs:label xml:lang="en">Swing_phase</rdfs:label>
    </owl:Class>
    


    <!-- http://www.semanticweb.org/marthinust/ontologies/2022/8/Gait_Ontology#Terminal_stance -->

    <owl:Class rdf:about="http://www.semanticweb.org/marthinust/ontologies/2022/8/Gait_Ontology#Terminal_stance">
        <rdfs:subClassOf rdf:resource="http://www.semanticweb.org/marthinust/ontologies/2022/8/Gait_Ontology#Stance_phase"/>
        <opla-sd:entityPosition>
            <rdf:Description>
                <opla-sd:entityPositionX rdf:datatype="http://www.w3.org/2001/XMLSchema#double">159.6944694206963</opla-sd:entityPositionX>
                <opla-sd:entityPositionY rdf:datatype="http://www.w3.org/2001/XMLSchema#double">44.009753012354395</opla-sd:entityPositionY>
                <rdfs:comment xml:lang="en">This is an entity positioning annotation generated by CoModIDE (https://comodide.com/). Removing this annotation will break rendering the CoModIDE schema diagram view.</rdfs:comment>
            </rdf:Description>
        </opla-sd:entityPosition>
        <rdfs:comment xml:lang="en">Terminal stance begins when the center of gravity is over the supporting foot and ends when the contralateral foot contacts the ground. During terminal stance, around 35 percent of the gait cycle, the heel rises from the ground.</rdfs:comment>
        <rdfs:label xml:lang="en">Terminal_stance</rdfs:label>
    </owl:Class>
    


    <!-- http://www.semanticweb.org/marthinust/ontologies/2022/8/Gait_Ontology#Terminal_swing -->

    <owl:Class rdf:about="http://www.semanticweb.org/marthinust/ontologies/2022/8/Gait_Ontology#Terminal_swing">
        <rdfs:subClassOf rdf:resource="http://www.semanticweb.org/marthinust/ontologies/2022/8/Gait_Ontology#Swing_phase"/>
        <opla-sd:entityPosition>
            <rdf:Description>
                <opla-sd:entityPositionX rdf:datatype="http://www.w3.org/2001/XMLSchema#double">82.95191618921763</opla-sd:entityPositionX>
                <opla-sd:entityPositionY rdf:datatype="http://www.w3.org/2001/XMLSchema#double">31.242396078136935</opla-sd:entityPositionY>
                <rdfs:comment xml:lang="en">This is an entity positioning annotation generated by CoModIDE (https://comodide.com/). Removing this annotation will break rendering the CoModIDE schema diagram view.</rdfs:comment>
            </rdf:Description>
        </opla-sd:entityPosition>
        <rdfs:comment xml:lang="en">The terminal swing phase is the phase of the gait cycle that occurs after the initial swing phase and before the foot makes contact with the ground again at the beginning of the next stance phase. It begins when the leg is fully extended at the end of the initial swing phase and ends when the foot makes contact with the ground at the beginning of the next stance phase.

During the terminal swing phase, the hip, knee, and ankle joints undergo a rapid series of movements as the leg prepares for foot strike. The toes of the swinging leg may be pointed downward, and the ankle joint may undergo plantarflexion (pointing the toes downward) in preparation for landing.


Terminal swing is the final phase of the gait cycle going from 87-100% of the cycle. During terminal swing, the final advancement of the shank takes place and the foot is positioned for initial foot contact to start the next gait cycle.</rdfs:comment>
        <rdfs:label xml:lang="en">Terminal_swing</rdfs:label>
    </owl:Class>
    


    <!-- http://www.semanticweb.org/marthinust/ontologies/2022/8/Gait_Ontology#Tip-toe_gait -->

    <owl:Class rdf:about="http://www.semanticweb.org/marthinust/ontologies/2022/8/Gait_Ontology#Tip-toe_gait">
        <rdfs:subClassOf rdf:resource="http://www.semanticweb.org/marthinust/ontologies/2022/8/Gait_Ontology#Gait_Disturbance"/>
        <opla-sd:entityPosition>
            <rdf:Description>
                <opla-sd:entityPositionX rdf:datatype="http://www.w3.org/2001/XMLSchema#double">9.827549951499075</opla-sd:entityPositionX>
                <opla-sd:entityPositionY rdf:datatype="http://www.w3.org/2001/XMLSchema#double">269.6799679840805</opla-sd:entityPositionY>
                <rdfs:comment xml:lang="en">This is an entity positioning annotation generated by CoModIDE (https://comodide.com/). Removing this annotation will break rendering the CoModIDE schema diagram view.</rdfs:comment>
            </rdf:Description>
        </opla-sd:entityPosition>
        <rdfs:comment xml:lang="en">An abnormal gait pattern characterized by the failure of the heel to contact the floor at the onset of stance during gait.

Tip-toe walking (or simply toe-walking) is common in healthy young children, and should resolve spontaneously by 3 years of age. After this age, tip-toe gait must be differentiated from habitual toe gait, congenital short tendo calcaneus, cerebral palsy, syringomyelia, spinal tumor, hematoma in a lower limb muscle, or neuromuscular diseases like muscular dystrophy, Charcot-Marie-Tooth disease and hereditary sensorimotor neuropathies. If the toe gait persists for 2-3 years, this gait pattern is not considered to be habitual. Therefore, the judgment of habitual toe gait should not be determined without evaluation for other diseases.</rdfs:comment>
        <rdfs:label xml:lang="en">Tip-toe_gait</rdfs:label>
    </owl:Class>
    


    <!-- http://www.semanticweb.org/marthinust/ontologies/2022/8/Gait_Ontology#Treadmill -->

    <owl:Class rdf:about="http://www.semanticweb.org/marthinust/ontologies/2022/8/Gait_Ontology#Treadmill">
        <rdfs:subClassOf rdf:resource="http://www.semanticweb.org/marthinust/ontologies/2022/8/Gait_Ontology#Gait_Analysis_Equipment"/>
        <opla-sd:entityPosition>
            <rdf:Description>
                <opla-sd:entityPositionX rdf:datatype="http://www.w3.org/2001/XMLSchema#double">147.79803987978076</opla-sd:entityPositionX>
                <opla-sd:entityPositionY rdf:datatype="http://www.w3.org/2001/XMLSchema#double">59.31042595469892</opla-sd:entityPositionY>
                <rdfs:comment xml:lang="en">This is an entity positioning annotation generated by CoModIDE (https://comodide.com/). Removing this annotation will break rendering the CoModIDE schema diagram view.</rdfs:comment>
            </rdf:Description>
        </opla-sd:entityPosition>
        <rdfs:comment xml:lang="en">Some gait analysis facilities use instrumented treadmills to assess gait in a controlled environment. Examples include h/p/cosmos, Woodway, and Bertec treadmills.</rdfs:comment>
        <rdfs:label xml:lang="en">Treadmill</rdfs:label>
    </owl:Class>
    


    <!-- http://www.semanticweb.org/marthinust/ontologies/2022/8/Gait_Ontology#Treatment -->

    <owl:Class rdf:about="http://www.semanticweb.org/marthinust/ontologies/2022/8/Gait_Ontology#Treatment">
        <rdfs:subClassOf rdf:resource="http://www.semanticweb.org/marthinust/ontologies/2022/8/Gait_Ontology#Gait_Assistive_Technology"/>
        <opla-sd:entityPosition>
            <rdf:Description>
                <opla-sd:entityPositionX rdf:datatype="http://www.w3.org/2001/XMLSchema#double">63.49353974142389</opla-sd:entityPositionX>
                <opla-sd:entityPositionY rdf:datatype="http://www.w3.org/2001/XMLSchema#double">102.73394755307922</opla-sd:entityPositionY>
                <rdfs:comment xml:lang="en">This is an entity positioning annotation generated by CoModIDE (https://comodide.com/). Removing this annotation will break rendering the CoModIDE schema diagram view.</rdfs:comment>
            </rdf:Description>
        </opla-sd:entityPosition>
        <rdfs:comment xml:lang="en">Treatment for gait and balance issues depends on the cause. Treatments may include medications and physical therapy. You may require rehabilitation to learn to move muscles, to compensate for a lack of balance, and to learn how to prevent falls. 

Treating the underlying cause of the abnormal gait may help you recover some function. Medicines are available to treat arthritis, Parkinsons disease and multiple sclerosis.</rdfs:comment>
        <rdfs:label xml:lang="en">Treatment</rdfs:label>
    </owl:Class>
    


    <!-- http://www.semanticweb.org/marthinust/ontologies/2022/8/Gait_Ontology#Trendelenburg_gait -->

    <owl:Class rdf:about="http://www.semanticweb.org/marthinust/ontologies/2022/8/Gait_Ontology#Trendelenburg_gait">
        <rdfs:subClassOf rdf:resource="http://www.semanticweb.org/marthinust/ontologies/2022/8/Gait_Ontology#Type_of_Gait"/>
        <opla-sd:entityPosition>
            <rdf:Description>
                <opla-sd:entityPositionX rdf:datatype="http://www.w3.org/2001/XMLSchema#double">214.0026699295207</opla-sd:entityPositionX>
                <opla-sd:entityPositionY rdf:datatype="http://www.w3.org/2001/XMLSchema#double">161.53469229664233</opla-sd:entityPositionY>
                <rdfs:comment xml:lang="en">This is an entity positioning annotation generated by CoModIDE (https://comodide.com/). Removing this annotation will break rendering the CoModIDE schema diagram view.</rdfs:comment>
            </rdf:Description>
        </opla-sd:entityPosition>
        <rdfs:comment xml:lang="en">Trendelenburg gait (also known as Gluteus Medius Gait) occurs when the gluteus medius is weak. Gluteus medius weakness can be the result of dysfunctions or diagnoses related to back pain or lumbopelvic pain, chronic hip dysfunctions, or lumbopelvic surgery. The weakness of the involved side causes a contralateral pelvic hip drop during swing phase.

A trendelenburg gait is characterized by trunk shift over the affected hip during stance and away during the swing phase of gait and it is best visualized from behind or in front of the patient. During gait, the pelvis tilts downwards instead of upwards on the non-weight bearing extremity. In an attempt to lessen this effect, the person compensates by lateral tilt of the trunk away from the affected hip, thus center of gravity is mostly on the stance limb causing a reduction of the pelvic drop.

The trendelenburg gait is caused by a unilateral weakness of the hip abductors, mostly the gluteal musculature. This weakness could be due to superior gluteal nerve damage or in 5th lumbar spine lesion. This condition makes it difficult to support the bodys weight on the affected side.</rdfs:comment>
        <rdfs:label xml:lang="en">Trendelenburg_gait</rdfs:label>
    </owl:Class>
    


    <!-- http://www.semanticweb.org/marthinust/ontologies/2022/8/Gait_Ontology#Type_of_Gait -->

    <owl:Class rdf:about="http://www.semanticweb.org/marthinust/ontologies/2022/8/Gait_Ontology#Type_of_Gait">
        <rdfs:subClassOf>
            <owl:Restriction>
                <owl:onProperty rdf:resource="http://www.semanticweb.org/marthinust/ontologies/2022/8/Gait_Ontology#isDetectedIn"/>
                <owl:someValuesFrom rdf:resource="http://www.semanticweb.org/marthinust/ontologies/2022/8/Gait_Ontology#Gait_Analysis_Method"/>
            </owl:Restriction>
        </rdfs:subClassOf>
        <rdfs:subClassOf>
            <owl:Restriction>
                <owl:onProperty rdf:resource="http://www.semanticweb.org/marthinust/ontologies/2022/8/Gait_Ontology#isExhibitedBy"/>
                <owl:someValuesFrom rdf:resource="http://www.semanticweb.org/marthinust/ontologies/2022/8/Gait_Ontology#Gait_patient"/>
            </owl:Restriction>
        </rdfs:subClassOf>
        <rdfs:subClassOf>
            <owl:Restriction>
                <owl:onProperty rdf:resource="http://www.semanticweb.org/marthinust/ontologies/2022/8/Gait_Ontology#isInfluencedBy"/>
                <owl:someValuesFrom rdf:resource="http://www.semanticweb.org/marthinust/ontologies/2022/8/Gait_Ontology#Gait-related_Disease"/>
            </owl:Restriction>
        </rdfs:subClassOf>
        <rdfs:subClassOf>
            <owl:Restriction>
                <owl:onProperty rdf:resource="http://www.semanticweb.org/marthinust/ontologies/2022/8/Gait_Ontology#isRelatedTo"/>
                <owl:someValuesFrom rdf:resource="http://www.semanticweb.org/marthinust/ontologies/2022/8/Gait_Ontology#Gait_Disturbance"/>
            </owl:Restriction>
        </rdfs:subClassOf>
        <opla-sd:entityPosition>
            <rdf:Description>
                <opla-sd:entityPositionX rdf:datatype="http://www.w3.org/2001/XMLSchema#double">143.6486696091671</opla-sd:entityPositionX>
                <opla-sd:entityPositionY rdf:datatype="http://www.w3.org/2001/XMLSchema#double">227.46892201358392</opla-sd:entityPositionY>
                <rdfs:comment xml:lang="en">This is an entity positioning annotation generated by CoModIDE (https://comodide.com/). Removing this annotation will break rendering the CoModIDE schema diagram view.</rdfs:comment>
            </rdf:Description>
        </opla-sd:entityPosition>
        <rdfs:comment xml:lang="en">Abnormal or improper gait is categorised in different types of gait, which is based on the symptoms or appearance of an individual&apos;s walk through assessment and observation.</rdfs:comment>
        <rdfs:label xml:lang="en">Type_of_Gait</rdfs:label>
    </owl:Class>
    


    <!-- http://www.semanticweb.org/marthinust/ontologies/2022/8/Gait_Ontology#Unsteady_gait -->

    <owl:Class rdf:about="http://www.semanticweb.org/marthinust/ontologies/2022/8/Gait_Ontology#Unsteady_gait">
        <rdfs:subClassOf rdf:resource="http://www.semanticweb.org/marthinust/ontologies/2022/8/Gait_Ontology#Gait_Disturbance"/>
        <opla-sd:entityPosition>
            <rdf:Description>
                <opla-sd:entityPositionX rdf:datatype="http://www.w3.org/2001/XMLSchema#double">285.5340604661784</opla-sd:entityPositionX>
                <opla-sd:entityPositionY rdf:datatype="http://www.w3.org/2001/XMLSchema#double">137.01910091690812</opla-sd:entityPositionY>
                <rdfs:comment xml:lang="en">This is an entity positioning annotation generated by CoModIDE (https://comodide.com/). Removing this annotation will break rendering the CoModIDE schema diagram view.</rdfs:comment>
            </rdf:Description>
        </opla-sd:entityPosition>
        <rdfs:comment xml:lang="en">Gait instability, Unsteady walk</rdfs:comment>
        <rdfs:label xml:lang="en">Unsteady_gait</rdfs:label>
    </owl:Class>
    


    <!-- http://www.semanticweb.org/marthinust/ontologies/2022/8/Gait_Ontology#Vascular -->

    <owl:Class rdf:about="http://www.semanticweb.org/marthinust/ontologies/2022/8/Gait_Ontology#Vascular">
        <rdfs:subClassOf rdf:resource="http://www.semanticweb.org/marthinust/ontologies/2022/8/Gait_Ontology#Calcification"/>
        <opla-sd:entityPosition>
            <rdf:Description>
                <opla-sd:entityPositionX rdf:datatype="http://www.w3.org/2001/XMLSchema#double">203.95390363761965</opla-sd:entityPositionX>
                <opla-sd:entityPositionY rdf:datatype="http://www.w3.org/2001/XMLSchema#double">102.46366182328165</opla-sd:entityPositionY>
                <rdfs:comment xml:lang="en">This is an entity positioning annotation generated by CoModIDE (https://comodide.com/). Removing this annotation will break rendering the CoModIDE schema diagram view.</rdfs:comment>
            </rdf:Description>
        </opla-sd:entityPosition>
        <rdfs:comment xml:lang="en">Vascular calcification, a hallmark of aging, is accelerated in patients with hypertension, diabetes, and chronic kidney disease. It may be viewed as the result of disturbances of the complex and subtle balance between inhibitors and promoters, acting at both the systemic and local levels.</rdfs:comment>
        <rdfs:label xml:lang="en">Vascular</rdfs:label>
    </owl:Class>
    


    <!-- http://www.semanticweb.org/marthinust/ontologies/2022/8/Gait_Ontology#Velocity -->

    <owl:Class rdf:about="http://www.semanticweb.org/marthinust/ontologies/2022/8/Gait_Ontology#Velocity">
        <rdfs:subClassOf rdf:resource="http://www.semanticweb.org/marthinust/ontologies/2022/8/Gait_Ontology#Gait_Parameter"/>
        <opla-sd:entityPosition>
            <rdf:Description>
                <opla-sd:entityPositionX rdf:datatype="http://www.w3.org/2001/XMLSchema#double">242.93800902961692</opla-sd:entityPositionX>
                <opla-sd:entityPositionY rdf:datatype="http://www.w3.org/2001/XMLSchema#double">45.37355398307246</opla-sd:entityPositionY>
                <rdfs:comment xml:lang="en">This is an entity positioning annotation generated by CoModIDE (https://comodide.com/). Removing this annotation will break rendering the CoModIDE schema diagram view.</rdfs:comment>
            </rdf:Description>
        </opla-sd:entityPosition>
        <rdfs:comment xml:lang="en">Gait Velocity or Walking Speed is the fundamental walking measure that defines the person&apos;s basic walking ability. Walking Speed is the time required for a person to traverse a specific distance. The term velocity indicates not only the speed of travel but also the specific direction of travel.

Acceleration and deceleration curves - how quickly people are able to get up to speed and then come to a stop can provide insight into explosive power and musculoskeletal stability.</rdfs:comment>
        <rdfs:label xml:lang="en">Velocity</rdfs:label>
    </owl:Class>
    


    <!-- http://www.semanticweb.org/marthinust/ontologies/2022/8/Gait_Ontology#Waddling_gait -->

    <owl:Class rdf:about="http://www.semanticweb.org/marthinust/ontologies/2022/8/Gait_Ontology#Waddling_gait">
        <rdfs:subClassOf rdf:resource="http://www.semanticweb.org/marthinust/ontologies/2022/8/Gait_Ontology#Gait_Disturbance"/>
        <rdfs:subClassOf rdf:resource="http://www.semanticweb.org/marthinust/ontologies/2022/8/Gait_Ontology#Myopathic_gait"/>
    </owl:Class>
    


    <!-- http://www.semanticweb.org/marthinust/ontologies/2022/8/Gait_Ontology#Walker -->

    <owl:Class rdf:about="http://www.semanticweb.org/marthinust/ontologies/2022/8/Gait_Ontology#Walker">
        <rdfs:subClassOf rdf:resource="http://www.semanticweb.org/marthinust/ontologies/2022/8/Gait_Ontology#Gait_Assistive_Technology"/>
    </owl:Class>
    


    <!-- http://www.semanticweb.org/marthinust/ontologies/2022/8/Gait_Ontology#Weak_quadriceps -->

    <owl:Class rdf:about="http://www.semanticweb.org/marthinust/ontologies/2022/8/Gait_Ontology#Weak_quadriceps">
        <rdfs:subClassOf rdf:resource="http://www.semanticweb.org/marthinust/ontologies/2022/8/Gait_Ontology#Knee"/>
        <opla-sd:entityPosition>
            <rdf:Description>
                <opla-sd:entityPositionX rdf:datatype="http://www.w3.org/2001/XMLSchema#double">10.837889066756377</opla-sd:entityPositionX>
                <opla-sd:entityPositionY rdf:datatype="http://www.w3.org/2001/XMLSchema#double">59.36556350830208</opla-sd:entityPositionY>
                <rdfs:comment xml:lang="en">This is an entity positioning annotation generated by CoModIDE (https://comodide.com/). Removing this annotation will break rendering the CoModIDE schema diagram view.</rdfs:comment>
            </rdf:Description>
        </opla-sd:entityPosition>
        <rdfs:comment xml:lang="en">The quadriceps role is to eccentrically control the knee during flexion through the stance phase. If these muscles are weak the hip extensors will compensate by bringing the limb back into a more extended position, reducing the amount of flexion at the knee during stance phase. Alternatively heel strike will occur earlier increasing the ankle of plantar flexion at the ankle, preventing the forward movement of the tibia, to help stabilise the knee joint.</rdfs:comment>
        <rdfs:label xml:lang="en">Weak_quadriceps</rdfs:label>
    </owl:Class>
    


    <!-- http://www.semanticweb.org/marthinust/ontologies/2022/8/Gait_Ontology#Wheelchair -->

    <owl:Class rdf:about="http://www.semanticweb.org/marthinust/ontologies/2022/8/Gait_Ontology#Wheelchair">
        <rdfs:subClassOf rdf:resource="http://www.semanticweb.org/marthinust/ontologies/2022/8/Gait_Ontology#Gait_Assistive_Technology"/>
        <opla-sd:entityPosition>
            <rdf:Description>
                <opla-sd:entityPositionX rdf:datatype="http://www.w3.org/2001/XMLSchema#double">170.3046745265607</opla-sd:entityPositionX>
                <opla-sd:entityPositionY rdf:datatype="http://www.w3.org/2001/XMLSchema#double">89.74032481134117</opla-sd:entityPositionY>
                <rdfs:comment xml:lang="en">This is an entity positioning annotation generated by CoModIDE (https://comodide.com/). Removing this annotation will break rendering the CoModIDE schema diagram view.</rdfs:comment>
            </rdf:Description>
        </opla-sd:entityPosition>
        <rdfs:comment xml:lang="en">The wheelchair is one of the most commonly used assistive devices to promote mobility and enhance quality of life for people who have difficulties in walking (e.g. a person with spinal cord injuries resulting in quadriplegia or paraplegia, muscular dystrophy,etc).

Wheelchairs are devices that allow users to sit and be transported without having to walk. They can be manual or powered, and they can be customized to meet the individual&apos;s needs and preferences.</rdfs:comment>
        <rdfs:label xml:lang="en">Wheelchair</rdfs:label>
    </owl:Class>
    


    <!-- http://www.semanticweb.org/marthinust/ontologies/2022/8/Gait_Ontology#3D_scanner -->

    <owl:Class rdf:about="http://www.semanticweb.org/marthinust/ontologies/2022/8/Gait_Ontology#3D_scanner">
        <rdfs:subClassOf rdf:resource="http://www.semanticweb.org/marthinust/ontologies/2022/8/Gait_Ontology#Gait_Analysis_Equipment"/>
        <opla-sd:entityPosition>
            <rdf:Description>
                <opla-sd:entityPositionX rdf:datatype="http://www.w3.org/2001/XMLSchema#double">104.64779131405577</opla-sd:entityPositionX>
                <opla-sd:entityPositionY rdf:datatype="http://www.w3.org/2001/XMLSchema#double">96.88340793804164</opla-sd:entityPositionY>
                <rdfs:comment xml:lang="en">This is an entity positioning annotation generated by CoModIDE (https://comodide.com/). Removing this annotation will break rendering the CoModIDE schema diagram view.</rdfs:comment>
            </rdf:Description>
        </opla-sd:entityPosition>
        <rdfs:comment xml:lang="en">These systems capture the shape and size of an individual&apos;s feet, helping to identify potential issues related to footwear and orthotics. Examples include Artec, Fuel3D, and EinScan systems.</rdfs:comment>
        <rdfs:label xml:lang="en">3D_scanner</rdfs:label>
    </owl:Class>
    


    <!-- http://www.semanticweb.org/marthinust/ontologies/2022/8/Gait_Ontology#Alzheimer&apos;s -->

    <owl:Class rdf:about="http://www.semanticweb.org/marthinust/ontologies/2022/8/Gait_Ontology#Alzheimer&apos;s">
        <rdfs:subClassOf rdf:resource="http://www.semanticweb.org/marthinust/ontologies/2022/8/Gait_Ontology#Dementia"/>
        <opla-sd:entityPosition>
            <rdf:Description>
                <opla-sd:entityPositionX rdf:datatype="http://www.w3.org/2001/XMLSchema#double">240.32912157406943</opla-sd:entityPositionX>
                <opla-sd:entityPositionY rdf:datatype="http://www.w3.org/2001/XMLSchema#double">211.73659173017248</opla-sd:entityPositionY>
                <rdfs:comment xml:lang="en">This is an entity positioning annotation generated by CoModIDE (https://comodide.com/). Removing this annotation will break rendering the CoModIDE schema diagram view.</rdfs:comment>
            </rdf:Description>
        </opla-sd:entityPosition>
        <rdfs:comment xml:lang="en">Alzheimer&apos;s disease is a progressive neurologic disorder that causes the brain to shrink (atrophy) and brain cells to die. Alzheimer&apos;s disease is the most common cause of dementia  a continuous decline in thinking, behavioral and social skills that affects a person&apos;s ability to function independently.

Alzheimers disease is a brain disorder that slowly destroys memory and thinking skills, and, eventually, the ability to carry out the simplest tasks. In most people with Alzheimers, symptoms first appear later in life during old age.</rdfs:comment>
        <rdfs:label xml:lang="en">Alzheimer&apos;s</rdfs:label>
    </owl:Class>
    


    <!-- http://www.semanticweb.org/marthinust/ontologies/2022/8/Gait_Ontology#Amyotrophic_lateral_sclerosis_(ALS) -->

    <owl:Class rdf:about="http://www.semanticweb.org/marthinust/ontologies/2022/8/Gait_Ontology#Amyotrophic_lateral_sclerosis_(ALS)">
        <rdfs:subClassOf rdf:resource="http://www.semanticweb.org/marthinust/ontologies/2022/8/Gait_Ontology#Gait-related_Disease"/>
        <opla-sd:entityPosition>
            <rdf:Description>
                <opla-sd:entityPositionX rdf:datatype="http://www.w3.org/2001/XMLSchema#double">87.61917054034673</opla-sd:entityPositionX>
                <opla-sd:entityPositionY rdf:datatype="http://www.w3.org/2001/XMLSchema#double">243.79876286088228</opla-sd:entityPositionY>
                <rdfs:comment xml:lang="en">This is an entity positioning annotation generated by CoModIDE (https://comodide.com/). Removing this annotation will break rendering the CoModIDE schema diagram view.</rdfs:comment>
            </rdf:Description>
        </opla-sd:entityPosition>
        <rdfs:comment xml:lang="en">Amyotrophic lateral sclerosis (ALS) is a degenerative disease that affects the brain and spinal cord. ALS causes a loss of voluntary muscle control that worsens over time. This affects movements like talking, swallowing, and walking. Unfortunately, no cure has been found yet. But treatments are available that can reduce symptoms and may help people with ALS to live longer.

Its a progressive neurological disease that damages nerve cells and often begins with muscle twitching and weakness in the legs.

Other early symptoms include:

difficulty walking or performing daily tasks
trouble swallowing
slurred speech
difficulty holding up your head</rdfs:comment>
        <rdfs:label xml:lang="en">Amyotrophic_lateral_sclerosis_(ALS)</rdfs:label>
    </owl:Class>
    


    <!-- http://www.semanticweb.org/marthinust/ontologies/2022/8/Gait_Ontology#Calcaneal_fracture_(Broken_heel_bone) -->

    <owl:Class rdf:about="http://www.semanticweb.org/marthinust/ontologies/2022/8/Gait_Ontology#Calcaneal_fracture_(Broken_heel_bone)">
        <rdfs:subClassOf rdf:resource="http://www.semanticweb.org/marthinust/ontologies/2022/8/Gait_Ontology#Calcaneus/Heel_bone"/>
        <opla-sd:entityPosition>
            <rdf:Description>
                <opla-sd:entityPositionX rdf:datatype="http://www.w3.org/2001/XMLSchema#double">50.53487019592191</opla-sd:entityPositionX>
                <opla-sd:entityPositionY rdf:datatype="http://www.w3.org/2001/XMLSchema#double">7.592032815904538</opla-sd:entityPositionY>
                <rdfs:comment xml:lang="en">This is an entity positioning annotation generated by CoModIDE (https://comodide.com/). Removing this annotation will break rendering the CoModIDE schema diagram view.</rdfs:comment>
            </rdf:Description>
        </opla-sd:entityPosition>
        <rdfs:comment xml:lang="en">A fracture of the calcaneus, or heel bone, can be a painful and disabling injury. This type of fracture commonly occurs during a high-energy event  such as a car crash or a fall from a ladder  when the heel is crushed under the weight of the body. When this occurs, the heel can widen, shorten, and become deformed.

Calcaneus fractures are the most common fractured tarsal bone and are associated with a high degree of morbidity and disability.</rdfs:comment>
        <rdfs:label xml:lang="en">Calcaneal_fracture/Broken_heel</rdfs:label>
    </owl:Class>
    


    <!-- http://www.semanticweb.org/marthinust/ontologies/2022/8/Gait_Ontology#Calcaneus/Heel_bone -->

    <owl:Class rdf:about="http://www.semanticweb.org/marthinust/ontologies/2022/8/Gait_Ontology#Calcaneus/Heel_bone">
        <rdfs:subClassOf rdf:resource="http://www.semanticweb.org/marthinust/ontologies/2022/8/Gait_Ontology#Musculoskeletal"/>
        <opla-sd:entityPosition>
            <rdf:Description>
                <opla-sd:entityPositionX rdf:datatype="http://www.w3.org/2001/XMLSchema#double">6.29198978279456</opla-sd:entityPositionX>
                <opla-sd:entityPositionY rdf:datatype="http://www.w3.org/2001/XMLSchema#double">104.00946123975473</opla-sd:entityPositionY>
                <rdfs:comment xml:lang="en">This is an entity positioning annotation generated by CoModIDE (https://comodide.com/). Removing this annotation will break rendering the CoModIDE schema diagram view.</rdfs:comment>
            </rdf:Description>
        </opla-sd:entityPosition>
        <rdfs:comment xml:lang="en">The calcaneus, or heel bone, is a complex shaped bone located just below your ankle and extending to the back of your foot. The calcaneus not only provides support as you walk, but also connects your calf muscles to your foot. This allows you to push off as you take a step forward. The calcaneus is the largest bone in the foot. It projects posterior to the tibia and fibula and acts as a short lever for the calf muscles (gastrocnemius and soleus) which insert onto its posterior surface via the Achilles tendon. It also plays an important role in weight bearing and stability.</rdfs:comment>
        <rdfs:label xml:lang="en">Calcaneus/Heel_bone</rdfs:label>
    </owl:Class>
    


    <!-- http://www.semanticweb.org/marthinust/ontologies/2022/8/Gait_Ontology#Footdrop/Dropfoot -->

    <owl:Class rdf:about="http://www.semanticweb.org/marthinust/ontologies/2022/8/Gait_Ontology#Footdrop/Dropfoot">
        <rdfs:subClassOf rdf:resource="http://www.semanticweb.org/marthinust/ontologies/2022/8/Gait_Ontology#Foot"/>
        <opla-sd:entityPosition>
            <rdf:Description>
                <opla-sd:entityPositionX rdf:datatype="http://www.w3.org/2001/XMLSchema#double">1.9340047131029139</opla-sd:entityPositionX>
                <opla-sd:entityPositionY rdf:datatype="http://www.w3.org/2001/XMLSchema#double">47.31443615689929</opla-sd:entityPositionY>
                <rdfs:comment xml:lang="en">This is an entity positioning annotation generated by CoModIDE (https://comodide.com/). Removing this annotation will break rendering the CoModIDE schema diagram view.</rdfs:comment>
            </rdf:Description>
        </opla-sd:entityPosition>
        <rdfs:comment xml:lang="en">Foot drop, sometimes called drop foot, is a general term for difficulty lifting the front part of the foot. If you have foot drop, the front of your foot might drag on the ground when you walk. Foot drop isn&apos;t a disease. Rather, foot drop is a sign of an underlying neurological, muscular or anatomical problem.</rdfs:comment>
        <rdfs:label xml:lang="en">Drop_foot/Foot_drop</rdfs:label>
    </owl:Class>
    


    <!-- http://www.semanticweb.org/marthinust/ontologies/2022/8/Gait_Ontology#Force_platform/Forceplate -->

    <owl:Class rdf:about="http://www.semanticweb.org/marthinust/ontologies/2022/8/Gait_Ontology#Force_platform/Forceplate">
        <rdfs:subClassOf rdf:resource="http://www.semanticweb.org/marthinust/ontologies/2022/8/Gait_Ontology#Gait_Analysis_Equipment"/>
        <opla-sd:entityPosition>
            <rdf:Description>
                <opla-sd:entityPositionX rdf:datatype="http://www.w3.org/2001/XMLSchema#double">141.13916577810699</opla-sd:entityPositionX>
                <opla-sd:entityPositionY rdf:datatype="http://www.w3.org/2001/XMLSchema#double">240.34687370472076</opla-sd:entityPositionY>
                <rdfs:comment xml:lang="en">This is an entity positioning annotation generated by CoModIDE (https://comodide.com/). Removing this annotation will break rendering the CoModIDE schema diagram view.</rdfs:comment>
            </rdf:Description>
        </opla-sd:entityPosition>
        <rdfs:comment xml:lang="en">A force platform is a device that is used to measure the forces acting on a body or object. It consists of a flat surface that is mounted on load cells, which are sensors that measure force. The load cells are typically connected to a computer or other data acquisition system, which is used to collect and analyse the force data.

Force platforms are commonly used in the field of biomechanics, which is the study of the mechanics of living organisms. They can be used to measure forces acting on the body during activities such as walking, running, and jumping, and can provide important information on the kinematics (movement) and kinetics (forces and moments) of these activities.

The force platform (or forceplate) is an instrument commonly used in gait analysis. It gives the total force applied by the foot to the ground, although it does not show the distribution of different parts of this force (e.g. heel and forefoot) on the walking surface. Some force platforms give only one component of the force (usually vertical), but most give a full three dimensional description of the ground reaction force vector.</rdfs:comment>
        <rdfs:label xml:lang="en">Force _platform/Forceplate</rdfs:label>
    </owl:Class>
    


    <!-- http://www.semanticweb.org/marthinust/ontologies/2022/8/Gait_Ontology#Haglund&apos;s_deformity -->

    <owl:Class rdf:about="http://www.semanticweb.org/marthinust/ontologies/2022/8/Gait_Ontology#Haglund&apos;s_deformity">
        <rdfs:subClassOf rdf:resource="http://www.semanticweb.org/marthinust/ontologies/2022/8/Gait_Ontology#Calcaneus/Heel_bone"/>
        <opla-sd:entityPosition>
            <rdf:Description>
                <opla-sd:entityPositionX rdf:datatype="http://www.w3.org/2001/XMLSchema#double">192.85500783949416</opla-sd:entityPositionX>
                <opla-sd:entityPositionY rdf:datatype="http://www.w3.org/2001/XMLSchema#double">22.834179736183373</opla-sd:entityPositionY>
                <rdfs:comment xml:lang="en">This is an entity positioning annotation generated by CoModIDE (https://comodide.com/). Removing this annotation will break rendering the CoModIDE schema diagram view.</rdfs:comment>
            </rdf:Description>
        </opla-sd:entityPosition>
        <rdfs:comment xml:lang="en">Haglund&apos;s deformity is an abnormality of the bone and soft tissues in the foot. An enlargement of the bony section of the heel (where the Achilles tendon is inserted) triggers this condition. The soft tissue near the back of the heel can become irritated when the large, bony lump rubs against rigid shoes.

Haglunds deformity is a symptomatic osseous prominence of the posterolateral corner of the calcaneus resulting in posterior heel pain and swelling around the insertion of the Achilles Tendon. 

You may be genetically disposed to Haglunds Deformity by your foot shape, or it can be caused by muscle tightness or friction from shoes.</rdfs:comment>
        <rdfs:label xml:lang="en">Haglund&apos;s_deformity</rdfs:label>
    </owl:Class>
    


    <!-- http://www.semanticweb.org/marthinust/ontologies/2022/8/Gait_Ontology#Huntington&apos;s_disease -->

    <owl:Class rdf:about="http://www.semanticweb.org/marthinust/ontologies/2022/8/Gait_Ontology#Huntington&apos;s_disease">
        <rdfs:subClassOf rdf:resource="http://www.semanticweb.org/marthinust/ontologies/2022/8/Gait_Ontology#Gait-related_Disease"/>
        <opla-sd:entityPosition>
            <rdf:Description>
                <opla-sd:entityPositionX rdf:datatype="http://www.w3.org/2001/XMLSchema#double">9.639784223347574</opla-sd:entityPositionX>
                <opla-sd:entityPositionY rdf:datatype="http://www.w3.org/2001/XMLSchema#double">211.57376627842098</opla-sd:entityPositionY>
                <rdfs:comment xml:lang="en">This is an entity positioning annotation generated by CoModIDE (https://comodide.com/). Removing this annotation will break rendering the CoModIDE schema diagram view.</rdfs:comment>
            </rdf:Description>
        </opla-sd:entityPosition>
        <rdfs:comment xml:lang="en">Huntington&apos;s disease (HD) is an inherited disease that causes certain nerve cells in the brain to waste away. Huntington&apos;s disease is a rare, inherited disease that causes the progressive breakdown (degeneration) of nerve cells in the brain. Huntington&apos;s disease has a wide impact on a person&apos;s functional abilities and usually results in movement, thinking (cognitive) and psychiatric disorders. A general lack of coordination and an unsteady gait often follow. People are born with the defective gene, but symptoms usually don&apos;t appear until middle age. Early symptoms of HD may include uncontrolled movements, clumsiness, and balance problems. Later, HD can take away the ability to walk, talk, and swallow. Some people stop recognizing family members. Others are aware of their environment and are able to express emotions.</rdfs:comment>
        <rdfs:label xml:lang="en">Huntington&apos;s_disease</rdfs:label>
    </owl:Class>
    


    <!-- http://www.semanticweb.org/marthinust/ontologies/2022/8/Gait_Ontology#Inability_to_walk_by_childhood/adolescence -->

    <owl:Class rdf:about="http://www.semanticweb.org/marthinust/ontologies/2022/8/Gait_Ontology#Inability_to_walk_by_childhood/adolescence">
        <rdfs:subClassOf rdf:resource="http://www.semanticweb.org/marthinust/ontologies/2022/8/Gait_Ontology#Inability_to_walk"/>
        <opla-sd:entityPosition>
            <rdf:Description>
                <opla-sd:entityPositionX rdf:datatype="http://www.w3.org/2001/XMLSchema#double">277.98177604333154</opla-sd:entityPositionX>
                <opla-sd:entityPositionY rdf:datatype="http://www.w3.org/2001/XMLSchema#double">201.0154291125712</opla-sd:entityPositionY>
                <rdfs:comment xml:lang="en">This is an entity positioning annotation generated by CoModIDE (https://comodide.com/). Removing this annotation will break rendering the CoModIDE schema diagram view.</rdfs:comment>
            </rdf:Description>
        </opla-sd:entityPosition>
        <rdfs:comment>Inability to walk by childhood/adolescence</rdfs:comment>
        <rdfs:label xml:lang="en">Inability_to_walk_by_childhood/adolescence</rdfs:label>
    </owl:Class>
    


    <!-- http://www.semanticweb.org/marthinust/ontologies/2022/8/Gait_Ontology#Parkinson&apos;s_disease -->

    <owl:Class rdf:about="http://www.semanticweb.org/marthinust/ontologies/2022/8/Gait_Ontology#Parkinson&apos;s_disease">
        <rdfs:subClassOf rdf:resource="http://www.semanticweb.org/marthinust/ontologies/2022/8/Gait_Ontology#Gait-related_Disease"/>
        <opla-sd:entityPosition>
            <rdf:Description>
                <opla-sd:entityPositionX rdf:datatype="http://www.w3.org/2001/XMLSchema#double">7.857746170321769</opla-sd:entityPositionX>
                <opla-sd:entityPositionY rdf:datatype="http://www.w3.org/2001/XMLSchema#double">100.14120129685811</opla-sd:entityPositionY>
                <rdfs:comment xml:lang="en">This is an entity positioning annotation generated by CoModIDE (https://comodide.com/). Removing this annotation will break rendering the CoModIDE schema diagram view.</rdfs:comment>
            </rdf:Description>
        </opla-sd:entityPosition>
        <rdfs:comment xml:lang="en">Parkinson&apos;s disease (PD) is a type of movement disorder. It happens when nerve cells in the brain don&apos;t produce enough of a brain chemical called dopamine. Sometimes it is genetic, but most cases do not seem to run in families. Exposure to chemicals in the environment might play a role. As symptoms get worse, people with the disease may have trouble walking, talking, or doing simple tasks. They may also have problems such as depression, sleep problems, or trouble chewing, swallowing, or speaking. 

Parkinson&apos;s disease is a brain disorder that causes unintended or uncontrollable movements, such as shaking, stiffness, and difficulty with balance and coordination. Symptoms usually begin gradually and worsen over time. As the disease progresses, people may have difficulty walking and talking.</rdfs:comment>
        <rdfs:label xml:lang="en">Parkinson&apos;s_disease</rdfs:label>
    </owl:Class>
    


    <!-- http://www.semanticweb.org/marthinust/ontologies/2022/8/Gait_Ontology#Wilson&apos;s_disease -->

    <owl:Class rdf:about="http://www.semanticweb.org/marthinust/ontologies/2022/8/Gait_Ontology#Wilson&apos;s_disease">
        <rdfs:subClassOf rdf:resource="http://www.semanticweb.org/marthinust/ontologies/2022/8/Gait_Ontology#Gait-related_Disease"/>
        <opla-sd:entityPosition>
            <rdf:Description>
                <opla-sd:entityPositionX rdf:datatype="http://www.w3.org/2001/XMLSchema#double">130.77820651484788</opla-sd:entityPositionX>
                <opla-sd:entityPositionY rdf:datatype="http://www.w3.org/2001/XMLSchema#double">36.29251043535202</opla-sd:entityPositionY>
                <rdfs:comment xml:lang="en">This is an entity positioning annotation generated by CoModIDE (https://comodide.com/). Removing this annotation will break rendering the CoModIDE schema diagram view.</rdfs:comment>
            </rdf:Description>
        </opla-sd:entityPosition>
        <rdfs:comment xml:lang="en">Wilson disease is a rare genetic disorder characterized by excess copper stored in various body tissues, particularly the liver, brain, and corneas of the eyes. The disease is progressive and, if left untreated, it may cause liver (hepatic) disease, central nervous system dysfunction, and death. Early diagnosis and treatment may prevent serious long-term disability and life threatening complications.

In Wilson&apos;s disease, copper isn&apos;t eliminated properly and instead accumulates, possibly to a life-threatening level. Symptoms include swelling, fatigue, abdominal pain and uncontrolled or poorly coordinated movements.

Common neurological symptoms of Wilson disease that may appear and progress with time include tremor, involuntary movements, difficulty swallowing (dysphagia), difficulty speaking and poor articulation (dysarthria), lack of coordination, spasticity, dystonic postures, and muscle rigidity.</rdfs:comment>
        <rdfs:label xml:lang="en">Wilson&apos;s_disease</rdfs:label>
    </owl:Class>
    


    <!-- 
    ///////////////////////////////////////////////////////////////////////////////////////
    //
    // Individuals
    //
    ///////////////////////////////////////////////////////////////////////////////////////
     -->

    


    <!-- http://www.semanticweb.org/marthinust/ontologies/2022/8/Gait_Ontology#AI_method -->

    <owl:NamedIndividual rdf:about="http://www.semanticweb.org/marthinust/ontologies/2022/8/Gait_Ontology#AI_method">
        <rdf:type rdf:resource="http://www.semanticweb.org/marthinust/ontologies/2022/8/Gait_Ontology#Gait_Analysis_Method"/>
        <Gait_Ontology:isBasedOn rdf:resource="http://www.semanticweb.org/marthinust/ontologies/2022/8/Gait_Ontology#Gyroscope"/>
        <Gait_Ontology:hasAnalysis_method rdf:datatype="http://www.w3.org/2001/XMLSchema#string">AI-based gait analysis</Gait_Ontology:hasAnalysis_method>
        <rdfs:comment xml:lang="en">AI algorithms, particularly machine learning and deep learning techniques, can be used to analyse and interpret data collected by gait analysis equipment, such as motion capture systems, force plates, and wearable sensors.</rdfs:comment>
        <rdfs:label xml:lang="en">AI_method</rdfs:label>
    </owl:NamedIndividual>
    


    <!-- http://www.semanticweb.org/marthinust/ontologies/2022/8/Gait_Ontology#Acute -->

    <owl:NamedIndividual rdf:about="http://www.semanticweb.org/marthinust/ontologies/2022/8/Gait_Ontology#Acute">
        <rdf:type rdf:resource="http://www.semanticweb.org/marthinust/ontologies/2022/8/Gait_Ontology#Severity_Scale"/>
        <Gait_Ontology:isMilderThan rdf:resource="http://www.semanticweb.org/marthinust/ontologies/2022/8/Gait_Ontology#Severe"/>
        <Gait_Ontology:isSevereThan rdf:resource="http://www.semanticweb.org/marthinust/ontologies/2022/8/Gait_Ontology#Mild"/>
        <rdfs:comment xml:lang="en">Acute pain typically has a specific, treatable cause. Acute (pain) acts as a warning to your body that it is unsafe and its health has been compromised. A common belief is that acute pain is a bit mild and temporary.</rdfs:comment>
        <rdfs:label xml:lang="en">Acute</rdfs:label>
    </owl:NamedIndividual>
    


    <!-- http://www.semanticweb.org/marthinust/ontologies/2022/8/Gait_Ontology#Adolescent -->

    <owl:NamedIndividual rdf:about="http://www.semanticweb.org/marthinust/ontologies/2022/8/Gait_Ontology#Adolescent">
        <rdf:type rdf:resource="http://www.semanticweb.org/marthinust/ontologies/2022/8/Gait_Ontology#Gait_patient"/>
        <Gait_Ontology:demonstrates rdf:resource="http://www.semanticweb.org/marthinust/ontologies/2022/8/Gait_Ontology#Gait_walk"/>
        <Gait_Ontology:exhibits rdf:resource="http://www.semanticweb.org/marthinust/ontologies/2022/8/Gait_Ontology#Limp_gait"/>
        <Gait_Ontology:isAffectedBy rdf:resource="http://www.semanticweb.org/marthinust/ontologies/2022/8/Gait_Ontology#Gait_imbalance"/>
        <Gait_Ontology:isAssessedIn rdf:resource="http://www.semanticweb.org/marthinust/ontologies/2022/8/Gait_Ontology#Gait_assessment"/>
        <Gait_Ontology:isAssignedWith rdf:resource="http://www.semanticweb.org/marthinust/ontologies/2022/8/Gait_Ontology#Orthotic"/>
        <Gait_Ontology:isClassedIn rdf:resource="http://www.semanticweb.org/marthinust/ontologies/2022/8/Gait_Ontology#Musculoskeletal"/>
        <Gait_Ontology:isInvolvedIn rdf:resource="http://www.semanticweb.org/marthinust/ontologies/2022/8/Gait_Ontology#Session"/>
        <Gait_Ontology:isLinkedWith rdf:resource="http://www.semanticweb.org/marthinust/ontologies/2022/8/Gait_Ontology#Scoliosis"/>
        <Gait_Ontology:isMonitoredBy rdf:resource="http://www.semanticweb.org/marthinust/ontologies/2022/8/Gait_Ontology#GRF_sensor"/>
        <Gait_Ontology:isOlderThan rdf:resource="http://www.semanticweb.org/marthinust/ontologies/2022/8/Gait_Ontology#Child"/>
        <Gait_Ontology:isTreatedBy rdf:resource="http://www.semanticweb.org/marthinust/ontologies/2022/8/Gait_Ontology#Podiatrist"/>
        <Gait_Ontology:isYoungerThan rdf:resource="http://www.semanticweb.org/marthinust/ontologies/2022/8/Gait_Ontology#Adult"/>
        <Gait_Ontology:isYoungerThan rdf:resource="http://www.semanticweb.org/marthinust/ontologies/2022/8/Gait_Ontology#Athlete"/>
        <Gait_Ontology:isYoungerThan rdf:resource="http://www.semanticweb.org/marthinust/ontologies/2022/8/Gait_Ontology#Elderly"/>
        <Gait_Ontology:hasAffected_leg_side rdf:datatype="http://www.w3.org/2001/XMLSchema#string">Left</Gait_Ontology:hasAffected_leg_side>
        <Gait_Ontology:hasAge_in_years rdf:datatype="http://www.w3.org/2001/XMLSchema#integer">15</Gait_Ontology:hasAge_in_years>
        <Gait_Ontology:hasAge_range rdf:datatype="http://www.w3.org/2001/XMLSchema#string">Between the age of 12 and 21</Gait_Ontology:hasAge_range>
        <Gait_Ontology:hasGender rdf:datatype="http://www.w3.org/2001/XMLSchema#string">Male</Gait_Ontology:hasGender>
        <Gait_Ontology:hasHeight_in_meters rdf:datatype="http://www.w3.org/2001/XMLSchema#double">1.64</Gait_Ontology:hasHeight_in_meters>
        <Gait_Ontology:hasWeight_in_kilograms rdf:datatype="http://www.w3.org/2001/XMLSchema#double">55.6</Gait_Ontology:hasWeight_in_kilograms>
        <rdfs:comment xml:lang="en">An adolescent is a person who is going through puberty and the transition from childhood to adulthood. This typically occurs during the teenage years, between the ages of 13 and 20. Adolescents are characterised by physical, cognitive, and social changes that can be both exciting and challenging.</rdfs:comment>
        <rdfs:label xml:lang="en">Adolescent</rdfs:label>
    </owl:NamedIndividual>
    


    <!-- http://www.semanticweb.org/marthinust/ontologies/2022/8/Gait_Ontology#Adult -->

    <owl:NamedIndividual rdf:about="http://www.semanticweb.org/marthinust/ontologies/2022/8/Gait_Ontology#Adult">
        <rdf:type rdf:resource="http://www.semanticweb.org/marthinust/ontologies/2022/8/Gait_Ontology#Gait_patient"/>
        <Gait_Ontology:demonstrates rdf:resource="http://www.semanticweb.org/marthinust/ontologies/2022/8/Gait_Ontology#Gait_walk"/>
        <Gait_Ontology:exhibits rdf:resource="http://www.semanticweb.org/marthinust/ontologies/2022/8/Gait_Ontology#Ataxic_gait"/>
        <Gait_Ontology:isAffectedBy rdf:resource="http://www.semanticweb.org/marthinust/ontologies/2022/8/Gait_Ontology#Progressive_ataxia"/>
        <Gait_Ontology:isAssessedIn rdf:resource="http://www.semanticweb.org/marthinust/ontologies/2022/8/Gait_Ontology#Gait_assessment"/>
        <Gait_Ontology:isAssignedWith rdf:resource="http://www.semanticweb.org/marthinust/ontologies/2022/8/Gait_Ontology#Walking_stick"/>
        <Gait_Ontology:isClassedIn rdf:resource="http://www.semanticweb.org/marthinust/ontologies/2022/8/Gait_Ontology#Neurological"/>
        <Gait_Ontology:isInvolvedIn rdf:resource="http://www.semanticweb.org/marthinust/ontologies/2022/8/Gait_Ontology#Session"/>
        <Gait_Ontology:isLinkedWith rdf:resource="http://www.semanticweb.org/marthinust/ontologies/2022/8/Gait_Ontology#Ataxia"/>
        <Gait_Ontology:isMonitoredBy rdf:resource="http://www.semanticweb.org/marthinust/ontologies/2022/8/Gait_Ontology#EM_tracking_system"/>
        <Gait_Ontology:isOlderThan rdf:resource="http://www.semanticweb.org/marthinust/ontologies/2022/8/Gait_Ontology#Adolescent"/>
        <Gait_Ontology:isOlderThan rdf:resource="http://www.semanticweb.org/marthinust/ontologies/2022/8/Gait_Ontology#Child"/>
        <Gait_Ontology:isTreatedBy rdf:resource="http://www.semanticweb.org/marthinust/ontologies/2022/8/Gait_Ontology#Physical_therapist"/>
        <Gait_Ontology:isYoungerThan rdf:resource="http://www.semanticweb.org/marthinust/ontologies/2022/8/Gait_Ontology#Elderly"/>
        <Gait_Ontology:hasAffected_leg_side rdf:datatype="http://www.w3.org/2001/XMLSchema#string">Both</Gait_Ontology:hasAffected_leg_side>
        <Gait_Ontology:hasAge_in_years rdf:datatype="http://www.w3.org/2001/XMLSchema#integer">42</Gait_Ontology:hasAge_in_years>
        <Gait_Ontology:hasAge_range rdf:datatype="http://www.w3.org/2001/XMLSchema#string">The age can be from 21 until 65</Gait_Ontology:hasAge_range>
        <Gait_Ontology:hasGender rdf:datatype="http://www.w3.org/2001/XMLSchema#string">Male</Gait_Ontology:hasGender>
        <Gait_Ontology:hasHeight_in_meters rdf:datatype="http://www.w3.org/2001/XMLSchema#double">1.75</Gait_Ontology:hasHeight_in_meters>
        <Gait_Ontology:hasWeight_in_kilograms rdf:datatype="http://www.w3.org/2001/XMLSchema#double">69.0</Gait_Ontology:hasWeight_in_kilograms>
        <rdfs:comment xml:lang="en">An adult is a person who has reached physical and mental maturity. In most societies, a person is considered an adult when they reach the age of 18 OR 21. Adults are self-sufficient and responsible for their own actions. They are expected to make their own decisions and to take care of themselves and any dependents they may have. Adults also have more life experience and are generally more mature than children and adolescents.</rdfs:comment>
        <rdfs:label xml:lang="en">Adult</rdfs:label>
    </owl:NamedIndividual>
    


    <!-- http://www.semanticweb.org/marthinust/ontologies/2022/8/Gait_Ontology#Ataxia -->

    <owl:NamedIndividual rdf:about="http://www.semanticweb.org/marthinust/ontologies/2022/8/Gait_Ontology#Ataxia">
        <rdf:type rdf:resource="http://www.semanticweb.org/marthinust/ontologies/2022/8/Gait_Ontology#Gait-related_Disease"/>
        <Gait_Ontology:isAssociatedTo rdf:resource="http://www.semanticweb.org/marthinust/ontologies/2022/8/Gait_Ontology#Adult"/>
        <Gait_Ontology:hasDisease_description rdf:datatype="http://www.w3.org/2001/XMLSchema#string">Cerebellar disease</Gait_Ontology:hasDisease_description>
    </owl:NamedIndividual>
    


    <!-- http://www.semanticweb.org/marthinust/ontologies/2022/8/Gait_Ontology#Ataxic_gait -->

    <owl:NamedIndividual rdf:about="http://www.semanticweb.org/marthinust/ontologies/2022/8/Gait_Ontology#Ataxic_gait">
        <rdf:type rdf:resource="http://www.semanticweb.org/marthinust/ontologies/2022/8/Gait_Ontology#Type_of_Gait"/>
        <Gait_Ontology:isDetectedIn rdf:resource="http://www.semanticweb.org/marthinust/ontologies/2022/8/Gait_Ontology#Kinematography"/>
        <Gait_Ontology:isExhibitedBy rdf:resource="http://www.semanticweb.org/marthinust/ontologies/2022/8/Gait_Ontology#Adult"/>
        <Gait_Ontology:isInfluencedBy rdf:resource="http://www.semanticweb.org/marthinust/ontologies/2022/8/Gait_Ontology#Ataxia"/>
        <Gait_Ontology:isRelatedTo rdf:resource="http://www.semanticweb.org/marthinust/ontologies/2022/8/Gait_Ontology#Progressive_ataxia"/>
        <Gait_Ontology:hasGait_type rdf:datatype="http://www.w3.org/2001/XMLSchema#string">Cerebellar</Gait_Ontology:hasGait_type>
    </owl:NamedIndividual>
    


    <!-- http://www.semanticweb.org/marthinust/ontologies/2022/8/Gait_Ontology#Athlete -->

    <owl:NamedIndividual rdf:about="http://www.semanticweb.org/marthinust/ontologies/2022/8/Gait_Ontology#Athlete">
        <rdf:type rdf:resource="http://www.semanticweb.org/marthinust/ontologies/2022/8/Gait_Ontology#Gait_patient"/>
        <Gait_Ontology:demonstrates rdf:resource="http://www.semanticweb.org/marthinust/ontologies/2022/8/Gait_Ontology#Gait_walk"/>
        <Gait_Ontology:exhibits rdf:resource="http://www.semanticweb.org/marthinust/ontologies/2022/8/Gait_Ontology#Normal_gait"/>
        <Gait_Ontology:isAffectedBy rdf:resource="http://www.semanticweb.org/marthinust/ontologies/2022/8/Gait_Ontology#Dystonic_gait"/>
        <Gait_Ontology:isAssessedIn rdf:resource="http://www.semanticweb.org/marthinust/ontologies/2022/8/Gait_Ontology#Gait_assessment"/>
        <Gait_Ontology:isAssignedWith rdf:resource="http://www.semanticweb.org/marthinust/ontologies/2022/8/Gait_Ontology#Pharmaceutical"/>
        <Gait_Ontology:isClassedIn rdf:resource="http://www.semanticweb.org/marthinust/ontologies/2022/8/Gait_Ontology#Musculoskeletal"/>
        <Gait_Ontology:isInvolvedIn rdf:resource="http://www.semanticweb.org/marthinust/ontologies/2022/8/Gait_Ontology#Session"/>
        <Gait_Ontology:isLinkedWith rdf:resource="http://www.semanticweb.org/marthinust/ontologies/2022/8/Gait_Ontology#Dystonia"/>
        <Gait_Ontology:isMonitoredBy rdf:resource="http://www.semanticweb.org/marthinust/ontologies/2022/8/Gait_Ontology#Electromyography"/>
        <Gait_Ontology:isOlderThan rdf:resource="http://www.semanticweb.org/marthinust/ontologies/2022/8/Gait_Ontology#Adolescent"/>
        <Gait_Ontology:isOlderThan rdf:resource="http://www.semanticweb.org/marthinust/ontologies/2022/8/Gait_Ontology#Child"/>
        <Gait_Ontology:isTreatedBy rdf:resource="http://www.semanticweb.org/marthinust/ontologies/2022/8/Gait_Ontology#Biomechanist"/>
        <Gait_Ontology:isYoungerThan rdf:resource="http://www.semanticweb.org/marthinust/ontologies/2022/8/Gait_Ontology#Elderly"/>
        <Gait_Ontology:hasAffected_leg_side rdf:datatype="http://www.w3.org/2001/XMLSchema#string">Left</Gait_Ontology:hasAffected_leg_side>
        <Gait_Ontology:hasAge_in_years rdf:datatype="http://www.w3.org/2001/XMLSchema#integer">27</Gait_Ontology:hasAge_in_years>
        <Gait_Ontology:hasAge_range rdf:datatype="http://www.w3.org/2001/XMLSchema#string">The age can be from 21 until 65</Gait_Ontology:hasAge_range>
        <Gait_Ontology:hasGender rdf:datatype="http://www.w3.org/2001/XMLSchema#string">Gender neutral</Gait_Ontology:hasGender>
        <Gait_Ontology:hasHeight_in_meters rdf:datatype="http://www.w3.org/2001/XMLSchema#double">1.88</Gait_Ontology:hasHeight_in_meters>
        <Gait_Ontology:hasWeight_in_kilograms rdf:datatype="http://www.w3.org/2001/XMLSchema#double">81.0</Gait_Ontology:hasWeight_in_kilograms>
        <rdfs:comment xml:lang="en">An athlete is a person who is proficient in a physical sport or activity that requires strength, speed, endurance, agility, and/or coordination. Athletes can participate in various competitions, such as the Olympics, professional leagues, and amateur events. They often dedicate themselves to rigorous training regimes to improve their skills and performance in their chosen sport. Athletes can range from professional players to amateur enthusiasts, and they can compete individually or as part of a team.

An athlete is a person who is trained or skilled in exercises, sports, or games requiring physical strength, agility, stamina, or endurance. Athletes typically compete in organised events or tournaments, and use their physical and mental abilities to achieve success in their chosen sport.</rdfs:comment>
        <rdfs:label xml:lang="en">Athlete</rdfs:label>
    </owl:NamedIndividual>
    


    <!-- http://www.semanticweb.org/marthinust/ontologies/2022/8/Gait_Ontology#Biomechanist -->

    <owl:NamedIndividual rdf:about="http://www.semanticweb.org/marthinust/ontologies/2022/8/Gait_Ontology#Biomechanist">
        <rdf:type rdf:resource="http://www.semanticweb.org/marthinust/ontologies/2022/8/Gait_Ontology#Gait_expert"/>
        <Gait_Ontology:administers rdf:resource="http://www.semanticweb.org/marthinust/ontologies/2022/8/Gait_Ontology#Gait_assessment"/>
        <Gait_Ontology:analyzes rdf:resource="http://www.semanticweb.org/marthinust/ontologies/2022/8/Gait_Ontology#Clinical_data"/>
        <Gait_Ontology:facilitates rdf:resource="http://www.semanticweb.org/marthinust/ontologies/2022/8/Gait_Ontology#Clinical_evaluation"/>
        <Gait_Ontology:observes rdf:resource="http://www.semanticweb.org/marthinust/ontologies/2022/8/Gait_Ontology#Gait_walk"/>
        <Gait_Ontology:prescribes rdf:resource="http://www.semanticweb.org/marthinust/ontologies/2022/8/Gait_Ontology#Pharmaceutical"/>
        <Gait_Ontology:treats rdf:resource="http://www.semanticweb.org/marthinust/ontologies/2022/8/Gait_Ontology#Athlete"/>
        <Gait_Ontology:hasGait_expert rdf:datatype="http://www.w3.org/2001/XMLSchema#string">Biomechanist</Gait_Ontology:hasGait_expert>
        <Gait_Ontology:hasGender rdf:datatype="http://www.w3.org/2001/XMLSchema#string">Female</Gait_Ontology:hasGender>
        <rdfs:comment xml:lang="en">A biomechanist is an expert in human motion. They use their expertise to solve medical and mobility problems and improve the quality of life for people who are injured. A clinical biomechanist in a biomechanics laboratory at a hospital might work with physicians and therapists to understand how best to help patients regain normal walking patterns with medical treatment.

A biomechanist is a scientist who studies the mechanical aspects of biological systems, such as the movement and function of muscles, bones, and joints in the body. Biomechanists use principles of engineering, physics, and mathematics to understand and analyse the mechanics of living mammals. They may study the movement of humans or animals, and may focus on issues such as posture, balance, and gait (the way a person walks). Biomechanists may work in a variety of settings, including universities, hospitals, research institutes, and sports organisations. They may also work in industries such as healthcare, athletic equipment design, or military research.</rdfs:comment>
        <rdfs:label xml:lang="en">Biomechanist</rdfs:label>
    </owl:NamedIndividual>
    


    <!-- http://www.semanticweb.org/marthinust/ontologies/2022/8/Gait_Ontology#Braces -->

    <owl:NamedIndividual rdf:about="http://www.semanticweb.org/marthinust/ontologies/2022/8/Gait_Ontology#Braces">
        <rdf:type rdf:resource="http://www.semanticweb.org/marthinust/ontologies/2022/8/Gait_Ontology#Gait_Assistive_Technology"/>
        <Gait_Ontology:isAscertainedIn rdf:resource="http://www.semanticweb.org/marthinust/ontologies/2022/8/Gait_Ontology#Gait_assessment"/>
        <Gait_Ontology:isPrescribedBy rdf:resource="http://www.semanticweb.org/marthinust/ontologies/2022/8/Gait_Ontology#Orthopedist"/>
        <Gait_Ontology:isRecommendedTo rdf:resource="http://www.semanticweb.org/marthinust/ontologies/2022/8/Gait_Ontology#Child"/>
        <Gait_Ontology:hasGait_assistive_solution rdf:datatype="http://www.w3.org/2001/XMLSchema#string">Orthotic braces</Gait_Ontology:hasGait_assistive_solution>
        <Gait_Ontology:hasType_of_material rdf:datatype="http://www.w3.org/2001/XMLSchema#string">Composite materials</Gait_Ontology:hasType_of_material>
        <rdfs:comment xml:lang="en">For example, ankle braces that allow a person to stand straight are orthotics. Also, wrist braces, arm braces, spinal orthotics, and heel casts are orthotic devices. They all work to help those who have pain or difficulty with basic movements to be able to perform these activities again.

An orthosis is a device designed to improve biomechanical function, encourage proper joint alignment or to protect an existing limb.</rdfs:comment>
        <rdfs:label xml:lang="en">Braces</rdfs:label>
    </owl:NamedIndividual>
    


    <!-- http://www.semanticweb.org/marthinust/ontologies/2022/8/Gait_Ontology#Child -->

    <owl:NamedIndividual rdf:about="http://www.semanticweb.org/marthinust/ontologies/2022/8/Gait_Ontology#Child">
        <rdf:type rdf:resource="http://www.semanticweb.org/marthinust/ontologies/2022/8/Gait_Ontology#Gait_patient"/>
        <Gait_Ontology:demonstrates rdf:resource="http://www.semanticweb.org/marthinust/ontologies/2022/8/Gait_Ontology#Gait_walk"/>
        <Gait_Ontology:exhibits rdf:resource="http://www.semanticweb.org/marthinust/ontologies/2022/8/Gait_Ontology#Waddling_gait"/>
        <Gait_Ontology:isAffectedBy rdf:resource="http://www.semanticweb.org/marthinust/ontologies/2022/8/Gait_Ontology#Waddling"/>
        <Gait_Ontology:isAssessedIn rdf:resource="http://www.semanticweb.org/marthinust/ontologies/2022/8/Gait_Ontology#Gait_assessment"/>
        <Gait_Ontology:isAssignedWith rdf:resource="http://www.semanticweb.org/marthinust/ontologies/2022/8/Gait_Ontology#Braces"/>
        <Gait_Ontology:isClassedIn rdf:resource="http://www.semanticweb.org/marthinust/ontologies/2022/8/Gait_Ontology#Neuromuscular"/>
        <Gait_Ontology:isInvolvedIn rdf:resource="http://www.semanticweb.org/marthinust/ontologies/2022/8/Gait_Ontology#Session"/>
        <Gait_Ontology:isLinkedWith rdf:resource="http://www.semanticweb.org/marthinust/ontologies/2022/8/Gait_Ontology#Hip_spina_bifida"/>
        <Gait_Ontology:isMonitoredBy rdf:resource="http://www.semanticweb.org/marthinust/ontologies/2022/8/Gait_Ontology#Gonio"/>
        <Gait_Ontology:isTreatedBy rdf:resource="http://www.semanticweb.org/marthinust/ontologies/2022/8/Gait_Ontology#Orthopedist"/>
        <Gait_Ontology:isYoungerThan rdf:resource="http://www.semanticweb.org/marthinust/ontologies/2022/8/Gait_Ontology#Adolescent"/>
        <Gait_Ontology:isYoungerThan rdf:resource="http://www.semanticweb.org/marthinust/ontologies/2022/8/Gait_Ontology#Adult"/>
        <Gait_Ontology:isYoungerThan rdf:resource="http://www.semanticweb.org/marthinust/ontologies/2022/8/Gait_Ontology#Athlete"/>
        <Gait_Ontology:isYoungerThan rdf:resource="http://www.semanticweb.org/marthinust/ontologies/2022/8/Gait_Ontology#Elderly"/>
        <Gait_Ontology:hasAffected_leg_side rdf:datatype="http://www.w3.org/2001/XMLSchema#string">Both</Gait_Ontology:hasAffected_leg_side>
        <Gait_Ontology:hasAge_in_years rdf:datatype="http://www.w3.org/2001/XMLSchema#integer">8</Gait_Ontology:hasAge_in_years>
        <Gait_Ontology:hasAge_range rdf:datatype="http://www.w3.org/2001/XMLSchema#string">From newborn baby until 12 years old.</Gait_Ontology:hasAge_range>
        <Gait_Ontology:hasGender rdf:datatype="http://www.w3.org/2001/XMLSchema#string">Female</Gait_Ontology:hasGender>
        <Gait_Ontology:hasHeight_in_meters rdf:datatype="http://www.w3.org/2001/XMLSchema#double">1.2</Gait_Ontology:hasHeight_in_meters>
        <Gait_Ontology:hasWeight_in_kilograms rdf:datatype="http://www.w3.org/2001/XMLSchema#double">38.4</Gait_Ontology:hasWeight_in_kilograms>
        <rdfs:comment xml:lang="en">A child is a young person who is not yet an adult. Children are usually considered to be between the ages of newborn and 12 years old. Children are dependent on their caregivers for their physical, emotional, and social needs. They are typically curious and eager to learn about the world around them. Children are generally less mature and have less life experience than adolescents and adults, and they may need guidance and support as they develop and grow.</rdfs:comment>
        <rdfs:label xml:lang="en">Child</rdfs:label>
    </owl:NamedIndividual>
    


    <!-- http://www.semanticweb.org/marthinust/ontologies/2022/8/Gait_Ontology#Clinical_data -->

    <owl:NamedIndividual rdf:about="http://www.semanticweb.org/marthinust/ontologies/2022/8/Gait_Ontology#Clinical_data">
        <rdf:type rdf:resource="http://www.semanticweb.org/marthinust/ontologies/2022/8/Gait_Ontology#Gait_data"/>
        <Gait_Ontology:isAcquiredFrom rdf:resource="http://www.semanticweb.org/marthinust/ontologies/2022/8/Gait_Ontology#Adolescent"/>
        <Gait_Ontology:isAcquiredFrom rdf:resource="http://www.semanticweb.org/marthinust/ontologies/2022/8/Gait_Ontology#Adult"/>
        <Gait_Ontology:isAcquiredFrom rdf:resource="http://www.semanticweb.org/marthinust/ontologies/2022/8/Gait_Ontology#Athlete"/>
        <Gait_Ontology:isAcquiredFrom rdf:resource="http://www.semanticweb.org/marthinust/ontologies/2022/8/Gait_Ontology#Child"/>
        <Gait_Ontology:isAcquiredFrom rdf:resource="http://www.semanticweb.org/marthinust/ontologies/2022/8/Gait_Ontology#Elderly"/>
        <Gait_Ontology:isAnalysedBy rdf:resource="http://www.semanticweb.org/marthinust/ontologies/2022/8/Gait_Ontology#Biomechanist"/>
        <Gait_Ontology:isAnalysedBy rdf:resource="http://www.semanticweb.org/marthinust/ontologies/2022/8/Gait_Ontology#Healthcare_practitioner"/>
        <Gait_Ontology:isAnalysedBy rdf:resource="http://www.semanticweb.org/marthinust/ontologies/2022/8/Gait_Ontology#Orthopedist"/>
        <Gait_Ontology:isAnalysedBy rdf:resource="http://www.semanticweb.org/marthinust/ontologies/2022/8/Gait_Ontology#Physical_therapist"/>
        <Gait_Ontology:isAnalysedBy rdf:resource="http://www.semanticweb.org/marthinust/ontologies/2022/8/Gait_Ontology#Podiatrist"/>
        <Gait_Ontology:isCollectedBy rdf:resource="http://www.semanticweb.org/marthinust/ontologies/2022/8/Gait_Ontology#Session"/>
        <Gait_Ontology:isObtainedBy rdf:resource="http://www.semanticweb.org/marthinust/ontologies/2022/8/Gait_Ontology#EM_tracking_system"/>
        <Gait_Ontology:isObtainedBy rdf:resource="http://www.semanticweb.org/marthinust/ontologies/2022/8/Gait_Ontology#Electromyography"/>
        <Gait_Ontology:isObtainedBy rdf:resource="http://www.semanticweb.org/marthinust/ontologies/2022/8/Gait_Ontology#GRF_sensor"/>
        <Gait_Ontology:isObtainedBy rdf:resource="http://www.semanticweb.org/marthinust/ontologies/2022/8/Gait_Ontology#Gonio"/>
        <Gait_Ontology:isObtainedBy rdf:resource="http://www.semanticweb.org/marthinust/ontologies/2022/8/Gait_Ontology#Gyroscope"/>
        <Gait_Ontology:hasGait_data rdf:datatype="http://www.w3.org/2001/XMLSchema#string">Gait data readings</Gait_Ontology:hasGait_data>
        <rdfs:comment xml:lang="en">The collection of dynamical data during human walking has a long history beginning with the first motion pictures and now with modern marker(s) based motion capture techniques, wearable sensors, and high fidelity ground reaction load measurements. This data can likely be useful for validating or generating mathematical models that are capable of simulating normal periodic gait and non-periodic, perturbed gaits that results in clinical gait data for analysis.

Gait data is often used to evaluate various aspects of gait, such as efficiency, symmetry, and stability. It can also be used to diagnose and treat gait abnormalities, to evaluate the effectiveness of interventions such as orthotic devices or physical therapy, and to assess the impact of aging or diseases on gait. Gait data can be collected and analyzed both in the laboratory, and in more naturalistic environments, such as the individual&apos;s home or community.</rdfs:comment>
        <rdfs:label xml:lang="en">Clinical_data</rdfs:label>
    </owl:NamedIndividual>
    


    <!-- http://www.semanticweb.org/marthinust/ontologies/2022/8/Gait_Ontology#Clinical_evaluation -->

    <owl:NamedIndividual rdf:about="http://www.semanticweb.org/marthinust/ontologies/2022/8/Gait_Ontology#Clinical_evaluation">
        <rdf:type rdf:resource="http://www.semanticweb.org/marthinust/ontologies/2022/8/Gait_Ontology#Gait_analysis"/>
        <Gait_Ontology:isFacilitatedBy rdf:resource="http://www.semanticweb.org/marthinust/ontologies/2022/8/Gait_Ontology#Biomechanist"/>
        <Gait_Ontology:isFacilitatedBy rdf:resource="http://www.semanticweb.org/marthinust/ontologies/2022/8/Gait_Ontology#Healthcare_practitioner"/>
        <Gait_Ontology:isFacilitatedBy rdf:resource="http://www.semanticweb.org/marthinust/ontologies/2022/8/Gait_Ontology#Orthopedist"/>
        <Gait_Ontology:isFacilitatedBy rdf:resource="http://www.semanticweb.org/marthinust/ontologies/2022/8/Gait_Ontology#Physical_therapist"/>
        <Gait_Ontology:isFacilitatedBy rdf:resource="http://www.semanticweb.org/marthinust/ontologies/2022/8/Gait_Ontology#Podiatrist"/>
        <Gait_Ontology:isGeneratedIn rdf:resource="http://www.semanticweb.org/marthinust/ontologies/2022/8/Gait_Ontology#Gait_assessment"/>
        <Gait_Ontology:hasGait_analysis rdf:datatype="http://www.w3.org/2001/XMLSchema#string">Clinical gait analysis</Gait_Ontology:hasGait_analysis>
        <rdfs:comment xml:lang="en">Clinical gait analysis allows the measurement and assessment of walking biomechanics, which facilitates the identification of abnormal characteristics and the recommendation of treatment alternatives.</rdfs:comment>
        <rdfs:label xml:lang="en">Clinical_evaluation</rdfs:label>
    </owl:NamedIndividual>
    


    <!-- http://www.semanticweb.org/marthinust/ontologies/2022/8/Gait_Ontology#Dystonia -->

    <owl:NamedIndividual rdf:about="http://www.semanticweb.org/marthinust/ontologies/2022/8/Gait_Ontology#Dystonia">
        <rdf:type rdf:resource="http://www.semanticweb.org/marthinust/ontologies/2022/8/Gait_Ontology#Gait-related_Disease"/>
        <Gait_Ontology:isAssociatedTo rdf:resource="http://www.semanticweb.org/marthinust/ontologies/2022/8/Gait_Ontology#Athlete"/>
        <Gait_Ontology:hasDisease_description rdf:datatype="http://www.w3.org/2001/XMLSchema#string">Muscle contraction cramps</Gait_Ontology:hasDisease_description>
    </owl:NamedIndividual>
    


    <!-- http://www.semanticweb.org/marthinust/ontologies/2022/8/Gait_Ontology#Dystonic_gait -->

    <owl:NamedIndividual rdf:about="http://www.semanticweb.org/marthinust/ontologies/2022/8/Gait_Ontology#Dystonic_gait">
        <rdf:type rdf:resource="http://www.semanticweb.org/marthinust/ontologies/2022/8/Gait_Ontology#Gait_Disturbance"/>
        <Gait_Ontology:affects rdf:resource="http://www.semanticweb.org/marthinust/ontologies/2022/8/Gait_Ontology#Athlete"/>
        <Gait_Ontology:isDiagnosedBy rdf:resource="http://www.semanticweb.org/marthinust/ontologies/2022/8/Gait_Ontology#Biomechanist"/>
        <Gait_Ontology:isVerifiedBy rdf:resource="http://www.semanticweb.org/marthinust/ontologies/2022/8/Gait_Ontology#Electromyography"/>
        <Gait_Ontology:hasClinical_term rdf:datatype="http://www.w3.org/2001/XMLSchema#string">Hobby horse gait</Gait_Ontology:hasClinical_term>
    </owl:NamedIndividual>
    


    <!-- http://www.semanticweb.org/marthinust/ontologies/2022/8/Gait_Ontology#EM_tracking_system -->

    <owl:NamedIndividual rdf:about="http://www.semanticweb.org/marthinust/ontologies/2022/8/Gait_Ontology#EM_tracking_system">
        <rdf:type rdf:resource="http://www.semanticweb.org/marthinust/ontologies/2022/8/Gait_Ontology#Gait_Analysis_Equipment"/>
        <Gait_Ontology:isLinkedTo rdf:resource="http://www.semanticweb.org/marthinust/ontologies/2022/8/Gait_Ontology#Adult"/>
        <Gait_Ontology:isUsedFor rdf:resource="http://www.semanticweb.org/marthinust/ontologies/2022/8/Gait_Ontology#Gait_assessment"/>
        <Gait_Ontology:isUsedIn rdf:resource="http://www.semanticweb.org/marthinust/ontologies/2022/8/Gait_Ontology#Kinematography"/>
        <Gait_Ontology:hasEquipment_type rdf:datatype="http://www.w3.org/2001/XMLSchema#string">Electromagnetic tracking</Gait_Ontology:hasEquipment_type>
        <rdfs:comment xml:lang="en">The electromagnetic tracking system is a kind of 3D measurement device based on Faradays law of magnetic induction. When an object carrying sensor coils performs a motion inside controlled magnetic fields, the induced voltages in the sensor coils will change, with respect to the change of the objects position and orientation, relative to the source of controlled magnetic fields. In the ETS, the controlled magnetic fields are generated by a fixed transmitter and detected by the receivers fixed on the object in motion. Therefore, the positions and orientations of the object in relation to the transmitter can be calculated. Based on this working principle, some developed commercialised ETSs have been applied in bioengineering, including gait analysis and the kinematic study of body segments.</rdfs:comment>
        <rdfs:label xml:lang="en">EM_tracking_system</rdfs:label>
    </owl:NamedIndividual>
    


    <!-- http://www.semanticweb.org/marthinust/ontologies/2022/8/Gait_Ontology#Elderly -->

    <owl:NamedIndividual rdf:about="http://www.semanticweb.org/marthinust/ontologies/2022/8/Gait_Ontology#Elderly">
        <rdf:type rdf:resource="http://www.semanticweb.org/marthinust/ontologies/2022/8/Gait_Ontology#Gait_patient"/>
        <Gait_Ontology:demonstrates rdf:resource="http://www.semanticweb.org/marthinust/ontologies/2022/8/Gait_Ontology#Gait_walk"/>
        <Gait_Ontology:exhibits rdf:resource="http://www.semanticweb.org/marthinust/ontologies/2022/8/Gait_Ontology#Parkinsonian_gait"/>
        <Gait_Ontology:isAffectedBy rdf:resource="http://www.semanticweb.org/marthinust/ontologies/2022/8/Gait_Ontology#Freezing_of_gait"/>
        <Gait_Ontology:isAssessedIn rdf:resource="http://www.semanticweb.org/marthinust/ontologies/2022/8/Gait_Ontology#Gait_assessment"/>
        <Gait_Ontology:isAssignedWith rdf:resource="http://www.semanticweb.org/marthinust/ontologies/2022/8/Gait_Ontology#Walker"/>
        <Gait_Ontology:isClassedIn rdf:resource="http://www.semanticweb.org/marthinust/ontologies/2022/8/Gait_Ontology#Neurological"/>
        <Gait_Ontology:isInvolvedIn rdf:resource="http://www.semanticweb.org/marthinust/ontologies/2022/8/Gait_Ontology#Session"/>
        <Gait_Ontology:isLinkedWith rdf:resource="http://www.semanticweb.org/marthinust/ontologies/2022/8/Gait_Ontology#Parkinson&apos;s"/>
        <Gait_Ontology:isMonitoredBy rdf:resource="http://www.semanticweb.org/marthinust/ontologies/2022/8/Gait_Ontology#Gyroscope"/>
        <Gait_Ontology:isOlderThan rdf:resource="http://www.semanticweb.org/marthinust/ontologies/2022/8/Gait_Ontology#Adolescent"/>
        <Gait_Ontology:isOlderThan rdf:resource="http://www.semanticweb.org/marthinust/ontologies/2022/8/Gait_Ontology#Adult"/>
        <Gait_Ontology:isOlderThan rdf:resource="http://www.semanticweb.org/marthinust/ontologies/2022/8/Gait_Ontology#Athlete"/>
        <Gait_Ontology:isOlderThan rdf:resource="http://www.semanticweb.org/marthinust/ontologies/2022/8/Gait_Ontology#Child"/>
        <Gait_Ontology:isTreatedBy rdf:resource="http://www.semanticweb.org/marthinust/ontologies/2022/8/Gait_Ontology#Healthcare_practitioner"/>
        <Gait_Ontology:hasAffected_leg_side rdf:datatype="http://www.w3.org/2001/XMLSchema#string">Right</Gait_Ontology:hasAffected_leg_side>
        <Gait_Ontology:hasAge_in_years rdf:datatype="http://www.w3.org/2001/XMLSchema#integer">69</Gait_Ontology:hasAge_in_years>
        <Gait_Ontology:hasAge_range rdf:datatype="http://www.w3.org/2001/XMLSchema#string">Person from 65 years and older</Gait_Ontology:hasAge_range>
        <Gait_Ontology:hasGender rdf:datatype="http://www.w3.org/2001/XMLSchema#string">Female</Gait_Ontology:hasGender>
        <Gait_Ontology:hasHeight_in_meters rdf:datatype="http://www.w3.org/2001/XMLSchema#double">1.75</Gait_Ontology:hasHeight_in_meters>
        <Gait_Ontology:hasWeight_in_kilograms rdf:datatype="http://www.w3.org/2001/XMLSchema#double">70.4</Gait_Ontology:hasWeight_in_kilograms>
        <rdfs:comment xml:lang="en">The term &quot;elderly&quot; generally refers to people who are older, usually in their later years of life. The age at which someone is considered elderly can vary, but it is often used to describe people who are in their 60s or older. Elderly people may need more support and assistance with daily activities due to physical or cognitive decline.</rdfs:comment>
        <rdfs:label xml:lang="en">Elderly</rdfs:label>
    </owl:NamedIndividual>
    


    <!-- http://www.semanticweb.org/marthinust/ontologies/2022/8/Gait_Ontology#Electromyography -->

    <owl:NamedIndividual rdf:about="http://www.semanticweb.org/marthinust/ontologies/2022/8/Gait_Ontology#Electromyography">
        <rdf:type rdf:resource="http://www.semanticweb.org/marthinust/ontologies/2022/8/Gait_Ontology#Gait_Analysis_Equipment"/>
        <Gait_Ontology:isLinkedTo rdf:resource="http://www.semanticweb.org/marthinust/ontologies/2022/8/Gait_Ontology#Athlete"/>
        <Gait_Ontology:isUsedFor rdf:resource="http://www.semanticweb.org/marthinust/ontologies/2022/8/Gait_Ontology#Gait_assessment"/>
        <Gait_Ontology:isUsedIn rdf:resource="http://www.semanticweb.org/marthinust/ontologies/2022/8/Gait_Ontology#Sensory"/>
        <Gait_Ontology:hasEquipment_type rdf:datatype="http://www.w3.org/2001/XMLSchema#string">Leg and foot muscle sensors</Gait_Ontology:hasEquipment_type>
    </owl:NamedIndividual>
    


    <!-- http://www.semanticweb.org/marthinust/ontologies/2022/8/Gait_Ontology#Foot_pronation -->

    <owl:NamedIndividual rdf:about="http://www.semanticweb.org/marthinust/ontologies/2022/8/Gait_Ontology#Foot_pronation">
        <rdf:type rdf:resource="http://www.semanticweb.org/marthinust/ontologies/2022/8/Gait_Ontology#Gait_Measurement_Point"/>
        <Gait_Ontology:isAnalysedIn rdf:resource="http://www.semanticweb.org/marthinust/ontologies/2022/8/Gait_Ontology#Gait_walk"/>
        <Gait_Ontology:hasMeasurement rdf:datatype="http://www.w3.org/2001/XMLSchema#string">Over or under pronation</Gait_Ontology:hasMeasurement>
        <rdfs:comment xml:lang="en">Pronation is how your foot rolls from heel to toe as you walk or run. There are three different types of pronation  neutral, over, and under.

Gait measurement point of a connecting strip along the outside edges of your footprint indicates a neutral arch and normal pronation.</rdfs:comment>
        <rdfs:label xml:lang="en">Foot_pronation</rdfs:label>
    </owl:NamedIndividual>
    


    <!-- http://www.semanticweb.org/marthinust/ontologies/2022/8/Gait_Ontology#Freezing_of_gait -->

    <owl:NamedIndividual rdf:about="http://www.semanticweb.org/marthinust/ontologies/2022/8/Gait_Ontology#Freezing_of_gait">
        <rdf:type rdf:resource="http://www.semanticweb.org/marthinust/ontologies/2022/8/Gait_Ontology#Gait_Disturbance"/>
        <Gait_Ontology:affects rdf:resource="http://www.semanticweb.org/marthinust/ontologies/2022/8/Gait_Ontology#Elderly"/>
        <Gait_Ontology:isDiagnosedBy rdf:resource="http://www.semanticweb.org/marthinust/ontologies/2022/8/Gait_Ontology#Healthcare_practitioner"/>
        <Gait_Ontology:isVerifiedBy rdf:resource="http://www.semanticweb.org/marthinust/ontologies/2022/8/Gait_Ontology#Gyroscope"/>
        <Gait_Ontology:hasClinical_term rdf:datatype="http://www.w3.org/2001/XMLSchema#string">Freezing of gait</Gait_Ontology:hasClinical_term>
    </owl:NamedIndividual>
    


    <!-- http://www.semanticweb.org/marthinust/ontologies/2022/8/Gait_Ontology#Frontal_lobe_injury -->

    <owl:NamedIndividual rdf:about="http://www.semanticweb.org/marthinust/ontologies/2022/8/Gait_Ontology#Frontal_lobe_injury">
        <rdf:type rdf:resource="http://www.semanticweb.org/marthinust/ontologies/2022/8/Gait_Ontology#Gait_Pathology"/>
        <Gait_Ontology:isCategorisedIn rdf:resource="http://www.semanticweb.org/marthinust/ontologies/2022/8/Gait_Ontology#Neurological"/>
        <Gait_Ontology:hasPathology_trait rdf:datatype="http://www.w3.org/2001/XMLSchema#string">Frontal gait ataxia</Gait_Ontology:hasPathology_trait>
        <rdfs:comment xml:lang="en">Usually secondary to injury to frontal lobe and connecting networks. May be secondary to vascular disease or hydrocephalus. May involve other lobes of brain and associated with Alzheimers disease. Difficult to classify condition. Not Parkinsons disease or any neurologic tremor. Patients have lost the ability to walk, change positions from sit to stand, and have a broad base gait with short stride length and are unable to initiate gait on own. Will also have en bloc gait, freezing episodes, and retropulsion.</rdfs:comment>
        <rdfs:label xml:lang="en">Frontal_lobe_injury</rdfs:label>
    </owl:NamedIndividual>
    


    <!-- http://www.semanticweb.org/marthinust/ontologies/2022/8/Gait_Ontology#GRF_sensor -->

    <owl:NamedIndividual rdf:about="http://www.semanticweb.org/marthinust/ontologies/2022/8/Gait_Ontology#GRF_sensor">
        <rdf:type rdf:resource="http://www.semanticweb.org/marthinust/ontologies/2022/8/Gait_Ontology#Gait_Analysis_Equipment"/>
        <Gait_Ontology:isLinkedTo rdf:resource="http://www.semanticweb.org/marthinust/ontologies/2022/8/Gait_Ontology#Adolescent"/>
        <Gait_Ontology:isUsedFor rdf:resource="http://www.semanticweb.org/marthinust/ontologies/2022/8/Gait_Ontology#Gait_assessment"/>
        <Gait_Ontology:isUsedIn rdf:resource="http://www.semanticweb.org/marthinust/ontologies/2022/8/Gait_Ontology#Image_sensing"/>
        <Gait_Ontology:hasEquipment_type rdf:datatype="http://www.w3.org/2001/XMLSchema#string">Force (transducer) sensor</Gait_Ontology:hasEquipment_type>
        <rdfs:comment xml:lang="en">Force sensors can be embedded into footwear to realize ambulatory measurements of Ground Reaction Force (GRF) during the gait. This GRF is a 3D vector, with the actual direction depending on the nature of the interface between the foot and the ground.

In the development of wearable force sensors, various implementations of the force transducer, including piezoelectrics, strain gauged and capacitive transducerd , are feasible. In addition, Hessert et al. designed a type of wearable force sensor based on a photoelastic triaxial force transducer to measure GRF in gait analysis. Force sensors based on the optical fiber matrix were developed to detect the shear and compressive force during human walking.

There are several different types of force sensors, including load cells, strain gauges, and piezoelectric sensors. Load cells are sensors that are used to measure force by converting it into an electrical signal. They are commonly used in force platforms, which are devices that measure the forces acting on a body or object. Strain gauges are sensors that are used to measure the deformation or strain of an object when it is subjected to a force.</rdfs:comment>
        <rdfs:label xml:lang="en">Ground Reaction Force sensor</rdfs:label>
    </owl:NamedIndividual>
    


    <!-- http://www.semanticweb.org/marthinust/ontologies/2022/8/Gait_Ontology#Gait_assessment -->

    <owl:NamedIndividual rdf:about="http://www.semanticweb.org/marthinust/ontologies/2022/8/Gait_Ontology#Gait_assessment">
        <rdf:type rdf:resource="http://www.semanticweb.org/marthinust/ontologies/2022/8/Gait_Ontology#Gait-based_Process"/>
        <Gait_Ontology:isAdministeredBy rdf:resource="http://www.semanticweb.org/marthinust/ontologies/2022/8/Gait_Ontology#Biomechanist"/>
        <Gait_Ontology:isAdministeredBy rdf:resource="http://www.semanticweb.org/marthinust/ontologies/2022/8/Gait_Ontology#Healthcare_practitioner"/>
        <Gait_Ontology:isAdministeredBy rdf:resource="http://www.semanticweb.org/marthinust/ontologies/2022/8/Gait_Ontology#Orthopedist"/>
        <Gait_Ontology:isAdministeredBy rdf:resource="http://www.semanticweb.org/marthinust/ontologies/2022/8/Gait_Ontology#Physical_therapist"/>
        <Gait_Ontology:isAdministeredBy rdf:resource="http://www.semanticweb.org/marthinust/ontologies/2022/8/Gait_Ontology#Podiatrist"/>
        <Gait_Ontology:isCapturedIn rdf:resource="http://www.semanticweb.org/marthinust/ontologies/2022/8/Gait_Ontology#Image_sensing"/>
        <Gait_Ontology:isCapturedIn rdf:resource="http://www.semanticweb.org/marthinust/ontologies/2022/8/Gait_Ontology#Kinematography"/>
        <Gait_Ontology:isCapturedIn rdf:resource="http://www.semanticweb.org/marthinust/ontologies/2022/8/Gait_Ontology#Motion_system"/>
        <Gait_Ontology:isCapturedIn rdf:resource="http://www.semanticweb.org/marthinust/ontologies/2022/8/Gait_Ontology#Sensory"/>
        <Gait_Ontology:hasGait-based_process rdf:datatype="http://www.w3.org/2001/XMLSchema#string">Gait data assimilation</Gait_Ontology:hasGait-based_process>
        <rdfs:comment xml:lang="en">Gait (analysis) process assessment is administered by the gait expert.

By simply observing the gait and noting abnormalities is of little value by itself. It needs to be followed by gait assessment, which is the synthesis of these observations with other information about the subject, obtained from the history and physical examination, combined with the intelligence and experience of the observer. Visual gait analysis is entirely subjective and the quality of the analysis depends on the skill of the person performing it. It can be an interesting exercise to perform visual gait analysis on people walking past in the street, but without knowing their clinical details it is easy to misinterpret what is wrong with them. When performing any type of gait analysis, one thing that must be constantly borne in mind is that you are observing effects and not causes.</rdfs:comment>
        <rdfs:label xml:lang="en">Gait_assessment</rdfs:label>
    </owl:NamedIndividual>
    


    <!-- http://www.semanticweb.org/marthinust/ontologies/2022/8/Gait_Ontology#Gait_imbalance -->

    <owl:NamedIndividual rdf:about="http://www.semanticweb.org/marthinust/ontologies/2022/8/Gait_Ontology#Gait_imbalance">
        <rdf:type rdf:resource="http://www.semanticweb.org/marthinust/ontologies/2022/8/Gait_Ontology#Gait_Disturbance"/>
        <Gait_Ontology:affects rdf:resource="http://www.semanticweb.org/marthinust/ontologies/2022/8/Gait_Ontology#Adolescent"/>
        <Gait_Ontology:isDiagnosedBy rdf:resource="http://www.semanticweb.org/marthinust/ontologies/2022/8/Gait_Ontology#Podiatrist"/>
        <Gait_Ontology:isVerifiedBy rdf:resource="http://www.semanticweb.org/marthinust/ontologies/2022/8/Gait_Ontology#GRF_sensor"/>
        <Gait_Ontology:hasClinical_term rdf:datatype="http://www.w3.org/2001/XMLSchema#string">Imbalanced walking</Gait_Ontology:hasClinical_term>
    </owl:NamedIndividual>
    


    <!-- http://www.semanticweb.org/marthinust/ontologies/2022/8/Gait_Ontology#Gait_walk -->

    <owl:NamedIndividual rdf:about="http://www.semanticweb.org/marthinust/ontologies/2022/8/Gait_Ontology#Gait_walk">
        <rdf:type rdf:resource="http://www.semanticweb.org/marthinust/ontologies/2022/8/Gait_Ontology#Gait_Cycle"/>
        <Gait_Ontology:isDemonstratedBy rdf:resource="http://www.semanticweb.org/marthinust/ontologies/2022/8/Gait_Ontology#Adolescent"/>
        <Gait_Ontology:isDemonstratedBy rdf:resource="http://www.semanticweb.org/marthinust/ontologies/2022/8/Gait_Ontology#Adult"/>
        <Gait_Ontology:isDemonstratedBy rdf:resource="http://www.semanticweb.org/marthinust/ontologies/2022/8/Gait_Ontology#Athlete"/>
        <Gait_Ontology:isDemonstratedBy rdf:resource="http://www.semanticweb.org/marthinust/ontologies/2022/8/Gait_Ontology#Child"/>
        <Gait_Ontology:isDemonstratedBy rdf:resource="http://www.semanticweb.org/marthinust/ontologies/2022/8/Gait_Ontology#Elderly"/>
        <Gait_Ontology:isObservedBy rdf:resource="http://www.semanticweb.org/marthinust/ontologies/2022/8/Gait_Ontology#Biomechanist"/>
        <Gait_Ontology:isObservedBy rdf:resource="http://www.semanticweb.org/marthinust/ontologies/2022/8/Gait_Ontology#Healthcare_practitioner"/>
        <Gait_Ontology:isObservedBy rdf:resource="http://www.semanticweb.org/marthinust/ontologies/2022/8/Gait_Ontology#Orthopedist"/>
        <Gait_Ontology:isObservedBy rdf:resource="http://www.semanticweb.org/marthinust/ontologies/2022/8/Gait_Ontology#Physical_therapist"/>
        <Gait_Ontology:isObservedBy rdf:resource="http://www.semanticweb.org/marthinust/ontologies/2022/8/Gait_Ontology#Podiatrist"/>
        <Gait_Ontology:isObservedIn rdf:resource="http://www.semanticweb.org/marthinust/ontologies/2022/8/Gait_Ontology#Gait_assessment"/>
        <Gait_Ontology:hasGait_phase_cycle rdf:datatype="http://www.w3.org/2001/XMLSchema#string">Striding</Gait_Ontology:hasGait_phase_cycle>
        <rdfs:comment xml:lang="en">A manner of walking or moving on foot. : a sequence of foot movements (such as a walk, trot, pace, or canter) by which a human, horse or a dog moves forward. Gait is a person&apos;s pattern of walking. Walking involves balance and coordination of muscles so that the body is propelled forward in a rhythm, called the stride.</rdfs:comment>
        <rdfs:label xml:lang="en">Gait_walk</rdfs:label>
    </owl:NamedIndividual>
    


    <!-- http://www.semanticweb.org/marthinust/ontologies/2022/8/Gait_Ontology#Gonio -->

    <owl:NamedIndividual rdf:about="http://www.semanticweb.org/marthinust/ontologies/2022/8/Gait_Ontology#Gonio">
        <rdf:type rdf:resource="http://www.semanticweb.org/marthinust/ontologies/2022/8/Gait_Ontology#Gait_Analysis_Equipment"/>
        <Gait_Ontology:isLinkedTo rdf:resource="http://www.semanticweb.org/marthinust/ontologies/2022/8/Gait_Ontology#Child"/>
        <Gait_Ontology:isUsedFor rdf:resource="http://www.semanticweb.org/marthinust/ontologies/2022/8/Gait_Ontology#Gait_assessment"/>
        <Gait_Ontology:isUsedIn rdf:resource="http://www.semanticweb.org/marthinust/ontologies/2022/8/Gait_Ontology#Motion_system"/>
        <Gait_Ontology:hasEquipment_type rdf:datatype="http://www.w3.org/2001/XMLSchema#string">Goniometer</Gait_Ontology:hasEquipment_type>
        <rdfs:comment xml:lang="en">Unlike the inertial sensor, the flexible goniometer is operated by measuring the change in the physical signal resulting from the angular change. A flexible goniometer can be used to measure the relative rotation between two human body segments.

The flexible goniometers used in gait analysis can be divided into strain gauges, mechanical flexible, inductive, and optical fiber goniometers. A number of flexible electrogoniometers based on a strain gauge have been developed and used for angle measurement in gait analysis since the 1980s. At present, numerous commercialized flexible electrogoniometers are available for the measurement of human posture and spinal motion. A mechanical flexible goniometer is designed to obtain angular change by measuring the longitudinal displacement of two parallel wires bent in the plane of rotation, which is demonstrated by measuring the knee joint during human walking.</rdfs:comment>
        <rdfs:label xml:lang="en">Gonio</rdfs:label>
    </owl:NamedIndividual>
    


    <!-- http://www.semanticweb.org/marthinust/ontologies/2022/8/Gait_Ontology#Gyroscope -->

    <owl:NamedIndividual rdf:about="http://www.semanticweb.org/marthinust/ontologies/2022/8/Gait_Ontology#Gyroscope">
        <rdf:type rdf:resource="http://www.semanticweb.org/marthinust/ontologies/2022/8/Gait_Ontology#Gait_Analysis_Equipment"/>
        <Gait_Ontology:isLinkedTo rdf:resource="http://www.semanticweb.org/marthinust/ontologies/2022/8/Gait_Ontology#Elderly"/>
        <Gait_Ontology:isUsedFor rdf:resource="http://www.semanticweb.org/marthinust/ontologies/2022/8/Gait_Ontology#Gait_assessment"/>
        <Gait_Ontology:isUsedIn rdf:resource="http://www.semanticweb.org/marthinust/ontologies/2022/8/Gait_Ontology#AI_method"/>
        <Gait_Ontology:hasEquipment_type rdf:datatype="http://www.w3.org/2001/XMLSchema#string">Gyroscopic sensor</Gait_Ontology:hasEquipment_type>
        <rdfs:comment xml:lang="en">A gyroscope is an angular velocity sensor. The micromachined gyroscope is based on the concept of measuring the Coriolis force, which is an apparent force proportional to the angular rate of rotation in a rotating reference frame. By detecting the linear motion from the Coriolis effort and performing an integration of the gyroscopic signal, the angular rate can be obtained. In addition, gyroscopes based on other operating principles also exist, such as the electronic, microchip-packaged MEMS gyroscope devices found in consumer electronic devices, solid-state ring lasers, fiber optic gyroscopes, and the extremely sensitive quantum gyroscope. A gyroscope can be applied for the measurement of the motion and posture of the human segment in gait analysis by measuring the angular rate. For example, by attaching a gyroscope to human feet or legs, the angular velocity and angle of feet or legs during the gait can be determined to realise the reorganisation of the various gait phases. In the gait analysis, a gyroscope is usually combined with an accelerometer to construct a complete initial sensing system.</rdfs:comment>
        <rdfs:label xml:lang="en">Gyroscope</rdfs:label>
    </owl:NamedIndividual>
    


    <!-- http://www.semanticweb.org/marthinust/ontologies/2022/8/Gait_Ontology#Hallux_rigidus -->

    <owl:NamedIndividual rdf:about="http://www.semanticweb.org/marthinust/ontologies/2022/8/Gait_Ontology#Hallux_rigidus">
        <rdf:type rdf:resource="http://www.semanticweb.org/marthinust/ontologies/2022/8/Gait_Ontology#Gait_Pathology"/>
        <Gait_Ontology:isCategorisedIn rdf:resource="http://www.semanticweb.org/marthinust/ontologies/2022/8/Gait_Ontology#Musculoskeletal"/>
        <Gait_Ontology:hasPathology_trait rdf:datatype="http://www.w3.org/2001/XMLSchema#string">Reduced rang of motion in foot.</Gait_Ontology:hasPathology_trait>
    </owl:NamedIndividual>
    


    <!-- http://www.semanticweb.org/marthinust/ontologies/2022/8/Gait_Ontology#Healthcare_practitioner -->

    <owl:NamedIndividual rdf:about="http://www.semanticweb.org/marthinust/ontologies/2022/8/Gait_Ontology#Healthcare_practitioner">
        <rdf:type rdf:resource="http://www.semanticweb.org/marthinust/ontologies/2022/8/Gait_Ontology#Gait_expert"/>
        <Gait_Ontology:administers rdf:resource="http://www.semanticweb.org/marthinust/ontologies/2022/8/Gait_Ontology#Gait_assessment"/>
        <Gait_Ontology:analyzes rdf:resource="http://www.semanticweb.org/marthinust/ontologies/2022/8/Gait_Ontology#Clinical_data"/>
        <Gait_Ontology:facilitates rdf:resource="http://www.semanticweb.org/marthinust/ontologies/2022/8/Gait_Ontology#Clinical_evaluation"/>
        <Gait_Ontology:observes rdf:resource="http://www.semanticweb.org/marthinust/ontologies/2022/8/Gait_Ontology#Gait_walk"/>
        <Gait_Ontology:prescribes rdf:resource="http://www.semanticweb.org/marthinust/ontologies/2022/8/Gait_Ontology#Walker"/>
        <Gait_Ontology:treats rdf:resource="http://www.semanticweb.org/marthinust/ontologies/2022/8/Gait_Ontology#Elderly"/>
        <Gait_Ontology:hasGait_expert rdf:datatype="http://www.w3.org/2001/XMLSchema#string">Healthcare practitioner</Gait_Ontology:hasGait_expert>
        <Gait_Ontology:hasGender rdf:datatype="http://www.w3.org/2001/XMLSchema#string">Male</Gait_Ontology:hasGender>
        <rdfs:comment xml:lang="en">A healthcare practitioner is a person who is trained and licensed to provide medical treatment to individuals. This can include doctors, nurses, surgeons, and other professionals who are qualified to diagnose and treat patients. Healthcare practitioners typically work in a variety of settings, such as hospitals, clinics, private practices, and other healthcare facilities. They may also work in specialised areas of medicine, such as pediatrics, surgery, or mental health. The specific duties and responsibilities of a healthcare practitioner will depend on their specific area of practice and the needs of their patients.</rdfs:comment>
        <rdfs:label xml:lang="en">Healthcare_practitioner</rdfs:label>
    </owl:NamedIndividual>
    


    <!-- http://www.semanticweb.org/marthinust/ontologies/2022/8/Gait_Ontology#Hip_abductor_weakness -->

    <owl:NamedIndividual rdf:about="http://www.semanticweb.org/marthinust/ontologies/2022/8/Gait_Ontology#Hip_abductor_weakness">
        <rdf:type rdf:resource="http://www.semanticweb.org/marthinust/ontologies/2022/8/Gait_Ontology#Gait_Pathology"/>
        <Gait_Ontology:isCategorisedIn rdf:resource="http://www.semanticweb.org/marthinust/ontologies/2022/8/Gait_Ontology#Neuromuscular"/>
        <Gait_Ontology:hasPathology_trait rdf:datatype="http://www.w3.org/2001/XMLSchema#string">Hip abductor weakness</Gait_Ontology:hasPathology_trait>
    </owl:NamedIndividual>
    


    <!-- http://www.semanticweb.org/marthinust/ontologies/2022/8/Gait_Ontology#Hip_spina_bifida -->

    <owl:NamedIndividual rdf:about="http://www.semanticweb.org/marthinust/ontologies/2022/8/Gait_Ontology#Hip_spina_bifida">
        <rdf:type rdf:resource="http://www.semanticweb.org/marthinust/ontologies/2022/8/Gait_Ontology#Gait-related_Disease"/>
        <Gait_Ontology:isAssociatedTo rdf:resource="http://www.semanticweb.org/marthinust/ontologies/2022/8/Gait_Ontology#Child"/>
        <Gait_Ontology:hasDisease_description rdf:datatype="http://www.w3.org/2001/XMLSchema#string">Spina bifida</Gait_Ontology:hasDisease_description>
        <rdfs:comment xml:lang="en">Spina bifida is a gait-related disease, meaning that it can cause gait disturbances. Individuals with spina bifida often experience gait impairments due to the neurological deficits associated with the condition. These impairments can include reduced muscle strength and coordination, as well as decreased sensation, which can all lead to impaired gait patterns.

Spina bifida is a congenital birth defect that affects the spinal column and spinal cord. It occurs when the neural tube, which forms during the early stages of fetal development, does not close properly, resulting in a gap or opening in the spinal column. This can lead to damage or malformation of the spinal cord and nerves, which can cause a range of physical and neurological problems.

The condition can cause weakness or paralysis in the legs, as well as other neurological problems that can affect an individual&apos;s ability to walk and maintain balance. Some individuals with spina bifida may require assistive devices such as braces, crutches, or wheelchairs to help with mobility, while others may be able to walk independently. Treatment for spina bifida often involves physical therapy and other interventions to improve gait and mobility, as well as manage other symptoms of the condition.</rdfs:comment>
        <rdfs:label xml:lang="en">Hip_spina_bifida</rdfs:label>
    </owl:NamedIndividual>
    


    <!-- http://www.semanticweb.org/marthinust/ontologies/2022/8/Gait_Ontology#Image_sensing -->

    <owl:NamedIndividual rdf:about="http://www.semanticweb.org/marthinust/ontologies/2022/8/Gait_Ontology#Image_sensing">
        <rdf:type rdf:resource="http://www.semanticweb.org/marthinust/ontologies/2022/8/Gait_Ontology#Gait_Analysis_Method"/>
        <Gait_Ontology:isBasedOn rdf:resource="http://www.semanticweb.org/marthinust/ontologies/2022/8/Gait_Ontology#GRF_sensor"/>
        <Gait_Ontology:hasAnalysis_method rdf:datatype="http://www.w3.org/2001/XMLSchema#string">Multi camera image capture</Gait_Ontology:hasAnalysis_method>
    </owl:NamedIndividual>
    


    <!-- http://www.semanticweb.org/marthinust/ontologies/2022/8/Gait_Ontology#Kinematography -->

    <owl:NamedIndividual rdf:about="http://www.semanticweb.org/marthinust/ontologies/2022/8/Gait_Ontology#Kinematography">
        <rdf:type rdf:resource="http://www.semanticweb.org/marthinust/ontologies/2022/8/Gait_Ontology#Gait_Analysis_Method"/>
        <Gait_Ontology:isBasedOn rdf:resource="http://www.semanticweb.org/marthinust/ontologies/2022/8/Gait_Ontology#EM_tracking_system"/>
        <Gait_Ontology:hasAnalysis_method rdf:datatype="http://www.w3.org/2001/XMLSchema#string">Kinematics</Gait_Ontology:hasAnalysis_method>
        <rdfs:comment xml:lang="en">A three-in-one device that could record, develop and project motion (moving) pictures of individuals.</rdfs:comment>
        <rdfs:label xml:lang="en">Kinematography</rdfs:label>
    </owl:NamedIndividual>
    


    <!-- http://www.semanticweb.org/marthinust/ontologies/2022/8/Gait_Ontology#LL_discrepancy -->

    <owl:NamedIndividual rdf:about="http://www.semanticweb.org/marthinust/ontologies/2022/8/Gait_Ontology#LL_discrepancy">
        <rdf:type rdf:resource="http://www.semanticweb.org/marthinust/ontologies/2022/8/Gait_Ontology#Gait_Pathology"/>
        <Gait_Ontology:isCategorisedIn rdf:resource="http://www.semanticweb.org/marthinust/ontologies/2022/8/Gait_Ontology#Musculoskeletal"/>
        <Gait_Ontology:hasPathology_trait rdf:datatype="http://www.w3.org/2001/XMLSchema#string">Leg length discrepancy</Gait_Ontology:hasPathology_trait>
        <rdfs:comment xml:lang="en">Leg length discrepancy (LLD) refers to a condition in which the length of one leg is significantly different from the length of the other leg. This can be due to a number of factors, including congenital differences (present at birth), developmental conditions, injuries, or diseases. The difference in leg length can be measured in millimeters or centimeters and is usually determined by a physical examination, x-ray, or other imaging modality.

LLD can lead to a number of symptoms, such as pain in the back, hips, knees, or ankles, as well as problems with walking or standing. In some cases, LLD can be treated with the use of shoe lifts or orthotic devices, while in other cases, surgical intervention may be necessary.

Leg length discrepancy can be as a result of an asymmetrical pelvic, tibia, or femur length or for other reasons such as scoliosis or contractures. The gait pattern will present as a pelvic dip to the shortened side during the stance phase with possible toe walking on that limb. The opposite leg is likely to increase its knee and hip flexion to reduce its length.</rdfs:comment>
        <rdfs:label xml:lang="en">Leg_length_discrepency</rdfs:label>
    </owl:NamedIndividual>
    


    <!-- http://www.semanticweb.org/marthinust/ontologies/2022/8/Gait_Ontology#Limp_gait -->

    <owl:NamedIndividual rdf:about="http://www.semanticweb.org/marthinust/ontologies/2022/8/Gait_Ontology#Limp_gait">
        <rdf:type rdf:resource="http://www.semanticweb.org/marthinust/ontologies/2022/8/Gait_Ontology#Type_of_Gait"/>
        <Gait_Ontology:isDetectedIn rdf:resource="http://www.semanticweb.org/marthinust/ontologies/2022/8/Gait_Ontology#Image_sensing"/>
        <Gait_Ontology:isExhibitedBy rdf:resource="http://www.semanticweb.org/marthinust/ontologies/2022/8/Gait_Ontology#Adolescent"/>
        <Gait_Ontology:isInfluencedBy rdf:resource="http://www.semanticweb.org/marthinust/ontologies/2022/8/Gait_Ontology#Scoliosis"/>
        <Gait_Ontology:isRelatedTo rdf:resource="http://www.semanticweb.org/marthinust/ontologies/2022/8/Gait_Ontology#Gait_imbalance"/>
        <Gait_Ontology:hasGait_type rdf:datatype="http://www.w3.org/2001/XMLSchema#string">Limping due to leg length discrepancy</Gait_Ontology:hasGait_type>
    </owl:NamedIndividual>
    


    <!-- http://www.semanticweb.org/marthinust/ontologies/2022/8/Gait_Ontology#Mild -->

    <owl:NamedIndividual rdf:about="http://www.semanticweb.org/marthinust/ontologies/2022/8/Gait_Ontology#Mild">
        <rdf:type rdf:resource="http://www.semanticweb.org/marthinust/ontologies/2022/8/Gait_Ontology#Severity_Scale"/>
        <Gait_Ontology:isMilderThan rdf:resource="http://www.semanticweb.org/marthinust/ontologies/2022/8/Gait_Ontology#Acute"/>
        <Gait_Ontology:isMilderThan rdf:resource="http://www.semanticweb.org/marthinust/ontologies/2022/8/Gait_Ontology#Severe"/>
        <rdfs:comment xml:lang="en">A mild condition, illness or injury is one that is not as painful or serious.</rdfs:comment>
        <rdfs:label xml:lang="en">Mild</rdfs:label>
    </owl:NamedIndividual>
    


    <!-- http://www.semanticweb.org/marthinust/ontologies/2022/8/Gait_Ontology#Motion_system -->

    <owl:NamedIndividual rdf:about="http://www.semanticweb.org/marthinust/ontologies/2022/8/Gait_Ontology#Motion_system">
        <rdf:type rdf:resource="http://www.semanticweb.org/marthinust/ontologies/2022/8/Gait_Ontology#Gait_Analysis_Method"/>
        <Gait_Ontology:isBasedOn rdf:resource="http://www.semanticweb.org/marthinust/ontologies/2022/8/Gait_Ontology#Gonio"/>
        <Gait_Ontology:hasAnalysis_method rdf:datatype="http://www.w3.org/2001/XMLSchema#string">Electronic Motion System</Gait_Ontology:hasAnalysis_method>
        <rdfs:comment xml:lang="en">Gait analysis has used different types of motion sensors and systems, such as the accelerometer, gyroscope, magnetoresistive sensors, flexible goniometer, electromagnetic tracking system (ETS), sensing fabric, force sensor, and sensors for electromyography (EMG). Based on these sensors, a single type or a combined sensor system of multiple types of sensors may be used for various gait analysis applications.</rdfs:comment>
        <rdfs:label xml:lang="en">Motion_system</rdfs:label>
    </owl:NamedIndividual>
    


    <!-- http://www.semanticweb.org/marthinust/ontologies/2022/8/Gait_Ontology#Musculoskeletal -->

    <owl:NamedIndividual rdf:about="http://www.semanticweb.org/marthinust/ontologies/2022/8/Gait_Ontology#Musculoskeletal">
        <rdf:type rdf:resource="http://www.semanticweb.org/marthinust/ontologies/2022/8/Gait_Ontology#Gait_Classification"/>
        <Gait_Ontology:isIdentifiedIn rdf:resource="http://www.semanticweb.org/marthinust/ontologies/2022/8/Gait_Ontology#Image_sensing"/>
        <Gait_Ontology:isIdentifiedIn rdf:resource="http://www.semanticweb.org/marthinust/ontologies/2022/8/Gait_Ontology#Sensory"/>
        <Gait_Ontology:hasGait_classification rdf:datatype="http://www.w3.org/2001/XMLSchema#string">Leg and foot stiffness</Gait_Ontology:hasGait_classification>
        <Gait_Ontology:hasGait_classification rdf:datatype="http://www.w3.org/2001/XMLSchema#string">Leg limb discrepancy</Gait_Ontology:hasGait_classification>
    </owl:NamedIndividual>
    


    <!-- http://www.semanticweb.org/marthinust/ontologies/2022/8/Gait_Ontology#Neurological -->

    <owl:NamedIndividual rdf:about="http://www.semanticweb.org/marthinust/ontologies/2022/8/Gait_Ontology#Neurological">
        <rdf:type rdf:resource="http://www.semanticweb.org/marthinust/ontologies/2022/8/Gait_Ontology#Gait_Classification"/>
        <Gait_Ontology:isIdentifiedIn rdf:resource="http://www.semanticweb.org/marthinust/ontologies/2022/8/Gait_Ontology#AI_method"/>
        <Gait_Ontology:isIdentifiedIn rdf:resource="http://www.semanticweb.org/marthinust/ontologies/2022/8/Gait_Ontology#Kinematography"/>
        <Gait_Ontology:hasGait_classification rdf:datatype="http://www.w3.org/2001/XMLSchema#string">Neurological gait dysfunction</Gait_Ontology:hasGait_classification>
        <Gait_Ontology:hasGait_classification rdf:datatype="http://www.w3.org/2001/XMLSchema#string">Parkinsonian</Gait_Ontology:hasGait_classification>
    </owl:NamedIndividual>
    


    <!-- http://www.semanticweb.org/marthinust/ontologies/2022/8/Gait_Ontology#Neuromuscular -->

    <owl:NamedIndividual rdf:about="http://www.semanticweb.org/marthinust/ontologies/2022/8/Gait_Ontology#Neuromuscular">
        <rdf:type rdf:resource="http://www.semanticweb.org/marthinust/ontologies/2022/8/Gait_Ontology#Gait_Classification"/>
        <Gait_Ontology:isIdentifiedIn rdf:resource="http://www.semanticweb.org/marthinust/ontologies/2022/8/Gait_Ontology#Motion_system"/>
        <Gait_Ontology:hasGait_classification rdf:datatype="http://www.w3.org/2001/XMLSchema#string">Hip abductor weakness</Gait_Ontology:hasGait_classification>
    </owl:NamedIndividual>
    


    <!-- http://www.semanticweb.org/marthinust/ontologies/2022/8/Gait_Ontology#Normal_gait -->

    <owl:NamedIndividual rdf:about="http://www.semanticweb.org/marthinust/ontologies/2022/8/Gait_Ontology#Normal_gait">
        <rdf:type rdf:resource="http://www.semanticweb.org/marthinust/ontologies/2022/8/Gait_Ontology#Type_of_Gait"/>
        <Gait_Ontology:isDetectedIn rdf:resource="http://www.semanticweb.org/marthinust/ontologies/2022/8/Gait_Ontology#Sensory"/>
        <Gait_Ontology:isExhibitedBy rdf:resource="http://www.semanticweb.org/marthinust/ontologies/2022/8/Gait_Ontology#Athlete"/>
        <Gait_Ontology:isInfluencedBy rdf:resource="http://www.semanticweb.org/marthinust/ontologies/2022/8/Gait_Ontology#Dystonia"/>
        <Gait_Ontology:isRelatedTo rdf:resource="http://www.semanticweb.org/marthinust/ontologies/2022/8/Gait_Ontology#Dystonic_gait"/>
        <Gait_Ontology:hasGait_type rdf:datatype="http://www.w3.org/2001/XMLSchema#string">Temporary stiffness before normal gait returns</Gait_Ontology:hasGait_type>
    </owl:NamedIndividual>
    


    <!-- http://www.semanticweb.org/marthinust/ontologies/2022/8/Gait_Ontology#Orthopedist -->

    <owl:NamedIndividual rdf:about="http://www.semanticweb.org/marthinust/ontologies/2022/8/Gait_Ontology#Orthopedist">
        <rdf:type rdf:resource="http://www.semanticweb.org/marthinust/ontologies/2022/8/Gait_Ontology#Gait_expert"/>
        <Gait_Ontology:administers rdf:resource="http://www.semanticweb.org/marthinust/ontologies/2022/8/Gait_Ontology#Gait_assessment"/>
        <Gait_Ontology:analyzes rdf:resource="http://www.semanticweb.org/marthinust/ontologies/2022/8/Gait_Ontology#Clinical_data"/>
        <Gait_Ontology:facilitates rdf:resource="http://www.semanticweb.org/marthinust/ontologies/2022/8/Gait_Ontology#Clinical_evaluation"/>
        <Gait_Ontology:observes rdf:resource="http://www.semanticweb.org/marthinust/ontologies/2022/8/Gait_Ontology#Gait_walk"/>
        <Gait_Ontology:prescribes rdf:resource="http://www.semanticweb.org/marthinust/ontologies/2022/8/Gait_Ontology#Braces"/>
        <Gait_Ontology:treats rdf:resource="http://www.semanticweb.org/marthinust/ontologies/2022/8/Gait_Ontology#Child"/>
        <Gait_Ontology:hasGait_expert rdf:datatype="http://www.w3.org/2001/XMLSchema#string">Orthopedist</Gait_Ontology:hasGait_expert>
        <Gait_Ontology:hasGender rdf:datatype="http://www.w3.org/2001/XMLSchema#string">Female</Gait_Ontology:hasGender>
        <rdfs:comment xml:lang="en">An orthopedist is a medical doctor who specialises in the diagnosis and treatment of disorders of the musculoskeletal system, which includes bones, joints, muscles, tendons, and ligaments. Orthopedists are trained to diagnose and treat a wide range of conditions, including fractures, dislocations, sprains and strains, tendonitis, bursitis, and osteoarthritis. They may use a variety of treatments, including medications, physical therapy, and surgery to treat their patients.</rdfs:comment>
        <rdfs:label xml:lang="en">Orthopedist</rdfs:label>
    </owl:NamedIndividual>
    


    <!-- http://www.semanticweb.org/marthinust/ontologies/2022/8/Gait_Ontology#Orthotic -->

    <owl:NamedIndividual rdf:about="http://www.semanticweb.org/marthinust/ontologies/2022/8/Gait_Ontology#Orthotic">
        <rdf:type rdf:resource="http://www.semanticweb.org/marthinust/ontologies/2022/8/Gait_Ontology#Gait_Assistive_Technology"/>
        <Gait_Ontology:isAscertainedIn rdf:resource="http://www.semanticweb.org/marthinust/ontologies/2022/8/Gait_Ontology#Gait_assessment"/>
        <Gait_Ontology:isPrescribedBy rdf:resource="http://www.semanticweb.org/marthinust/ontologies/2022/8/Gait_Ontology#Podiatrist"/>
        <Gait_Ontology:isRecommendedTo rdf:resource="http://www.semanticweb.org/marthinust/ontologies/2022/8/Gait_Ontology#Adolescent"/>
        <Gait_Ontology:hasGait_assistive_solution rdf:datatype="http://www.w3.org/2001/XMLSchema#string">Specialised shoe</Gait_Ontology:hasGait_assistive_solution>
        <Gait_Ontology:hasType_of_material rdf:datatype="http://www.w3.org/2001/XMLSchema#string">Soft leather</Gait_Ontology:hasType_of_material>
        <rdfs:comment xml:lang="en">Orthotics are used for correcting foot deformities, providing ankle support, and promoting better foot or ankle function, among other important purposes. Although orthotics can be purchased in stores, podiatrists (foot doctors) highly recommend custom orthotics, as these are designed to fit your feet perfectly.

They are prescription medical devices that you wear inside your shoes to correct biomechanical foot issues such as problems with how you walk, stand, or run. They can also help with foot pain caused by medical conditions such as diabetes, plantar fasciitis, bursitis, and arthritis.</rdfs:comment>
        <rdfs:label xml:lang="en">Orthotic</rdfs:label>
    </owl:NamedIndividual>
    


    <!-- http://www.semanticweb.org/marthinust/ontologies/2022/8/Gait_Ontology#Pace -->

    <owl:NamedIndividual rdf:about="http://www.semanticweb.org/marthinust/ontologies/2022/8/Gait_Ontology#Pace">
        <rdf:type rdf:resource="http://www.semanticweb.org/marthinust/ontologies/2022/8/Gait_Ontology#Gait_Parameter"/>
        <Gait_Ontology:isDeterminedBy rdf:resource="http://www.semanticweb.org/marthinust/ontologies/2022/8/Gait_Ontology#Foot_pronation"/>
        <Gait_Ontology:isEvaluatedIn rdf:resource="http://www.semanticweb.org/marthinust/ontologies/2022/8/Gait_Ontology#Gait_walk"/>
        <Gait_Ontology:hasParameter rdf:datatype="http://www.w3.org/2001/XMLSchema#string">Tempo</Gait_Ontology:hasParameter>
        <rdfs:comment xml:lang="en">Pace - speed in walking, running, or moving.
Pace - the speed or rate at which something happens or develops.
Pace - a unit of length representing the distance between two successive steps in walking.</rdfs:comment>
        <rdfs:label xml:lang="en">Pace</rdfs:label>
    </owl:NamedIndividual>
    


    <!-- http://www.semanticweb.org/marthinust/ontologies/2022/8/Gait_Ontology#Parkinsonian_gait -->

    <owl:NamedIndividual rdf:about="http://www.semanticweb.org/marthinust/ontologies/2022/8/Gait_Ontology#Parkinsonian_gait">
        <rdf:type rdf:resource="http://www.semanticweb.org/marthinust/ontologies/2022/8/Gait_Ontology#Type_of_Gait"/>
        <Gait_Ontology:isDetectedIn rdf:resource="http://www.semanticweb.org/marthinust/ontologies/2022/8/Gait_Ontology#AI_method"/>
        <Gait_Ontology:isExhibitedBy rdf:resource="http://www.semanticweb.org/marthinust/ontologies/2022/8/Gait_Ontology#Elderly"/>
        <Gait_Ontology:isInfluencedBy rdf:resource="http://www.semanticweb.org/marthinust/ontologies/2022/8/Gait_Ontology#Parkinson&apos;s"/>
        <Gait_Ontology:isRelatedTo rdf:resource="http://www.semanticweb.org/marthinust/ontologies/2022/8/Gait_Ontology#Freezing_of_gait"/>
        <Gait_Ontology:hasGait_type rdf:datatype="http://www.w3.org/2001/XMLSchema#string">Festinating gait pattern</Gait_Ontology:hasGait_type>
    </owl:NamedIndividual>
    


    <!-- http://www.semanticweb.org/marthinust/ontologies/2022/8/Gait_Ontology#Pharmaceutical -->

    <owl:NamedIndividual rdf:about="http://www.semanticweb.org/marthinust/ontologies/2022/8/Gait_Ontology#Pharmaceutical">
        <rdf:type rdf:resource="http://www.semanticweb.org/marthinust/ontologies/2022/8/Gait_Ontology#Gait_Assistive_Technology"/>
        <Gait_Ontology:isAscertainedIn rdf:resource="http://www.semanticweb.org/marthinust/ontologies/2022/8/Gait_Ontology#Gait_assessment"/>
        <Gait_Ontology:isPrescribedBy rdf:resource="http://www.semanticweb.org/marthinust/ontologies/2022/8/Gait_Ontology#Biomechanist"/>
        <Gait_Ontology:isRecommendedTo rdf:resource="http://www.semanticweb.org/marthinust/ontologies/2022/8/Gait_Ontology#Athlete"/>
        <Gait_Ontology:hasGait_assistive_solution rdf:datatype="http://www.w3.org/2001/XMLSchema#string">Pharmacotherapy</Gait_Ontology:hasGait_assistive_solution>
        <Gait_Ontology:hasType_of_material rdf:datatype="http://www.w3.org/2001/XMLSchema#string">Natural</Gait_Ontology:hasType_of_material>
        <rdfs:comment xml:lang="en">Pharmaceutical (pharmacology) is the treatment of a disorder or disease with medication.

Pharmacotherapy is the treatment of health conditions by using pharmaceutical products (drugs) as medication.</rdfs:comment>
        <rdfs:label xml:lang="en">Pharmaceutical</rdfs:label>
    </owl:NamedIndividual>
    


    <!-- http://www.semanticweb.org/marthinust/ontologies/2022/8/Gait_Ontology#Physical_therapist -->

    <owl:NamedIndividual rdf:about="http://www.semanticweb.org/marthinust/ontologies/2022/8/Gait_Ontology#Physical_therapist">
        <rdf:type rdf:resource="http://www.semanticweb.org/marthinust/ontologies/2022/8/Gait_Ontology#Gait_expert"/>
        <Gait_Ontology:administers rdf:resource="http://www.semanticweb.org/marthinust/ontologies/2022/8/Gait_Ontology#Gait_assessment"/>
        <Gait_Ontology:analyzes rdf:resource="http://www.semanticweb.org/marthinust/ontologies/2022/8/Gait_Ontology#Clinical_data"/>
        <Gait_Ontology:facilitates rdf:resource="http://www.semanticweb.org/marthinust/ontologies/2022/8/Gait_Ontology#Clinical_evaluation"/>
        <Gait_Ontology:observes rdf:resource="http://www.semanticweb.org/marthinust/ontologies/2022/8/Gait_Ontology#Gait_walk"/>
        <Gait_Ontology:prescribes rdf:resource="http://www.semanticweb.org/marthinust/ontologies/2022/8/Gait_Ontology#Walking_stick"/>
        <Gait_Ontology:treats rdf:resource="http://www.semanticweb.org/marthinust/ontologies/2022/8/Gait_Ontology#Adult"/>
        <Gait_Ontology:hasGait_expert rdf:datatype="http://www.w3.org/2001/XMLSchema#string">Physical therapist</Gait_Ontology:hasGait_expert>
        <Gait_Ontology:hasGender rdf:datatype="http://www.w3.org/2001/XMLSchema#string">Male</Gait_Ontology:hasGender>
        <rdfs:comment xml:lang="en">A physical therapist is a healthcare professional who helps patients recover from injuries, disabilities, and surgeries by using various techniques to improve mobility, reduce pain, and increase strength. Physical therapists use a variety of treatments, such as exercise, stretching, and massage, to help patients achieve their goals and improve their overall quality of life. They may work with patients who have a wide range of conditions, including sports injuries, chronic pain, arthritis, stroke, and orthopedic injuries. Physical therapists may work in hospitals, outpatient clinics, rehabilitation centers, or private practice.</rdfs:comment>
        <rdfs:label xml:lang="en">Physical_therapist</rdfs:label>
    </owl:NamedIndividual>
    


    <!-- http://www.semanticweb.org/marthinust/ontologies/2022/8/Gait_Ontology#Podiatrist -->

    <owl:NamedIndividual rdf:about="http://www.semanticweb.org/marthinust/ontologies/2022/8/Gait_Ontology#Podiatrist">
        <rdf:type rdf:resource="http://www.semanticweb.org/marthinust/ontologies/2022/8/Gait_Ontology#Gait_expert"/>
        <Gait_Ontology:administers rdf:resource="http://www.semanticweb.org/marthinust/ontologies/2022/8/Gait_Ontology#Gait_assessment"/>
        <Gait_Ontology:analyzes rdf:resource="http://www.semanticweb.org/marthinust/ontologies/2022/8/Gait_Ontology#Clinical_data"/>
        <Gait_Ontology:facilitates rdf:resource="http://www.semanticweb.org/marthinust/ontologies/2022/8/Gait_Ontology#Clinical_evaluation"/>
        <Gait_Ontology:observes rdf:resource="http://www.semanticweb.org/marthinust/ontologies/2022/8/Gait_Ontology#Gait_walk"/>
        <Gait_Ontology:prescribes rdf:resource="http://www.semanticweb.org/marthinust/ontologies/2022/8/Gait_Ontology#Orthotic"/>
        <Gait_Ontology:treats rdf:resource="http://www.semanticweb.org/marthinust/ontologies/2022/8/Gait_Ontology#Adolescent"/>
        <Gait_Ontology:hasGait_expert>Podiatrist</Gait_Ontology:hasGait_expert>
        <Gait_Ontology:hasGender rdf:datatype="http://www.w3.org/2001/XMLSchema#string">Female</Gait_Ontology:hasGender>
        <rdfs:comment xml:lang="en">A podiatrist is a medical doctor who specialises in the diagnosis and treatment of conditions affecting the foot, ankle, and lower leg. Podiatrists are trained to diagnose and treat a wide range of foot and ankle conditions, including foot and ankle injuries, toenail and skin conditions, and deformities such as bunions and hammertoes. They may use a variety of treatments, including medications, physical therapy, and surgery to treat their patients. Podiatrists are also trained to fit and prescribe orthotic devices to help correct foot and ankle problems.</rdfs:comment>
        <rdfs:label xml:lang="en">Podiatrist</rdfs:label>
    </owl:NamedIndividual>
    


    <!-- http://www.semanticweb.org/marthinust/ontologies/2022/8/Gait_Ontology#Progressive_ataxia -->

    <owl:NamedIndividual rdf:about="http://www.semanticweb.org/marthinust/ontologies/2022/8/Gait_Ontology#Progressive_ataxia">
        <rdf:type rdf:resource="http://www.semanticweb.org/marthinust/ontologies/2022/8/Gait_Ontology#Gait_Disturbance"/>
        <Gait_Ontology:affects rdf:resource="http://www.semanticweb.org/marthinust/ontologies/2022/8/Gait_Ontology#Adult"/>
        <Gait_Ontology:isDiagnosedBy rdf:resource="http://www.semanticweb.org/marthinust/ontologies/2022/8/Gait_Ontology#Physical_therapist"/>
        <Gait_Ontology:isVerifiedBy rdf:resource="http://www.semanticweb.org/marthinust/ontologies/2022/8/Gait_Ontology#EM_tracking_system"/>
        <Gait_Ontology:hasClinical_term rdf:datatype="http://www.w3.org/2001/XMLSchema#string">Progressive gait ataxia</Gait_Ontology:hasClinical_term>
        <rdfs:comment xml:lang="en">A type of gait ataxia displaying progression of clinical severity. A type of gait ataxia displaying progression of clinical severity. Progressive ataxia describes a group of uncommon neurological disorders, characterised by problems with balance and coordination.

Progressive cerebellar ataxia is a degenerative neurological condition that affects the nervous system. It occurs when the cerebellum is damaged due to exposure to certain medications, autoimmune disorders, genetics, or other factors.</rdfs:comment>
        <rdfs:label xml:lang="en">Progressive_ataxia</rdfs:label>
    </owl:NamedIndividual>
    


    <!-- http://www.semanticweb.org/marthinust/ontologies/2022/8/Gait_Ontology#Scoliosis -->

    <owl:NamedIndividual rdf:about="http://www.semanticweb.org/marthinust/ontologies/2022/8/Gait_Ontology#Scoliosis">
        <rdf:type rdf:resource="http://www.semanticweb.org/marthinust/ontologies/2022/8/Gait_Ontology#Gait-related_Disease"/>
        <Gait_Ontology:isAssociatedTo rdf:resource="http://www.semanticweb.org/marthinust/ontologies/2022/8/Gait_Ontology#Adolescent"/>
        <Gait_Ontology:hasDisease_description rdf:datatype="http://www.w3.org/2001/XMLSchema#string">Scoliosis is a tri-planar deformity.</Gait_Ontology:hasDisease_description>
    </owl:NamedIndividual>
    


    <!-- http://www.semanticweb.org/marthinust/ontologies/2022/8/Gait_Ontology#Sensory -->

    <owl:NamedIndividual rdf:about="http://www.semanticweb.org/marthinust/ontologies/2022/8/Gait_Ontology#Sensory">
        <rdf:type rdf:resource="http://www.semanticweb.org/marthinust/ontologies/2022/8/Gait_Ontology#Gait_Analysis_Method"/>
        <Gait_Ontology:isBasedOn rdf:resource="http://www.semanticweb.org/marthinust/ontologies/2022/8/Gait_Ontology#Electromyography"/>
        <Gait_Ontology:hasAnalysis_method rdf:datatype="http://www.w3.org/2001/XMLSchema#string">Sensory sensing</Gait_Ontology:hasAnalysis_method>
        <rdfs:comment xml:lang="en">In gait analysis using wearable sensors, motion sensors are worn or attached to various parts of the patients body, such as the foot and waist. These sensors, which may be accelerometers, gyrosensors, force sensors, strain gauges, inclinometers, goniometers, and so on, can measure various characteristics of the human gait. The temporal characteristics of gait are collected and estimated from body-worn accelerometers and pressure sensors inside footwear, on leg sections such as the knee, ankle or foot.</rdfs:comment>
        <rdfs:label xml:lang="en">Sensory</rdfs:label>
    </owl:NamedIndividual>
    


    <!-- http://www.semanticweb.org/marthinust/ontologies/2022/8/Gait_Ontology#Session -->

    <owl:NamedIndividual rdf:about="http://www.semanticweb.org/marthinust/ontologies/2022/8/Gait_Ontology#Session">
        <rdf:type rdf:resource="http://www.semanticweb.org/marthinust/ontologies/2022/8/Gait_Ontology#Gait_acquisition"/>
        <Gait_Ontology:collects rdf:resource="http://www.semanticweb.org/marthinust/ontologies/2022/8/Gait_Ontology#Clinical_data"/>
        <Gait_Ontology:involves rdf:resource="http://www.semanticweb.org/marthinust/ontologies/2022/8/Gait_Ontology#Adolescent"/>
        <Gait_Ontology:involves rdf:resource="http://www.semanticweb.org/marthinust/ontologies/2022/8/Gait_Ontology#Adult"/>
        <Gait_Ontology:involves rdf:resource="http://www.semanticweb.org/marthinust/ontologies/2022/8/Gait_Ontology#Athlete"/>
        <Gait_Ontology:involves rdf:resource="http://www.semanticweb.org/marthinust/ontologies/2022/8/Gait_Ontology#Child"/>
        <Gait_Ontology:involves rdf:resource="http://www.semanticweb.org/marthinust/ontologies/2022/8/Gait_Ontology#Elderly"/>
        <Gait_Ontology:isPartOf rdf:resource="http://www.semanticweb.org/marthinust/ontologies/2022/8/Gait_Ontology#Clinical_evaluation"/>
        <Gait_Ontology:hasGait_acquisition rdf:datatype="http://www.w3.org/2001/XMLSchema#string">Gait (data) aquisition</Gait_Ontology:hasGait_acquisition>
        <rdfs:comment xml:lang="en">Gait acquisition is the process of collecting and analyzing data on an individual&apos;s gait, or the way in which they walk.

Gait (data) acquisition is the process where a patient&apos;s gait assessment  or measurements are obtained in acquisition sessions and observations for quantitative recording and functional description.</rdfs:comment>
        <rdfs:label xml:lang="en">Session</rdfs:label>
    </owl:NamedIndividual>
    


    <!-- http://www.semanticweb.org/marthinust/ontologies/2022/8/Gait_Ontology#Severe -->

    <owl:NamedIndividual rdf:about="http://www.semanticweb.org/marthinust/ontologies/2022/8/Gait_Ontology#Severe">
        <rdf:type rdf:resource="http://www.semanticweb.org/marthinust/ontologies/2022/8/Gait_Ontology#Severity_Scale"/>
        <Gait_Ontology:isSevereThan rdf:resource="http://www.semanticweb.org/marthinust/ontologies/2022/8/Gait_Ontology#Acute"/>
        <Gait_Ontology:isSevereThan rdf:resource="http://www.semanticweb.org/marthinust/ontologies/2022/8/Gait_Ontology#Mild"/>
        <rdfs:comment xml:lang="en">Severewhen you are in pain and it&apos;s getting worse 
causing very great pain, difficulty, worry, damage, etc.</rdfs:comment>
        <rdfs:label xml:lang="en">Severe</rdfs:label>
    </owl:NamedIndividual>
    


    <!-- http://www.semanticweb.org/marthinust/ontologies/2022/8/Gait_Ontology#Tremor -->

    <owl:NamedIndividual rdf:about="http://www.semanticweb.org/marthinust/ontologies/2022/8/Gait_Ontology#Tremor">
        <rdf:type rdf:resource="http://www.semanticweb.org/marthinust/ontologies/2022/8/Gait_Ontology#Gait_Pathology"/>
        <Gait_Ontology:isCategorisedIn rdf:resource="http://www.semanticweb.org/marthinust/ontologies/2022/8/Gait_Ontology#Neurological"/>
        <Gait_Ontology:hasPathology_trait rdf:datatype="http://www.w3.org/2001/XMLSchema#string">Parkinsonism</Gait_Ontology:hasPathology_trait>
        <rdfs:comment xml:lang="en">Parkinsonism comprises a clinical syndrome that presents with a varying degree of rigidity, and a variety of symptoms that include bradykinesia, tremor, and unstable posture, all of which can cause a profound gait impairment. Parkinsonism is an umbrella term that refers to conditions with similar, movement-related effects. These conditions involve slowed movements, and other symptoms are possible depending on the condition.</rdfs:comment>
        <rdfs:label xml:lang="en">Tremor</rdfs:label>
    </owl:NamedIndividual>
    


    <!-- http://www.semanticweb.org/marthinust/ontologies/2022/8/Gait_Ontology#Waddling -->

    <owl:NamedIndividual rdf:about="http://www.semanticweb.org/marthinust/ontologies/2022/8/Gait_Ontology#Waddling">
        <rdf:type rdf:resource="http://www.semanticweb.org/marthinust/ontologies/2022/8/Gait_Ontology#Gait_Disturbance"/>
        <Gait_Ontology:affects rdf:resource="http://www.semanticweb.org/marthinust/ontologies/2022/8/Gait_Ontology#Child"/>
        <Gait_Ontology:isDiagnosedBy rdf:resource="http://www.semanticweb.org/marthinust/ontologies/2022/8/Gait_Ontology#Orthopedist"/>
        <Gait_Ontology:isVerifiedBy rdf:resource="http://www.semanticweb.org/marthinust/ontologies/2022/8/Gait_Ontology#Gonio"/>
        <Gait_Ontology:hasClinical_term rdf:datatype="http://www.w3.org/2001/XMLSchema#string">Wide-based gait</Gait_Ontology:hasClinical_term>
        <rdfs:comment xml:lang="en">Weakness of the hip girdle and upper thigh muscles, for instance in myopathies, leads to an instability of the pelvis on standing and walking. If the muscles extending the hip joint are affected, the posture in that joint becomes flexed and lumbar lordosis increases. The patients usually have difficulties standing up from a sitting position. Due to weakness in the gluteus medius muscle, the hip on the side of the swinging leg drops with each step (referred to as Trendelenburg sign). The gait appears waddling. The patients frequently attempt to counteract the dropping of the hip on the swinging side by bending the trunk towards the side which is in the stance phase (in the German language literature this is referred to as Duchenne sign). Similar gait patterns can be caused by orthopedic conditions when the origin and the insertion site of the gluteus medius muscle are closer to each other than normal, for instance due to a posttraumatic elevation of the trochanter or pseudarthrosis of the femoral neck.</rdfs:comment>
        <rdfs:label xml:lang="en">Waddling</rdfs:label>
    </owl:NamedIndividual>
    


    <!-- http://www.semanticweb.org/marthinust/ontologies/2022/8/Gait_Ontology#Waddling_gait -->

    <owl:NamedIndividual rdf:about="http://www.semanticweb.org/marthinust/ontologies/2022/8/Gait_Ontology#Waddling_gait">
        <rdf:type rdf:resource="http://www.semanticweb.org/marthinust/ontologies/2022/8/Gait_Ontology#Type_of_Gait"/>
        <Gait_Ontology:isDetectedIn rdf:resource="http://www.semanticweb.org/marthinust/ontologies/2022/8/Gait_Ontology#Motion_system"/>
        <Gait_Ontology:isExhibitedBy rdf:resource="http://www.semanticweb.org/marthinust/ontologies/2022/8/Gait_Ontology#Child"/>
        <Gait_Ontology:isInfluencedBy rdf:resource="http://www.semanticweb.org/marthinust/ontologies/2022/8/Gait_Ontology#Hip_spina_bifida"/>
        <Gait_Ontology:isRelatedTo rdf:resource="http://www.semanticweb.org/marthinust/ontologies/2022/8/Gait_Ontology#Waddling"/>
        <Gait_Ontology:hasGait_type rdf:datatype="http://www.w3.org/2001/XMLSchema#string">Myopathic gait</Gait_Ontology:hasGait_type>
    </owl:NamedIndividual>
    


    <!-- http://www.semanticweb.org/marthinust/ontologies/2022/8/Gait_Ontology#Walker -->

    <owl:NamedIndividual rdf:about="http://www.semanticweb.org/marthinust/ontologies/2022/8/Gait_Ontology#Walker">
        <rdf:type rdf:resource="http://www.semanticweb.org/marthinust/ontologies/2022/8/Gait_Ontology#Gait_Assistive_Technology"/>
        <Gait_Ontology:isAscertainedIn rdf:resource="http://www.semanticweb.org/marthinust/ontologies/2022/8/Gait_Ontology#Gait_assessment"/>
        <Gait_Ontology:isPrescribedBy rdf:resource="http://www.semanticweb.org/marthinust/ontologies/2022/8/Gait_Ontology#Healthcare_practitioner"/>
        <Gait_Ontology:isRecommendedTo rdf:resource="http://www.semanticweb.org/marthinust/ontologies/2022/8/Gait_Ontology#Elderly"/>
        <Gait_Ontology:hasGait_assistive_solution rdf:datatype="http://www.w3.org/2001/XMLSchema#string">Standard walker</Gait_Ontology:hasGait_assistive_solution>
        <Gait_Ontology:hasType_of_material rdf:datatype="http://www.w3.org/2001/XMLSchema#string">Metal</Gait_Ontology:hasType_of_material>
    </owl:NamedIndividual>
    


    <!-- http://www.semanticweb.org/marthinust/ontologies/2022/8/Gait_Ontology#Walking_stick -->

    <owl:NamedIndividual rdf:about="http://www.semanticweb.org/marthinust/ontologies/2022/8/Gait_Ontology#Walking_stick">
        <rdf:type rdf:resource="http://www.semanticweb.org/marthinust/ontologies/2022/8/Gait_Ontology#Gait_Assistive_Technology"/>
        <Gait_Ontology:isAscertainedIn rdf:resource="http://www.semanticweb.org/marthinust/ontologies/2022/8/Gait_Ontology#Gait_assessment"/>
        <Gait_Ontology:isPrescribedBy rdf:resource="http://www.semanticweb.org/marthinust/ontologies/2022/8/Gait_Ontology#Physical_therapist"/>
        <Gait_Ontology:isRecommendedTo rdf:resource="http://www.semanticweb.org/marthinust/ontologies/2022/8/Gait_Ontology#Adult"/>
        <Gait_Ontology:hasGait_assistive_solution rdf:datatype="http://www.w3.org/2001/XMLSchema#string">Stick cane</Gait_Ontology:hasGait_assistive_solution>
        <Gait_Ontology:hasType_of_material rdf:datatype="http://www.w3.org/2001/XMLSchema#string">Wooden</Gait_Ontology:hasType_of_material>
        <rdfs:comment xml:lang="en">A cane or stick can be helpful if you have minor problems with balance or stability, some weakness in your leg or trunk, an injury, or a pain. If you are elderly, using a single point cane may help you to walk more comfortably and safely and, in some cases, may make it easier for you to continue living independently.</rdfs:comment>
        <rdfs:label xml:lang="en">Walking_stick</rdfs:label>
    </owl:NamedIndividual>
    


    <!-- http://www.semanticweb.org/marthinust/ontologies/2022/8/Gait_Ontology#Parkinson&apos;s -->

    <owl:NamedIndividual rdf:about="http://www.semanticweb.org/marthinust/ontologies/2022/8/Gait_Ontology#Parkinson&apos;s">
        <rdf:type rdf:resource="http://www.semanticweb.org/marthinust/ontologies/2022/8/Gait_Ontology#Gait-related_Disease"/>
        <Gait_Ontology:isAssociatedTo rdf:resource="http://www.semanticweb.org/marthinust/ontologies/2022/8/Gait_Ontology#Elderly"/>
        <Gait_Ontology:hasDisease_description rdf:datatype="http://www.w3.org/2001/XMLSchema#string">Parkinsonism</Gait_Ontology:hasDisease_description>
        <rdfs:comment xml:lang="en">Parkinson&apos;s disease (PD) is a type of movement disorder. It happens when nerve cells in the brain don&apos;t produce enough of a brain chemical called dopamine. Sometimes it is genetic, but most cases do not seem to run in families. Exposure to chemicals in the environment might play a role. As symptoms get worse, people with the disease may have trouble walking, talking, or doing simple tasks. They may also have problems such as depression, sleep problems, or trouble chewing, swallowing, or speaking. 

Parkinson&apos;s disease is a brain disorder that causes unintended or uncontrollable movements, such as shaking, stiffness, and difficulty with balance and coordination. Symptoms usually begin gradually and worsen over time. As the disease progresses, people may have difficulty walking and talking.</rdfs:comment>
        <rdfs:label xml:lang="en">Parkinson&apos;s</rdfs:label>
    </owl:NamedIndividual>
    <rdf:Description>
        <Gait_Ontology:hasAgeGroup rdf:resource="http://www.semanticweb.org/marthinust/ontologies/2022/8/Gait_Ontology#Child"/>
    </rdf:Description>
    <rdf:Description>
        <Gait_Ontology:hasAgeGroup rdf:resource="http://www.semanticweb.org/marthinust/ontologies/2022/8/Gait_Ontology#Adolescent"/>
    </rdf:Description>
    <rdf:Description>
        <Gait_Ontology:hasAgeGroup rdf:resource="http://www.semanticweb.org/marthinust/ontologies/2022/8/Gait_Ontology#Elderly"/>
    </rdf:Description>
    <rdf:Description>
        <opla-sd:entityPositionX rdf:datatype="http://www.w3.org/2001/XMLSchema#double">259.08886439337294</opla-sd:entityPositionX>
        <opla-sd:entityPositionY rdf:datatype="http://www.w3.org/2001/XMLSchema#double">56.21693028620965</opla-sd:entityPositionY>
        <rdfs:comment xml:lang="en">This is an entity positioning annotation generated by CoModIDE (https://comodide.com/). Removing this annotation will break rendering the CoModIDE schema diagram view.</rdfs:comment>
    </rdf:Description>
    <rdf:Description>
        <opla-sd:entityPositionX rdf:datatype="http://www.w3.org/2001/XMLSchema#double">79.2458402424517</opla-sd:entityPositionX>
        <opla-sd:entityPositionY rdf:datatype="http://www.w3.org/2001/XMLSchema#double">269.67445065953854</opla-sd:entityPositionY>
        <rdfs:comment xml:lang="en">This is an entity positioning annotation generated by CoModIDE (https://comodide.com/). Removing this annotation will break rendering the CoModIDE schema diagram view.</rdfs:comment>
    </rdf:Description>
    <rdf:Description>
        <opla-sd:entityPositionX rdf:datatype="http://www.w3.org/2001/XMLSchema#double">16.803569313406495</opla-sd:entityPositionX>
        <opla-sd:entityPositionY rdf:datatype="http://www.w3.org/2001/XMLSchema#double">91.0975250159648</opla-sd:entityPositionY>
        <rdfs:comment xml:lang="en">This is an entity positioning annotation generated by CoModIDE (https://comodide.com/). Removing this annotation will break rendering the CoModIDE schema diagram view.</rdfs:comment>
    </rdf:Description>
    <rdf:Description>
        <opla-sd:entityPositionX rdf:datatype="http://www.w3.org/2001/XMLSchema#double">90.9877361680386</opla-sd:entityPositionX>
        <opla-sd:entityPositionY rdf:datatype="http://www.w3.org/2001/XMLSchema#double">267.9692849963406</opla-sd:entityPositionY>
        <rdfs:comment xml:lang="en">This is an entity positioning annotation generated by CoModIDE (https://comodide.com/). Removing this annotation will break rendering the CoModIDE schema diagram view.</rdfs:comment>
    </rdf:Description>
    <rdf:Description>
        <opla-sd:entityPositionX rdf:datatype="http://www.w3.org/2001/XMLSchema#double">60.264499049883646</opla-sd:entityPositionX>
        <opla-sd:entityPositionY rdf:datatype="http://www.w3.org/2001/XMLSchema#double">206.98101300589775</opla-sd:entityPositionY>
        <rdfs:comment xml:lang="en">This is an entity positioning annotation generated by CoModIDE (https://comodide.com/). Removing this annotation will break rendering the CoModIDE schema diagram view.</rdfs:comment>
    </rdf:Description>
    


    <!-- 
    ///////////////////////////////////////////////////////////////////////////////////////
    //
    // Annotations
    //
    ///////////////////////////////////////////////////////////////////////////////////////
     -->

    <rdf:Description rdf:about="http://www.semanticweb.org/marthinust/ontologies/2022/8/Gait_Ontology#Ataxia">
        <rdfs:label xml:lang="en">Ataxia</rdfs:label>
        <rdfs:comment>Ataxia is a degenerative disease of the nervous system. Many symptoms of Ataxia mimic those of being drunk, such as slurred speech, stumbling, falling, and incoordination. These symptoms are caused by damage to the cerebellum, the part of the brain that is responsible for coordinating movement. People affected by Ataxia may experience problems with using their fingers and hands, arms, legs, walking, speaking or moving their eyes. Ataxia affects people of all ages. Age of symptom-onset can vary widely, from childhood to late-adulthood. Complications from the disease are serious and oftentimes debilitating. Some types of Ataxia can lead to an early death.</rdfs:comment>
        <opla-sd:entityPosition>
            <rdf:Description>
                <opla-sd:entityPositionX rdf:datatype="http://www.w3.org/2001/XMLSchema#double">18.85038540278317</opla-sd:entityPositionX>
                <opla-sd:entityPositionY rdf:datatype="http://www.w3.org/2001/XMLSchema#double">114.82223573701026</opla-sd:entityPositionY>
                <rdfs:comment xml:lang="en">This is an entity positioning annotation generated by CoModIDE (https://comodide.com/). Removing this annotation will break rendering the CoModIDE schema diagram view.</rdfs:comment>
            </rdf:Description>
        </opla-sd:entityPosition>
    </rdf:Description>
    <rdf:Description rdf:about="http://www.semanticweb.org/marthinust/ontologies/2022/8/Gait_Ontology#Ataxic_gait">
        <opla-sd:entityPosition>
            <rdf:Description>
                <opla-sd:entityPositionX rdf:datatype="http://www.w3.org/2001/XMLSchema#double">152.50616207032508</opla-sd:entityPositionX>
                <opla-sd:entityPositionY rdf:datatype="http://www.w3.org/2001/XMLSchema#double">272.8179275348511</opla-sd:entityPositionY>
                <rdfs:comment xml:lang="en">This is an entity positioning annotation generated by CoModIDE (https://comodide.com/). Removing this annotation will break rendering the CoModIDE schema diagram view.</rdfs:comment>
            </rdf:Description>
        </opla-sd:entityPosition>
        <rdfs:label xml:lang="en">Ataxic_gait</rdfs:label>
        <rdfs:comment xml:lang="en">Most commonly seen in cerebellar disease, this gait is described as clumsy, staggering movements with a wide-based gait. While standing still, the patient&apos;s body may swagger back and forth and from side to side, known as titubation. Patients will not be able to walk from heel to toe or in a straight line. The gait of acute alcohol intoxication will resemble the gait of cerebellar disease. Patients with more truncal instability are more likely to have midline cerebellar disease at the vermis.

(Cerebellar)</rdfs:comment>
    </rdf:Description>
    <rdf:Description rdf:about="http://www.semanticweb.org/marthinust/ontologies/2022/8/Gait_Ontology#Dystonia">
        <rdfs:label xml:lang="en">Dystonia</rdfs:label>
        <rdfs:comment xml:lang="en">Dystonia is a very complex, highly variable neurological movement disorder characterized by involuntary muscle contractions. Dystonia is a movement disorder in which a person&apos;s muscles contract uncontrollably. The contraction causes the affected body part to twist involuntarily, resulting in repetitive movements or abnormal postures. Dystonia can affect one muscle, a muscle group, or the entire body. Dystonia affects about 1% of the population, and women are more prone to it than men.

Dystonia is a disorder characterised by involuntary muscle contractions that cause slow repetitive movements or abnormal postures. The movements may be painful, and some individuals with dystonia may have a tremor or other neurological symptoms. 

Symptoms may include a foot cramp or a tendency for one foot to turn or drageither sporadically or after running or walking some distance.</rdfs:comment>
        <opla-sd:entityPosition>
            <rdf:Description>
                <opla-sd:entityPositionX rdf:datatype="http://www.w3.org/2001/XMLSchema#double">209.55049235509736</opla-sd:entityPositionX>
                <opla-sd:entityPositionY rdf:datatype="http://www.w3.org/2001/XMLSchema#double">121.59159018685122</opla-sd:entityPositionY>
                <rdfs:comment xml:lang="en">This is an entity positioning annotation generated by CoModIDE (https://comodide.com/). Removing this annotation will break rendering the CoModIDE schema diagram view.</rdfs:comment>
            </rdf:Description>
        </opla-sd:entityPosition>
    </rdf:Description>
    <rdf:Description rdf:about="http://www.semanticweb.org/marthinust/ontologies/2022/8/Gait_Ontology#Dystonic_gait">
        <rdfs:comment xml:lang="en">Dystonic gait disorders frequently appear bizarre, particularly because activity increases dystonic tonus and posture. The abnormal posture of the foot in dystonic gait typically involves inversion, plantar flexion and tonic extension of the big toe. In many patients complex types of walking, such as walking backwards and running are paradoxically less impaired than walking forward and may seem completely unaffected. Sensory tricks, for instance, if the affected individual rests a hand on his or her neck, may improve or even normalise dystonic gait in some patients.</rdfs:comment>
        <rdfs:label xml:lang="en">Dystonic_gait</rdfs:label>
        <opla-sd:entityPosition>
            <rdf:Description>
                <opla-sd:entityPositionX rdf:datatype="http://www.w3.org/2001/XMLSchema#double">75.82209884890511</opla-sd:entityPositionX>
                <opla-sd:entityPositionY rdf:datatype="http://www.w3.org/2001/XMLSchema#double">284.4845136355521</opla-sd:entityPositionY>
                <rdfs:comment xml:lang="en">This is an entity positioning annotation generated by CoModIDE (https://comodide.com/). Removing this annotation will break rendering the CoModIDE schema diagram view.</rdfs:comment>
            </rdf:Description>
        </opla-sd:entityPosition>
    </rdf:Description>
    <rdf:Description rdf:about="http://www.semanticweb.org/marthinust/ontologies/2022/8/Gait_Ontology#Electromyography">
        <rdfs:comment xml:lang="en">To measure the action of the muscles in the lower extremity in a human gait, the Electromyography (EMG) was developed to perform an indirect measurement of muscle activity using surface or wire electrodes. These electrodes are a kind of sensor for EMG and can detect voltage potentials to provide information on the timing and intensity of muscle contraction, which have been commercialised in combination with wireless technology. Generally, surface electrodes are used when only general information on muscle activity is required, whereas wire electrodes must be inserted into the designated muscle using a hypodermic needle to measure specific information on a particular muscle. As a result, EMG sensors can be used to realise the assessment of muscle activity in human gait and play an important role in evaluating the walking performance of individuals with problems in their lower extremities.</rdfs:comment>
        <rdfs:label xml:lang="en">Electromyography</rdfs:label>
        <opla-sd:entityPosition>
            <rdf:Description>
                <opla-sd:entityPositionX rdf:datatype="http://www.w3.org/2001/XMLSchema#double">80.45256607278827</opla-sd:entityPositionX>
                <opla-sd:entityPositionY rdf:datatype="http://www.w3.org/2001/XMLSchema#double">82.83099092823711</opla-sd:entityPositionY>
                <rdfs:comment xml:lang="en">This is an entity positioning annotation generated by CoModIDE (https://comodide.com/). Removing this annotation will break rendering the CoModIDE schema diagram view.</rdfs:comment>
            </rdf:Description>
        </opla-sd:entityPosition>
    </rdf:Description>
    <rdf:Description rdf:about="http://www.semanticweb.org/marthinust/ontologies/2022/8/Gait_Ontology#Freezing_of_gait">
        <rdfs:label xml:lang="en">Freezing_of_gait</rdfs:label>
        <opla-sd:entityPosition>
            <rdf:Description>
                <opla-sd:entityPositionX rdf:datatype="http://www.w3.org/2001/XMLSchema#double">89.72226907123033</opla-sd:entityPositionX>
                <opla-sd:entityPositionY rdf:datatype="http://www.w3.org/2001/XMLSchema#double">17.389533513264855</opla-sd:entityPositionY>
                <rdfs:comment xml:lang="en">This is an entity positioning annotation generated by CoModIDE (https://comodide.com/). Removing this annotation will break rendering the CoModIDE schema diagram view.</rdfs:comment>
            </rdf:Description>
        </opla-sd:entityPosition>
        <rdfs:comment xml:lang="en">Freezing of gait is defined as a brief, episodic absence or marked reduction of forward progression of the feet despite the intention to walk.

Freezing of gait is one of the most debilitating motor symptoms in patients with Parkinson&apos;s disease as it may lead to falls and a loss of independence. Patients may report that their feet are stuck to the floor as if held by magnets when trying to walk, resulting in a temporary blockage of the motor function involved in ambulation.</rdfs:comment>
    </rdf:Description>
    <rdf:Description rdf:about="http://www.semanticweb.org/marthinust/ontologies/2022/8/Gait_Ontology#Gait_imbalance">
        <rdfs:comment>Abnormality of equilibrium. Imbalanced walk. Abnormality of balance.</rdfs:comment>
        <opla-sd:entityPosition>
            <rdf:Description>
                <opla-sd:entityPositionX rdf:datatype="http://www.w3.org/2001/XMLSchema#double">56.61717725369067</opla-sd:entityPositionX>
                <opla-sd:entityPositionY rdf:datatype="http://www.w3.org/2001/XMLSchema#double">177.84124689850958</opla-sd:entityPositionY>
                <rdfs:comment xml:lang="en">This is an entity positioning annotation generated by CoModIDE (https://comodide.com/). Removing this annotation will break rendering the CoModIDE schema diagram view.</rdfs:comment>
            </rdf:Description>
        </opla-sd:entityPosition>
        <rdfs:label xml:lang="en">Gait_imbalance</rdfs:label>
    </rdf:Description>
    <rdf:Description rdf:about="http://www.semanticweb.org/marthinust/ontologies/2022/8/Gait_Ontology#Hallux_rigidus">
        <opla-sd:entityPosition>
            <rdf:Description>
                <opla-sd:entityPositionX rdf:datatype="http://www.w3.org/2001/XMLSchema#double">256.0726880338156</opla-sd:entityPositionX>
                <opla-sd:entityPositionY rdf:datatype="http://www.w3.org/2001/XMLSchema#double">299.0876917478438</opla-sd:entityPositionY>
                <rdfs:comment xml:lang="en">This is an entity positioning annotation generated by CoModIDE (https://comodide.com/). Removing this annotation will break rendering the CoModIDE schema diagram view.</rdfs:comment>
            </rdf:Description>
        </opla-sd:entityPosition>
        <rdfs:comment xml:lang="en">Hallux Rigidus (also referred to as Hallux Limitus) is a degenerative condition leading to reduced rang of motion in the first metatarsophalangeal (MTP) joint of the big toe or great toe. This can impair normal gait function, particularly during the propulsive phase.

Hallux Rigidus results in a lack of dorsiflexion of the great toe.  The windlass effect to raise the arch and stiffen the foot during dorsiflexion of the hallux. This stiffness increases the efficiency of the propulsion portion of the gait cycle. To be efficient in creating stiffness, the hallux should be able to dorsiflex at least 65 degrees.</rdfs:comment>
        <rdfs:label xml:lang="en">Hallux_rigidus</rdfs:label>
    </rdf:Description>
    <rdf:Description rdf:about="http://www.semanticweb.org/marthinust/ontologies/2022/8/Gait_Ontology#Hip_abductor_weakness">
        <rdfs:comment xml:lang="en">The abductor muscles stabilise the pelvis to allow the opposite leg to lift during the swing phase. Weak abductor muscles will cause the hip to drop towards the side of the leg swinging forward. This is also known as Trendelenburg gait.

Hip abductor weakness (Trendelenburg gait): Excessive downward drop of the contralateral pelvis during stance. Referred to as positive Trendelenburg sign if present during single-limb standing.
Pathomechanism: Compensated gait causes the trunk to lean laterally toward the stance lower extremity of the weak side. If bilateral, it is referred to as a waddling gait.</rdfs:comment>
        <opla-sd:entityPosition>
            <rdf:Description>
                <opla-sd:entityPositionX rdf:datatype="http://www.w3.org/2001/XMLSchema#double">259.6025366844974</opla-sd:entityPositionX>
                <opla-sd:entityPositionY rdf:datatype="http://www.w3.org/2001/XMLSchema#double">30.855143042967015</opla-sd:entityPositionY>
                <rdfs:comment xml:lang="en">This is an entity positioning annotation generated by CoModIDE (https://comodide.com/). Removing this annotation will break rendering the CoModIDE schema diagram view.</rdfs:comment>
            </rdf:Description>
        </opla-sd:entityPosition>
        <rdfs:label xml:lang="en">Hip_abductor_weakness</rdfs:label>
    </rdf:Description>
    <rdf:Description rdf:about="http://www.semanticweb.org/marthinust/ontologies/2022/8/Gait_Ontology#Image_sensing">
        <rdfs:comment>A standard gait analysis method based on the multi-camera motion capture system and force platform with the capability of measuring ground-reaction forces was successfully developed and applied in a number of gait laboratories.</rdfs:comment>
        <rdfs:label xml:lang="en">Image_sensing</rdfs:label>
        <opla-sd:entityPosition>
            <rdf:Description>
                <opla-sd:entityPositionX rdf:datatype="http://www.w3.org/2001/XMLSchema#double">277.80650066908066</opla-sd:entityPositionX>
                <opla-sd:entityPositionY rdf:datatype="http://www.w3.org/2001/XMLSchema#double">157.8917533236596</opla-sd:entityPositionY>
                <rdfs:comment xml:lang="en">This is an entity positioning annotation generated by CoModIDE (https://comodide.com/). Removing this annotation will break rendering the CoModIDE schema diagram view.</rdfs:comment>
            </rdf:Description>
        </opla-sd:entityPosition>
    </rdf:Description>
    <rdf:Description rdf:about="http://www.semanticweb.org/marthinust/ontologies/2022/8/Gait_Ontology#Limp_gait">
        <rdfs:label xml:lang="en">Limp_gait</rdfs:label>
        <opla-sd:entityPosition>
            <rdf:Description>
                <opla-sd:entityPositionX rdf:datatype="http://www.w3.org/2001/XMLSchema#double">275.91513350457535</opla-sd:entityPositionX>
                <opla-sd:entityPositionY rdf:datatype="http://www.w3.org/2001/XMLSchema#double">169.65957161925414</opla-sd:entityPositionY>
                <rdfs:comment xml:lang="en">This is an entity positioning annotation generated by CoModIDE (https://comodide.com/). Removing this annotation will break rendering the CoModIDE schema diagram view.</rdfs:comment>
            </rdf:Description>
        </opla-sd:entityPosition>
        <rdfs:comment xml:lang="en">This is a gait pattern characterised by a reduced weight-bearing on one limb, often due to pain or injury.</rdfs:comment>
    </rdf:Description>
    <rdf:Description rdf:about="http://www.semanticweb.org/marthinust/ontologies/2022/8/Gait_Ontology#Musculoskeletal">
        <rdfs:comment xml:lang="en">Musculoskeletal health refers to the performance of the locomotor system, comprising intact muscles, bones, joints and adjacent connective tissues.

Your musculoskeletal system includes bones, muscles, tendons, ligaments and soft tissues.</rdfs:comment>
        <rdfs:label xml:lang="en">Musculoskeletal</rdfs:label>
        <opla-sd:entityPosition>
            <rdf:Description>
                <opla-sd:entityPositionX rdf:datatype="http://www.w3.org/2001/XMLSchema#double">26.096504953841485</opla-sd:entityPositionX>
                <opla-sd:entityPositionY rdf:datatype="http://www.w3.org/2001/XMLSchema#double">246.04300278102784</opla-sd:entityPositionY>
                <rdfs:comment xml:lang="en">This is an entity positioning annotation generated by CoModIDE (https://comodide.com/). Removing this annotation will break rendering the CoModIDE schema diagram view.</rdfs:comment>
            </rdf:Description>
        </opla-sd:entityPosition>
        <rdfs:comment xml:lang="en">The term musculoskeletal refers to the muscles and the bones and their associated structures, such as tendons, ligaments, and cartilage. The musculoskeletal system is responsible for movement, support, and protection of the body. It includes the bones of the skeleton, the muscles that move the bones, and the tendons, ligaments, and cartilage that connect the bones and muscles and help to stabilize the joints.

The term musculoskeletal is often used to describe conditions that affect the muscles, bones, and associated structures, such as musculoskeletal disorders or diseases. These conditions can cause a wide range of symptoms, including pain, stiffness, and difficulty with movement. Musculoskeletal conditions can be caused by a variety of factors, including genetics, injury, overuse, and degenerative diseases. Treatment may involve medications, physical therapy, and other interventions.</rdfs:comment>
    </rdf:Description>
    <rdf:Description rdf:about="http://www.semanticweb.org/marthinust/ontologies/2022/8/Gait_Ontology#Neurological">
        <rdfs:comment xml:lang="en">The term neurological comes from neurology  the branch of medicine that deals with problems affecting the nervous system. The word neuro means nerve and nervous system. Neurological disorders are medically defined as disorders that affect the brain as well as the nerves found throughout the human body and the spinal cord. Structural, biochemical or electrical abnormalities in the brain, spinal cord or other nerves can result in a range of symptoms.</rdfs:comment>
        <opla-sd:entityPosition>
            <rdf:Description>
                <opla-sd:entityPositionX rdf:datatype="http://www.w3.org/2001/XMLSchema#double">10.654550012271528</opla-sd:entityPositionX>
                <opla-sd:entityPositionY rdf:datatype="http://www.w3.org/2001/XMLSchema#double">271.9795268055477</opla-sd:entityPositionY>
                <rdfs:comment xml:lang="en">This is an entity positioning annotation generated by CoModIDE (https://comodide.com/). Removing this annotation will break rendering the CoModIDE schema diagram view.</rdfs:comment>
            </rdf:Description>
        </opla-sd:entityPosition>
        <rdfs:comment xml:lang="en">The term neurological refers to the nervous system, which is the body&apos;s system for communicating and coordinating functions. The nervous system is made up of the brain, the spinal cord, and a network of nerves that extend throughout the body. It is responsible for transmitting information between the brain and the rest of the body, as well as for controlling many of the body&apos;s functions, such as movement, sensation, and organ function.

The term neurological is often used to describe conditions that affect the nervous system, such as neurological disorders or diseases. These conditions can affect the brain, the spinal cord, or the nerves, and can cause a wide range of symptoms, such as muscle weakness, numbness, and difficulty with coordination and balance. Neurological conditions can be caused by a variety of factors, including genetics, infection, trauma, and degenerative diseases.</rdfs:comment>
        <rdfs:label xml:lang="en">Neurological</rdfs:label>
    </rdf:Description>
    <rdf:Description rdf:about="http://www.semanticweb.org/marthinust/ontologies/2022/8/Gait_Ontology#Neuromuscular">
        <rdfs:label xml:lang="en">Neuromuscular</rdfs:label>
        <opla-sd:entityPosition>
            <rdf:Description>
                <opla-sd:entityPositionX rdf:datatype="http://www.w3.org/2001/XMLSchema#double">188.9595167078593</opla-sd:entityPositionX>
                <opla-sd:entityPositionY rdf:datatype="http://www.w3.org/2001/XMLSchema#double">128.67219772092892</opla-sd:entityPositionY>
                <rdfs:comment xml:lang="en">This is an entity positioning annotation generated by CoModIDE (https://comodide.com/). Removing this annotation will break rendering the CoModIDE schema diagram view.</rdfs:comment>
            </rdf:Description>
        </opla-sd:entityPosition>
        <rdfs:comment>Neuromuscular diseases affect the function of muscles due to problems with the nerves and muscles in your body.</rdfs:comment>
    </rdf:Description>
    <rdf:Description rdf:about="http://www.semanticweb.org/marthinust/ontologies/2022/8/Gait_Ontology#Normal_gait">
        <opla-sd:entityPosition>
            <rdf:Description>
                <opla-sd:entityPositionX rdf:datatype="http://www.w3.org/2001/XMLSchema#double">127.34738472032292</opla-sd:entityPositionX>
                <opla-sd:entityPositionY rdf:datatype="http://www.w3.org/2001/XMLSchema#double">204.04657631479668</opla-sd:entityPositionY>
                <rdfs:comment xml:lang="en">This is an entity positioning annotation generated by CoModIDE (https://comodide.com/). Removing this annotation will break rendering the CoModIDE schema diagram view.</rdfs:comment>
            </rdf:Description>
        </opla-sd:entityPosition>
        <rdfs:comment xml:lang="en">This is the typical standard gait pattern seen in a healthy individual. It is characterised by smooth and coordinated movement of the limbs and a symmetrical stride.</rdfs:comment>
        <rdfs:label xml:lang="en">Normal_gait</rdfs:label>
    </rdf:Description>
    <rdf:Description rdf:about="http://www.semanticweb.org/marthinust/ontologies/2022/8/Gait_Ontology#Parkinsonian_gait">
        <rdfs:label xml:lang="en">Parkinsonian_gait</rdfs:label>
        <rdfs:comment xml:lang="en">In this gait, the patient will have rigidity and bradykinesia. He or she will be stooped with the head and neck forward, with flexion at the knees. The whole upper extremity is also in flexion with the fingers usually extended. The patient walks with slow little steps known at marche a petits pas (walk of little steps). Patient may also have difficulty initiating steps. The patient may show an involuntary inclination to take accelerating steps, known as festination. This gait is seen in Parkinson&apos;s disease or any other condition causing parkinsonism, such as side effects from drugs.

(Festinating Gait, Propulsive Gait)</rdfs:comment>
        <opla-sd:entityPosition>
            <rdf:Description>
                <opla-sd:entityPositionX rdf:datatype="http://www.w3.org/2001/XMLSchema#double">219.03672191612606</opla-sd:entityPositionX>
                <opla-sd:entityPositionY rdf:datatype="http://www.w3.org/2001/XMLSchema#double">97.77812924613833</opla-sd:entityPositionY>
                <rdfs:comment xml:lang="en">This is an entity positioning annotation generated by CoModIDE (https://comodide.com/). Removing this annotation will break rendering the CoModIDE schema diagram view.</rdfs:comment>
            </rdf:Description>
        </opla-sd:entityPosition>
    </rdf:Description>
    <rdf:Description rdf:about="http://www.semanticweb.org/marthinust/ontologies/2022/8/Gait_Ontology#Scoliosis">
        <rdfs:label xml:lang="en">Scoliosis</rdfs:label>
        <opla-sd:entityPosition>
            <rdf:Description>
                <opla-sd:entityPositionX rdf:datatype="http://www.w3.org/2001/XMLSchema#double">135.08747420375346</opla-sd:entityPositionX>
                <opla-sd:entityPositionY rdf:datatype="http://www.w3.org/2001/XMLSchema#double">179.85908777497016</opla-sd:entityPositionY>
                <rdfs:comment xml:lang="en">This is an entity positioning annotation generated by CoModIDE (https://comodide.com/). Removing this annotation will break rendering the CoModIDE schema diagram view.</rdfs:comment>
            </rdf:Description>
        </opla-sd:entityPosition>
        <rdfs:comment xml:lang="en">Scoliosis is a sideways curvature of the spine that most often is diagnosed in adolescents. While scoliosis can occur in people with conditions such as cerebral palsy and muscular dystrophy, the cause of most childhood scoliosis is unknown. Most cases of scoliosis are mild, but some curves worsen as children grow.

A sideways curvature of the spine.
Scoliosis occurs most often during the growth spurt just before puberty.
Most cases are mild with few symptoms. Some children develop spine deformities that get more severe as they grow. Severe scoliosis can be painful and disabling.
Often, no treatment is necessary. Sometimes a brace or surgery is required.</rdfs:comment>
    </rdf:Description>
    <rdf:Description rdf:about="http://www.semanticweb.org/marthinust/ontologies/2022/8/Gait_Ontology#Waddling_gait">
        <opla-sd:entityPosition>
            <rdf:Description>
                <opla-sd:entityPositionX rdf:datatype="http://www.w3.org/2001/XMLSchema#double">88.02137804692497</opla-sd:entityPositionX>
                <opla-sd:entityPositionY rdf:datatype="http://www.w3.org/2001/XMLSchema#double">119.2672495059423</opla-sd:entityPositionY>
                <rdfs:comment xml:lang="en">This is an entity positioning annotation generated by CoModIDE (https://comodide.com/). Removing this annotation will break rendering the CoModIDE schema diagram view.</rdfs:comment>
            </rdf:Description>
        </opla-sd:entityPosition>
        <rdfs:label xml:lang="en">Waddling_gait</rdfs:label>
        <rdfs:comment xml:lang="en">Weakness of the hip girdle and upper thigh muscles, for instance in myopathies, leads to an instability of the pelvis on standing and walking. If the muscles extending the hip joint are affected, the posture in that joint becomes flexed and lumbar lordosis increases. The patients usually have difficulties standing up from a sitting position. Due to weakness in the gluteus medius muscle, the hip on the side of the swinging leg drops with each step (referred to as Trendelenburg sign). The gait appears waddling. The patients frequently attempt to counteract the dropping of the hip on the swinging side by bending the trunk towards the side which is in the stance phase (in the German language literature this is referred to as Duchenne sign). Similar gait patterns can be caused by orthopedic conditions when the origin and the insertion site of the gluteus medius muscle are closer to each other than normal, for instance due to a posttraumatic elevation of the trochanter or pseudarthrosis of the femoral neck.</rdfs:comment>
    </rdf:Description>
    <rdf:Description rdf:about="http://www.semanticweb.org/marthinust/ontologies/2022/8/Gait_Ontology#Walker">
        <rdfs:label xml:lang="en">Walker</rdfs:label>
        <rdfs:comment xml:lang="en">A walker is an assistive device that provides the patient with a wide base of support, increased anterior and lateral stability, and a reduction in weight-bearing on one or both lower extremities. The walker is the most stable ambulatory assistive device.</rdfs:comment>
        <opla-sd:entityPosition>
            <rdf:Description>
                <opla-sd:entityPositionX rdf:datatype="http://www.w3.org/2001/XMLSchema#double">231.61533810370958</opla-sd:entityPositionX>
                <opla-sd:entityPositionY rdf:datatype="http://www.w3.org/2001/XMLSchema#double">133.6536931920414</opla-sd:entityPositionY>
                <rdfs:comment xml:lang="en">This is an entity positioning annotation generated by CoModIDE (https://comodide.com/). Removing this annotation will break rendering the CoModIDE schema diagram view.</rdfs:comment>
            </rdf:Description>
        </opla-sd:entityPosition>
    </rdf:Description>
</rdf:RDF>



<!-- Generated by the OWL API (version 4.5.9.2019-02-01T07:24:44Z) https://github.com/owlcs/owlapi -->

